<?xml version="1.0"?>
<rdf:RDF xmlns="http://www.semanticweb.org/audunvennesland/ontologies/2019/0/untitled-ontology-214#"
     xml:base="http://www.semanticweb.org/audunvennesland/ontologies/2019/0/untitled-ontology-214"
     xmlns:rdf="http://www.w3.org/1999/02/22-rdf-syntax-ns#"
     xmlns:owl="http://www.w3.org/2002/07/owl#"
     xmlns:xml="http://www.w3.org/XML/1998/namespace"
     xmlns:xsd="http://www.w3.org/2001/XMLSchema#"
     xmlns:rdfs="http://www.w3.org/2000/01/rdf-schema#">
    <owl:Ontology rdf:about="http://www.semanticweb.org/audunvennesland/ontologies/2019/0/untitled-ontology-214"/>
    


    <!-- 
    ///////////////////////////////////////////////////////////////////////////////////////
    //
    // Object Properties
    //
    ///////////////////////////////////////////////////////////////////////////////////////
     -->

    


    <!-- http://www.semanticweb.org/audunvennesland/ontologies/2019/0/untitled-ontology-214#hasTopic -->

    <owl:ObjectProperty rdf:about="http://www.semanticweb.org/audunvennesland/ontologies/2019/0/untitled-ontology-214#hasTopic">
        <rdfs:domain rdf:resource="http://www.semanticweb.org/audunvennesland/ontologies/2019/0/untitled-ontology-214#Entry"/>
        <rdfs:range rdf:resource="http://www.semanticweb.org/audunvennesland/ontologies/2019/0/untitled-ontology-214#Topic"/>
    </owl:ObjectProperty>
    


    <!-- http://www.semanticweb.org/audunvennesland/ontologies/2019/0/untitled-ontology-214#organizedBy -->

    <owl:ObjectProperty rdf:about="http://www.semanticweb.org/audunvennesland/ontologies/2019/0/untitled-ontology-214#organizedBy">
        <rdfs:domain rdf:resource="http://www.semanticweb.org/audunvennesland/ontologies/2019/0/untitled-ontology-214#Conference"/>
        <rdfs:domain rdf:resource="http://www.semanticweb.org/audunvennesland/ontologies/2019/0/untitled-ontology-214#Journal"/>
        <rdfs:range rdf:resource="http://www.semanticweb.org/audunvennesland/ontologies/2019/0/untitled-ontology-214#Organization"/>
    </owl:ObjectProperty>
    


    <!-- http://www.semanticweb.org/audunvennesland/ontologies/2019/0/untitled-ontology-214#publishedIn -->

    <owl:ObjectProperty rdf:about="http://www.semanticweb.org/audunvennesland/ontologies/2019/0/untitled-ontology-214#publishedIn">
        <rdfs:domain rdf:resource="http://www.semanticweb.org/audunvennesland/ontologies/2019/0/untitled-ontology-214#Monography"/>
        <rdfs:domain rdf:resource="http://www.semanticweb.org/audunvennesland/ontologies/2019/0/untitled-ontology-214#Proceedings"/>
        <rdfs:domain rdf:resource="http://www.semanticweb.org/audunvennesland/ontologies/2019/0/untitled-ontology-214#Text"/>
        <rdfs:domain rdf:resource="http://www.semanticweb.org/audunvennesland/ontologies/2019/0/untitled-ontology-214#Thesis"/>
        <rdfs:range rdf:resource="http://www.semanticweb.org/audunvennesland/ontologies/2019/0/untitled-ontology-214#Entry"/>
    </owl:ObjectProperty>
    


    <!-- http://www.semanticweb.org/audunvennesland/ontologies/2019/0/untitled-ontology-214#reviewedBy -->

    <owl:ObjectProperty rdf:about="http://www.semanticweb.org/audunvennesland/ontologies/2019/0/untitled-ontology-214#reviewedBy">
        <rdfs:domain rdf:resource="http://www.semanticweb.org/audunvennesland/ontologies/2019/0/untitled-ontology-214#Academic"/>
        <rdfs:domain rdf:resource="http://www.semanticweb.org/audunvennesland/ontologies/2019/0/untitled-ontology-214#Book"/>
        <rdfs:domain rdf:resource="http://www.semanticweb.org/audunvennesland/ontologies/2019/0/untitled-ontology-214#Text"/>
        <rdfs:range rdf:resource="http://www.semanticweb.org/audunvennesland/ontologies/2019/0/untitled-ontology-214#Person"/>
    </owl:ObjectProperty>
    


    <!-- http://www.semanticweb.org/audunvennesland/ontologies/2019/0/untitled-ontology-214#writtenBy -->

    <owl:ObjectProperty rdf:about="http://www.semanticweb.org/audunvennesland/ontologies/2019/0/untitled-ontology-214#writtenBy">
        <rdfs:domain rdf:resource="http://www.semanticweb.org/audunvennesland/ontologies/2019/0/untitled-ontology-214#Academic"/>
        <rdfs:domain rdf:resource="http://www.semanticweb.org/audunvennesland/ontologies/2019/0/untitled-ontology-214#Book"/>
        <rdfs:domain rdf:resource="http://www.semanticweb.org/audunvennesland/ontologies/2019/0/untitled-ontology-214#Booklet"/>
        <rdfs:domain rdf:resource="http://www.semanticweb.org/audunvennesland/ontologies/2019/0/untitled-ontology-214#LectureNotes"/>
        <rdfs:domain rdf:resource="http://www.semanticweb.org/audunvennesland/ontologies/2019/0/untitled-ontology-214#Manual"/>
        <rdfs:domain rdf:resource="http://www.semanticweb.org/audunvennesland/ontologies/2019/0/untitled-ontology-214#TechReport"/>
        <rdfs:domain rdf:resource="http://www.semanticweb.org/audunvennesland/ontologies/2019/0/untitled-ontology-214#Text"/>
        <rdfs:domain rdf:resource="http://www.semanticweb.org/audunvennesland/ontologies/2019/0/untitled-ontology-214#Unpublished"/>
        <rdfs:range rdf:resource="http://www.semanticweb.org/audunvennesland/ontologies/2019/0/untitled-ontology-214#Person"/>
    </owl:ObjectProperty>
    


    <!-- 
    ///////////////////////////////////////////////////////////////////////////////////////
    //
    // Classes
    //
    ///////////////////////////////////////////////////////////////////////////////////////
     -->

    


    <!-- http://www.semanticweb.org/audunvennesland/ontologies/2019/0/untitled-ontology-214#Academic -->

    <owl:Class rdf:about="http://www.semanticweb.org/audunvennesland/ontologies/2019/0/untitled-ontology-214#Academic">
        <rdfs:subClassOf rdf:resource="http://www.semanticweb.org/audunvennesland/ontologies/2019/0/untitled-ontology-214#Entry"/>
        <rdfs:comment>Relating to education and scholarship.</rdfs:comment>
    </owl:Class>
    


    <!-- http://www.semanticweb.org/audunvennesland/ontologies/2019/0/untitled-ontology-214#Book -->

    <owl:Class rdf:about="http://www.semanticweb.org/audunvennesland/ontologies/2019/0/untitled-ontology-214#Book">
        <rdfs:subClassOf rdf:resource="http://www.semanticweb.org/audunvennesland/ontologies/2019/0/untitled-ontology-214#Entry"/>
        <rdfs:comment>A written text that can be published in printed or electronic form.</rdfs:comment>
    </owl:Class>
    


    <!-- http://www.semanticweb.org/audunvennesland/ontologies/2019/0/untitled-ontology-214#Booklet -->

    <owl:Class rdf:about="http://www.semanticweb.org/audunvennesland/ontologies/2019/0/untitled-ontology-214#Booklet">
        <rdfs:subClassOf rdf:resource="http://www.semanticweb.org/audunvennesland/ontologies/2019/0/untitled-ontology-214#Informal"/>
        <rdfs:comment>A small, thin book with paper covers, typically giving information on a particular subject.</rdfs:comment>
    </owl:Class>
    


    <!-- http://www.semanticweb.org/audunvennesland/ontologies/2019/0/untitled-ontology-214#Chapter -->

    <owl:Class rdf:about="http://www.semanticweb.org/audunvennesland/ontologies/2019/0/untitled-ontology-214#Chapter">
        <rdfs:comment>A main division of a book, typically with a number or title.</rdfs:comment>
    </owl:Class>
    


    <!-- http://www.semanticweb.org/audunvennesland/ontologies/2019/0/untitled-ontology-214#Collection -->

    <owl:Class rdf:about="http://www.semanticweb.org/audunvennesland/ontologies/2019/0/untitled-ontology-214#Collection">
        <rdfs:subClassOf rdf:resource="http://www.semanticweb.org/audunvennesland/ontologies/2019/0/untitled-ontology-214#Book"/>
        <rdfs:comment>A group of written objects that have been collected by one person or in one place.</rdfs:comment>
    </owl:Class>
    


    <!-- http://www.semanticweb.org/audunvennesland/ontologies/2019/0/untitled-ontology-214#Conference -->

    <owl:Class rdf:about="http://www.semanticweb.org/audunvennesland/ontologies/2019/0/untitled-ontology-214#Conference">
        <rdfs:subClassOf rdf:resource="http://www.semanticweb.org/audunvennesland/ontologies/2019/0/untitled-ontology-214#Informal"/>
        <rdfs:comment>A formal meeting of people with a shared interest, typically one that takes place over several days.</rdfs:comment>
    </owl:Class>
    


    <!-- http://www.semanticweb.org/audunvennesland/ontologies/2019/0/untitled-ontology-214#Date -->

    <owl:Class rdf:about="http://www.semanticweb.org/audunvennesland/ontologies/2019/0/untitled-ontology-214#Date">
        <rdfs:comment>The day of the month or year as specified by a number.</rdfs:comment>
    </owl:Class>
    


    <!-- http://www.semanticweb.org/audunvennesland/ontologies/2019/0/untitled-ontology-214#Entry -->

    <owl:Class rdf:about="http://www.semanticweb.org/audunvennesland/ontologies/2019/0/untitled-ontology-214#Entry">
        <rdfs:comment>An item written or printed.</rdfs:comment>
    </owl:Class>
    


    <!-- http://www.semanticweb.org/audunvennesland/ontologies/2019/0/untitled-ontology-214#Informal -->

    <owl:Class rdf:about="http://www.semanticweb.org/audunvennesland/ontologies/2019/0/untitled-ontology-214#Informal">
        <rdfs:subClassOf rdf:resource="http://www.semanticweb.org/audunvennesland/ontologies/2019/0/untitled-ontology-214#Entry"/>
    </owl:Class>
    


    <!-- http://www.semanticweb.org/audunvennesland/ontologies/2019/0/untitled-ontology-214#Institution -->

    <owl:Class rdf:about="http://www.semanticweb.org/audunvennesland/ontologies/2019/0/untitled-ontology-214#Institution">
        <rdfs:comment>An organization founded for a religious, educational, professional, or social purpose.</rdfs:comment>
    </owl:Class>
    


    <!-- http://www.semanticweb.org/audunvennesland/ontologies/2019/0/untitled-ontology-214#Journal -->

    <owl:Class rdf:about="http://www.semanticweb.org/audunvennesland/ontologies/2019/0/untitled-ontology-214#Journal">
        <rdfs:subClassOf rdf:resource="http://www.semanticweb.org/audunvennesland/ontologies/2019/0/untitled-ontology-214#Entry"/>
        <rdfs:comment>A newspaper or magazine that deals with a particular subject or professional activity</rdfs:comment>
    </owl:Class>
    


    <!-- http://www.semanticweb.org/audunvennesland/ontologies/2019/0/untitled-ontology-214#LectureNotes -->

    <owl:Class rdf:about="http://www.semanticweb.org/audunvennesland/ontologies/2019/0/untitled-ontology-214#LectureNotes">
        <rdfs:subClassOf rdf:resource="http://www.semanticweb.org/audunvennesland/ontologies/2019/0/untitled-ontology-214#Academic"/>
        <rdfs:subClassOf rdf:resource="http://www.semanticweb.org/audunvennesland/ontologies/2019/0/untitled-ontology-214#Informal"/>
        <owl:disjointWith rdf:resource="http://www.semanticweb.org/audunvennesland/ontologies/2019/0/untitled-ontology-214#Thesis"/>
        <rdfs:comment>Notes made by a person who is attending a lecture.</rdfs:comment>
    </owl:Class>
    


    <!-- http://www.semanticweb.org/audunvennesland/ontologies/2019/0/untitled-ontology-214#Manual -->

    <owl:Class rdf:about="http://www.semanticweb.org/audunvennesland/ontologies/2019/0/untitled-ontology-214#Manual">
        <rdfs:subClassOf rdf:resource="http://www.semanticweb.org/audunvennesland/ontologies/2019/0/untitled-ontology-214#Informal"/>
        <rdfs:comment>A book giving instructions or information.</rdfs:comment>
    </owl:Class>
    


    <!-- http://www.semanticweb.org/audunvennesland/ontologies/2019/0/untitled-ontology-214#Misc -->

    <owl:Class rdf:about="http://www.semanticweb.org/audunvennesland/ontologies/2019/0/untitled-ontology-214#Misc">
        <rdfs:subClassOf rdf:resource="http://www.semanticweb.org/audunvennesland/ontologies/2019/0/untitled-ontology-214#Informal"/>
        <rdfs:comment>Consisting of a mixture of various things that are not usually connected with each other</rdfs:comment>
    </owl:Class>
    


    <!-- http://www.semanticweb.org/audunvennesland/ontologies/2019/0/untitled-ontology-214#Monography -->

    <owl:Class rdf:about="http://www.semanticweb.org/audunvennesland/ontologies/2019/0/untitled-ontology-214#Monography">
        <rdfs:subClassOf rdf:resource="http://www.semanticweb.org/audunvennesland/ontologies/2019/0/untitled-ontology-214#Book"/>
        <rdfs:comment>A long article or a short book on a particular subject.</rdfs:comment>
    </owl:Class>
    


    <!-- http://www.semanticweb.org/audunvennesland/ontologies/2019/0/untitled-ontology-214#Organization -->

    <owl:Class rdf:about="http://www.semanticweb.org/audunvennesland/ontologies/2019/0/untitled-ontology-214#Organization">
        <rdfs:comment>An organized group of people with a particular purpose, such as a business or government department</rdfs:comment>
    </owl:Class>
    


    <!-- http://www.semanticweb.org/audunvennesland/ontologies/2019/0/untitled-ontology-214#PageRange -->

    <owl:Class rdf:about="http://www.semanticweb.org/audunvennesland/ontologies/2019/0/untitled-ontology-214#PageRange"/>
    


    <!-- http://www.semanticweb.org/audunvennesland/ontologies/2019/0/untitled-ontology-214#Person -->

    <owl:Class rdf:about="http://www.semanticweb.org/audunvennesland/ontologies/2019/0/untitled-ontology-214#Person">
        <rdfs:comment>Human or individual, sometimes used in combination especially by those who prefer to avoid man in compounds applicable to both sexes</rdfs:comment>
    </owl:Class>
    


    <!-- http://www.semanticweb.org/audunvennesland/ontologies/2019/0/untitled-ontology-214#PersonList -->

    <owl:Class rdf:about="http://www.semanticweb.org/audunvennesland/ontologies/2019/0/untitled-ontology-214#PersonList">
        <rdfs:comment>A list of persons, that is, human beings regarded as individuals.</rdfs:comment>
    </owl:Class>
    


    <!-- http://www.semanticweb.org/audunvennesland/ontologies/2019/0/untitled-ontology-214#Proceedings -->

    <owl:Class rdf:about="http://www.semanticweb.org/audunvennesland/ontologies/2019/0/untitled-ontology-214#Proceedings">
        <rdfs:subClassOf rdf:resource="http://www.semanticweb.org/audunvennesland/ontologies/2019/0/untitled-ontology-214#Book"/>
        <rdfs:comment>A published report of a set of meetings or a conference.</rdfs:comment>
    </owl:Class>
    


    <!-- http://www.semanticweb.org/audunvennesland/ontologies/2019/0/untitled-ontology-214#Publisher -->

    <owl:Class rdf:about="http://www.semanticweb.org/audunvennesland/ontologies/2019/0/untitled-ontology-214#Publisher">
        <rdfs:comment>A company or person that prepares and issues books, journals, or music for sale</rdfs:comment>
    </owl:Class>
    


    <!-- http://www.semanticweb.org/audunvennesland/ontologies/2019/0/untitled-ontology-214#ResearchProject -->

    <owl:Class rdf:about="http://www.semanticweb.org/audunvennesland/ontologies/2019/0/untitled-ontology-214#ResearchProject">
        <rdfs:comment>An individual or collaborative enterprise that is carefully planned to achieve a particular research goal.</rdfs:comment>
    </owl:Class>
    


    <!-- http://www.semanticweb.org/audunvennesland/ontologies/2019/0/untitled-ontology-214#School -->

    <owl:Class rdf:about="http://www.semanticweb.org/audunvennesland/ontologies/2019/0/untitled-ontology-214#School">
        <rdfs:comment>Any institution at which instruction is given in a particular discipline.</rdfs:comment>
    </owl:Class>
    


    <!-- http://www.semanticweb.org/audunvennesland/ontologies/2019/0/untitled-ontology-214#TechReport -->

    <owl:Class rdf:about="http://www.semanticweb.org/audunvennesland/ontologies/2019/0/untitled-ontology-214#TechReport">
        <rdfs:subClassOf rdf:resource="http://www.semanticweb.org/audunvennesland/ontologies/2019/0/untitled-ontology-214#Informal"/>
        <rdfs:comment>A technical report (also scientific report) is a document that describes the process, progress, or results of technical or scientific research or the state of a technical or scientific research problem.</rdfs:comment>
    </owl:Class>
    


    <!-- http://www.semanticweb.org/audunvennesland/ontologies/2019/0/untitled-ontology-214#Text -->

    <owl:Class rdf:about="http://www.semanticweb.org/audunvennesland/ontologies/2019/0/untitled-ontology-214#Text">
        <rdfs:comment>A book or other written or printed work, regarded in terms of its content rather than its physical form.</rdfs:comment>
    </owl:Class>
    


    <!-- http://www.semanticweb.org/audunvennesland/ontologies/2019/0/untitled-ontology-214#Thesis -->

    <owl:Class rdf:about="http://www.semanticweb.org/audunvennesland/ontologies/2019/0/untitled-ontology-214#Thesis">
        <rdfs:subClassOf rdf:resource="http://www.semanticweb.org/audunvennesland/ontologies/2019/0/untitled-ontology-214#Academic"/>
        <rdfs:comment>A long piece of writing on a particular subject, especially one that is done for a higher college or university degree.</rdfs:comment>
    </owl:Class>
    


    <!-- http://www.semanticweb.org/audunvennesland/ontologies/2019/0/untitled-ontology-214#Title -->

    <owl:Class rdf:about="http://www.semanticweb.org/audunvennesland/ontologies/2019/0/untitled-ontology-214#Title">
        <rdfs:subClassOf rdf:resource="http://www.semanticweb.org/audunvennesland/ontologies/2019/0/untitled-ontology-214#Text"/>
        <rdfs:comment>The name of a book, composition, or other artistic work.</rdfs:comment>
    </owl:Class>
    


    <!-- http://www.semanticweb.org/audunvennesland/ontologies/2019/0/untitled-ontology-214#Topic -->

    <owl:Class rdf:about="http://www.semanticweb.org/audunvennesland/ontologies/2019/0/untitled-ontology-214#Topic">
        <rdfs:comment>A matter dealt with in a text, discourse, or conversation; a subject.</rdfs:comment>
    </owl:Class>
    


    <!-- http://www.semanticweb.org/audunvennesland/ontologies/2019/0/untitled-ontology-214#UnprintedCopy -->

    <owl:Class rdf:about="http://www.semanticweb.org/audunvennesland/ontologies/2019/0/untitled-ontology-214#UnprintedCopy">
        <rdfs:subClassOf rdf:resource="http://www.semanticweb.org/audunvennesland/ontologies/2019/0/untitled-ontology-214#Entry"/>
        <rdfs:comment>A legible version of a piece of information not printed on a physical medium, especially as stored or displayed on a computer.</rdfs:comment>
    </owl:Class>
    


    <!-- http://www.semanticweb.org/audunvennesland/ontologies/2019/0/untitled-ontology-214#Unpublished -->

    <owl:Class rdf:about="http://www.semanticweb.org/audunvennesland/ontologies/2019/0/untitled-ontology-214#Unpublished">
        <rdfs:subClassOf rdf:resource="http://www.semanticweb.org/audunvennesland/ontologies/2019/0/untitled-ontology-214#Informal"/>
        <rdfs:comment>Written research works that have not been published anywhere.</rdfs:comment>
    </owl:Class>
    


    <!-- 
    ///////////////////////////////////////////////////////////////////////////////////////
    //
    // General axioms
    //
    ///////////////////////////////////////////////////////////////////////////////////////
     -->

    <rdf:Description>
        <rdf:type rdf:resource="http://www.w3.org/2002/07/owl#AllDisjointClasses"/>
        <owl:members rdf:parseType="Collection">
            <rdf:Description rdf:about="http://www.semanticweb.org/audunvennesland/ontologies/2019/0/untitled-ontology-214#Academic"/>
            <rdf:Description rdf:about="http://www.semanticweb.org/audunvennesland/ontologies/2019/0/untitled-ontology-214#Book"/>
            <rdf:Description rdf:about="http://www.semanticweb.org/audunvennesland/ontologies/2019/0/untitled-ontology-214#Informal"/>
        </owl:members>
    </rdf:Description>
    <rdf:Description>
        <rdf:type rdf:resource="http://www.w3.org/2002/07/owl#AllDisjointClasses"/>
        <owl:members rdf:parseType="Collection">
            <rdf:Description rdf:about="http://www.semanticweb.org/audunvennesland/ontologies/2019/0/untitled-ontology-214#Booklet"/>
            <rdf:Description rdf:about="http://www.semanticweb.org/audunvennesland/ontologies/2019/0/untitled-ontology-214#Conference"/>
            <rdf:Description rdf:about="http://www.semanticweb.org/audunvennesland/ontologies/2019/0/untitled-ontology-214#LectureNotes"/>
            <rdf:Description rdf:about="http://www.semanticweb.org/audunvennesland/ontologies/2019/0/untitled-ontology-214#Manual"/>
            <rdf:Description rdf:about="http://www.semanticweb.org/audunvennesland/ontologies/2019/0/untitled-ontology-214#Misc"/>
            <rdf:Description rdf:about="http://www.semanticweb.org/audunvennesland/ontologies/2019/0/untitled-ontology-214#TechReport"/>
            <rdf:Description rdf:about="http://www.semanticweb.org/audunvennesland/ontologies/2019/0/untitled-ontology-214#Unpublished"/>
        </owl:members>
    </rdf:Description>
    <rdf:Description>
        <rdf:type rdf:resource="http://www.w3.org/2002/07/owl#AllDisjointClasses"/>
        <owl:members rdf:parseType="Collection">
            <rdf:Description rdf:about="http://www.semanticweb.org/audunvennesland/ontologies/2019/0/untitled-ontology-214#Chapter"/>
            <rdf:Description rdf:about="http://www.semanticweb.org/audunvennesland/ontologies/2019/0/untitled-ontology-214#Date"/>
            <rdf:Description rdf:about="http://www.semanticweb.org/audunvennesland/ontologies/2019/0/untitled-ontology-214#Entry"/>
            <rdf:Description rdf:about="http://www.semanticweb.org/audunvennesland/ontologies/2019/0/untitled-ontology-214#Institution"/>
            <rdf:Description rdf:about="http://www.semanticweb.org/audunvennesland/ontologies/2019/0/untitled-ontology-214#Journal"/>
            <rdf:Description rdf:about="http://www.semanticweb.org/audunvennesland/ontologies/2019/0/untitled-ontology-214#Organization"/>
            <rdf:Description rdf:about="http://www.semanticweb.org/audunvennesland/ontologies/2019/0/untitled-ontology-214#PageRange"/>
            <rdf:Description rdf:about="http://www.semanticweb.org/audunvennesland/ontologies/2019/0/untitled-ontology-214#Person"/>
            <rdf:Description rdf:about="http://www.semanticweb.org/audunvennesland/ontologies/2019/0/untitled-ontology-214#PersonList"/>
            <rdf:Description rdf:about="http://www.semanticweb.org/audunvennesland/ontologies/2019/0/untitled-ontology-214#Publisher"/>
            <rdf:Description rdf:about="http://www.semanticweb.org/audunvennesland/ontologies/2019/0/untitled-ontology-214#School"/>
            <rdf:Description rdf:about="http://www.semanticweb.org/audunvennesland/ontologies/2019/0/untitled-ontology-214#Text"/>
        </owl:members>
    </rdf:Description>
    <rdf:Description>
        <rdf:type rdf:resource="http://www.w3.org/2002/07/owl#AllDisjointClasses"/>
        <owl:members rdf:parseType="Collection">
            <rdf:Description rdf:about="http://www.semanticweb.org/audunvennesland/ontologies/2019/0/untitled-ontology-214#Collection"/>
            <rdf:Description rdf:about="http://www.semanticweb.org/audunvennesland/ontologies/2019/0/untitled-ontology-214#Monography"/>
            <rdf:Description rdf:about="http://www.semanticweb.org/audunvennesland/ontologies/2019/0/untitled-ontology-214#Proceedings"/>
        </owl:members>
    </rdf:Description>
</rdf:RDF>



<!-- Generated by the OWL API (version 4.2.8.20170104-2310) https://github.com/owlcs/owlapi -->

