<?xml version="1.0"?>
<rdf:RDF xmlns="http://www.project-best.eu/owl/aixm-mod/airportheliport#"
     xml:base="http://www.project-best.eu/owl/aixm-mod/airportheliport"
     xmlns:aixm-ah="http://www.project-best.eu/owl/aixm-mod/airportheliport#"
     xmlns:rdf="http://www.w3.org/1999/02/22-rdf-syntax-ns#"
     xmlns:owl="http://www.w3.org/2002/07/owl#"
     xmlns:xsd="http://www.w3.org/2001/XMLSchema#"
     xmlns:rdfs="http://www.w3.org/2000/01/rdf-schema#">
    <owl:Ontology rdf:about="http://www.project-best.eu/owl/aixm-mod/airportheliport">
        <rdfs:comment xml:lang="en">At the moment the AIXM AbstractFeatures are not in use. Not sure
            if we need to associate the features with this abstract representation. There are no
            generalisations from features to abstracts, only stereotypes. </rdfs:comment>
    </owl:Ontology>
    


    <!-- 
    ///////////////////////////////////////////////////////////////////////////////////////
    //
    // Object Properties
    //
    ///////////////////////////////////////////////////////////////////////////////////////
     -->

    


    <!-- http://www.project-best.eu/owl/aixm-mod/airportheliport#AircraftStand-apronLocation -->

    <owl:ObjectProperty rdf:about="http://www.project-best.eu/owl/aixm-mod/airportheliport#AircraftStand-apronLocation">
        <rdfs:comment xml:lang="en">(DO272/ED99) Each ParkingStandArea feature?s attribute idstd shall provide an idstd object identifier value that holds the idstd object identifier values of all corresponding ParkingStandLocations (Rule 13)</rdfs:comment>
        <rdfs:comment xml:lang="en">Association to Geometry::ElevatedPoint</rdfs:comment>
        <rdfs:domain rdf:resource="http://www.project-best.eu/owl/aixm-mod/airportheliport#AircraftStand"/>
        <rdfs:range rdf:resource="http://www.project-best.eu/owl/aixm-mod/airportheliport#ApronElement"/>
    </owl:ObjectProperty>
    


    <!-- http://www.project-best.eu/owl/aixm-mod/airportheliport#AircraftStand-availability -->

    <owl:ObjectProperty rdf:about="http://www.project-best.eu/owl/aixm-mod/airportheliport#AircraftStand-availability">
        <rdfs:domain rdf:resource="http://www.project-best.eu/owl/aixm-mod/airportheliport#AircraftStand"/>
        <rdfs:range rdf:resource="http://www.project-best.eu/owl/aixm-mod/airportheliport#ApronAreaAvailability"/>
    </owl:ObjectProperty>
    


    <!-- http://www.project-best.eu/owl/aixm-mod/airportheliport#AircraftStand-contaminant -->

    <owl:ObjectProperty rdf:about="http://www.project-best.eu/owl/aixm-mod/airportheliport#AircraftStand-contaminant">
        <rdfs:comment xml:lang="en">Identifies the contaminant of the gate stand.</rdfs:comment>
        <rdfs:domain rdf:resource="http://www.project-best.eu/owl/aixm-mod/airportheliport#AircraftStand"/>
        <rdfs:range rdf:resource="http://www.project-best.eu/owl/aixm-mod/airportheliport#AircraftStandContamination"/>
    </owl:ObjectProperty>
    


    <!-- http://www.project-best.eu/owl/aixm-mod/airportheliport#AircraftStand-extent -->

    <owl:ObjectProperty rdf:about="http://www.project-best.eu/owl/aixm-mod/airportheliport#AircraftStand-extent">
        <rdfs:comment xml:lang="en">Association to Geometry::ElevatedSurface</rdfs:comment>
        <rdfs:comment xml:lang="en">Identifies the surface area of the Gate Stand.</rdfs:comment>
        <rdfs:domain rdf:resource="http://www.project-best.eu/owl/aixm-mod/airportheliport#AircraftStand"/>
    </owl:ObjectProperty>
    


    <!-- http://www.project-best.eu/owl/aixm-mod/airportheliport#AircraftStand-location -->

    <owl:ObjectProperty rdf:about="http://www.project-best.eu/owl/aixm-mod/airportheliport#AircraftStand-location">
        <rdfs:comment xml:lang="en">Association to Geometry::ElevatedPoint</rdfs:comment>
        <rdfs:comment xml:lang="en">The geographical reference position for the parking position.</rdfs:comment>
        <rdfs:domain rdf:resource="http://www.project-best.eu/owl/aixm-mod/airportheliport#AircraftStand"/>
    </owl:ObjectProperty>
    


    <!-- http://www.project-best.eu/owl/aixm-mod/airportheliport#AircraftStand-surfaceProperties -->

    <owl:ObjectProperty rdf:about="http://www.project-best.eu/owl/aixm-mod/airportheliport#AircraftStand-surfaceProperties">
        <rdfs:comment xml:lang="en">Identifies the Surface Characteristics for which the Gate Stand is described by.</rdfs:comment>
        <rdfs:domain rdf:resource="http://www.project-best.eu/owl/aixm-mod/airportheliport#AircraftStand"/>
        <rdfs:range rdf:resource="http://www.project-best.eu/owl/aixm-mod/airportheliport#SurfaceCharacteristics"/>
    </owl:ObjectProperty>
    


    <!-- http://www.project-best.eu/owl/aixm-mod/airportheliport#AircraftStand-type -->

    <owl:ObjectProperty rdf:about="http://www.project-best.eu/owl/aixm-mod/airportheliport#AircraftStand-type">
        <rdfs:comment xml:lang="en">A code identifying the characteristics of a stand. Examples: parking position on the apron, isolated aircraft stand, terminal building gate.</rdfs:comment>
        <rdfs:domain rdf:resource="http://www.project-best.eu/owl/aixm-mod/airportheliport#AircraftStand"/>
        <rdfs:range rdf:resource="http://www.project-best.eu/owl/aixm-mod/airportheliport#CodeAircraftStandType"/>
    </owl:ObjectProperty>
    


    <!-- http://www.project-best.eu/owl/aixm-mod/airportheliport#AircraftStand-visualDockingSystem -->

    <owl:ObjectProperty rdf:about="http://www.project-best.eu/owl/aixm-mod/airportheliport#AircraftStand-visualDockingSystem">
        <rdfs:comment xml:lang="en">A device used at the aircraft stands in order to help the pilot align and position the aircraft.</rdfs:comment>
        <rdfs:domain rdf:resource="http://www.project-best.eu/owl/aixm-mod/airportheliport#AircraftStand"/>
        <rdfs:range rdf:resource="http://www.project-best.eu/owl/aixm-mod/airportheliport#CodeVisualDockingGuidanceType"/>
    </owl:ObjectProperty>
    


    <!-- http://www.project-best.eu/owl/aixm-mod/airportheliport#AirportHeliport-ARP -->

    <owl:ObjectProperty rdf:about="http://www.project-best.eu/owl/aixm-mod/airportheliport#AirportHeliport-ARP">
        <rdfs:comment xml:lang="en">Association to Geometry::ElevatedPoint</rdfs:comment>
        <rdfs:comment xml:lang="en">Identifies the Airport Reference Point.</rdfs:comment>
        <rdfs:domain rdf:resource="http://www.project-best.eu/owl/aixm-mod/airportheliport#AirportHeliport"/>
    </owl:ObjectProperty>
    


    <!-- http://www.project-best.eu/owl/aixm-mod/airportheliport#AirportHeliport-altimeterSource -->

    <owl:ObjectProperty rdf:about="http://www.project-best.eu/owl/aixm-mod/airportheliport#AirportHeliport-altimeterSource">
        <rdfs:comment xml:lang="en">Indicates the Altimeter Source(s) located at a particular AirportHeliport.</rdfs:comment>
        <rdfs:domain rdf:resource="http://www.project-best.eu/owl/aixm-mod/airportheliport#AirportHeliport"/>
        <rdfs:range rdf:resource="http://www.project-best.eu/owl/aixm-mod/airportheliport#AltimeterSource"/>
    </owl:ObjectProperty>
    


    <!-- http://www.project-best.eu/owl/aixm-mod/airportheliport#AirportHeliport-availability -->

    <owl:ObjectProperty rdf:about="http://www.project-best.eu/owl/aixm-mod/airportheliport#AirportHeliport-availability">
        <rdfs:domain rdf:resource="http://www.project-best.eu/owl/aixm-mod/airportheliport#AirportHeliport"/>
        <rdfs:range rdf:resource="http://www.project-best.eu/owl/aixm-mod/airportheliport#AirportHeliportAvailability"/>
    </owl:ObjectProperty>
    


    <!-- http://www.project-best.eu/owl/aixm-mod/airportheliport#AirportHeliport-aviationBoundary -->

    <owl:ObjectProperty rdf:about="http://www.project-best.eu/owl/aixm-mod/airportheliport#AirportHeliport-aviationBoundary">
        <rdfs:comment xml:lang="en">Association to Geometry::ElevatedSurface</rdfs:comment>
        <rdfs:comment xml:lang="en">Defines the Airport boundaries.</rdfs:comment>
        <rdfs:domain rdf:resource="http://www.project-best.eu/owl/aixm-mod/airportheliport#AirportHeliport"/>
    </owl:ObjectProperty>
    


    <!-- http://www.project-best.eu/owl/aixm-mod/airportheliport#AirportHeliport-contact -->

    <owl:ObjectProperty rdf:about="http://www.project-best.eu/owl/aixm-mod/airportheliport#AirportHeliport-contact">
        <rdfs:comment xml:lang="en">Association to Shared::Address::ContactInformation</rdfs:comment>
        <rdfs:comment xml:lang="en">Identifies the Airport Contact.</rdfs:comment>
        <rdfs:domain rdf:resource="http://www.project-best.eu/owl/aixm-mod/airportheliport#AirportHeliport"/>
    </owl:ObjectProperty>
    


    <!-- http://www.project-best.eu/owl/aixm-mod/airportheliport#AirportHeliport-contaminant -->

    <owl:ObjectProperty rdf:about="http://www.project-best.eu/owl/aixm-mod/airportheliport#AirportHeliport-contaminant">
        <rdfs:domain rdf:resource="http://www.project-best.eu/owl/aixm-mod/airportheliport#AirportHeliport"/>
        <rdfs:range rdf:resource="http://www.project-best.eu/owl/aixm-mod/airportheliport#AirportHeliportContamination"/>
    </owl:ObjectProperty>
    


    <!-- http://www.project-best.eu/owl/aixm-mod/airportheliport#AirportHeliport-controlType -->

    <owl:ObjectProperty rdf:about="http://www.project-best.eu/owl/aixm-mod/airportheliport#AirportHeliport-controlType">
        <rdfs:comment xml:lang="en">The primary organization type in terms of civil or military, which controls the airport.</rdfs:comment>
        <rdfs:domain rdf:resource="http://www.project-best.eu/owl/aixm-mod/airportheliport#AirportHeliport"/>
        <rdfs:range rdf:resource="http://www.project-best.eu/owl/aixm-mod/airportheliport#CodeMilitaryOperationsType"/>
    </owl:ObjectProperty>
    


    <!-- http://www.project-best.eu/owl/aixm-mod/airportheliport#AirportHeliport-responsibleOrganisation -->

    <owl:ObjectProperty rdf:about="http://www.project-best.eu/owl/aixm-mod/airportheliport#AirportHeliport-responsibleOrganisation">
        <rdfs:comment xml:lang="en">Association to Organisation::OrganisationAuthority</rdfs:comment>
        <rdfs:domain rdf:resource="http://www.project-best.eu/owl/aixm-mod/airportheliport#AirportHeliport"/>
    </owl:ObjectProperty>
    


    <!-- http://www.project-best.eu/owl/aixm-mod/airportheliport#AirportHeliport-servedCity -->

    <owl:ObjectProperty rdf:about="http://www.project-best.eu/owl/aixm-mod/airportheliport#AirportHeliport-servedCity">
        <rdfs:comment xml:lang="en">Identifies the Cities that the Airport serves.</rdfs:comment>
        <rdfs:domain rdf:resource="http://www.project-best.eu/owl/aixm-mod/airportheliport#AirportHeliport"/>
        <rdfs:range rdf:resource="http://www.project-best.eu/owl/aixm-mod/airportheliport#City"/>
    </owl:ObjectProperty>
    


    <!-- http://www.project-best.eu/owl/aixm-mod/airportheliport#AirportHeliportAvailability-operationalStatus -->

    <owl:ObjectProperty rdf:about="http://www.project-best.eu/owl/aixm-mod/airportheliport#AirportHeliportAvailability-operationalStatus">
        <rdfs:comment xml:lang="en">Indicates the availability of the facility for specific flight operations.</rdfs:comment>
        <rdfs:domain rdf:resource="http://www.project-best.eu/owl/aixm-mod/airportheliport#AirportHeliportAvailability"/>
        <rdfs:range rdf:resource="http://www.project-best.eu/owl/aixm-mod/airportheliport#CodeStatusAirportType"/>
    </owl:ObjectProperty>
    


    <!-- http://www.project-best.eu/owl/aixm-mod/airportheliport#AirportHeliportAvailability-usage -->

    <owl:ObjectProperty rdf:about="http://www.project-best.eu/owl/aixm-mod/airportheliport#AirportHeliportAvailability-usage">
        <rdfs:domain rdf:resource="http://www.project-best.eu/owl/aixm-mod/airportheliport#AirportHeliportAvailability"/>
        <rdfs:range rdf:resource="http://www.project-best.eu/owl/aixm-mod/airportheliport#AirportHeliportUsage"/>
    </owl:ObjectProperty>
    


    <!-- http://www.project-best.eu/owl/aixm-mod/airportheliport#AirportHeliportAvailability-warning -->

    <owl:ObjectProperty rdf:about="http://www.project-best.eu/owl/aixm-mod/airportheliport#AirportHeliportAvailability-warning">
        <rdfs:comment xml:lang="en">A reason for caution when operating at the facility.</rdfs:comment>
        <rdfs:domain rdf:resource="http://www.project-best.eu/owl/aixm-mod/airportheliport#AirportHeliportAvailability"/>
        <rdfs:range rdf:resource="http://www.project-best.eu/owl/aixm-mod/airportheliport#CodeAirportWarningType"/>
    </owl:ObjectProperty>
    


    <!-- http://www.project-best.eu/owl/aixm-mod/airportheliport#AirportHeliportCollocation-dependentAirport -->

    <owl:ObjectProperty rdf:about="http://www.project-best.eu/owl/aixm-mod/airportheliport#AirportHeliportCollocation-dependentAirport">
        <rdfs:comment xml:lang="en">This is the dependant airport which is using the facilities of the host airport.</rdfs:comment>
        <rdfs:range rdf:resource="http://www.project-best.eu/owl/aixm-mod/airportheliport#AirportHeliport"/>
        <rdfs:domain rdf:resource="http://www.project-best.eu/owl/aixm-mod/airportheliport#AirportHeliportCollocation"/>
    </owl:ObjectProperty>
    


    <!-- http://www.project-best.eu/owl/aixm-mod/airportheliport#AirportHeliportCollocation-hostAirport -->

    <owl:ObjectProperty rdf:about="http://www.project-best.eu/owl/aixm-mod/airportheliport#AirportHeliportCollocation-hostAirport">
        <rdfs:comment xml:lang="en">This is the main aerodrome.</rdfs:comment>
        <rdfs:range rdf:resource="http://www.project-best.eu/owl/aixm-mod/airportheliport#AirportHeliport"/>
        <rdfs:domain rdf:resource="http://www.project-best.eu/owl/aixm-mod/airportheliport#AirportHeliportCollocation"/>
    </owl:ObjectProperty>
    


    <!-- http://www.project-best.eu/owl/aixm-mod/airportheliport#AirportHeliportCollocation-type -->

    <owl:ObjectProperty rdf:about="http://www.project-best.eu/owl/aixm-mod/airportheliport#AirportHeliportCollocation-type">
        <rdfs:comment xml:lang="en">A code indicating the extent of the collocation situation of the two aerodrome/heliports.</rdfs:comment>
        <rdfs:domain rdf:resource="http://www.project-best.eu/owl/aixm-mod/airportheliport#AirportHeliportCollocation"/>
        <rdfs:range rdf:resource="http://www.project-best.eu/owl/aixm-mod/airportheliport#CodeAirportHeliportCollocationType"/>
    </owl:ObjectProperty>
    


    <!-- http://www.project-best.eu/owl/aixm-mod/airportheliport#AirportHeliportProtectionArea-extent -->

    <owl:ObjectProperty rdf:about="http://www.project-best.eu/owl/aixm-mod/airportheliport#AirportHeliportProtectionArea-extent">
        <rdfs:comment xml:lang="en">Association to Geometry::ElevatedSurface
</rdfs:comment>
        <rdfs:comment xml:lang="en">Identifies the surface area of the Airport Heliport Protection Area.</rdfs:comment>
        <rdfs:domain rdf:resource="http://www.project-best.eu/owl/aixm-mod/airportheliport#AirportHeliportProtectionArea"/>
    </owl:ObjectProperty>
    


    <!-- http://www.project-best.eu/owl/aixm-mod/airportheliport#AirportHeliportProtectionArea-surfaceProperties -->

    <owl:ObjectProperty rdf:about="http://www.project-best.eu/owl/aixm-mod/airportheliport#AirportHeliportProtectionArea-surfaceProperties">
        <rdfs:comment xml:lang="en">Identifies the Surface Characteristics that describe the Airport Heliport Protection Area.</rdfs:comment>
        <rdfs:domain rdf:resource="http://www.project-best.eu/owl/aixm-mod/airportheliport#AirportHeliportProtectionArea"/>
        <rdfs:range rdf:resource="http://www.project-best.eu/owl/aixm-mod/airportheliport#SurfaceCharacteristics"/>
    </owl:ObjectProperty>
    


    <!-- http://www.project-best.eu/owl/aixm-mod/airportheliport#AirportHeliportResponsibilityOrganisation-role -->

    <owl:ObjectProperty rdf:about="http://www.project-best.eu/owl/aixm-mod/airportheliport#AirportHeliportResponsibilityOrganisation-role">
        <rdfs:comment xml:lang="en">An indication of the responsibility that the Organization or Authority has over the facility.</rdfs:comment>
        <rdfs:domain rdf:resource="http://www.project-best.eu/owl/aixm-mod/airportheliport#AirportHeliportResponsibilityOrganisation"/>
        <rdfs:range rdf:resource="http://www.project-best.eu/owl/aixm-mod/airportheliport#CodeAuthorityRoleType"/>
    </owl:ObjectProperty>
    


    <!-- http://www.project-best.eu/owl/aixm-mod/airportheliport#AirportHeliportUsage-operation -->

    <owl:ObjectProperty rdf:about="http://www.project-best.eu/owl/aixm-mod/airportheliport#AirportHeliportUsage-operation">
        <rdfs:comment xml:lang="en">A type of activity for which a usage rule is specified.</rdfs:comment>
        <rdfs:domain rdf:resource="http://www.project-best.eu/owl/aixm-mod/airportheliport#AirportHeliportUsage"/>
        <rdfs:range rdf:resource="http://www.project-best.eu/owl/aixm-mod/airportheliport#CodeOperationAirportHeliportType"/>
    </owl:ObjectProperty>
    


    <!-- http://www.project-best.eu/owl/aixm-mod/airportheliport#AirportHotSpot-affectedAirport -->

    <owl:ObjectProperty rdf:about="http://www.project-best.eu/owl/aixm-mod/airportheliport#AirportHotSpot-affectedAirport">
        <rdfs:comment xml:lang="en">The AirportHeliport where the hot spot has been identified.</rdfs:comment>
        <rdfs:range rdf:resource="http://www.project-best.eu/owl/aixm-mod/airportheliport#AirportHeliport"/>
        <rdfs:domain rdf:resource="http://www.project-best.eu/owl/aixm-mod/airportheliport#AirportHotSpot"/>
    </owl:ObjectProperty>
    


    <!-- http://www.project-best.eu/owl/aixm-mod/airportheliport#AirportHotSpot-area -->

    <owl:ObjectProperty rdf:about="http://www.project-best.eu/owl/aixm-mod/airportheliport#AirportHotSpot-area">
        <rdfs:comment xml:lang="en">Association to Geometry::ElevatedSurface</rdfs:comment>
        <rdfs:comment xml:lang="en">The area on the airport/heliport that has been identified as a hot spot</rdfs:comment>
        <rdfs:domain rdf:resource="http://www.project-best.eu/owl/aixm-mod/airportheliport#AirportHotSpot"/>
    </owl:ObjectProperty>
    


    <!-- http://www.project-best.eu/owl/aixm-mod/airportheliport#AirportProtectionAreaMarking-markedProtectionArea -->

    <owl:ObjectProperty rdf:about="http://www.project-best.eu/owl/aixm-mod/airportheliport#AirportProtectionAreaMarking-markedProtectionArea">
        <rdfs:comment xml:lang="en">Identifies the Airport Heliport Protection Area that is marked.</rdfs:comment>
        <rdfs:range rdf:resource="http://www.project-best.eu/owl/aixm-mod/airportheliport#AirportHeliportProtectionArea"/>
        <rdfs:domain rdf:resource="http://www.project-best.eu/owl/aixm-mod/airportheliport#AirportProtectionAreaMarking"/>
    </owl:ObjectProperty>
    


    <!-- http://www.project-best.eu/owl/aixm-mod/airportheliport#AirportProtectionAreaMarking-markingLocation -->

    <owl:ObjectProperty rdf:about="http://www.project-best.eu/owl/aixm-mod/airportheliport#AirportProtectionAreaMarking-markingLocation">
        <rdfs:comment xml:lang="en">The location of the marking.</rdfs:comment>
        <rdfs:domain rdf:resource="http://www.project-best.eu/owl/aixm-mod/airportheliport#AirportProtectionAreaMarking"/>
        <rdfs:range rdf:resource="http://www.project-best.eu/owl/aixm-mod/airportheliport#CodeProtectAreaSectionType"/>
    </owl:ObjectProperty>
    


    <!-- http://www.project-best.eu/owl/aixm-mod/airportheliport#AltimeterSource-availability -->

    <owl:ObjectProperty rdf:about="http://www.project-best.eu/owl/aixm-mod/airportheliport#AltimeterSource-availability">
        <rdfs:domain rdf:resource="http://www.project-best.eu/owl/aixm-mod/airportheliport#AltimeterSource"/>
        <rdfs:range rdf:resource="http://www.project-best.eu/owl/aixm-mod/airportheliport#AltimeterSourceStatus"/>
    </owl:ObjectProperty>
    


    <!-- http://www.project-best.eu/owl/aixm-mod/airportheliport#AltimeterSourceStatus-operationalStatus -->

    <owl:ObjectProperty rdf:about="http://www.project-best.eu/owl/aixm-mod/airportheliport#AltimeterSourceStatus-operationalStatus">
        <rdfs:comment xml:lang="en">Operational status.</rdfs:comment>
        <rdfs:domain rdf:resource="http://www.project-best.eu/owl/aixm-mod/airportheliport#AltimeterSourceStatus"/>
        <rdfs:range rdf:resource="http://www.project-best.eu/owl/aixm-mod/airportheliport#CodeStatusOperationsType"/>
    </owl:ObjectProperty>
    


    <!-- http://www.project-best.eu/owl/aixm-mod/airportheliport#ApproachLightingSystem-classICAO -->

    <owl:ObjectProperty rdf:about="http://www.project-best.eu/owl/aixm-mod/airportheliport#ApproachLightingSystem-classICAO">
        <rdfs:comment xml:lang="en">Classification of the approach lighting system using as criteria the ICAO Annex 14 standards and recommended practices</rdfs:comment>
        <rdfs:domain rdf:resource="http://www.project-best.eu/owl/aixm-mod/airportheliport#ApproachLightingSystem"/>
        <rdfs:range rdf:resource="http://www.project-best.eu/owl/aixm-mod/airportheliport#CodeApproachLightingICAOType"/>
    </owl:ObjectProperty>
    


    <!-- http://www.project-best.eu/owl/aixm-mod/airportheliport#ApproachLightingSystem-servedRunwayDirection -->

    <owl:ObjectProperty rdf:about="http://www.project-best.eu/owl/aixm-mod/airportheliport#ApproachLightingSystem-servedRunwayDirection">
        <rdfs:comment xml:lang="en">Identifies the Runway Direction that the ALS serves.</rdfs:comment>
        <rdfs:domain rdf:resource="http://www.project-best.eu/owl/aixm-mod/airportheliport#ApproachLightingSystem"/>
        <rdfs:range rdf:resource="http://www.project-best.eu/owl/aixm-mod/airportheliport#RunwayDirection"/>
    </owl:ObjectProperty>
    


    <!-- http://www.project-best.eu/owl/aixm-mod/airportheliport#ApproachLightingSystem-type -->

    <owl:ObjectProperty rdf:about="http://www.project-best.eu/owl/aixm-mod/airportheliport#ApproachLightingSystem-type">
        <rdfs:comment xml:lang="en">A regional or organisation specific classification of the approach lighting system equipment. Could also be a brand name</rdfs:comment>
        <rdfs:domain rdf:resource="http://www.project-best.eu/owl/aixm-mod/airportheliport#ApproachLightingSystem"/>
        <rdfs:range rdf:resource="http://www.project-best.eu/owl/aixm-mod/airportheliport#CodeApproachLightingType"/>
    </owl:ObjectProperty>
    


    <!-- http://www.project-best.eu/owl/aixm-mod/airportheliport#Apron-associatedAirportHeliport -->

    <owl:ObjectProperty rdf:about="http://www.project-best.eu/owl/aixm-mod/airportheliport#Apron-associatedAirportHeliport">
        <rdfs:comment xml:lang="en">Identifies the Airport where the Apron is situated.</rdfs:comment>
        <rdfs:range rdf:resource="http://www.project-best.eu/owl/aixm-mod/airportheliport#AirportHeliport"/>
        <rdfs:domain rdf:resource="http://www.project-best.eu/owl/aixm-mod/airportheliport#Apron"/>
    </owl:ObjectProperty>
    


    <!-- http://www.project-best.eu/owl/aixm-mod/airportheliport#Apron-availability -->

    <owl:ObjectProperty rdf:about="http://www.project-best.eu/owl/aixm-mod/airportheliport#Apron-availability">
        <rdfs:domain rdf:resource="http://www.project-best.eu/owl/aixm-mod/airportheliport#Apron"/>
        <rdfs:range rdf:resource="http://www.project-best.eu/owl/aixm-mod/airportheliport#ApronAreaAvailability"/>
    </owl:ObjectProperty>
    


    <!-- http://www.project-best.eu/owl/aixm-mod/airportheliport#Apron-contaminant -->

    <owl:ObjectProperty rdf:about="http://www.project-best.eu/owl/aixm-mod/airportheliport#Apron-contaminant">
        <rdfs:comment xml:lang="en">Identifies the contaminant of the apron.</rdfs:comment>
        <rdfs:domain rdf:resource="http://www.project-best.eu/owl/aixm-mod/airportheliport#Apron"/>
        <rdfs:range rdf:resource="http://www.project-best.eu/owl/aixm-mod/airportheliport#ApronContamination"/>
    </owl:ObjectProperty>
    


    <!-- http://www.project-best.eu/owl/aixm-mod/airportheliport#Apron-surfaceProperties -->

    <owl:ObjectProperty rdf:about="http://www.project-best.eu/owl/aixm-mod/airportheliport#Apron-surfaceProperties">
        <rdfs:comment xml:lang="en">Identifies the surface characteristics of which the Apron is described by.</rdfs:comment>
        <rdfs:domain rdf:resource="http://www.project-best.eu/owl/aixm-mod/airportheliport#Apron"/>
        <rdfs:range rdf:resource="http://www.project-best.eu/owl/aixm-mod/airportheliport#SurfaceCharacteristics"/>
    </owl:ObjectProperty>
    


    <!-- http://www.project-best.eu/owl/aixm-mod/airportheliport#ApronAreaAvailability-operationalStatus -->

    <owl:ObjectProperty rdf:about="http://www.project-best.eu/owl/aixm-mod/airportheliport#ApronAreaAvailability-operationalStatus">
        <rdfs:comment xml:lang="en">Indicates the availability of the facility for specific flight operations.</rdfs:comment>
        <rdfs:domain rdf:resource="http://www.project-best.eu/owl/aixm-mod/airportheliport#ApronAreaAvailability"/>
        <rdfs:range rdf:resource="http://www.project-best.eu/owl/aixm-mod/airportheliport#CodeStatusAirportType"/>
    </owl:ObjectProperty>
    


    <!-- http://www.project-best.eu/owl/aixm-mod/airportheliport#ApronAreaAvailability-usage -->

    <owl:ObjectProperty rdf:about="http://www.project-best.eu/owl/aixm-mod/airportheliport#ApronAreaAvailability-usage">
        <rdfs:domain rdf:resource="http://www.project-best.eu/owl/aixm-mod/airportheliport#ApronAreaAvailability"/>
        <rdfs:range rdf:resource="http://www.project-best.eu/owl/aixm-mod/airportheliport#ApronAreaUsage"/>
    </owl:ObjectProperty>
    


    <!-- http://www.project-best.eu/owl/aixm-mod/airportheliport#ApronAreaAvailability-warning -->

    <owl:ObjectProperty rdf:about="http://www.project-best.eu/owl/aixm-mod/airportheliport#ApronAreaAvailability-warning">
        <rdfs:comment xml:lang="en">A reason for caution when operating at the facility.</rdfs:comment>
        <rdfs:domain rdf:resource="http://www.project-best.eu/owl/aixm-mod/airportheliport#ApronAreaAvailability"/>
        <rdfs:range rdf:resource="http://www.project-best.eu/owl/aixm-mod/airportheliport#CodeAirportWarningType"/>
    </owl:ObjectProperty>
    


    <!-- http://www.project-best.eu/owl/aixm-mod/airportheliport#ApronElement-associatedApron -->

    <owl:ObjectProperty rdf:about="http://www.project-best.eu/owl/aixm-mod/airportheliport#ApronElement-associatedApron">
        <rdfs:comment xml:lang="en">(DO272/ED99) The value of a ParkingStandArea feature?s attribute idapron shall be identical to the value of the operationally corresponding ApronElement feature?s attribute idapron (Rule 23).</rdfs:comment>
        <rdfs:range rdf:resource="http://www.project-best.eu/owl/aixm-mod/airportheliport#Apron"/>
        <rdfs:domain rdf:resource="http://www.project-best.eu/owl/aixm-mod/airportheliport#ApronElement"/>
    </owl:ObjectProperty>
    


    <!-- http://www.project-best.eu/owl/aixm-mod/airportheliport#ApronElement-availability -->

    <owl:ObjectProperty rdf:about="http://www.project-best.eu/owl/aixm-mod/airportheliport#ApronElement-availability">
        <rdfs:range rdf:resource="http://www.project-best.eu/owl/aixm-mod/airportheliport#ApronAreaAvailability"/>
        <rdfs:domain rdf:resource="http://www.project-best.eu/owl/aixm-mod/airportheliport#ApronElement"/>
    </owl:ObjectProperty>
    


    <!-- http://www.project-best.eu/owl/aixm-mod/airportheliport#ApronElement-extent -->

    <owl:ObjectProperty rdf:about="http://www.project-best.eu/owl/aixm-mod/airportheliport#ApronElement-extent">
        <rdfs:comment xml:lang="en">Association to Geometry::ElevatedSurface</rdfs:comment>
        <rdfs:comment xml:lang="en">Identifies the extent of the apron element.</rdfs:comment>
        <rdfs:domain rdf:resource="http://www.project-best.eu/owl/aixm-mod/airportheliport#ApronElement"/>
    </owl:ObjectProperty>
    


    <!-- http://www.project-best.eu/owl/aixm-mod/airportheliport#ApronElement-surfaceProperties -->

    <owl:ObjectProperty rdf:about="http://www.project-best.eu/owl/aixm-mod/airportheliport#ApronElement-surfaceProperties">
        <rdfs:comment xml:lang="en">Identifies the surface characteristics of which the Apron Element is described by.</rdfs:comment>
        <rdfs:domain rdf:resource="http://www.project-best.eu/owl/aixm-mod/airportheliport#ApronElement"/>
        <rdfs:range rdf:resource="http://www.project-best.eu/owl/aixm-mod/airportheliport#SurfaceCharacteristics"/>
    </owl:ObjectProperty>
    


    <!-- http://www.project-best.eu/owl/aixm-mod/airportheliport#ApronElement-type -->

    <owl:ObjectProperty rdf:about="http://www.project-best.eu/owl/aixm-mod/airportheliport#ApronElement-type">
        <rdfs:comment xml:lang="en">The type of an apron based upon its location on an aerodrome and its general purpose.</rdfs:comment>
        <rdfs:domain rdf:resource="http://www.project-best.eu/owl/aixm-mod/airportheliport#ApronElement"/>
        <rdfs:range rdf:resource="http://www.project-best.eu/owl/aixm-mod/airportheliport#CodeApronElementType"/>
    </owl:ObjectProperty>
    


    <!-- http://www.project-best.eu/owl/aixm-mod/airportheliport#ApronLightSystem-lightedApron -->

    <owl:ObjectProperty rdf:about="http://www.project-best.eu/owl/aixm-mod/airportheliport#ApronLightSystem-lightedApron">
        <rdfs:comment xml:lang="en">Identifies the Apron for which the Lighting System is provided.</rdfs:comment>
        <rdfs:range rdf:resource="http://www.project-best.eu/owl/aixm-mod/airportheliport#Apron"/>
        <rdfs:domain rdf:resource="http://www.project-best.eu/owl/aixm-mod/airportheliport#ApronLightSystem"/>
    </owl:ObjectProperty>
    


    <!-- http://www.project-best.eu/owl/aixm-mod/airportheliport#ApronLightSystem-position -->

    <owl:ObjectProperty rdf:about="http://www.project-best.eu/owl/aixm-mod/airportheliport#ApronLightSystem-position">
        <rdfs:comment xml:lang="en">A code indicating the part of the apron served by the lighting system.</rdfs:comment>
        <rdfs:domain rdf:resource="http://www.project-best.eu/owl/aixm-mod/airportheliport#ApronLightSystem"/>
        <rdfs:range rdf:resource="http://www.project-best.eu/owl/aixm-mod/airportheliport#CodeApronSectionType"/>
    </owl:ObjectProperty>
    


    <!-- http://www.project-best.eu/owl/aixm-mod/airportheliport#ApronMarking-markedApron -->

    <owl:ObjectProperty rdf:about="http://www.project-best.eu/owl/aixm-mod/airportheliport#ApronMarking-markedApron">
        <rdfs:comment xml:lang="en">Identifies the Apron on which the Apron Marking is marked.</rdfs:comment>
        <rdfs:range rdf:resource="http://www.project-best.eu/owl/aixm-mod/airportheliport#Apron"/>
        <rdfs:domain rdf:resource="http://www.project-best.eu/owl/aixm-mod/airportheliport#ApronMarking"/>
    </owl:ObjectProperty>
    


    <!-- http://www.project-best.eu/owl/aixm-mod/airportheliport#ApronMarking-markingLocation -->

    <owl:ObjectProperty rdf:about="http://www.project-best.eu/owl/aixm-mod/airportheliport#ApronMarking-markingLocation">
        <rdfs:comment xml:lang="en">A code indicating the location of the marking relative to the surface.</rdfs:comment>
        <rdfs:domain rdf:resource="http://www.project-best.eu/owl/aixm-mod/airportheliport#ApronMarking"/>
        <rdfs:range rdf:resource="http://www.project-best.eu/owl/aixm-mod/airportheliport#CodeApronSectionType"/>
    </owl:ObjectProperty>
    


    <!-- http://www.project-best.eu/owl/aixm-mod/airportheliport#ArrestingGear-absorbType -->

    <owl:ObjectProperty rdf:about="http://www.project-best.eu/owl/aixm-mod/airportheliport#ArrestingGear-absorbType">
        <rdfs:comment xml:lang="en">The type of energy absorber (for example: a rotary brake) by which the arresting gear system rapidly dissipates the kinetic energy of a moving aircraft that engages the arresting system, bringing the aircraft to a stop.</rdfs:comment>
        <rdfs:domain rdf:resource="http://www.project-best.eu/owl/aixm-mod/airportheliport#ArrestingGear"/>
        <rdfs:range rdf:resource="http://www.project-best.eu/owl/aixm-mod/airportheliport#CodeArrestingGearEnergyAbsorbType"/>
    </owl:ObjectProperty>
    


    <!-- http://www.project-best.eu/owl/aixm-mod/airportheliport#ArrestingGear-engageDevice -->

    <owl:ObjectProperty rdf:about="http://www.project-best.eu/owl/aixm-mod/airportheliport#ArrestingGear-engageDevice">
        <rdfs:comment xml:lang="en">The type of device (for example: a hook) that is used to engage an aircraft upon landing in order to immediately stop it.</rdfs:comment>
        <rdfs:domain rdf:resource="http://www.project-best.eu/owl/aixm-mod/airportheliport#ArrestingGear"/>
        <rdfs:range rdf:resource="http://www.project-best.eu/owl/aixm-mod/airportheliport#CodeArrestingGearEngageDeviceType"/>
    </owl:ObjectProperty>
    


    <!-- http://www.project-best.eu/owl/aixm-mod/airportheliport#ArrestingGear-extent -->

    <owl:ObjectProperty rdf:about="http://www.project-best.eu/owl/aixm-mod/airportheliport#ArrestingGear-extent">
        <rdfs:comment xml:lang="en">Identifies the shape of the arresting gear.</rdfs:comment>
        <rdfs:domain rdf:resource="http://www.project-best.eu/owl/aixm-mod/airportheliport#ArrestingGear"/>
        <rdfs:range rdf:resource="http://www.project-best.eu/owl/aixm-mod/airportheliport#ArrestingGearExtent"/>
    </owl:ObjectProperty>
    


    <!-- http://www.project-best.eu/owl/aixm-mod/airportheliport#ArrestingGear-runwayDirection -->

    <owl:ObjectProperty rdf:about="http://www.project-best.eu/owl/aixm-mod/airportheliport#ArrestingGear-runwayDirection">
        <rdfs:comment xml:lang="en">Identifies the runway direction on which the arresting gear is used.</rdfs:comment>
        <rdfs:domain rdf:resource="http://www.project-best.eu/owl/aixm-mod/airportheliport#ArrestingGear"/>
        <rdfs:range rdf:resource="http://www.project-best.eu/owl/aixm-mod/airportheliport#RunwayDirection"/>
    </owl:ObjectProperty>
    


    <!-- http://www.project-best.eu/owl/aixm-mod/airportheliport#ArrestingGear-status -->

    <owl:ObjectProperty rdf:about="http://www.project-best.eu/owl/aixm-mod/airportheliport#ArrestingGear-status">
        <rdfs:comment xml:lang="en">The operational status of the arresting gear device.</rdfs:comment>
        <rdfs:domain rdf:resource="http://www.project-best.eu/owl/aixm-mod/airportheliport#ArrestingGear"/>
        <rdfs:range rdf:resource="http://www.project-best.eu/owl/aixm-mod/airportheliport#CodeStatusOperationsType"/>
    </owl:ObjectProperty>
    


    <!-- http://www.project-best.eu/owl/aixm-mod/airportheliport#ArrestingGear-surfaceProperties -->

    <owl:ObjectProperty rdf:about="http://www.project-best.eu/owl/aixm-mod/airportheliport#ArrestingGear-surfaceProperties">
        <rdfs:comment xml:lang="en">Describes the surface characteristics of the arresting gear.</rdfs:comment>
        <rdfs:domain rdf:resource="http://www.project-best.eu/owl/aixm-mod/airportheliport#ArrestingGear"/>
        <rdfs:range rdf:resource="http://www.project-best.eu/owl/aixm-mod/airportheliport#SurfaceCharacteristics"/>
    </owl:ObjectProperty>
    


    <!-- http://www.project-best.eu/owl/aixm-mod/airportheliport#ArrestingGearExtent-surfaceExtent -->

    <owl:ObjectProperty rdf:about="http://www.project-best.eu/owl/aixm-mod/airportheliport#ArrestingGearExtent-surfaceExtent">
        <rdfs:comment xml:lang="en">Association to Geometry::ElevatedSurface</rdfs:comment>
        <rdfs:comment xml:lang="en">Identifies the polygon of the arresting gear extent.</rdfs:comment>
        <rdfs:domain rdf:resource="http://www.project-best.eu/owl/aixm-mod/airportheliport#ArrestingGearExtent"/>
    </owl:ObjectProperty>
    


    <!-- http://www.project-best.eu/owl/aixm-mod/airportheliport#ConditionCombination-logicalOperator -->

    <owl:ObjectProperty rdf:about="http://www.project-best.eu/owl/aixm-mod/airportheliport#ConditionCombination-logicalOperator">
        <rdfs:comment xml:lang="en">The type of operation combining an elementary condition or a previously defined combination with other elementary conditions or previously defined combinations.</rdfs:comment>
        <rdfs:range rdf:resource="http://www.project-best.eu/owl/aixm-mod/airportheliport#CodeLogicalOperatorType"/>
        <rdfs:domain rdf:resource="http://www.project-best.eu/owl/aixm-mod/airportheliport#ConditionCombination"/>
    </owl:ObjectProperty>
    


    <!-- http://www.project-best.eu/owl/aixm-mod/airportheliport#ConditionCombination-subCondition -->

    <owl:ObjectProperty rdf:about="http://www.project-best.eu/owl/aixm-mod/airportheliport#ConditionCombination-subCondition">
        <rdfs:range rdf:resource="http://www.project-best.eu/owl/aixm-mod/airportheliport#ConditionCombination"/>
        <rdfs:domain rdf:resource="http://www.project-best.eu/owl/aixm-mod/airportheliport#ConditionCombination"/>
    </owl:ObjectProperty>
    


    <!-- http://www.project-best.eu/owl/aixm-mod/airportheliport#ConditionCombination-weather -->

    <owl:ObjectProperty rdf:about="http://www.project-best.eu/owl/aixm-mod/airportheliport#ConditionCombination-weather">
        <rdfs:comment xml:lang="en">Association to Meteorology::Meteorology</rdfs:comment>
        <rdfs:domain rdf:resource="http://www.project-best.eu/owl/aixm-mod/airportheliport#ConditionCombination"/>
    </owl:ObjectProperty>
    


    <!-- http://www.project-best.eu/owl/aixm-mod/airportheliport#DeicingArea-associatedApron -->

    <owl:ObjectProperty rdf:about="http://www.project-best.eu/owl/aixm-mod/airportheliport#DeicingArea-associatedApron">
        <rdfs:comment xml:lang="en">Identifies the Apron on which the Deicing Area is located on.</rdfs:comment>
        <rdfs:range rdf:resource="http://www.project-best.eu/owl/aixm-mod/airportheliport#Apron"/>
        <rdfs:domain rdf:resource="http://www.project-best.eu/owl/aixm-mod/airportheliport#DeicingArea"/>
    </owl:ObjectProperty>
    


    <!-- http://www.project-best.eu/owl/aixm-mod/airportheliport#DeicingArea-availability -->

    <owl:ObjectProperty rdf:about="http://www.project-best.eu/owl/aixm-mod/airportheliport#DeicingArea-availability">
        <rdfs:range rdf:resource="http://www.project-best.eu/owl/aixm-mod/airportheliport#ApronAreaAvailability"/>
        <rdfs:domain rdf:resource="http://www.project-best.eu/owl/aixm-mod/airportheliport#DeicingArea"/>
    </owl:ObjectProperty>
    


    <!-- http://www.project-best.eu/owl/aixm-mod/airportheliport#DeicingArea-extent -->

    <owl:ObjectProperty rdf:about="http://www.project-best.eu/owl/aixm-mod/airportheliport#DeicingArea-extent">
        <rdfs:comment xml:lang="en">Association to Geometry::ElevatedSurface</rdfs:comment>
        <rdfs:comment xml:lang="en">Identifies the extent of the deicing area.</rdfs:comment>
        <rdfs:domain rdf:resource="http://www.project-best.eu/owl/aixm-mod/airportheliport#DeicingArea"/>
    </owl:ObjectProperty>
    


    <!-- http://www.project-best.eu/owl/aixm-mod/airportheliport#DeicingArea-standLocation -->

    <owl:ObjectProperty rdf:about="http://www.project-best.eu/owl/aixm-mod/airportheliport#DeicingArea-standLocation">
        <rdfs:comment xml:lang="en">Identifies the Gate Stand at which the Deicing Area is located.</rdfs:comment>
        <rdfs:range rdf:resource="http://www.project-best.eu/owl/aixm-mod/airportheliport#AircraftStand"/>
        <rdfs:domain rdf:resource="http://www.project-best.eu/owl/aixm-mod/airportheliport#DeicingArea"/>
    </owl:ObjectProperty>
    


    <!-- http://www.project-best.eu/owl/aixm-mod/airportheliport#DeicingArea-surfaceProperties -->

    <owl:ObjectProperty rdf:about="http://www.project-best.eu/owl/aixm-mod/airportheliport#DeicingArea-surfaceProperties">
        <rdfs:comment xml:lang="en">Identifies the surface characteristics of which the Deicing Area is described by.</rdfs:comment>
        <rdfs:domain rdf:resource="http://www.project-best.eu/owl/aixm-mod/airportheliport#DeicingArea"/>
        <rdfs:range rdf:resource="http://www.project-best.eu/owl/aixm-mod/airportheliport#SurfaceCharacteristics"/>
    </owl:ObjectProperty>
    


    <!-- http://www.project-best.eu/owl/aixm-mod/airportheliport#DeicingArea-taxiwayLocation -->

    <owl:ObjectProperty rdf:about="http://www.project-best.eu/owl/aixm-mod/airportheliport#DeicingArea-taxiwayLocation">
        <rdfs:comment xml:lang="en">Identifies the taxiway where the deicing area is located.</rdfs:comment>
        <rdfs:domain rdf:resource="http://www.project-best.eu/owl/aixm-mod/airportheliport#DeicingArea"/>
        <rdfs:range rdf:resource="http://www.project-best.eu/owl/aixm-mod/airportheliport#Taxiway"/>
    </owl:ObjectProperty>
    


    <!-- http://www.project-best.eu/owl/aixm-mod/airportheliport#DeicingAreaMarking-markedDeicingArea -->

    <owl:ObjectProperty rdf:about="http://www.project-best.eu/owl/aixm-mod/airportheliport#DeicingAreaMarking-markedDeicingArea">
        <rdfs:comment xml:lang="en">Identifies the Deicing Area that is marked.</rdfs:comment>
        <rdfs:range rdf:resource="http://www.project-best.eu/owl/aixm-mod/airportheliport#DeicingArea"/>
        <rdfs:domain rdf:resource="http://www.project-best.eu/owl/aixm-mod/airportheliport#DeicingAreaMarking"/>
    </owl:ObjectProperty>
    


    <!-- http://www.project-best.eu/owl/aixm-mod/airportheliport#FloatingDockSite-extent -->

    <owl:ObjectProperty rdf:about="http://www.project-best.eu/owl/aixm-mod/airportheliport#FloatingDockSite-extent">
        <rdfs:comment xml:lang="en">Association to Geometry::ElevatedSurface</rdfs:comment>
        <rdfs:comment xml:lang="en">Identifies the extent of the floating dock site.</rdfs:comment>
        <rdfs:domain rdf:resource="http://www.project-best.eu/owl/aixm-mod/airportheliport#FloatingDockSite"/>
    </owl:ObjectProperty>
    


    <!-- http://www.project-best.eu/owl/aixm-mod/airportheliport#GroundLightSystem-availability -->

    <owl:ObjectProperty rdf:about="http://www.project-best.eu/owl/aixm-mod/airportheliport#GroundLightSystem-availability">
        <rdfs:domain rdf:resource="http://www.project-best.eu/owl/aixm-mod/airportheliport#GroundLightSystem"/>
        <rdfs:range rdf:resource="http://www.project-best.eu/owl/aixm-mod/airportheliport#GroundLightingAvailability"/>
    </owl:ObjectProperty>
    


    <!-- http://www.project-best.eu/owl/aixm-mod/airportheliport#GroundLightSystem-colour -->

    <owl:ObjectProperty rdf:about="http://www.project-best.eu/owl/aixm-mod/airportheliport#GroundLightSystem-colour">
        <rdfs:comment xml:lang="en">A code indicating the global colour of the lighting system.</rdfs:comment>
        <rdfs:range rdf:resource="http://www.project-best.eu/owl/aixm-mod/airportheliport#CodeColourType"/>
        <rdfs:domain rdf:resource="http://www.project-best.eu/owl/aixm-mod/airportheliport#GroundLightSystem"/>
    </owl:ObjectProperty>
    


    <!-- http://www.project-best.eu/owl/aixm-mod/airportheliport#GroundLightSystem-element -->

    <owl:ObjectProperty rdf:about="http://www.project-best.eu/owl/aixm-mod/airportheliport#GroundLightSystem-element">
        <rdfs:comment xml:lang="en">Association to Shared::LightElement</rdfs:comment>
        <rdfs:comment xml:lang="en">Identifies the LightElements that make up the Ground Light System</rdfs:comment>
        <rdfs:domain rdf:resource="http://www.project-best.eu/owl/aixm-mod/airportheliport#GroundLightSystem"/>
    </owl:ObjectProperty>
    


    <!-- http://www.project-best.eu/owl/aixm-mod/airportheliport#GroundLightSystem-intensityLevel -->

    <owl:ObjectProperty rdf:about="http://www.project-best.eu/owl/aixm-mod/airportheliport#GroundLightSystem-intensityLevel">
        <rdfs:comment xml:lang="en">A code indicating the relative intensity of the lighting system.</rdfs:comment>
        <rdfs:range rdf:resource="http://www.project-best.eu/owl/aixm-mod/airportheliport#CodeLightIntensityType"/>
        <rdfs:domain rdf:resource="http://www.project-best.eu/owl/aixm-mod/airportheliport#GroundLightSystem"/>
    </owl:ObjectProperty>
    


    <!-- http://www.project-best.eu/owl/aixm-mod/airportheliport#GroundLightingAvailability-operationalStatus -->

    <owl:ObjectProperty rdf:about="http://www.project-best.eu/owl/aixm-mod/airportheliport#GroundLightingAvailability-operationalStatus">
        <rdfs:comment xml:lang="en">An indication of the operational status of the lighting system. The list of values include: &quot;in construction&quot;, &quot;operational&quot;, &quot;unavailable&quot;.</rdfs:comment>
        <rdfs:range rdf:resource="http://www.project-best.eu/owl/aixm-mod/airportheliport#CodeStatusOperationsType"/>
        <rdfs:domain rdf:resource="http://www.project-best.eu/owl/aixm-mod/airportheliport#GroundLightingAvailability"/>
    </owl:ObjectProperty>
    


    <!-- http://www.project-best.eu/owl/aixm-mod/airportheliport#GuidanceLine-connectedRunwayCentrelinePoint -->

    <owl:ObjectProperty rdf:about="http://www.project-best.eu/owl/aixm-mod/airportheliport#GuidanceLine-connectedRunwayCentrelinePoint">
        <rdfs:comment xml:lang="en">(OD272/ED99) The value of a RunwayExitLine feature?s attribute idthr shall be identical to the value of the operationally corresponding RunwayThresholds feature?s attribute idthr (Rule 21).</rdfs:comment>
        <rdfs:domain rdf:resource="http://www.project-best.eu/owl/aixm-mod/airportheliport#GuidanceLine"/>
        <rdfs:range rdf:resource="http://www.project-best.eu/owl/aixm-mod/airportheliport#RunwayCentrelinePoint"/>
    </owl:ObjectProperty>
    


    <!-- http://www.project-best.eu/owl/aixm-mod/airportheliport#GuidanceLine-extent -->

    <owl:ObjectProperty rdf:about="http://www.project-best.eu/owl/aixm-mod/airportheliport#GuidanceLine-extent">
        <rdfs:comment xml:lang="en">Association to Geometry::ElevatedSurface</rdfs:comment>
        <rdfs:comment xml:lang="en">Identifies the extent of the guidance line.</rdfs:comment>
        <rdfs:domain rdf:resource="http://www.project-best.eu/owl/aixm-mod/airportheliport#GuidanceLine"/>
    </owl:ObjectProperty>
    


    <!-- http://www.project-best.eu/owl/aixm-mod/airportheliport#GuidanceLine-type -->

    <owl:ObjectProperty rdf:about="http://www.project-best.eu/owl/aixm-mod/airportheliport#GuidanceLine-type">
        <rdfs:comment xml:lang="en">The type of guidance line.</rdfs:comment>
        <rdfs:range rdf:resource="http://www.project-best.eu/owl/aixm-mod/airportheliport#CodeGuidanceLineType"/>
        <rdfs:domain rdf:resource="http://www.project-best.eu/owl/aixm-mod/airportheliport#GuidanceLine"/>
    </owl:ObjectProperty>
    


    <!-- http://www.project-best.eu/owl/aixm-mod/airportheliport#GuidanceLine-usageDirection -->

    <owl:ObjectProperty rdf:about="http://www.project-best.eu/owl/aixm-mod/airportheliport#GuidanceLine-usageDirection">
        <rdfs:comment xml:lang="en">Indicates the direction in which the guidance line can be used with reference to the start and end points of the associated ElevatedCurve.</rdfs:comment>
        <rdfs:range rdf:resource="http://www.project-best.eu/owl/aixm-mod/airportheliport#CodeDirectionType"/>
        <rdfs:domain rdf:resource="http://www.project-best.eu/owl/aixm-mod/airportheliport#GuidanceLine"/>
    </owl:ObjectProperty>
    


    <!-- http://www.project-best.eu/owl/aixm-mod/airportheliport#GuidanceLineLightSystem-lightedGuidanceLine -->

    <owl:ObjectProperty rdf:about="http://www.project-best.eu/owl/aixm-mod/airportheliport#GuidanceLineLightSystem-lightedGuidanceLine">
        <rdfs:comment xml:lang="en">Identifies the Guidance Line for which the Lighting System is provided.</rdfs:comment>
        <rdfs:range rdf:resource="http://www.project-best.eu/owl/aixm-mod/airportheliport#GuidanceLine"/>
        <rdfs:domain rdf:resource="http://www.project-best.eu/owl/aixm-mod/airportheliport#GuidanceLineLightSystem"/>
    </owl:ObjectProperty>
    


    <!-- http://www.project-best.eu/owl/aixm-mod/airportheliport#GuidanceLineMarking-markedGuidanceLine -->

    <owl:ObjectProperty rdf:about="http://www.project-best.eu/owl/aixm-mod/airportheliport#GuidanceLineMarking-markedGuidanceLine">
        <rdfs:comment xml:lang="en">Identifies the Guidance Line on which the Guidance Marking Line is marked.</rdfs:comment>
        <rdfs:range rdf:resource="http://www.project-best.eu/owl/aixm-mod/airportheliport#GuidanceLine"/>
        <rdfs:domain rdf:resource="http://www.project-best.eu/owl/aixm-mod/airportheliport#GuidanceLineMarking"/>
    </owl:ObjectProperty>
    


    <!-- http://www.project-best.eu/owl/aixm-mod/airportheliport#GuidenceLine-connectedApron -->

    <owl:ObjectProperty rdf:about="http://www.project-best.eu/owl/aixm-mod/airportheliport#GuidenceLine-connectedApron">
        <rdfs:range rdf:resource="http://www.project-best.eu/owl/aixm-mod/airportheliport#Apron"/>
        <rdfs:domain rdf:resource="http://www.project-best.eu/owl/aixm-mod/airportheliport#GuidanceLine"/>
    </owl:ObjectProperty>
    


    <!-- http://www.project-best.eu/owl/aixm-mod/airportheliport#GuidenceLine-connectedStand -->

    <owl:ObjectProperty rdf:about="http://www.project-best.eu/owl/aixm-mod/airportheliport#GuidenceLine-connectedStand">
        <rdfs:range rdf:resource="http://www.project-best.eu/owl/aixm-mod/airportheliport#AircraftStand"/>
        <rdfs:domain rdf:resource="http://www.project-best.eu/owl/aixm-mod/airportheliport#GuidanceLine"/>
    </owl:ObjectProperty>
    


    <!-- http://www.project-best.eu/owl/aixm-mod/airportheliport#GuidenceLine-connectedTaxiway -->

    <owl:ObjectProperty rdf:about="http://www.project-best.eu/owl/aixm-mod/airportheliport#GuidenceLine-connectedTaxiway">
        <rdfs:domain rdf:resource="http://www.project-best.eu/owl/aixm-mod/airportheliport#GuidanceLine"/>
        <rdfs:range rdf:resource="http://www.project-best.eu/owl/aixm-mod/airportheliport#Taxiway"/>
    </owl:ObjectProperty>
    


    <!-- http://www.project-best.eu/owl/aixm-mod/airportheliport#GuidenceLine-connectedTouchDownLiftOff -->

    <owl:ObjectProperty rdf:about="http://www.project-best.eu/owl/aixm-mod/airportheliport#GuidenceLine-connectedTouchDownLiftOff">
        <rdfs:domain rdf:resource="http://www.project-best.eu/owl/aixm-mod/airportheliport#GuidanceLine"/>
        <rdfs:range rdf:resource="http://www.project-best.eu/owl/aixm-mod/airportheliport#TouchDownLiftOff"/>
    </owl:ObjectProperty>
    


    <!-- http://www.project-best.eu/owl/aixm-mod/airportheliport#LightActivation-activation -->

    <owl:ObjectProperty rdf:about="http://www.project-best.eu/owl/aixm-mod/airportheliport#LightActivation-activation">
        <rdfs:comment xml:lang="en">The status of the system (on or off) as result of the number of clicks.</rdfs:comment>
        <rdfs:range rdf:resource="http://www.project-best.eu/owl/aixm-mod/airportheliport#CodeSystemActivationType"/>
        <rdfs:domain rdf:resource="http://www.project-best.eu/owl/aixm-mod/airportheliport#LightActivation"/>
    </owl:ObjectProperty>
    


    <!-- http://www.project-best.eu/owl/aixm-mod/airportheliport#LightActivation-intensityLevel -->

    <owl:ObjectProperty rdf:about="http://www.project-best.eu/owl/aixm-mod/airportheliport#LightActivation-intensityLevel">
        <rdfs:comment xml:lang="en">The intensity step of the lighting system activated by the pilot, depending on the number of clicks.</rdfs:comment>
        <rdfs:range rdf:resource="http://www.project-best.eu/owl/aixm-mod/airportheliport#CodeLightIntensityType"/>
        <rdfs:domain rdf:resource="http://www.project-best.eu/owl/aixm-mod/airportheliport#LightActivation"/>
    </owl:ObjectProperty>
    


    <!-- http://www.project-best.eu/owl/aixm-mod/airportheliport#ManoeuvringAreaAvailability-operationalStatus -->

    <owl:ObjectProperty rdf:about="http://www.project-best.eu/owl/aixm-mod/airportheliport#ManoeuvringAreaAvailability-operationalStatus">
        <rdfs:comment xml:lang="en">Indicates the availability of the facility for specific flight operations.</rdfs:comment>
        <rdfs:range rdf:resource="http://www.project-best.eu/owl/aixm-mod/airportheliport#CodeStatusAirportType"/>
        <rdfs:domain rdf:resource="http://www.project-best.eu/owl/aixm-mod/airportheliport#ManoeuvringAreaAvailability"/>
    </owl:ObjectProperty>
    


    <!-- http://www.project-best.eu/owl/aixm-mod/airportheliport#ManoeuvringAreaAvailability-usage -->

    <owl:ObjectProperty rdf:about="http://www.project-best.eu/owl/aixm-mod/airportheliport#ManoeuvringAreaAvailability-usage">
        <rdfs:domain rdf:resource="http://www.project-best.eu/owl/aixm-mod/airportheliport#ManoeuvringAreaAvailability"/>
        <rdfs:range rdf:resource="http://www.project-best.eu/owl/aixm-mod/airportheliport#ManoeuvringAreaUsage"/>
    </owl:ObjectProperty>
    


    <!-- http://www.project-best.eu/owl/aixm-mod/airportheliport#ManoeuvringAreaAvailability-warning -->

    <owl:ObjectProperty rdf:about="http://www.project-best.eu/owl/aixm-mod/airportheliport#ManoeuvringAreaAvailability-warning">
        <rdfs:comment xml:lang="en">A reason for caution when operating at the facility.</rdfs:comment>
        <rdfs:range rdf:resource="http://www.project-best.eu/owl/aixm-mod/airportheliport#CodeAirportWarningType"/>
        <rdfs:domain rdf:resource="http://www.project-best.eu/owl/aixm-mod/airportheliport#ManoeuvringAreaAvailability"/>
    </owl:ObjectProperty>
    


    <!-- http://www.project-best.eu/owl/aixm-mod/airportheliport#ManoeuvringAreaUsage-isRegulatedBy -->

    <owl:ObjectProperty rdf:about="http://www.project-best.eu/owl/aixm-mod/airportheliport#ManoeuvringAreaUsage-isRegulatedBy">
        <rdfs:range rdf:resource="http://www.project-best.eu/owl/aixm-mod/airportheliport#ManoeuvringAreaAvailability"/>
        <rdfs:domain rdf:resource="http://www.project-best.eu/owl/aixm-mod/airportheliport#ManoeuvringAreaUsage"/>
    </owl:ObjectProperty>
    


    <!-- http://www.project-best.eu/owl/aixm-mod/airportheliport#ManoeuvringAreaUsage-operation -->

    <owl:ObjectProperty rdf:about="http://www.project-best.eu/owl/aixm-mod/airportheliport#ManoeuvringAreaUsage-operation">
        <rdfs:comment xml:lang="en">A type of activity for which a usage rule is specified.</rdfs:comment>
        <rdfs:range rdf:resource="http://www.project-best.eu/owl/aixm-mod/airportheliport#CodeOperationManoeuvringAreaType"/>
        <rdfs:domain rdf:resource="http://www.project-best.eu/owl/aixm-mod/airportheliport#ManoeuvringAreaUsage"/>
    </owl:ObjectProperty>
    


    <!-- http://www.project-best.eu/owl/aixm-mod/airportheliport#Marking-condition -->

    <owl:ObjectProperty rdf:about="http://www.project-best.eu/owl/aixm-mod/airportheliport#Marking-condition">
        <rdfs:comment xml:lang="en">The quality of the marking such as good, fair, poor and other.</rdfs:comment>
        <rdfs:range rdf:resource="http://www.project-best.eu/owl/aixm-mod/airportheliport#CodeMarkingConditionType"/>
        <rdfs:domain rdf:resource="http://www.project-best.eu/owl/aixm-mod/airportheliport#Marking"/>
    </owl:ObjectProperty>
    


    <!-- http://www.project-best.eu/owl/aixm-mod/airportheliport#Marking-element -->

    <owl:ObjectProperty rdf:about="http://www.project-best.eu/owl/aixm-mod/airportheliport#Marking-element">
        <rdfs:comment xml:lang="en">Identifies the Marking Elements of which the Marking is made.</rdfs:comment>
        <rdfs:domain rdf:resource="http://www.project-best.eu/owl/aixm-mod/airportheliport#Marking"/>
        <rdfs:range rdf:resource="http://www.project-best.eu/owl/aixm-mod/airportheliport#MarkingElement"/>
    </owl:ObjectProperty>
    


    <!-- http://www.project-best.eu/owl/aixm-mod/airportheliport#MarkingBuoy-colour -->

    <owl:ObjectProperty rdf:about="http://www.project-best.eu/owl/aixm-mod/airportheliport#MarkingBuoy-colour">
        <rdfs:comment xml:lang="en">Colour of the buoy</rdfs:comment>
        <rdfs:range rdf:resource="http://www.project-best.eu/owl/aixm-mod/airportheliport#CodeColourType"/>
        <rdfs:domain rdf:resource="http://www.project-best.eu/owl/aixm-mod/airportheliport#MarkingBuoy"/>
    </owl:ObjectProperty>
    


    <!-- http://www.project-best.eu/owl/aixm-mod/airportheliport#MarkingBuoy-location -->

    <owl:ObjectProperty rdf:about="http://www.project-best.eu/owl/aixm-mod/airportheliport#MarkingBuoy-location">
        <rdfs:comment xml:lang="en">Association to Geometry::ElevatedPoint</rdfs:comment>
        <rdfs:comment xml:lang="en">Identifies the geographical location of the marking buoy.</rdfs:comment>
        <rdfs:domain rdf:resource="http://www.project-best.eu/owl/aixm-mod/airportheliport#MarkingBuoy"/>
    </owl:ObjectProperty>
    


    <!-- http://www.project-best.eu/owl/aixm-mod/airportheliport#MarkingBuoy-markedSeaplaneLandingArea -->

    <owl:ObjectProperty rdf:about="http://www.project-best.eu/owl/aixm-mod/airportheliport#MarkingBuoy-markedSeaplaneLandingArea">
        <rdfs:domain rdf:resource="http://www.project-best.eu/owl/aixm-mod/airportheliport#MarkingBuoy"/>
        <rdfs:range rdf:resource="http://www.project-best.eu/owl/aixm-mod/airportheliport#SeaplaneLandingArea"/>
    </owl:ObjectProperty>
    


    <!-- http://www.project-best.eu/owl/aixm-mod/airportheliport#MarkingBuoy-type -->

    <owl:ObjectProperty rdf:about="http://www.project-best.eu/owl/aixm-mod/airportheliport#MarkingBuoy-type">
        <rdfs:comment xml:lang="en">The type of the buoy</rdfs:comment>
        <rdfs:range rdf:resource="http://www.project-best.eu/owl/aixm-mod/airportheliport#CodeBuoyType"/>
        <rdfs:domain rdf:resource="http://www.project-best.eu/owl/aixm-mod/airportheliport#MarkingBuoy"/>
    </owl:ObjectProperty>
    


    <!-- http://www.project-best.eu/owl/aixm-mod/airportheliport#MarkingElement-colour -->

    <owl:ObjectProperty rdf:about="http://www.project-best.eu/owl/aixm-mod/airportheliport#MarkingElement-colour">
        <rdfs:comment xml:lang="en">The colour of the marking.</rdfs:comment>
        <rdfs:range rdf:resource="http://www.project-best.eu/owl/aixm-mod/airportheliport#CodeColourType"/>
        <rdfs:domain rdf:resource="http://www.project-best.eu/owl/aixm-mod/airportheliport#MarkingElement"/>
    </owl:ObjectProperty>
    


    <!-- http://www.project-best.eu/owl/aixm-mod/airportheliport#MarkingElement-extent -->

    <owl:ObjectProperty rdf:about="http://www.project-best.eu/owl/aixm-mod/airportheliport#MarkingElement-extent">
        <rdfs:comment xml:lang="en">Identifies the the extent of the Marking Element.</rdfs:comment>
        <rdfs:domain rdf:resource="http://www.project-best.eu/owl/aixm-mod/airportheliport#MarkingElement"/>
        <rdfs:range rdf:resource="http://www.project-best.eu/owl/aixm-mod/airportheliport#MarkingExtent"/>
    </owl:ObjectProperty>
    


    <!-- http://www.project-best.eu/owl/aixm-mod/airportheliport#MarkingElement-style -->

    <owl:ObjectProperty rdf:about="http://www.project-best.eu/owl/aixm-mod/airportheliport#MarkingElement-style">
        <rdfs:comment xml:lang="en">The style of the marking line, such as continuous, dotted, etc.</rdfs:comment>
        <rdfs:range rdf:resource="http://www.project-best.eu/owl/aixm-mod/airportheliport#CodeMarkingStyleType"/>
        <rdfs:domain rdf:resource="http://www.project-best.eu/owl/aixm-mod/airportheliport#MarkingElement"/>
    </owl:ObjectProperty>
    


    <!-- http://www.project-best.eu/owl/aixm-mod/airportheliport#MarkingExtent-curveExtent -->

    <owl:ObjectProperty rdf:about="http://www.project-best.eu/owl/aixm-mod/airportheliport#MarkingExtent-curveExtent">
        <rdfs:comment xml:lang="en">Association to Geometry::ElevatedCurve</rdfs:comment>
        <rdfs:comment xml:lang="en">Identifies the marked curve.</rdfs:comment>
        <rdfs:domain rdf:resource="http://www.project-best.eu/owl/aixm-mod/airportheliport#MarkingExtent"/>
    </owl:ObjectProperty>
    


    <!-- http://www.project-best.eu/owl/aixm-mod/airportheliport#MarkingExtent-location -->

    <owl:ObjectProperty rdf:about="http://www.project-best.eu/owl/aixm-mod/airportheliport#MarkingExtent-location">
        <rdfs:comment xml:lang="en">Association to Geometry::ElevatedPoint</rdfs:comment>
        <rdfs:comment xml:lang="en">Identifies the marked point.</rdfs:comment>
        <rdfs:domain rdf:resource="http://www.project-best.eu/owl/aixm-mod/airportheliport#MarkingExtent"/>
    </owl:ObjectProperty>
    


    <!-- http://www.project-best.eu/owl/aixm-mod/airportheliport#MarkingExtent-surfaceExtent -->

    <owl:ObjectProperty rdf:about="http://www.project-best.eu/owl/aixm-mod/airportheliport#MarkingExtent-surfaceExtent">
        <rdfs:comment xml:lang="en">Association to Geometry::ElevatedSurface</rdfs:comment>
        <rdfs:comment xml:lang="en">Identifies the marked polygon.</rdfs:comment>
        <rdfs:domain rdf:resource="http://www.project-best.eu/owl/aixm-mod/airportheliport#MarkingExtent"/>
    </owl:ObjectProperty>
    


    <!-- http://www.project-best.eu/owl/aixm-mod/airportheliport#NonMovementArea-associatedAirportHeliport -->

    <owl:ObjectProperty rdf:about="http://www.project-best.eu/owl/aixm-mod/airportheliport#NonMovementArea-associatedAirportHeliport">
        <rdfs:comment xml:lang="en">Indicates the Airport where the Non-movement Area is situated.</rdfs:comment>
        <rdfs:range rdf:resource="http://www.project-best.eu/owl/aixm-mod/airportheliport#AirportHeliport"/>
        <rdfs:domain rdf:resource="http://www.project-best.eu/owl/aixm-mod/airportheliport#NonMovementArea"/>
    </owl:ObjectProperty>
    


    <!-- http://www.project-best.eu/owl/aixm-mod/airportheliport#NonMovementArea-extent -->

    <owl:ObjectProperty rdf:about="http://www.project-best.eu/owl/aixm-mod/airportheliport#NonMovementArea-extent">
        <rdfs:comment xml:lang="en">Association to Geometry::ElevatedSurface</rdfs:comment>
        <rdfs:comment xml:lang="en">Identifies the surface area of the Non-movement Area.</rdfs:comment>
        <rdfs:domain rdf:resource="http://www.project-best.eu/owl/aixm-mod/airportheliport#NonMovementArea"/>
    </owl:ObjectProperty>
    


    <!-- http://www.project-best.eu/owl/aixm-mod/airportheliport#PassengerLoadingBridge-extent -->

    <owl:ObjectProperty rdf:about="http://www.project-best.eu/owl/aixm-mod/airportheliport#PassengerLoadingBridge-extent">
        <rdfs:comment xml:lang="en">Association to Geometry::ElevatedSurface</rdfs:comment>
        <rdfs:comment xml:lang="en">Identifies the surface area of the Passenger Loading Bridge.</rdfs:comment>
        <rdfs:domain rdf:resource="http://www.project-best.eu/owl/aixm-mod/airportheliport#PassengerLoadingBridge"/>
    </owl:ObjectProperty>
    


    <!-- http://www.project-best.eu/owl/aixm-mod/airportheliport#PassengerLoadingBridge-type -->

    <owl:ObjectProperty rdf:about="http://www.project-best.eu/owl/aixm-mod/airportheliport#PassengerLoadingBridge-type">
        <rdfs:comment xml:lang="en">Type of bridge used passengers to board and deplane</rdfs:comment>
        <rdfs:range rdf:resource="http://www.project-best.eu/owl/aixm-mod/airportheliport#CodeLoadingBridgeType"/>
        <rdfs:domain rdf:resource="http://www.project-best.eu/owl/aixm-mod/airportheliport#PassengerLoadingBridge"/>
    </owl:ObjectProperty>
    


    <!-- http://www.project-best.eu/owl/aixm-mod/airportheliport#Ridge-side -->

    <owl:ObjectProperty rdf:about="http://www.project-best.eu/owl/aixm-mod/airportheliport#Ridge-side">
        <rdfs:comment xml:lang="en">The side of the runway where the deposited material is located.</rdfs:comment>
        <rdfs:range rdf:resource="http://www.project-best.eu/owl/aixm-mod/airportheliport#CodeSideType"/>
        <rdfs:domain rdf:resource="http://www.project-best.eu/owl/aixm-mod/airportheliport#Ridge"/>
    </owl:ObjectProperty>
    


    <!-- http://www.project-best.eu/owl/aixm-mod/airportheliport#Road-accessibleStand -->

    <owl:ObjectProperty rdf:about="http://www.project-best.eu/owl/aixm-mod/airportheliport#Road-accessibleStand">
        <rdfs:comment xml:lang="en">Identifies the Gate Stand(s) for which the Road gives access.</rdfs:comment>
        <rdfs:range rdf:resource="http://www.project-best.eu/owl/aixm-mod/airportheliport#AircraftStand"/>
        <rdfs:domain rdf:resource="http://www.project-best.eu/owl/aixm-mod/airportheliport#Road"/>
    </owl:ObjectProperty>
    


    <!-- http://www.project-best.eu/owl/aixm-mod/airportheliport#Road-associatedAirport -->

    <owl:ObjectProperty rdf:about="http://www.project-best.eu/owl/aixm-mod/airportheliport#Road-associatedAirport">
        <rdfs:comment xml:lang="en">Identifies the Airport where the Road is situated.</rdfs:comment>
        <rdfs:range rdf:resource="http://www.project-best.eu/owl/aixm-mod/airportheliport#AirportHeliport"/>
        <rdfs:domain rdf:resource="http://www.project-best.eu/owl/aixm-mod/airportheliport#Road"/>
    </owl:ObjectProperty>
    


    <!-- http://www.project-best.eu/owl/aixm-mod/airportheliport#Road-status -->

    <owl:ObjectProperty rdf:about="http://www.project-best.eu/owl/aixm-mod/airportheliport#Road-status">
        <rdfs:comment xml:lang="en">A code indicating the operational status of a service road. For example, serviceable, unserviceable,  work in progress, etc.</rdfs:comment>
        <rdfs:range rdf:resource="http://www.project-best.eu/owl/aixm-mod/airportheliport#CodeStatusOperationsType"/>
        <rdfs:domain rdf:resource="http://www.project-best.eu/owl/aixm-mod/airportheliport#Road"/>
    </owl:ObjectProperty>
    


    <!-- http://www.project-best.eu/owl/aixm-mod/airportheliport#Road-surfaceExtent -->

    <owl:ObjectProperty rdf:about="http://www.project-best.eu/owl/aixm-mod/airportheliport#Road-surfaceExtent">
        <rdfs:comment xml:lang="en">Association to Geometry::ElevatedSurface</rdfs:comment>
        <rdfs:comment xml:lang="en">Identifies the surface area of the Road.</rdfs:comment>
        <rdfs:domain rdf:resource="http://www.project-best.eu/owl/aixm-mod/airportheliport#Road"/>
    </owl:ObjectProperty>
    


    <!-- http://www.project-best.eu/owl/aixm-mod/airportheliport#Road-surfaceProperties -->

    <owl:ObjectProperty rdf:about="http://www.project-best.eu/owl/aixm-mod/airportheliport#Road-surfaceProperties">
        <rdfs:comment xml:lang="en">Identifies the Surface Characteristics of the Road.</rdfs:comment>
        <rdfs:domain rdf:resource="http://www.project-best.eu/owl/aixm-mod/airportheliport#Road"/>
        <rdfs:range rdf:resource="http://www.project-best.eu/owl/aixm-mod/airportheliport#SurfaceCharacteristics"/>
    </owl:ObjectProperty>
    


    <!-- http://www.project-best.eu/owl/aixm-mod/airportheliport#Road-type -->

    <owl:ObjectProperty rdf:about="http://www.project-best.eu/owl/aixm-mod/airportheliport#Road-type">
        <rdfs:comment xml:lang="en">Type of road</rdfs:comment>
        <rdfs:range rdf:resource="http://www.project-best.eu/owl/aixm-mod/airportheliport#CodeRoadType"/>
        <rdfs:domain rdf:resource="http://www.project-best.eu/owl/aixm-mod/airportheliport#Road"/>
    </owl:ObjectProperty>
    


    <!-- http://www.project-best.eu/owl/aixm-mod/airportheliport#Runway-areaContaminant -->

    <owl:ObjectProperty rdf:about="http://www.project-best.eu/owl/aixm-mod/airportheliport#Runway-areaContaminant">
        <rdfs:domain rdf:resource="http://www.project-best.eu/owl/aixm-mod/airportheliport#Runway"/>
        <rdfs:range rdf:resource="http://www.project-best.eu/owl/aixm-mod/airportheliport#RunwaySectionContamination"/>
    </owl:ObjectProperty>
    


    <!-- http://www.project-best.eu/owl/aixm-mod/airportheliport#Runway-associatedAirportHeliport -->

    <owl:ObjectProperty rdf:about="http://www.project-best.eu/owl/aixm-mod/airportheliport#Runway-associatedAirportHeliport">
        <rdfs:comment xml:lang="en">Identifies the Airport where the Runway is situated.</rdfs:comment>
        <rdfs:range rdf:resource="http://www.project-best.eu/owl/aixm-mod/airportheliport#AirportHeliport"/>
        <rdfs:domain rdf:resource="http://www.project-best.eu/owl/aixm-mod/airportheliport#Runway"/>
    </owl:ObjectProperty>
    


    <!-- http://www.project-best.eu/owl/aixm-mod/airportheliport#Runway-overallContaminant -->

    <owl:ObjectProperty rdf:about="http://www.project-best.eu/owl/aixm-mod/airportheliport#Runway-overallContaminant">
        <rdfs:comment xml:lang="en">Identifies the contaminant of the runway.</rdfs:comment>
        <rdfs:domain rdf:resource="http://www.project-best.eu/owl/aixm-mod/airportheliport#Runway"/>
        <rdfs:range rdf:resource="http://www.project-best.eu/owl/aixm-mod/airportheliport#RunwayContamination"/>
    </owl:ObjectProperty>
    


    <!-- http://www.project-best.eu/owl/aixm-mod/airportheliport#Runway-surfaceProperties -->

    <owl:ObjectProperty rdf:about="http://www.project-best.eu/owl/aixm-mod/airportheliport#Runway-surfaceProperties">
        <rdfs:comment xml:lang="en">Identifies the surface characteristics of the runway.</rdfs:comment>
        <rdfs:domain rdf:resource="http://www.project-best.eu/owl/aixm-mod/airportheliport#Runway"/>
        <rdfs:range rdf:resource="http://www.project-best.eu/owl/aixm-mod/airportheliport#SurfaceCharacteristics"/>
    </owl:ObjectProperty>
    


    <!-- http://www.project-best.eu/owl/aixm-mod/airportheliport#Runway-type -->

    <owl:ObjectProperty rdf:about="http://www.project-best.eu/owl/aixm-mod/airportheliport#Runway-type">
        <rdfs:comment xml:lang="en">The type can be either runway for airplanes or  final approach and take off area (FATO) for helicopters.</rdfs:comment>
        <rdfs:range rdf:resource="http://www.project-best.eu/owl/aixm-mod/airportheliport#CodeRunwayType"/>
        <rdfs:domain rdf:resource="http://www.project-best.eu/owl/aixm-mod/airportheliport#Runway"/>
    </owl:ObjectProperty>
    


    <!-- http://www.project-best.eu/owl/aixm-mod/airportheliport#RunwayBlastPad-extent -->

    <owl:ObjectProperty rdf:about="http://www.project-best.eu/owl/aixm-mod/airportheliport#RunwayBlastPad-extent">
        <rdfs:comment xml:lang="en">Association to Geometry::ElevatedSurface</rdfs:comment>
        <rdfs:comment xml:lang="en">Identifies the extent of the runway blast pad.</rdfs:comment>
        <rdfs:domain rdf:resource="http://www.project-best.eu/owl/aixm-mod/airportheliport#RunwayBlastPad"/>
    </owl:ObjectProperty>
    


    <!-- http://www.project-best.eu/owl/aixm-mod/airportheliport#RunwayBlastPad-status -->

    <owl:ObjectProperty rdf:about="http://www.project-best.eu/owl/aixm-mod/airportheliport#RunwayBlastPad-status">
        <rdfs:comment xml:lang="en">Temporal description of the operational state of the feature.  This attribute is used to describe real-time status</rdfs:comment>
        <rdfs:range rdf:resource="http://www.project-best.eu/owl/aixm-mod/airportheliport#CodeStatusOperationsType"/>
        <rdfs:domain rdf:resource="http://www.project-best.eu/owl/aixm-mod/airportheliport#RunwayBlastPad"/>
    </owl:ObjectProperty>
    


    <!-- http://www.project-best.eu/owl/aixm-mod/airportheliport#RunwayBlastPad-surfaceProperties -->

    <owl:ObjectProperty rdf:about="http://www.project-best.eu/owl/aixm-mod/airportheliport#RunwayBlastPad-surfaceProperties">
        <rdfs:comment xml:lang="en">Identifies the surface characteristics of the runway blast pad.</rdfs:comment>
        <rdfs:domain rdf:resource="http://www.project-best.eu/owl/aixm-mod/airportheliport#RunwayBlastPad"/>
        <rdfs:range rdf:resource="http://www.project-best.eu/owl/aixm-mod/airportheliport#SurfaceCharacteristics"/>
    </owl:ObjectProperty>
    


    <!-- http://www.project-best.eu/owl/aixm-mod/airportheliport#RunwayBlastPad-usedRunwayDirection -->

    <owl:ObjectProperty rdf:about="http://www.project-best.eu/owl/aixm-mod/airportheliport#RunwayBlastPad-usedRunwayDirection">
        <rdfs:comment xml:lang="en">Identifies the runway direction on which the blast pad is used.</rdfs:comment>
        <rdfs:domain rdf:resource="http://www.project-best.eu/owl/aixm-mod/airportheliport#RunwayBlastPad"/>
        <rdfs:range rdf:resource="http://www.project-best.eu/owl/aixm-mod/airportheliport#RunwayDirection"/>
    </owl:ObjectProperty>
    


    <!-- http://www.project-best.eu/owl/aixm-mod/airportheliport#RunwayCentrelinePoint-associatedDeclaredDistance -->

    <owl:ObjectProperty rdf:about="http://www.project-best.eu/owl/aixm-mod/airportheliport#RunwayCentrelinePoint-associatedDeclaredDistance">
        <rdfs:comment xml:lang="en">Identifies the ruwnay declared distance for which the runway centreline point ensures.</rdfs:comment>
        <rdfs:domain rdf:resource="http://www.project-best.eu/owl/aixm-mod/airportheliport#RunwayCentrelinePoint"/>
        <rdfs:range rdf:resource="http://www.project-best.eu/owl/aixm-mod/airportheliport#RunwayDeclaredDistance"/>
    </owl:ObjectProperty>
    


    <!-- http://www.project-best.eu/owl/aixm-mod/airportheliport#RunwayCentrelinePoint-location -->

    <owl:ObjectProperty rdf:about="http://www.project-best.eu/owl/aixm-mod/airportheliport#RunwayCentrelinePoint-location">
        <rdfs:comment xml:lang="en">Association to Geometry::ElevatedPoint</rdfs:comment>
        <rdfs:comment xml:lang="en">Identifies the geographical position of the runway centreline point.</rdfs:comment>
        <rdfs:domain rdf:resource="http://www.project-best.eu/owl/aixm-mod/airportheliport#RunwayCentrelinePoint"/>
    </owl:ObjectProperty>
    


    <!-- http://www.project-best.eu/owl/aixm-mod/airportheliport#RunwayCentrelinePoint-role -->

    <owl:ObjectProperty rdf:about="http://www.project-best.eu/owl/aixm-mod/airportheliport#RunwayCentrelinePoint-role">
        <rdfs:comment xml:lang="en">The role of the point along the runway direction centreline.</rdfs:comment>
        <rdfs:range rdf:resource="http://www.project-best.eu/owl/aixm-mod/airportheliport#CodeRunwayPointRoleType"/>
        <rdfs:domain rdf:resource="http://www.project-best.eu/owl/aixm-mod/airportheliport#RunwayCentrelinePoint"/>
    </owl:ObjectProperty>
    


    <!-- http://www.project-best.eu/owl/aixm-mod/airportheliport#RunwayContamination-clearedSide -->

    <owl:ObjectProperty rdf:about="http://www.project-best.eu/owl/aixm-mod/airportheliport#RunwayContamination-clearedSide">
        <rdfs:comment xml:lang="en">Indicates that the cleared width is offset left or right of centre line.</rdfs:comment>
        <rdfs:range rdf:resource="http://www.project-best.eu/owl/aixm-mod/airportheliport#CodeSideType"/>
        <rdfs:domain rdf:resource="http://www.project-best.eu/owl/aixm-mod/airportheliport#RunwayContamination"/>
    </owl:ObjectProperty>
    


    <!-- http://www.project-best.eu/owl/aixm-mod/airportheliport#RunwayContamination-obscuredLightsSide -->

    <owl:ObjectProperty rdf:about="http://www.project-best.eu/owl/aixm-mod/airportheliport#RunwayContamination-obscuredLightsSide">
        <rdfs:comment xml:lang="en">Indicates the side on which the lights are obscured.</rdfs:comment>
        <rdfs:range rdf:resource="http://www.project-best.eu/owl/aixm-mod/airportheliport#CodeSideType"/>
        <rdfs:domain rdf:resource="http://www.project-best.eu/owl/aixm-mod/airportheliport#RunwayContamination"/>
    </owl:ObjectProperty>
    


    <!-- http://www.project-best.eu/owl/aixm-mod/airportheliport#RunwayDeclaredDistance-declaredValue -->

    <owl:ObjectProperty rdf:about="http://www.project-best.eu/owl/aixm-mod/airportheliport#RunwayDeclaredDistance-declaredValue">
        <rdfs:domain rdf:resource="http://www.project-best.eu/owl/aixm-mod/airportheliport#RunwayDeclaredDistance"/>
        <rdfs:range rdf:resource="http://www.project-best.eu/owl/aixm-mod/airportheliport#RunwayDeclaredDistanceValue"/>
    </owl:ObjectProperty>
    


    <!-- http://www.project-best.eu/owl/aixm-mod/airportheliport#RunwayDeclaredDistance-type -->

    <owl:ObjectProperty rdf:about="http://www.project-best.eu/owl/aixm-mod/airportheliport#RunwayDeclaredDistance-type">
        <rdfs:comment xml:lang="en">A code indicating the type of a conventional declared distance.</rdfs:comment>
        <rdfs:range rdf:resource="http://www.project-best.eu/owl/aixm-mod/airportheliport#CodeDeclaredDistanceType"/>
        <rdfs:domain rdf:resource="http://www.project-best.eu/owl/aixm-mod/airportheliport#RunwayDeclaredDistance"/>
    </owl:ObjectProperty>
    


    <!-- http://www.project-best.eu/owl/aixm-mod/airportheliport#RunwayDirection-approachMarkingCondition -->

    <owl:ObjectProperty rdf:about="http://www.project-best.eu/owl/aixm-mod/airportheliport#RunwayDirection-approachMarkingCondition">
        <rdfs:comment xml:lang="en">The quality of the runway marking such as good, fair, poor and other.</rdfs:comment>
        <rdfs:range rdf:resource="http://www.project-best.eu/owl/aixm-mod/airportheliport#CodeMarkingConditionType"/>
        <rdfs:domain rdf:resource="http://www.project-best.eu/owl/aixm-mod/airportheliport#RunwayDirection"/>
    </owl:ObjectProperty>
    


    <!-- http://www.project-best.eu/owl/aixm-mod/airportheliport#RunwayDirection-approachMarkingType -->

    <owl:ObjectProperty rdf:about="http://www.project-best.eu/owl/aixm-mod/airportheliport#RunwayDirection-approachMarkingType">
        <rdfs:comment xml:lang="en">Type of marking related to landing categories such as precision, non-precision and basic.</rdfs:comment>
        <rdfs:range rdf:resource="http://www.project-best.eu/owl/aixm-mod/airportheliport#CodeRunwayMarkingType"/>
        <rdfs:domain rdf:resource="http://www.project-best.eu/owl/aixm-mod/airportheliport#RunwayDirection"/>
    </owl:ObjectProperty>
    


    <!-- http://www.project-best.eu/owl/aixm-mod/airportheliport#RunwayDirection-availability -->

    <owl:ObjectProperty rdf:about="http://www.project-best.eu/owl/aixm-mod/airportheliport#RunwayDirection-availability">
        <rdfs:range rdf:resource="http://www.project-best.eu/owl/aixm-mod/airportheliport#ManoeuvringAreaAvailability"/>
        <rdfs:domain rdf:resource="http://www.project-best.eu/owl/aixm-mod/airportheliport#RunwayDirection"/>
    </owl:ObjectProperty>
    


    <!-- http://www.project-best.eu/owl/aixm-mod/airportheliport#RunwayDirection-classLightingJAR -->

    <owl:ObjectProperty rdf:about="http://www.project-best.eu/owl/aixm-mod/airportheliport#RunwayDirection-classLightingJAR">
        <rdfs:comment xml:lang="en">Classification of the approach lighting system using as criteria JAR-OPS 1 - Subpart E, Appendix 1 to 1.430</rdfs:comment>
        <rdfs:range rdf:resource="http://www.project-best.eu/owl/aixm-mod/airportheliport#CodeLightingJARType"/>
        <rdfs:domain rdf:resource="http://www.project-best.eu/owl/aixm-mod/airportheliport#RunwayDirection"/>
    </owl:ObjectProperty>
    


    <!-- http://www.project-best.eu/owl/aixm-mod/airportheliport#RunwayDirection-precisionApproachGuidance -->

    <owl:ObjectProperty rdf:about="http://www.project-best.eu/owl/aixm-mod/airportheliport#RunwayDirection-precisionApproachGuidance">
        <rdfs:comment xml:lang="en">Degree to which navigation aids provide accurate approach guidance.  Precision approaches utilize both lateral (course) and vertical (glideslope) information</rdfs:comment>
        <rdfs:range rdf:resource="http://www.project-best.eu/owl/aixm-mod/airportheliport#CodeApproachGuidanceType"/>
        <rdfs:domain rdf:resource="http://www.project-best.eu/owl/aixm-mod/airportheliport#RunwayDirection"/>
    </owl:ObjectProperty>
    


    <!-- http://www.project-best.eu/owl/aixm-mod/airportheliport#RunwayDirection-startingElement -->

    <owl:ObjectProperty rdf:about="http://www.project-best.eu/owl/aixm-mod/airportheliport#RunwayDirection-startingElement">
        <rdfs:comment xml:lang="en">The runway element is the start of the runway direction.  Typically used to indicate the location of a displaced area.</rdfs:comment>
        <rdfs:domain rdf:resource="http://www.project-best.eu/owl/aixm-mod/airportheliport#RunwayDirection"/>
        <rdfs:range rdf:resource="http://www.project-best.eu/owl/aixm-mod/airportheliport#RunwayElement"/>
    </owl:ObjectProperty>
    


    <!-- http://www.project-best.eu/owl/aixm-mod/airportheliport#RunwayDirection-usedRunway -->

    <owl:ObjectProperty rdf:about="http://www.project-best.eu/owl/aixm-mod/airportheliport#RunwayDirection-usedRunway">
        <rdfs:comment xml:lang="en">(DO272/ED99) Each FinalApproachAndTakeOff feature?s attribute idthr shall provide the idrwy object identifier value of the corresponding HelipadThreshold (Rule 15).</rdfs:comment>
        <rdfs:range rdf:resource="http://www.project-best.eu/owl/aixm-mod/airportheliport#Runway"/>
        <rdfs:domain rdf:resource="http://www.project-best.eu/owl/aixm-mod/airportheliport#RunwayDirection"/>
    </owl:ObjectProperty>
    


    <!-- http://www.project-best.eu/owl/aixm-mod/airportheliport#RunwayDirectionLightSystem-associatedRunwayDirection -->

    <owl:ObjectProperty rdf:about="http://www.project-best.eu/owl/aixm-mod/airportheliport#RunwayDirectionLightSystem-associatedRunwayDirection">
        <rdfs:comment xml:lang="en">Identifies the Runway Direction for which the Lighting System is provided.</rdfs:comment>
        <rdfs:range rdf:resource="http://www.project-best.eu/owl/aixm-mod/airportheliport#RunwayDirection"/>
        <rdfs:domain rdf:resource="http://www.project-best.eu/owl/aixm-mod/airportheliport#RunwayDirectionLightSystem"/>
    </owl:ObjectProperty>
    


    <!-- http://www.project-best.eu/owl/aixm-mod/airportheliport#RunwayDirectionLightSystem-position -->

    <owl:ObjectProperty rdf:about="http://www.project-best.eu/owl/aixm-mod/airportheliport#RunwayDirectionLightSystem-position">
        <rdfs:comment xml:lang="en">A code indicating the part of the runway the lighting system is serving.</rdfs:comment>
        <rdfs:range rdf:resource="http://www.project-best.eu/owl/aixm-mod/airportheliport#CodeRunwaySectionType"/>
        <rdfs:domain rdf:resource="http://www.project-best.eu/owl/aixm-mod/airportheliport#RunwayDirectionLightSystem"/>
    </owl:ObjectProperty>
    


    <!-- http://www.project-best.eu/owl/aixm-mod/airportheliport#RunwayElement-associatedRunway -->

    <owl:ObjectProperty rdf:about="http://www.project-best.eu/owl/aixm-mod/airportheliport#RunwayElement-associatedRunway">
        <rdfs:comment xml:lang="en">Indicates which runways the Runway Element belongs to.  Note that Runway Intersection elements will belong to more than one Runway. </rdfs:comment>
        <rdfs:range rdf:resource="http://www.project-best.eu/owl/aixm-mod/airportheliport#Runway"/>
        <rdfs:domain rdf:resource="http://www.project-best.eu/owl/aixm-mod/airportheliport#RunwayElement"/>
    </owl:ObjectProperty>
    


    <!-- http://www.project-best.eu/owl/aixm-mod/airportheliport#RunwayElement-availability -->

    <owl:ObjectProperty rdf:about="http://www.project-best.eu/owl/aixm-mod/airportheliport#RunwayElement-availability">
        <rdfs:range rdf:resource="http://www.project-best.eu/owl/aixm-mod/airportheliport#ManoeuvringAreaAvailability"/>
        <rdfs:domain rdf:resource="http://www.project-best.eu/owl/aixm-mod/airportheliport#RunwayElement"/>
    </owl:ObjectProperty>
    


    <!-- http://www.project-best.eu/owl/aixm-mod/airportheliport#RunwayElement-extent -->

    <owl:ObjectProperty rdf:about="http://www.project-best.eu/owl/aixm-mod/airportheliport#RunwayElement-extent">
        <rdfs:comment xml:lang="en">Association to Geometry::ElevatedSurface</rdfs:comment>
        <rdfs:comment xml:lang="en">Identifies the extent of the Ruwnay Element.</rdfs:comment>
        <rdfs:domain rdf:resource="http://www.project-best.eu/owl/aixm-mod/airportheliport#RunwayElement"/>
    </owl:ObjectProperty>
    


    <!-- http://www.project-best.eu/owl/aixm-mod/airportheliport#RunwayElement-gradeSeparation -->

    <owl:ObjectProperty rdf:about="http://www.project-best.eu/owl/aixm-mod/airportheliport#RunwayElement-gradeSeparation">
        <rdfs:comment xml:lang="en">A code that indicates the placement of the element at a different height from another element.</rdfs:comment>
        <rdfs:range rdf:resource="http://www.project-best.eu/owl/aixm-mod/airportheliport#CodeGradeSeparationType"/>
        <rdfs:domain rdf:resource="http://www.project-best.eu/owl/aixm-mod/airportheliport#RunwayElement"/>
    </owl:ObjectProperty>
    


    <!-- http://www.project-best.eu/owl/aixm-mod/airportheliport#RunwayElement-surfaceProperties -->

    <owl:ObjectProperty rdf:about="http://www.project-best.eu/owl/aixm-mod/airportheliport#RunwayElement-surfaceProperties">
        <rdfs:comment xml:lang="en">Identifies the surface characteristics of the runway element.</rdfs:comment>
        <rdfs:domain rdf:resource="http://www.project-best.eu/owl/aixm-mod/airportheliport#RunwayElement"/>
        <rdfs:range rdf:resource="http://www.project-best.eu/owl/aixm-mod/airportheliport#SurfaceCharacteristics"/>
    </owl:ObjectProperty>
    


    <!-- http://www.project-best.eu/owl/aixm-mod/airportheliport#RunwayElement-type -->

    <owl:ObjectProperty rdf:about="http://www.project-best.eu/owl/aixm-mod/airportheliport#RunwayElement-type">
        <rdfs:comment xml:lang="en">The type of element.</rdfs:comment>
        <rdfs:range rdf:resource="http://www.project-best.eu/owl/aixm-mod/airportheliport#CodeRunwayElementType"/>
        <rdfs:domain rdf:resource="http://www.project-best.eu/owl/aixm-mod/airportheliport#RunwayElement"/>
    </owl:ObjectProperty>
    


    <!-- http://www.project-best.eu/owl/aixm-mod/airportheliport#RunwayMarking-markedRunway -->

    <owl:ObjectProperty rdf:about="http://www.project-best.eu/owl/aixm-mod/airportheliport#RunwayMarking-markedRunway">
        <rdfs:comment xml:lang="en">The runway having the runway markings.</rdfs:comment>
        <rdfs:range rdf:resource="http://www.project-best.eu/owl/aixm-mod/airportheliport#Runway"/>
        <rdfs:domain rdf:resource="http://www.project-best.eu/owl/aixm-mod/airportheliport#RunwayMarking"/>
    </owl:ObjectProperty>
    


    <!-- http://www.project-best.eu/owl/aixm-mod/airportheliport#RunwayMarking-markingLocation -->

    <owl:ObjectProperty rdf:about="http://www.project-best.eu/owl/aixm-mod/airportheliport#RunwayMarking-markingLocation">
        <rdfs:comment xml:lang="en">A code indicating the location of the marking relative to the surface.</rdfs:comment>
        <rdfs:range rdf:resource="http://www.project-best.eu/owl/aixm-mod/airportheliport#CodeRunwaySectionType"/>
        <rdfs:domain rdf:resource="http://www.project-best.eu/owl/aixm-mod/airportheliport#RunwayMarking"/>
    </owl:ObjectProperty>
    


    <!-- http://www.project-best.eu/owl/aixm-mod/airportheliport#RunwayProtectArea-status -->

    <owl:ObjectProperty rdf:about="http://www.project-best.eu/owl/aixm-mod/airportheliport#RunwayProtectArea-status">
        <rdfs:comment xml:lang="en">Temporal description of the operational state of the feature.  This attribute is used to describe real-time status.)</rdfs:comment>
        <rdfs:range rdf:resource="http://www.project-best.eu/owl/aixm-mod/airportheliport#CodeStatusOperationsType"/>
        <rdfs:domain rdf:resource="http://www.project-best.eu/owl/aixm-mod/airportheliport#RunwayProtectArea"/>
    </owl:ObjectProperty>
    


    <!-- http://www.project-best.eu/owl/aixm-mod/airportheliport#RunwayProtectArea-type -->

    <owl:ObjectProperty rdf:about="http://www.project-best.eu/owl/aixm-mod/airportheliport#RunwayProtectArea-type">
        <rdfs:comment xml:lang="en">A code indicating the type of protection area.</rdfs:comment>
        <rdfs:range rdf:resource="http://www.project-best.eu/owl/aixm-mod/airportheliport#CodeRunwayProtectionAreaType"/>
        <rdfs:domain rdf:resource="http://www.project-best.eu/owl/aixm-mod/airportheliport#RunwayProtectArea"/>
    </owl:ObjectProperty>
    


    <!-- http://www.project-best.eu/owl/aixm-mod/airportheliport#RunwayProtectAreaLightSystem-lightedArea -->

    <owl:ObjectProperty rdf:about="http://www.project-best.eu/owl/aixm-mod/airportheliport#RunwayProtectAreaLightSystem-lightedArea">
        <rdfs:comment xml:lang="en">Identifies the Runway Protect Area for which the Lighting System is provided.</rdfs:comment>
        <rdfs:range rdf:resource="http://www.project-best.eu/owl/aixm-mod/airportheliport#RunwayProtectArea"/>
        <rdfs:domain rdf:resource="http://www.project-best.eu/owl/aixm-mod/airportheliport#RunwayProtectAreaLightSystem"/>
    </owl:ObjectProperty>
    


    <!-- http://www.project-best.eu/owl/aixm-mod/airportheliport#RunwayProtectAreaLightSystem-position -->

    <owl:ObjectProperty rdf:about="http://www.project-best.eu/owl/aixm-mod/airportheliport#RunwayProtectAreaLightSystem-position">
        <rdfs:comment xml:lang="en">Location of the lighting.</rdfs:comment>
        <rdfs:range rdf:resource="http://www.project-best.eu/owl/aixm-mod/airportheliport#CodeProtectAreaSectionType"/>
        <rdfs:domain rdf:resource="http://www.project-best.eu/owl/aixm-mod/airportheliport#RunwayProtectAreaLightSystem"/>
    </owl:ObjectProperty>
    


    <!-- http://www.project-best.eu/owl/aixm-mod/airportheliport#RunwaySectionContamination-section -->

    <owl:ObjectProperty rdf:about="http://www.project-best.eu/owl/aixm-mod/airportheliport#RunwaySectionContamination-section">
        <rdfs:comment xml:lang="en">Indicates the part of the runway that is affected. This attribute supports the current SNOWTAM practice, which consists in reporting the contamination information on each third of the runway length, starting from the threshold of the runway direction having the lower designation number.</rdfs:comment>
        <rdfs:range rdf:resource="http://www.project-best.eu/owl/aixm-mod/airportheliport#CodeRunwaySectionType"/>
        <rdfs:domain rdf:resource="http://www.project-best.eu/owl/aixm-mod/airportheliport#RunwaySectionContamination"/>
    </owl:ObjectProperty>
    


    <!-- http://www.project-best.eu/owl/aixm-mod/airportheliport#RunwayVisualRange-associatedRunwayDirection -->

    <owl:ObjectProperty rdf:about="http://www.project-best.eu/owl/aixm-mod/airportheliport#RunwayVisualRange-associatedRunwayDirection">
        <rdfs:range rdf:resource="http://www.project-best.eu/owl/aixm-mod/airportheliport#RunwayDirection"/>
        <rdfs:domain rdf:resource="http://www.project-best.eu/owl/aixm-mod/airportheliport#RunwayVisualRange"/>
    </owl:ObjectProperty>
    


    <!-- http://www.project-best.eu/owl/aixm-mod/airportheliport#RunwayVisualRange-location -->

    <owl:ObjectProperty rdf:about="http://www.project-best.eu/owl/aixm-mod/airportheliport#RunwayVisualRange-location">
        <rdfs:comment xml:lang="en">Association to Geometry::ElevatedPoint</rdfs:comment>
        <rdfs:domain rdf:resource="http://www.project-best.eu/owl/aixm-mod/airportheliport#RunwayVisualRange"/>
    </owl:ObjectProperty>
    


    <!-- http://www.project-best.eu/owl/aixm-mod/airportheliport#RunwayVisualRange-readingPosition -->

    <owl:ObjectProperty rdf:about="http://www.project-best.eu/owl/aixm-mod/airportheliport#RunwayVisualRange-readingPosition">
        <rdfs:comment xml:lang="en">The position along the runway direction for which the reading is provided.</rdfs:comment>
        <rdfs:range rdf:resource="http://www.project-best.eu/owl/aixm-mod/airportheliport#CodeRVRReadingType"/>
        <rdfs:domain rdf:resource="http://www.project-best.eu/owl/aixm-mod/airportheliport#RunwayVisualRange"/>
    </owl:ObjectProperty>
    


    <!-- http://www.project-best.eu/owl/aixm-mod/airportheliport#SeaplaneLandingArea-availability -->

    <owl:ObjectProperty rdf:about="http://www.project-best.eu/owl/aixm-mod/airportheliport#SeaplaneLandingArea-availability">
        <rdfs:range rdf:resource="http://www.project-best.eu/owl/aixm-mod/airportheliport#ManoeuvringAreaAvailability"/>
        <rdfs:domain rdf:resource="http://www.project-best.eu/owl/aixm-mod/airportheliport#SeaplaneLandingArea"/>
    </owl:ObjectProperty>
    


    <!-- http://www.project-best.eu/owl/aixm-mod/airportheliport#SeaplaneLandingArea-dockSite -->

    <owl:ObjectProperty rdf:about="http://www.project-best.eu/owl/aixm-mod/airportheliport#SeaplaneLandingArea-dockSite">
        <rdfs:comment xml:lang="en">Identifies the dock site(s) associated with the seaplane landing area.</rdfs:comment>
        <rdfs:range rdf:resource="http://www.project-best.eu/owl/aixm-mod/airportheliport#FloatingDockSite"/>
        <rdfs:domain rdf:resource="http://www.project-best.eu/owl/aixm-mod/airportheliport#SeaplaneLandingArea"/>
    </owl:ObjectProperty>
    


    <!-- http://www.project-best.eu/owl/aixm-mod/airportheliport#SeaplaneLandingArea-extent -->

    <owl:ObjectProperty rdf:about="http://www.project-best.eu/owl/aixm-mod/airportheliport#SeaplaneLandingArea-extent">
        <rdfs:comment xml:lang="en">Association to Geometry::ElevatedSurface</rdfs:comment>
        <rdfs:comment xml:lang="en">Identifies the extent of the seaplane landing area.</rdfs:comment>
        <rdfs:domain rdf:resource="http://www.project-best.eu/owl/aixm-mod/airportheliport#SeaplaneLandingArea"/>
    </owl:ObjectProperty>
    


    <!-- http://www.project-best.eu/owl/aixm-mod/airportheliport#SeaplaneLandingArea-rampSite -->

    <owl:ObjectProperty rdf:about="http://www.project-best.eu/owl/aixm-mod/airportheliport#SeaplaneLandingArea-rampSite">
        <rdfs:comment xml:lang="en">Identifies the ramp site associated to the seaplane landing area.</rdfs:comment>
        <rdfs:domain rdf:resource="http://www.project-best.eu/owl/aixm-mod/airportheliport#SeaplaneLandingArea"/>
        <rdfs:range rdf:resource="http://www.project-best.eu/owl/aixm-mod/airportheliport#SeaplaneRampSite"/>
    </owl:ObjectProperty>
    


    <!-- http://www.project-best.eu/owl/aixm-mod/airportheliport#SeaplaneRampSite-centreline -->

    <owl:ObjectProperty rdf:about="http://www.project-best.eu/owl/aixm-mod/airportheliport#SeaplaneRampSite-centreline">
        <rdfs:comment xml:lang="en">Association to Geometry::ElevatedCurve</rdfs:comment>
        <rdfs:comment xml:lang="en">Identifies the centreline of the ramp site.</rdfs:comment>
        <rdfs:domain rdf:resource="http://www.project-best.eu/owl/aixm-mod/airportheliport#SeaplaneRampSite"/>
    </owl:ObjectProperty>
    


    <!-- http://www.project-best.eu/owl/aixm-mod/airportheliport#SeaplaneRampSite-extent -->

    <owl:ObjectProperty rdf:about="http://www.project-best.eu/owl/aixm-mod/airportheliport#SeaplaneRampSite-extent">
        <rdfs:comment xml:lang="en">Association to Geometry::ElevatedSurface</rdfs:comment>
        <rdfs:comment xml:lang="en">Identifies the extent of the ramp site.</rdfs:comment>
        <rdfs:domain rdf:resource="http://www.project-best.eu/owl/aixm-mod/airportheliport#SeaplaneRampSite"/>
    </owl:ObjectProperty>
    


    <!-- http://www.project-best.eu/owl/aixm-mod/airportheliport#StandMarking-markedStand -->

    <owl:ObjectProperty rdf:about="http://www.project-best.eu/owl/aixm-mod/airportheliport#StandMarking-markedStand">
        <rdfs:comment xml:lang="en">Identifies the Gate Stand at which the Gate Stand Markings are marked.</rdfs:comment>
        <rdfs:range rdf:resource="http://www.project-best.eu/owl/aixm-mod/airportheliport#AircraftStand"/>
        <rdfs:domain rdf:resource="http://www.project-best.eu/owl/aixm-mod/airportheliport#StandMarking"/>
    </owl:ObjectProperty>
    


    <!-- http://www.project-best.eu/owl/aixm-mod/airportheliport#SurfaceCharacteristics-composition -->

    <owl:ObjectProperty rdf:about="http://www.project-best.eu/owl/aixm-mod/airportheliport#SurfaceCharacteristics-composition">
        <rdfs:comment xml:lang="en">The type of the predominant material of which a surface of the movement area is composed.</rdfs:comment>
        <rdfs:range rdf:resource="http://www.project-best.eu/owl/aixm-mod/airportheliport#CodeSurfaceCompositionType"/>
        <rdfs:domain rdf:resource="http://www.project-best.eu/owl/aixm-mod/airportheliport#SurfaceCharacteristics"/>
    </owl:ObjectProperty>
    


    <!-- http://www.project-best.eu/owl/aixm-mod/airportheliport#SurfaceCharacteristics-evaluationMethodPCN -->

    <owl:ObjectProperty rdf:about="http://www.project-best.eu/owl/aixm-mod/airportheliport#SurfaceCharacteristics-evaluationMethodPCN">
        <rdfs:comment xml:lang="en">The method used to rate a runway pavement.</rdfs:comment>
        <rdfs:range rdf:resource="http://www.project-best.eu/owl/aixm-mod/airportheliport#CodePCNMethodType"/>
        <rdfs:domain rdf:resource="http://www.project-best.eu/owl/aixm-mod/airportheliport#SurfaceCharacteristics"/>
    </owl:ObjectProperty>
    


    <!-- http://www.project-best.eu/owl/aixm-mod/airportheliport#SurfaceCharacteristics-maxTyrePressurePCN -->

    <owl:ObjectProperty rdf:about="http://www.project-best.eu/owl/aixm-mod/airportheliport#SurfaceCharacteristics-maxTyrePressurePCN">
        <rdfs:comment xml:lang="en">The maximum allowable tire pressure category related to the Pavement Classification Number (PCN), as a category.</rdfs:comment>
        <rdfs:range rdf:resource="http://www.project-best.eu/owl/aixm-mod/airportheliport#CodePCNTyrePressureType"/>
        <rdfs:domain rdf:resource="http://www.project-best.eu/owl/aixm-mod/airportheliport#SurfaceCharacteristics"/>
    </owl:ObjectProperty>
    


    <!-- http://www.project-best.eu/owl/aixm-mod/airportheliport#SurfaceCharacteristics-pavementSubgradePCN -->

    <owl:ObjectProperty rdf:about="http://www.project-best.eu/owl/aixm-mod/airportheliport#SurfaceCharacteristics-pavementSubgradePCN">
        <rdfs:comment xml:lang="en">A categorized indication of the pavement subgrade strength related to the Pavement Classification Number (PCN).</rdfs:comment>
        <rdfs:range rdf:resource="http://www.project-best.eu/owl/aixm-mod/airportheliport#CodePCNSubgradeType"/>
        <rdfs:domain rdf:resource="http://www.project-best.eu/owl/aixm-mod/airportheliport#SurfaceCharacteristics"/>
    </owl:ObjectProperty>
    


    <!-- http://www.project-best.eu/owl/aixm-mod/airportheliport#SurfaceCharacteristics-pavementTypePCN -->

    <owl:ObjectProperty rdf:about="http://www.project-best.eu/owl/aixm-mod/airportheliport#SurfaceCharacteristics-pavementTypePCN">
        <rdfs:comment xml:lang="en">The pavement behaviour (rigid or flexible) used for the Pavement Classification Number (PCN) determination, as a category.</rdfs:comment>
        <rdfs:range rdf:resource="http://www.project-best.eu/owl/aixm-mod/airportheliport#CodePCNPavementType"/>
        <rdfs:domain rdf:resource="http://www.project-best.eu/owl/aixm-mod/airportheliport#SurfaceCharacteristics"/>
    </owl:ObjectProperty>
    


    <!-- http://www.project-best.eu/owl/aixm-mod/airportheliport#SurfaceCharacteristics-preparation -->

    <owl:ObjectProperty rdf:about="http://www.project-best.eu/owl/aixm-mod/airportheliport#SurfaceCharacteristics-preparation">
        <rdfs:comment xml:lang="en">The preparation technique(s) applied to a surface composition.</rdfs:comment>
        <rdfs:range rdf:resource="http://www.project-best.eu/owl/aixm-mod/airportheliport#CodeSurfacePreparationType"/>
        <rdfs:domain rdf:resource="http://www.project-best.eu/owl/aixm-mod/airportheliport#SurfaceCharacteristics"/>
    </owl:ObjectProperty>
    


    <!-- http://www.project-best.eu/owl/aixm-mod/airportheliport#SurfaceCharacteristics-surfaceCondition -->

    <owl:ObjectProperty rdf:about="http://www.project-best.eu/owl/aixm-mod/airportheliport#SurfaceCharacteristics-surfaceCondition">
        <rdfs:comment xml:lang="en">The quality of the surface, as a category.</rdfs:comment>
        <rdfs:range rdf:resource="http://www.project-best.eu/owl/aixm-mod/airportheliport#CodeSurfaceConditionType"/>
        <rdfs:domain rdf:resource="http://www.project-best.eu/owl/aixm-mod/airportheliport#SurfaceCharacteristics"/>
    </owl:ObjectProperty>
    


    <!-- http://www.project-best.eu/owl/aixm-mod/airportheliport#SurfaceContamination-criticalRidge -->

    <owl:ObjectProperty rdf:about="http://www.project-best.eu/owl/aixm-mod/airportheliport#SurfaceContamination-criticalRidge">
        <rdfs:comment xml:lang="en">Identifies the critical bank associated to the contaminant.</rdfs:comment>
        <rdfs:range rdf:resource="http://www.project-best.eu/owl/aixm-mod/airportheliport#Ridge"/>
        <rdfs:domain rdf:resource="http://www.project-best.eu/owl/aixm-mod/airportheliport#SurfaceContamination"/>
    </owl:ObjectProperty>
    


    <!-- http://www.project-best.eu/owl/aixm-mod/airportheliport#SurfaceContamination-frictionDevice -->

    <owl:ObjectProperty rdf:about="http://www.project-best.eu/owl/aixm-mod/airportheliport#SurfaceContamination-frictionDevice">
        <rdfs:comment xml:lang="en">The type of equipment used to determine the reported friction coefficient.</rdfs:comment>
        <rdfs:range rdf:resource="http://www.project-best.eu/owl/aixm-mod/airportheliport#CodeFrictionDeviceType"/>
        <rdfs:domain rdf:resource="http://www.project-best.eu/owl/aixm-mod/airportheliport#SurfaceContamination"/>
    </owl:ObjectProperty>
    


    <!-- http://www.project-best.eu/owl/aixm-mod/airportheliport#SurfaceContamination-frictionEstimation -->

    <owl:ObjectProperty rdf:about="http://www.project-best.eu/owl/aixm-mod/airportheliport#SurfaceContamination-frictionEstimation">
        <rdfs:comment xml:lang="en">A qualitative estimate of the friction.</rdfs:comment>
        <rdfs:range rdf:resource="http://www.project-best.eu/owl/aixm-mod/airportheliport#CodeFrictionEstimateType"/>
        <rdfs:domain rdf:resource="http://www.project-best.eu/owl/aixm-mod/airportheliport#SurfaceContamination"/>
    </owl:ObjectProperty>
    


    <!-- http://www.project-best.eu/owl/aixm-mod/airportheliport#SurfaceContamination-layer -->

    <owl:ObjectProperty rdf:about="http://www.project-best.eu/owl/aixm-mod/airportheliport#SurfaceContamination-layer">
        <rdfs:domain rdf:resource="http://www.project-best.eu/owl/aixm-mod/airportheliport#SurfaceContamination"/>
        <rdfs:range rdf:resource="http://www.project-best.eu/owl/aixm-mod/airportheliport#SurfaceContaminationLayer"/>
    </owl:ObjectProperty>
    


    <!-- http://www.project-best.eu/owl/aixm-mod/airportheliport#SurfaceContaminationLayer-extent -->

    <owl:ObjectProperty rdf:about="http://www.project-best.eu/owl/aixm-mod/airportheliport#SurfaceContaminationLayer-extent">
        <rdfs:comment xml:lang="en">Association to Geometry::ElevatedSurface</rdfs:comment>
        <rdfs:comment xml:lang="en">The surface covered by the contamination.  For runways this can be a runway third, such as in the current SNOWTAM reporting style..</rdfs:comment>
        <rdfs:domain rdf:resource="http://www.project-best.eu/owl/aixm-mod/airportheliport#SurfaceContaminationLayer"/>
    </owl:ObjectProperty>
    


    <!-- http://www.project-best.eu/owl/aixm-mod/airportheliport#SurfaceContaminationLayer-type -->

    <owl:ObjectProperty rdf:about="http://www.project-best.eu/owl/aixm-mod/airportheliport#SurfaceContaminationLayer-type">
        <rdfs:comment xml:lang="en">The type of contaminating substance on the movement area surface.</rdfs:comment>
        <rdfs:range rdf:resource="http://www.project-best.eu/owl/aixm-mod/airportheliport#CodeContaminationType"/>
        <rdfs:domain rdf:resource="http://www.project-best.eu/owl/aixm-mod/airportheliport#SurfaceContaminationLayer"/>
    </owl:ObjectProperty>
    


    <!-- http://www.project-best.eu/owl/aixm-mod/airportheliport#SurveyControlPoint-associatedAirportHeliport -->

    <owl:ObjectProperty rdf:about="http://www.project-best.eu/owl/aixm-mod/airportheliport#SurveyControlPoint-associatedAirportHeliport">
        <rdfs:comment xml:lang="en">Identifies the Airport at which the Survey Control Point is located.</rdfs:comment>
        <rdfs:range rdf:resource="http://www.project-best.eu/owl/aixm-mod/airportheliport#AirportHeliport"/>
        <rdfs:domain rdf:resource="http://www.project-best.eu/owl/aixm-mod/airportheliport#SurveyControlPoint"/>
    </owl:ObjectProperty>
    


    <!-- http://www.project-best.eu/owl/aixm-mod/airportheliport#SurveyControlPoint-location -->

    <owl:ObjectProperty rdf:about="http://www.project-best.eu/owl/aixm-mod/airportheliport#SurveyControlPoint-location">
        <rdfs:comment xml:lang="en">Association to Geometry::ElevatedPoint</rdfs:comment>
        <rdfs:comment xml:lang="en">Identifies the geospatial location of the Survey Control Point.</rdfs:comment>
        <rdfs:domain rdf:resource="http://www.project-best.eu/owl/aixm-mod/airportheliport#SurveyControlPoint"/>
    </owl:ObjectProperty>
    


    <!-- http://www.project-best.eu/owl/aixm-mod/airportheliport#TaxiHoldingPosition-associatedGuidenceLine -->

    <owl:ObjectProperty rdf:about="http://www.project-best.eu/owl/aixm-mod/airportheliport#TaxiHoldingPosition-associatedGuidenceLine">
        <rdfs:range rdf:resource="http://www.project-best.eu/owl/aixm-mod/airportheliport#GuidanceLine"/>
        <rdfs:domain rdf:resource="http://www.project-best.eu/owl/aixm-mod/airportheliport#TaxiHoldingPosition"/>
    </owl:ObjectProperty>
    


    <!-- http://www.project-best.eu/owl/aixm-mod/airportheliport#TaxiHoldingPosition-landingCategory -->

    <owl:ObjectProperty rdf:about="http://www.project-best.eu/owl/aixm-mod/airportheliport#TaxiHoldingPosition-landingCategory">
        <rdfs:comment xml:lang="en">Type of landing operations for which that holding position is relevant. For example, precision cat I, precision cat II, precision cat III.</rdfs:comment>
        <rdfs:range rdf:resource="http://www.project-best.eu/owl/aixm-mod/airportheliport#CodeHoldingCategoryType"/>
        <rdfs:domain rdf:resource="http://www.project-best.eu/owl/aixm-mod/airportheliport#TaxiHoldingPosition"/>
    </owl:ObjectProperty>
    


    <!-- http://www.project-best.eu/owl/aixm-mod/airportheliport#TaxiHoldingPosition-location -->

    <owl:ObjectProperty rdf:about="http://www.project-best.eu/owl/aixm-mod/airportheliport#TaxiHoldingPosition-location">
        <rdfs:comment xml:lang="en">Association to Geometry::ElevatedPoint</rdfs:comment>
        <rdfs:domain rdf:resource="http://www.project-best.eu/owl/aixm-mod/airportheliport#TaxiHoldingPosition"/>
    </owl:ObjectProperty>
    


    <!-- http://www.project-best.eu/owl/aixm-mod/airportheliport#TaxiHoldingPosition-protectedRunway -->

    <owl:ObjectProperty rdf:about="http://www.project-best.eu/owl/aixm-mod/airportheliport#TaxiHoldingPosition-protectedRunway">
        <rdfs:comment xml:lang="en">(DO272/ED99) The value of a TaxiwayHoldingPosition feature?s attribute idp shall be identical to the idrwy object identifier value of the protected real world runway (Rule 6).</rdfs:comment>
        <rdfs:range rdf:resource="http://www.project-best.eu/owl/aixm-mod/airportheliport#Runway"/>
        <rdfs:domain rdf:resource="http://www.project-best.eu/owl/aixm-mod/airportheliport#TaxiHoldingPosition"/>
    </owl:ObjectProperty>
    


    <!-- http://www.project-best.eu/owl/aixm-mod/airportheliport#TaxiHoldingPosition-status -->

    <owl:ObjectProperty rdf:about="http://www.project-best.eu/owl/aixm-mod/airportheliport#TaxiHoldingPosition-status">
        <rdfs:comment xml:lang="en">A code indicating the operational status of the holding position.</rdfs:comment>
        <rdfs:range rdf:resource="http://www.project-best.eu/owl/aixm-mod/airportheliport#CodeStatusOperationsType"/>
        <rdfs:domain rdf:resource="http://www.project-best.eu/owl/aixm-mod/airportheliport#TaxiHoldingPosition"/>
    </owl:ObjectProperty>
    


    <!-- http://www.project-best.eu/owl/aixm-mod/airportheliport#TaxiHoldingPositionLightSystem-taxiHolding -->

    <owl:ObjectProperty rdf:about="http://www.project-best.eu/owl/aixm-mod/airportheliport#TaxiHoldingPositionLightSystem-taxiHolding">
        <rdfs:comment xml:lang="en">Identifies the Taxi Holding Position for which the Lighting System is provided.</rdfs:comment>
        <rdfs:range rdf:resource="http://www.project-best.eu/owl/aixm-mod/airportheliport#TaxiHoldingPosition"/>
        <rdfs:domain rdf:resource="http://www.project-best.eu/owl/aixm-mod/airportheliport#TaxiHoldingPositionLightSystem"/>
    </owl:ObjectProperty>
    


    <!-- http://www.project-best.eu/owl/aixm-mod/airportheliport#TaxiHoldingPositionLightSystem-type -->

    <owl:ObjectProperty rdf:about="http://www.project-best.eu/owl/aixm-mod/airportheliport#TaxiHoldingPositionLightSystem-type">
        <rdfs:comment xml:lang="en">The kind of lighting aid provided for the taxiway holding position.</rdfs:comment>
        <rdfs:range rdf:resource="http://www.project-best.eu/owl/aixm-mod/airportheliport#CodeLightHoldingPositionType"/>
        <rdfs:domain rdf:resource="http://www.project-best.eu/owl/aixm-mod/airportheliport#TaxiHoldingPositionLightSystem"/>
    </owl:ObjectProperty>
    


    <!-- http://www.project-best.eu/owl/aixm-mod/airportheliport#TaxiHoldingPositionMarking-markedTaxiHold -->

    <owl:ObjectProperty rdf:about="http://www.project-best.eu/owl/aixm-mod/airportheliport#TaxiHoldingPositionMarking-markedTaxiHold">
        <rdfs:comment xml:lang="en">Identifies the Taxi Holding Position that is marked.</rdfs:comment>
        <rdfs:range rdf:resource="http://www.project-best.eu/owl/aixm-mod/airportheliport#TaxiHoldingPosition"/>
        <rdfs:domain rdf:resource="http://www.project-best.eu/owl/aixm-mod/airportheliport#TaxiHoldingPositionMarking"/>
    </owl:ObjectProperty>
    


    <!-- http://www.project-best.eu/owl/aixm-mod/airportheliport#Taxiway-associatedAirportHeliport -->

    <owl:ObjectProperty rdf:about="http://www.project-best.eu/owl/aixm-mod/airportheliport#Taxiway-associatedAirportHeliport">
        <rdfs:comment xml:lang="en">Identifies the Airport where the Taxiway is situated.</rdfs:comment>
        <rdfs:range rdf:resource="http://www.project-best.eu/owl/aixm-mod/airportheliport#AirportHeliport"/>
        <rdfs:domain rdf:resource="http://www.project-best.eu/owl/aixm-mod/airportheliport#Taxiway"/>
    </owl:ObjectProperty>
    


    <!-- http://www.project-best.eu/owl/aixm-mod/airportheliport#Taxiway-availability -->

    <owl:ObjectProperty rdf:about="http://www.project-best.eu/owl/aixm-mod/airportheliport#Taxiway-availability">
        <rdfs:range rdf:resource="http://www.project-best.eu/owl/aixm-mod/airportheliport#ManoeuvringAreaAvailability"/>
        <rdfs:domain rdf:resource="http://www.project-best.eu/owl/aixm-mod/airportheliport#Taxiway"/>
    </owl:ObjectProperty>
    


    <!-- http://www.project-best.eu/owl/aixm-mod/airportheliport#Taxiway-contaminant -->

    <owl:ObjectProperty rdf:about="http://www.project-best.eu/owl/aixm-mod/airportheliport#Taxiway-contaminant">
        <rdfs:comment xml:lang="en">Identifies the contaminant of the taxiway.</rdfs:comment>
        <rdfs:domain rdf:resource="http://www.project-best.eu/owl/aixm-mod/airportheliport#Taxiway"/>
        <rdfs:range rdf:resource="http://www.project-best.eu/owl/aixm-mod/airportheliport#TaxiwayContamination"/>
    </owl:ObjectProperty>
    


    <!-- http://www.project-best.eu/owl/aixm-mod/airportheliport#Taxiway-surfaceProperties -->

    <owl:ObjectProperty rdf:about="http://www.project-best.eu/owl/aixm-mod/airportheliport#Taxiway-surfaceProperties">
        <rdfs:comment xml:lang="en">Identifies the surface characteristics of the taxiway.</rdfs:comment>
        <rdfs:range rdf:resource="http://www.project-best.eu/owl/aixm-mod/airportheliport#SurfaceCharacteristics"/>
        <rdfs:domain rdf:resource="http://www.project-best.eu/owl/aixm-mod/airportheliport#Taxiway"/>
    </owl:ObjectProperty>
    


    <!-- http://www.project-best.eu/owl/aixm-mod/airportheliport#Taxiway-type -->

    <owl:ObjectProperty rdf:about="http://www.project-best.eu/owl/aixm-mod/airportheliport#Taxiway-type">
        <rdfs:comment xml:lang="en">A code indicating a type of taxiway. For example: air taxiway, ground exit/turnoff, rapid exit/turnoff, stub, turn around, etc.</rdfs:comment>
        <rdfs:range rdf:resource="http://www.project-best.eu/owl/aixm-mod/airportheliport#CodeTaxiwayType"/>
        <rdfs:domain rdf:resource="http://www.project-best.eu/owl/aixm-mod/airportheliport#Taxiway"/>
    </owl:ObjectProperty>
    


    <!-- http://www.project-best.eu/owl/aixm-mod/airportheliport#TaxiwayElement-availability -->

    <owl:ObjectProperty rdf:about="http://www.project-best.eu/owl/aixm-mod/airportheliport#TaxiwayElement-availability">
        <rdfs:range rdf:resource="http://www.project-best.eu/owl/aixm-mod/airportheliport#ManoeuvringAreaAvailability"/>
        <rdfs:domain rdf:resource="http://www.project-best.eu/owl/aixm-mod/airportheliport#TaxiwayElement"/>
    </owl:ObjectProperty>
    


    <!-- http://www.project-best.eu/owl/aixm-mod/airportheliport#TaxiwayElement-extent -->

    <owl:ObjectProperty rdf:about="http://www.project-best.eu/owl/aixm-mod/airportheliport#TaxiwayElement-extent">
        <rdfs:comment xml:lang="en">Association to Geometry::ElevatedSurface</rdfs:comment>
        <rdfs:comment xml:lang="en">Identifies the extent of the taxiway element.</rdfs:comment>
        <rdfs:domain rdf:resource="http://www.project-best.eu/owl/aixm-mod/airportheliport#TaxiwayElement"/>
    </owl:ObjectProperty>
    


    <!-- http://www.project-best.eu/owl/aixm-mod/airportheliport#TaxiwayElement-gradeSeparation -->

    <owl:ObjectProperty rdf:about="http://www.project-best.eu/owl/aixm-mod/airportheliport#TaxiwayElement-gradeSeparation">
        <rdfs:comment xml:lang="en">A code that indicates the placement of the element at a different height from another element.</rdfs:comment>
        <rdfs:range rdf:resource="http://www.project-best.eu/owl/aixm-mod/airportheliport#CodeGradeSeparationType"/>
        <rdfs:domain rdf:resource="http://www.project-best.eu/owl/aixm-mod/airportheliport#TaxiwayElement"/>
    </owl:ObjectProperty>
    


    <!-- http://www.project-best.eu/owl/aixm-mod/airportheliport#TaxiwayElement-surfaceProperties -->

    <owl:ObjectProperty rdf:about="http://www.project-best.eu/owl/aixm-mod/airportheliport#TaxiwayElement-surfaceProperties">
        <rdfs:comment xml:lang="en">Identifies the surface characteristics of the taxiway element.</rdfs:comment>
        <rdfs:range rdf:resource="http://www.project-best.eu/owl/aixm-mod/airportheliport#SurfaceCharacteristics"/>
        <rdfs:domain rdf:resource="http://www.project-best.eu/owl/aixm-mod/airportheliport#TaxiwayElement"/>
    </owl:ObjectProperty>
    


    <!-- http://www.project-best.eu/owl/aixm-mod/airportheliport#TaxiwayElement-type -->

    <owl:ObjectProperty rdf:about="http://www.project-best.eu/owl/aixm-mod/airportheliport#TaxiwayElement-type">
        <rdfs:comment xml:lang="en">The type of element.</rdfs:comment>
        <rdfs:range rdf:resource="http://www.project-best.eu/owl/aixm-mod/airportheliport#CodeTaxiwayElementType"/>
        <rdfs:domain rdf:resource="http://www.project-best.eu/owl/aixm-mod/airportheliport#TaxiwayElement"/>
    </owl:ObjectProperty>
    


    <!-- http://www.project-best.eu/owl/aixm-mod/airportheliport#TaxiwayLightSystem-lightedTaxiway -->

    <owl:ObjectProperty rdf:about="http://www.project-best.eu/owl/aixm-mod/airportheliport#TaxiwayLightSystem-lightedTaxiway">
        <rdfs:comment xml:lang="en">Identifies the Taxiway for which the Lighting System is provided.</rdfs:comment>
        <rdfs:range rdf:resource="http://www.project-best.eu/owl/aixm-mod/airportheliport#Taxiway"/>
        <rdfs:domain rdf:resource="http://www.project-best.eu/owl/aixm-mod/airportheliport#TaxiwayLightSystem"/>
    </owl:ObjectProperty>
    


    <!-- http://www.project-best.eu/owl/aixm-mod/airportheliport#TaxiwayLightSystem-position -->

    <owl:ObjectProperty rdf:about="http://www.project-best.eu/owl/aixm-mod/airportheliport#TaxiwayLightSystem-position">
        <rdfs:comment xml:lang="en">A code indicating the part of the TWY surface the lighting system is serving.</rdfs:comment>
        <rdfs:range rdf:resource="http://www.project-best.eu/owl/aixm-mod/airportheliport#CodeTaxiwaySectionType"/>
        <rdfs:domain rdf:resource="http://www.project-best.eu/owl/aixm-mod/airportheliport#TaxiwayLightSystem"/>
    </owl:ObjectProperty>
    


    <!-- http://www.project-best.eu/owl/aixm-mod/airportheliport#TaxiwayMarking-markedElement -->

    <owl:ObjectProperty rdf:about="http://www.project-best.eu/owl/aixm-mod/airportheliport#TaxiwayMarking-markedElement">
        <rdfs:comment xml:lang="en">Identifies the taxiway element that is marked.</rdfs:comment>
        <rdfs:range rdf:resource="http://www.project-best.eu/owl/aixm-mod/airportheliport#TaxiwayElement"/>
        <rdfs:domain rdf:resource="http://www.project-best.eu/owl/aixm-mod/airportheliport#TaxiwayMarking"/>
    </owl:ObjectProperty>
    


    <!-- http://www.project-best.eu/owl/aixm-mod/airportheliport#TaxiwayMarking-markedTaxiway -->

    <owl:ObjectProperty rdf:about="http://www.project-best.eu/owl/aixm-mod/airportheliport#TaxiwayMarking-markedTaxiway">
        <rdfs:comment xml:lang="en">(DO272/ED99) The value of a TaxiwayGuidanceLine feature?s attribute idlin shall be identical to the value of the corresponding TaxiwayElement feature?s attribute idlin (Rule 10).</rdfs:comment>
        <rdfs:range rdf:resource="http://www.project-best.eu/owl/aixm-mod/airportheliport#Taxiway"/>
        <rdfs:domain rdf:resource="http://www.project-best.eu/owl/aixm-mod/airportheliport#TaxiwayMarking"/>
    </owl:ObjectProperty>
    


    <!-- http://www.project-best.eu/owl/aixm-mod/airportheliport#TaxiwayMarking-markingLocation -->

    <owl:ObjectProperty rdf:about="http://www.project-best.eu/owl/aixm-mod/airportheliport#TaxiwayMarking-markingLocation">
        <rdfs:comment xml:lang="en">A code indicating the location of the marking relative to the surface.</rdfs:comment>
        <rdfs:range rdf:resource="http://www.project-best.eu/owl/aixm-mod/airportheliport#CodeTaxiwaySectionType"/>
        <rdfs:domain rdf:resource="http://www.project-best.eu/owl/aixm-mod/airportheliport#TaxiwayMarking"/>
    </owl:ObjectProperty>
    


    <!-- http://www.project-best.eu/owl/aixm-mod/airportheliport#TouchDownLiftOff-aimingPoint -->

    <owl:ObjectProperty rdf:about="http://www.project-best.eu/owl/aixm-mod/airportheliport#TouchDownLiftOff-aimingPoint">
        <rdfs:comment xml:lang="en">Association to Geometry::ElevatedPoint</rdfs:comment>
        <rdfs:comment xml:lang="en">Locates the aiming point of the TLOF.</rdfs:comment>
        <rdfs:domain rdf:resource="http://www.project-best.eu/owl/aixm-mod/airportheliport#TouchDownLiftOff"/>
    </owl:ObjectProperty>
    


    <!-- http://www.project-best.eu/owl/aixm-mod/airportheliport#TouchDownLiftOff-approachTakeOffArea -->

    <owl:ObjectProperty rdf:about="http://www.project-best.eu/owl/aixm-mod/airportheliport#TouchDownLiftOff-approachTakeOffArea">
        <rdfs:comment xml:lang="en">Only for runways of type FATO</rdfs:comment>
        <rdfs:range rdf:resource="http://www.project-best.eu/owl/aixm-mod/airportheliport#Runway"/>
        <rdfs:domain rdf:resource="http://www.project-best.eu/owl/aixm-mod/airportheliport#TouchDownLiftOff"/>
    </owl:ObjectProperty>
    


    <!-- http://www.project-best.eu/owl/aixm-mod/airportheliport#TouchDownLiftOff-associatedAirportHeliport -->

    <owl:ObjectProperty rdf:about="http://www.project-best.eu/owl/aixm-mod/airportheliport#TouchDownLiftOff-associatedAirportHeliport">
        <rdfs:comment xml:lang="en">Identifies the Airport where the Touch Down Lift Off is situated.</rdfs:comment>
        <rdfs:range rdf:resource="http://www.project-best.eu/owl/aixm-mod/airportheliport#AirportHeliport"/>
        <rdfs:domain rdf:resource="http://www.project-best.eu/owl/aixm-mod/airportheliport#TouchDownLiftOff"/>
    </owl:ObjectProperty>
    


    <!-- http://www.project-best.eu/owl/aixm-mod/airportheliport#TouchDownLiftOff-availability -->

    <owl:ObjectProperty rdf:about="http://www.project-best.eu/owl/aixm-mod/airportheliport#TouchDownLiftOff-availability">
        <rdfs:range rdf:resource="http://www.project-best.eu/owl/aixm-mod/airportheliport#ManoeuvringAreaAvailability"/>
        <rdfs:domain rdf:resource="http://www.project-best.eu/owl/aixm-mod/airportheliport#TouchDownLiftOff"/>
    </owl:ObjectProperty>
    


    <!-- http://www.project-best.eu/owl/aixm-mod/airportheliport#TouchDownLiftOff-contaminant -->

    <owl:ObjectProperty rdf:about="http://www.project-best.eu/owl/aixm-mod/airportheliport#TouchDownLiftOff-contaminant">
        <rdfs:comment xml:lang="en">Identifies the contaminant of the touch down lift off area.</rdfs:comment>
        <rdfs:domain rdf:resource="http://www.project-best.eu/owl/aixm-mod/airportheliport#TouchDownLiftOff"/>
        <rdfs:range rdf:resource="http://www.project-best.eu/owl/aixm-mod/airportheliport#TouchDownLiftOffContamination"/>
    </owl:ObjectProperty>
    


    <!-- http://www.project-best.eu/owl/aixm-mod/airportheliport#TouchDownLiftOff-extent -->

    <owl:ObjectProperty rdf:about="http://www.project-best.eu/owl/aixm-mod/airportheliport#TouchDownLiftOff-extent">
        <rdfs:comment xml:lang="en">Association to Geometry::ElevatedSurface</rdfs:comment>
        <rdfs:comment xml:lang="en">Identifies the surface area of the Touch Down Lift Off area.</rdfs:comment>
        <rdfs:domain rdf:resource="http://www.project-best.eu/owl/aixm-mod/airportheliport#TouchDownLiftOff"/>
    </owl:ObjectProperty>
    


    <!-- http://www.project-best.eu/owl/aixm-mod/airportheliport#TouchDownLiftOff-helicopterClass -->

    <owl:ObjectProperty rdf:about="http://www.project-best.eu/owl/aixm-mod/airportheliport#TouchDownLiftOff-helicopterClass">
        <rdfs:comment xml:lang="en">The class of a helicopter based on its performance during a critical power unit failure after take-off.</rdfs:comment>
        <rdfs:range rdf:resource="http://www.project-best.eu/owl/aixm-mod/airportheliport#CodeHelicopterPerformanceType"/>
        <rdfs:domain rdf:resource="http://www.project-best.eu/owl/aixm-mod/airportheliport#TouchDownLiftOff"/>
    </owl:ObjectProperty>
    


    <!-- http://www.project-best.eu/owl/aixm-mod/airportheliport#TouchDownLiftOff-isMarkedOn -->

    <owl:ObjectProperty rdf:about="http://www.project-best.eu/owl/aixm-mod/airportheliport#TouchDownLiftOff-isMarkedOn">
        <rdfs:domain rdf:resource="http://www.project-best.eu/owl/aixm-mod/airportheliport#TouchDownLiftOff"/>
        <rdfs:range rdf:resource="http://www.project-best.eu/owl/aixm-mod/airportheliport#TouchDownLiftOffMarking"/>
    </owl:ObjectProperty>
    


    <!-- http://www.project-best.eu/owl/aixm-mod/airportheliport#TouchDownLiftOff-isProvidedFor -->

    <owl:ObjectProperty rdf:about="http://www.project-best.eu/owl/aixm-mod/airportheliport#TouchDownLiftOff-isProvidedFor">
        <rdfs:domain rdf:resource="http://www.project-best.eu/owl/aixm-mod/airportheliport#TouchDownLiftOff"/>
        <rdfs:range rdf:resource="http://www.project-best.eu/owl/aixm-mod/airportheliport#TouchDownLiftOffLightSystem"/>
    </owl:ObjectProperty>
    


    <!-- http://www.project-best.eu/owl/aixm-mod/airportheliport#TouchDownLiftOff-surfaceProperties -->

    <owl:ObjectProperty rdf:about="http://www.project-best.eu/owl/aixm-mod/airportheliport#TouchDownLiftOff-surfaceProperties">
        <rdfs:comment xml:lang="en">Identifies the Surface Characteristics that describe the Touch Down Lift Off area.</rdfs:comment>
        <rdfs:range rdf:resource="http://www.project-best.eu/owl/aixm-mod/airportheliport#SurfaceCharacteristics"/>
        <rdfs:domain rdf:resource="http://www.project-best.eu/owl/aixm-mod/airportheliport#TouchDownLiftOff"/>
    </owl:ObjectProperty>
    


    <!-- http://www.project-best.eu/owl/aixm-mod/airportheliport#TouchDownLiftOffLightSystem-lightedTouchDownLiftOff -->

    <owl:ObjectProperty rdf:about="http://www.project-best.eu/owl/aixm-mod/airportheliport#TouchDownLiftOffLightSystem-lightedTouchDownLiftOff">
        <rdfs:comment xml:lang="en">Identifies the Touch Down Lift Off area for which the Lighting System is provided.</rdfs:comment>
        <rdfs:range rdf:resource="http://www.project-best.eu/owl/aixm-mod/airportheliport#TouchDownLiftOff"/>
        <rdfs:domain rdf:resource="http://www.project-best.eu/owl/aixm-mod/airportheliport#TouchDownLiftOffLightSystem"/>
    </owl:ObjectProperty>
    


    <!-- http://www.project-best.eu/owl/aixm-mod/airportheliport#TouchDownLiftOffLightSystem-position -->

    <owl:ObjectProperty rdf:about="http://www.project-best.eu/owl/aixm-mod/airportheliport#TouchDownLiftOffLightSystem-position">
        <rdfs:comment xml:lang="en">A code indicating the part of the TLOF surface the lighting system is serving.</rdfs:comment>
        <rdfs:range rdf:resource="http://www.project-best.eu/owl/aixm-mod/airportheliport#CodeTLOFSectionType"/>
        <rdfs:domain rdf:resource="http://www.project-best.eu/owl/aixm-mod/airportheliport#TouchDownLiftOffLightSystem"/>
    </owl:ObjectProperty>
    


    <!-- http://www.project-best.eu/owl/aixm-mod/airportheliport#TouchDownLiftOffMarking-markedTouchDownLiftOff -->

    <owl:ObjectProperty rdf:about="http://www.project-best.eu/owl/aixm-mod/airportheliport#TouchDownLiftOffMarking-markedTouchDownLiftOff">
        <rdfs:comment xml:lang="en">Identifies the Touch Down Lift Off area that is marked.</rdfs:comment>
        <rdfs:range rdf:resource="http://www.project-best.eu/owl/aixm-mod/airportheliport#TouchDownLiftOff"/>
        <rdfs:domain rdf:resource="http://www.project-best.eu/owl/aixm-mod/airportheliport#TouchDownLiftOffMarking"/>
    </owl:ObjectProperty>
    


    <!-- http://www.project-best.eu/owl/aixm-mod/airportheliport#TouchDownLiftOffMarking-markingLocation -->

    <owl:ObjectProperty rdf:about="http://www.project-best.eu/owl/aixm-mod/airportheliport#TouchDownLiftOffMarking-markingLocation">
        <rdfs:comment xml:lang="en">A code indicating the location of the marking relative to the surface.</rdfs:comment>
        <rdfs:range rdf:resource="http://www.project-best.eu/owl/aixm-mod/airportheliport#CodeTLOFSectionType"/>
        <rdfs:domain rdf:resource="http://www.project-best.eu/owl/aixm-mod/airportheliport#TouchDownLiftOffMarking"/>
    </owl:ObjectProperty>
    


    <!-- http://www.project-best.eu/owl/aixm-mod/airportheliport#TouchDownLiftOffSafeArea-protectedTouchDownLiftOff -->

    <owl:ObjectProperty rdf:about="http://www.project-best.eu/owl/aixm-mod/airportheliport#TouchDownLiftOffSafeArea-protectedTouchDownLiftOff">
        <rdfs:comment xml:lang="en">Identifies the Touch Down Lift Off area that is protected by the Safe Area.</rdfs:comment>
        <rdfs:range rdf:resource="http://www.project-best.eu/owl/aixm-mod/airportheliport#TouchDownLiftOff"/>
        <rdfs:domain rdf:resource="http://www.project-best.eu/owl/aixm-mod/airportheliport#TouchDownLiftOffSafeArea"/>
    </owl:ObjectProperty>
    


    <!-- http://www.project-best.eu/owl/aixm-mod/airportheliport#UsageCondition-contact -->

    <owl:ObjectProperty rdf:about="http://www.project-best.eu/owl/aixm-mod/airportheliport#UsageCondition-contact">
        <rdfs:comment xml:lang="en">Association to Shared::Address:ContactInformation</rdfs:comment>
        <rdfs:domain rdf:resource="http://www.project-best.eu/owl/aixm-mod/airportheliport#UsageCondition"/>
    </owl:ObjectProperty>
    


    <!-- http://www.project-best.eu/owl/aixm-mod/airportheliport#UsageCondition-selection -->

    <owl:ObjectProperty rdf:about="http://www.project-best.eu/owl/aixm-mod/airportheliport#UsageCondition-selection">
        <rdfs:range rdf:resource="http://www.project-best.eu/owl/aixm-mod/airportheliport#ConditionCombination"/>
        <rdfs:domain rdf:resource="http://www.project-best.eu/owl/aixm-mod/airportheliport#UsageCondition"/>
    </owl:ObjectProperty>
    


    <!-- http://www.project-best.eu/owl/aixm-mod/airportheliport#UsageCondition-type -->

    <owl:ObjectProperty rdf:about="http://www.project-best.eu/owl/aixm-mod/airportheliport#UsageCondition-type">
        <rdfs:comment xml:lang="en">A code indicating whether the limitation is a permission or an interdiction.</rdfs:comment>
        <rdfs:range rdf:resource="http://www.project-best.eu/owl/aixm-mod/airportheliport#CodeUsageLimitationType"/>
        <rdfs:domain rdf:resource="http://www.project-best.eu/owl/aixm-mod/airportheliport#UsageCondition"/>
    </owl:ObjectProperty>
    


    <!-- http://www.project-best.eu/owl/aixm-mod/airportheliport#VisualGlideSlopeIndicator-position -->

    <owl:ObjectProperty rdf:about="http://www.project-best.eu/owl/aixm-mod/airportheliport#VisualGlideSlopeIndicator-position">
        <rdfs:comment xml:lang="en">A code describing a position, relative to the centreline, of the visual approach slope indicator for a FATO/RWY direction.</rdfs:comment>
        <rdfs:range rdf:resource="http://www.project-best.eu/owl/aixm-mod/airportheliport#CodeSideType"/>
        <rdfs:domain rdf:resource="http://www.project-best.eu/owl/aixm-mod/airportheliport#VisualGlideSlopeIndicator"/>
    </owl:ObjectProperty>
    


    <!-- http://www.project-best.eu/owl/aixm-mod/airportheliport#VisualGlideSlopeIndicator-runwayDirection -->

    <owl:ObjectProperty rdf:about="http://www.project-best.eu/owl/aixm-mod/airportheliport#VisualGlideSlopeIndicator-runwayDirection">
        <rdfs:comment xml:lang="en">Identifies the Runway Direction for which the Visual Glide Slope Indicator provides guidance for.</rdfs:comment>
        <rdfs:range rdf:resource="http://www.project-best.eu/owl/aixm-mod/airportheliport#RunwayDirection"/>
        <rdfs:domain rdf:resource="http://www.project-best.eu/owl/aixm-mod/airportheliport#VisualGlideSlopeIndicator"/>
    </owl:ObjectProperty>
    


    <!-- http://www.project-best.eu/owl/aixm-mod/airportheliport#VisualGlideSlopeIndicator-type -->

    <owl:ObjectProperty rdf:about="http://www.project-best.eu/owl/aixm-mod/airportheliport#VisualGlideSlopeIndicator-type">
        <rdfs:comment xml:lang="en">A code indicating the type of the visual approach slope indicator system.</rdfs:comment>
        <rdfs:range rdf:resource="http://www.project-best.eu/owl/aixm-mod/airportheliport#CodeVASISType"/>
        <rdfs:domain rdf:resource="http://www.project-best.eu/owl/aixm-mod/airportheliport#VisualGlideSlopeIndicator"/>
    </owl:ObjectProperty>
    


    <!-- http://www.project-best.eu/owl/aixm-mod/airportheliport#WorkArea-activation -->

    <owl:ObjectProperty rdf:about="http://www.project-best.eu/owl/aixm-mod/airportheliport#WorkArea-activation">
        <rdfs:domain rdf:resource="http://www.project-best.eu/owl/aixm-mod/airportheliport#WorkArea"/>
        <rdfs:range rdf:resource="http://www.project-best.eu/owl/aixm-mod/airportheliport#WorkAreaActivity"/>
    </owl:ObjectProperty>
    


    <!-- http://www.project-best.eu/owl/aixm-mod/airportheliport#WorkArea-associatedAirportHeliport -->

    <owl:ObjectProperty rdf:about="http://www.project-best.eu/owl/aixm-mod/airportheliport#WorkArea-associatedAirportHeliport">
        <rdfs:comment xml:lang="en">Identifies the Airport where the Work Area is situated.</rdfs:comment>
        <rdfs:range rdf:resource="http://www.project-best.eu/owl/aixm-mod/airportheliport#AirportHeliport"/>
        <rdfs:domain rdf:resource="http://www.project-best.eu/owl/aixm-mod/airportheliport#WorkArea"/>
    </owl:ObjectProperty>
    


    <!-- http://www.project-best.eu/owl/aixm-mod/airportheliport#WorkArea-extent -->

    <owl:ObjectProperty rdf:about="http://www.project-best.eu/owl/aixm-mod/airportheliport#WorkArea-extent">
        <rdfs:comment xml:lang="en">Association to Geometry::ElevatedSurface
</rdfs:comment>
        <rdfs:domain rdf:resource="http://www.project-best.eu/owl/aixm-mod/airportheliport#WorkArea"/>
    </owl:ObjectProperty>
    


    <!-- http://www.project-best.eu/owl/aixm-mod/airportheliport#WorkArea-type -->

    <owl:ObjectProperty rdf:about="http://www.project-best.eu/owl/aixm-mod/airportheliport#WorkArea-type">
        <rdfs:comment xml:lang="en">The type of work performed in the work area.</rdfs:comment>
        <rdfs:range rdf:resource="http://www.project-best.eu/owl/aixm-mod/airportheliport#CodeWorkAreaType"/>
        <rdfs:domain rdf:resource="http://www.project-best.eu/owl/aixm-mod/airportheliport#WorkArea"/>
    </owl:ObjectProperty>
    


    <!-- 
    ///////////////////////////////////////////////////////////////////////////////////////
    //
    // Data properties
    //
    ///////////////////////////////////////////////////////////////////////////////////////
     -->

    


    <!-- http://www.project-best.eu/owl/aixm-mod/airportheliport#AirportHeliport-certificationDate -->

    <owl:DatatypeProperty rdf:about="http://www.project-best.eu/owl/aixm-mod/airportheliport#AirportHeliport-certificationDate">
        <rdfs:comment xml:lang="en">Range should be W3C Time</rdfs:comment>
        <rdfs:comment xml:lang="en">The date when the airport certification has been issued by the supervising authority.</rdfs:comment>
        <rdfs:domain rdf:resource="http://www.project-best.eu/owl/aixm-mod/airportheliport#AirportHeliport"/>
        <rdfs:range rdf:resource="http://www.w3.org/2001/XMLSchema#string"/>
    </owl:DatatypeProperty>
    


    <!-- http://www.project-best.eu/owl/aixm-mod/airportheliport#AirportHeliport-certificationExpirationDate -->

    <owl:DatatypeProperty rdf:about="http://www.project-best.eu/owl/aixm-mod/airportheliport#AirportHeliport-certificationExpirationDate">
        <rdfs:comment xml:lang="en">Range should be W3C Time</rdfs:comment>
        <rdfs:comment xml:lang="en">The date when the airport certification will become invalid.</rdfs:comment>
        <rdfs:domain rdf:resource="http://www.project-best.eu/owl/aixm-mod/airportheliport#AirportHeliport"/>
        <rdfs:range rdf:resource="http://www.w3.org/2001/XMLSchema#string"/>
    </owl:DatatypeProperty>
    


    <!-- http://www.project-best.eu/owl/aixm-mod/airportheliport#AirportHeliport-dateMagneticVariation -->

    <owl:DatatypeProperty rdf:about="http://www.project-best.eu/owl/aixm-mod/airportheliport#AirportHeliport-dateMagneticVariation">
        <rdfs:comment xml:lang="en">Range should be W3C Time</rdfs:comment>
        <rdfs:comment xml:lang="en">The date on which the magnetic variation had this value.</rdfs:comment>
        <rdfs:domain rdf:resource="http://www.project-best.eu/owl/aixm-mod/airportheliport#AirportHeliport"/>
        <rdfs:range rdf:resource="http://www.w3.org/2001/XMLSchema#string"/>
    </owl:DatatypeProperty>
    


    <!-- http://www.project-best.eu/owl/aixm-mod/airportheliport#AirportHeliport-designator -->

    <owl:DatatypeProperty rdf:about="http://www.project-best.eu/owl/aixm-mod/airportheliport#AirportHeliport-designator">
        <rdfs:comment xml:lang="en">A coded designator for an Aerodrome/Heliport.</rdfs:comment>
        <rdfs:domain rdf:resource="http://www.project-best.eu/owl/aixm-mod/airportheliport#AirportHeliport"/>
        <rdfs:range rdf:resource="http://www.w3.org/2001/XMLSchema#string"/>
    </owl:DatatypeProperty>
    


    <!-- http://www.project-best.eu/owl/aixm-mod/airportheliport#AirportHeliport-designatorIATA -->

    <owl:DatatypeProperty rdf:about="http://www.project-best.eu/owl/aixm-mod/airportheliport#AirportHeliport-designatorIATA">
        <rdfs:comment xml:lang="en">The identifier that is assigned to a location in accordance with rules (resolution 767) governed by the International Air Transport Association (IATA).</rdfs:comment>
        <rdfs:domain rdf:resource="http://www.project-best.eu/owl/aixm-mod/airportheliport#AirportHeliport"/>
        <rdfs:range rdf:resource="http://www.w3.org/2001/XMLSchema#string"/>
    </owl:DatatypeProperty>
    


    <!-- http://www.project-best.eu/owl/aixm-mod/airportheliport#AirportHeliport-fieldElevation -->

    <owl:DatatypeProperty rdf:about="http://www.project-best.eu/owl/aixm-mod/airportheliport#AirportHeliport-fieldElevation">
        <rdfs:comment xml:lang="en">The vertical distance above Mean Sea Level (MSL) of the highest point of the landing area.</rdfs:comment>
        <rdfs:domain rdf:resource="http://www.project-best.eu/owl/aixm-mod/airportheliport#AirportHeliport"/>
        <rdfs:range rdf:resource="http://www.w3.org/2001/XMLSchema#decimal"/>
    </owl:DatatypeProperty>
    


    <!-- http://www.project-best.eu/owl/aixm-mod/airportheliport#AirportHeliport-fieldElevationAccuracy -->

    <owl:DatatypeProperty rdf:about="http://www.project-best.eu/owl/aixm-mod/airportheliport#AirportHeliport-fieldElevationAccuracy">
        <rdfs:comment xml:lang="en">The vertical distance from the stated elevation within which there is a defined confidence of the true position falling.</rdfs:comment>
        <rdfs:domain rdf:resource="http://www.project-best.eu/owl/aixm-mod/airportheliport#AirportHeliport"/>
        <rdfs:range rdf:resource="http://www.w3.org/2001/XMLSchema#decimal"/>
    </owl:DatatypeProperty>
    


    <!-- http://www.project-best.eu/owl/aixm-mod/airportheliport#AirportHeliport-locationIndicatorICAO -->

    <owl:DatatypeProperty rdf:about="http://www.project-best.eu/owl/aixm-mod/airportheliport#AirportHeliport-locationIndicatorICAO">
        <rdfs:comment xml:lang="en">The four letter ICAO location indicator of the aerodrome/heliport, as listed in ICAO DOC 7910.</rdfs:comment>
        <rdfs:domain rdf:resource="http://www.project-best.eu/owl/aixm-mod/airportheliport#AirportHeliport"/>
        <rdfs:range rdf:resource="http://www.w3.org/2001/XMLSchema#string"/>
    </owl:DatatypeProperty>
    


    <!-- http://www.project-best.eu/owl/aixm-mod/airportheliport#AirportHeliport-lowestTemperature -->

    <owl:DatatypeProperty rdf:about="http://www.project-best.eu/owl/aixm-mod/airportheliport#AirportHeliport-lowestTemperature">
        <rdfs:comment xml:lang="en">The mean lowest temperature of the coldest month of the year.</rdfs:comment>
        <rdfs:domain rdf:resource="http://www.project-best.eu/owl/aixm-mod/airportheliport#AirportHeliport"/>
        <rdfs:range rdf:resource="http://www.w3.org/2001/XMLSchema#decimal"/>
    </owl:DatatypeProperty>
    


    <!-- http://www.project-best.eu/owl/aixm-mod/airportheliport#AirportHeliport-magneticVariation -->

    <owl:DatatypeProperty rdf:about="http://www.project-best.eu/owl/aixm-mod/airportheliport#AirportHeliport-magneticVariation">
        <rdfs:comment xml:lang="en">The angular difference between True North and Magnetic North measured at a given position and date.</rdfs:comment>
        <rdfs:domain rdf:resource="http://www.project-best.eu/owl/aixm-mod/airportheliport#AirportHeliport"/>
        <rdfs:range rdf:resource="http://www.w3.org/2001/XMLSchema#decimal"/>
    </owl:DatatypeProperty>
    


    <!-- http://www.project-best.eu/owl/aixm-mod/airportheliport#AirportHeliport-magneticVariationAccuracy -->

    <owl:DatatypeProperty rdf:about="http://www.project-best.eu/owl/aixm-mod/airportheliport#AirportHeliport-magneticVariationAccuracy">
        <rdfs:comment xml:lang="en">The accuracy of the Magnetic Variation in angle degrees.</rdfs:comment>
        <rdfs:domain rdf:resource="http://www.project-best.eu/owl/aixm-mod/airportheliport#AirportHeliport"/>
        <rdfs:range rdf:resource="http://www.w3.org/2001/XMLSchema#decimal"/>
    </owl:DatatypeProperty>
    


    <!-- http://www.project-best.eu/owl/aixm-mod/airportheliport#AirportHeliport-magneticVariationChange -->

    <owl:DatatypeProperty rdf:about="http://www.project-best.eu/owl/aixm-mod/airportheliport#AirportHeliport-magneticVariationChange">
        <rdfs:comment xml:lang="en">The annual rate of change of the magnetic variation.</rdfs:comment>
        <rdfs:domain rdf:resource="http://www.project-best.eu/owl/aixm-mod/airportheliport#AirportHeliport"/>
        <rdfs:range rdf:resource="http://www.w3.org/2001/XMLSchema#decimal"/>
    </owl:DatatypeProperty>
    


    <!-- http://www.project-best.eu/owl/aixm-mod/airportheliport#AirportHeliport-name -->

    <owl:DatatypeProperty rdf:about="http://www.project-best.eu/owl/aixm-mod/airportheliport#AirportHeliport-name">
        <rdfs:comment xml:lang="en">The primary official name of an aerodrome as designated by an appropriate authority.</rdfs:comment>
        <rdfs:domain rdf:resource="http://www.project-best.eu/owl/aixm-mod/airportheliport#AirportHeliport"/>
        <rdfs:range rdf:resource="http://www.w3.org/2001/XMLSchema#string"/>
    </owl:DatatypeProperty>
    


    <!-- http://www.project-best.eu/owl/aixm-mod/airportheliport#AirportHeliport-referenceTemperature -->

    <owl:DatatypeProperty rdf:about="http://www.project-best.eu/owl/aixm-mod/airportheliport#AirportHeliport-referenceTemperature">
        <rdfs:comment xml:lang="en">The monthly mean of the daily maximum temperatures for the hottest month of the year at an aerodrome.</rdfs:comment>
        <rdfs:domain rdf:resource="http://www.project-best.eu/owl/aixm-mod/airportheliport#AirportHeliport"/>
        <rdfs:range rdf:resource="http://www.w3.org/2001/XMLSchema#decimal"/>
    </owl:DatatypeProperty>
    


    <!-- http://www.project-best.eu/owl/aixm-mod/airportheliport#AirportHeliport-transitionAltitude -->

    <owl:DatatypeProperty rdf:about="http://www.project-best.eu/owl/aixm-mod/airportheliport#AirportHeliport-transitionAltitude">
        <rdfs:comment xml:lang="en">The altitude at or below which the vertical position of an aircraft is controlled by reference to altitudes.</rdfs:comment>
        <rdfs:domain rdf:resource="http://www.project-best.eu/owl/aixm-mod/airportheliport#AirportHeliport"/>
        <rdfs:range rdf:resource="http://www.w3.org/2001/XMLSchema#decimal"/>
    </owl:DatatypeProperty>
    


    <!-- http://www.project-best.eu/owl/aixm-mod/airportheliport#AirportHeliport-transitionLevel -->

    <owl:DatatypeProperty rdf:about="http://www.project-best.eu/owl/aixm-mod/airportheliport#AirportHeliport-transitionLevel">
        <rdfs:comment xml:lang="en">The lowest flight level available for use above the transition altitude.</rdfs:comment>
        <rdfs:domain rdf:resource="http://www.project-best.eu/owl/aixm-mod/airportheliport#AirportHeliport"/>
        <rdfs:range rdf:resource="http://www.w3.org/2001/XMLSchema#decimal"/>
    </owl:DatatypeProperty>
    


    <!-- http://www.project-best.eu/owl/aixm-mod/airportheliport#AirportHeliport-verticalDatum -->

    <owl:DatatypeProperty rdf:about="http://www.project-best.eu/owl/aixm-mod/airportheliport#AirportHeliport-verticalDatum">
        <rdfs:comment xml:lang="en">A reference surface with respect to which elevations and/or depths are specified.</rdfs:comment>
        <rdfs:comment xml:lang="en">Range should be W3C Time</rdfs:comment>
        <rdfs:domain rdf:resource="http://www.project-best.eu/owl/aixm-mod/airportheliport#AirportHeliport"/>
        <rdfs:range rdf:resource="http://www.w3.org/2001/XMLSchema#string"/>
    </owl:DatatypeProperty>
    


    <!-- http://www.project-best.eu/owl/aixm-mod/airportheliport#AirportHeliportProtectionArea-length -->

    <owl:DatatypeProperty rdf:about="http://www.project-best.eu/owl/aixm-mod/airportheliport#AirportHeliportProtectionArea-length">
        <rdfs:comment xml:lang="en">The value of the physical length of the protection area.</rdfs:comment>
        <rdfs:domain rdf:resource="http://www.project-best.eu/owl/aixm-mod/airportheliport#AirportHeliportProtectionArea"/>
        <rdfs:range rdf:resource="http://www.w3.org/2001/XMLSchema#decimal"/>
    </owl:DatatypeProperty>
    


    <!-- http://www.project-best.eu/owl/aixm-mod/airportheliport#AirportHeliportProtectionArea-width -->

    <owl:DatatypeProperty rdf:about="http://www.project-best.eu/owl/aixm-mod/airportheliport#AirportHeliportProtectionArea-width">
        <rdfs:comment xml:lang="en">The value of the physical width of the protection area.</rdfs:comment>
        <rdfs:domain rdf:resource="http://www.project-best.eu/owl/aixm-mod/airportheliport#AirportHeliportProtectionArea"/>
        <rdfs:range rdf:resource="http://www.w3.org/2001/XMLSchema#decimal"/>
    </owl:DatatypeProperty>
    


    <!-- http://www.project-best.eu/owl/aixm-mod/airportheliport#AirportHotSpot-designator -->

    <owl:DatatypeProperty rdf:about="http://www.project-best.eu/owl/aixm-mod/airportheliport#AirportHotSpot-designator">
        <rdfs:comment xml:lang="en">A coded identifier by which the hot spot is labelled on airport maps.</rdfs:comment>
        <rdfs:domain rdf:resource="http://www.project-best.eu/owl/aixm-mod/airportheliport#AirportHotSpot"/>
        <rdfs:range rdf:resource="http://www.w3.org/2001/XMLSchema#string"/>
    </owl:DatatypeProperty>
    


    <!-- http://www.project-best.eu/owl/aixm-mod/airportheliport#AirportHotSpot-instruction -->

    <owl:DatatypeProperty rdf:about="http://www.project-best.eu/owl/aixm-mod/airportheliport#AirportHotSpot-instruction">
        <rdfs:comment xml:lang="en">Action to be taken by the crew and/or vehicle drivers when approaching the hot spot.</rdfs:comment>
        <rdfs:domain rdf:resource="http://www.project-best.eu/owl/aixm-mod/airportheliport#AirportHotSpot"/>
        <rdfs:range rdf:resource="http://www.w3.org/2001/XMLSchema#string"/>
    </owl:DatatypeProperty>
    


    <!-- http://www.project-best.eu/owl/aixm-mod/airportheliport#ApproachLightingSystem-length -->

    <owl:DatatypeProperty rdf:about="http://www.project-best.eu/owl/aixm-mod/airportheliport#ApproachLightingSystem-length">
        <rdfs:comment xml:lang="en">The overall length of the approach lighting system.</rdfs:comment>
        <rdfs:domain rdf:resource="http://www.project-best.eu/owl/aixm-mod/airportheliport#ApproachLightingSystem"/>
        <rdfs:range rdf:resource="http://www.w3.org/2001/XMLSchema#decimal"/>
    </owl:DatatypeProperty>
    


    <!-- http://www.project-best.eu/owl/aixm-mod/airportheliport#Apron-name -->

    <owl:DatatypeProperty rdf:about="http://www.project-best.eu/owl/aixm-mod/airportheliport#Apron-name">
        <rdfs:comment xml:lang="en">The full textual name or designator used to identify an apron at an aerodrome/heliport which has more than one.</rdfs:comment>
        <rdfs:domain rdf:resource="http://www.project-best.eu/owl/aixm-mod/airportheliport#Apron"/>
        <rdfs:range rdf:resource="http://www.w3.org/2001/XMLSchema#string"/>
    </owl:DatatypeProperty>
    


    <!-- http://www.project-best.eu/owl/aixm-mod/airportheliport#ApronElement-length -->

    <owl:DatatypeProperty rdf:about="http://www.project-best.eu/owl/aixm-mod/airportheliport#ApronElement-length">
        <rdfs:comment xml:lang="en">The length of the runway element.</rdfs:comment>
        <rdfs:domain rdf:resource="http://www.project-best.eu/owl/aixm-mod/airportheliport#ApronElement"/>
        <rdfs:range rdf:resource="http://www.w3.org/2001/XMLSchema#decimal"/>
    </owl:DatatypeProperty>
    


    <!-- http://www.project-best.eu/owl/aixm-mod/airportheliport#ApronElement-width -->

    <owl:DatatypeProperty rdf:about="http://www.project-best.eu/owl/aixm-mod/airportheliport#ApronElement-width">
        <rdfs:comment xml:lang="en">The width of the runway element.</rdfs:comment>
        <rdfs:domain rdf:resource="http://www.project-best.eu/owl/aixm-mod/airportheliport#ApronElement"/>
        <rdfs:range rdf:resource="http://www.w3.org/2001/XMLSchema#decimal"/>
    </owl:DatatypeProperty>
    


    <!-- http://www.project-best.eu/owl/aixm-mod/airportheliport#ArrestingGear-length -->

    <owl:DatatypeProperty rdf:about="http://www.project-best.eu/owl/aixm-mod/airportheliport#ArrestingGear-length">
        <rdfs:comment xml:lang="en">Overall length of the feature.</rdfs:comment>
        <rdfs:domain rdf:resource="http://www.project-best.eu/owl/aixm-mod/airportheliport#ArrestingGear"/>
        <rdfs:range rdf:resource="http://www.w3.org/2001/XMLSchema#decimal"/>
    </owl:DatatypeProperty>
    


    <!-- http://www.project-best.eu/owl/aixm-mod/airportheliport#ArrestingGear-location -->

    <owl:DatatypeProperty rdf:about="http://www.project-best.eu/owl/aixm-mod/airportheliport#ArrestingGear-location">
        <rdfs:comment xml:lang="en">The distance of the arresting system from the closest threshold of the runway /landing area.</rdfs:comment>
        <rdfs:domain rdf:resource="http://www.project-best.eu/owl/aixm-mod/airportheliport#ArrestingGear"/>
        <rdfs:range rdf:resource="http://www.w3.org/2001/XMLSchema#decimal"/>
    </owl:DatatypeProperty>
    


    <!-- http://www.project-best.eu/owl/aixm-mod/airportheliport#ArrestingGear-width -->

    <owl:DatatypeProperty rdf:about="http://www.project-best.eu/owl/aixm-mod/airportheliport#ArrestingGear-width">
        <rdfs:comment xml:lang="en">Overall width of the feature.</rdfs:comment>
        <rdfs:domain rdf:resource="http://www.project-best.eu/owl/aixm-mod/airportheliport#ArrestingGear"/>
        <rdfs:range rdf:resource="http://www.w3.org/2001/XMLSchema#decimal"/>
    </owl:DatatypeProperty>
    


    <!-- http://www.project-best.eu/owl/aixm-mod/airportheliport#City-name -->

    <owl:DatatypeProperty rdf:about="http://www.project-best.eu/owl/aixm-mod/airportheliport#City-name">
        <rdfs:comment xml:lang="en">The full free text name of the city or town the aerodrome/heliport is serving.</rdfs:comment>
        <rdfs:domain rdf:resource="http://www.project-best.eu/owl/aixm-mod/airportheliport#City"/>
        <rdfs:range rdf:resource="http://www.w3.org/2001/XMLSchema#string"/>
    </owl:DatatypeProperty>
    


    <!-- http://www.project-best.eu/owl/aixm-mod/airportheliport#LightActivation-clicks -->

    <owl:DatatypeProperty rdf:about="http://www.project-best.eu/owl/aixm-mod/airportheliport#LightActivation-clicks">
        <rdfs:comment xml:lang="en">The number of clicks on the microphone required for activation of the lights at a particular intensity step.</rdfs:comment>
        <rdfs:domain rdf:resource="http://www.project-best.eu/owl/aixm-mod/airportheliport#LightActivation"/>
        <rdfs:range rdf:resource="http://www.w3.org/2001/XMLSchema#unsignedInt"/>
    </owl:DatatypeProperty>
    


    <!-- http://www.project-best.eu/owl/aixm-mod/airportheliport#MarkingBuoy-designator -->

    <owl:DatatypeProperty rdf:about="http://www.project-best.eu/owl/aixm-mod/airportheliport#MarkingBuoy-designator">
        <rdfs:comment xml:lang="en">Official number of the buoy</rdfs:comment>
        <rdfs:domain rdf:resource="http://www.project-best.eu/owl/aixm-mod/airportheliport#MarkingBuoy"/>
        <rdfs:range rdf:resource="http://www.w3.org/2001/XMLSchema#string"/>
    </owl:DatatypeProperty>
    


    <!-- http://www.project-best.eu/owl/aixm-mod/airportheliport#NavaidEquipmentDistance-distance -->

    <owl:DatatypeProperty rdf:about="http://www.project-best.eu/owl/aixm-mod/airportheliport#NavaidEquipmentDistance-distance">
        <rdfs:comment xml:lang="en">The measured or calculated distance between a Runway Centreline Point and a Navaid Equipment.</rdfs:comment>
        <rdfs:domain rdf:resource="http://www.project-best.eu/owl/aixm-mod/airportheliport#NavaidEquipmentDistance"/>
        <rdfs:range rdf:resource="http://www.w3.org/2001/XMLSchema#decimal"/>
    </owl:DatatypeProperty>
    


    <!-- http://www.project-best.eu/owl/aixm-mod/airportheliport#NavaidEquipmentDistance-distanceAccuracy -->

    <owl:DatatypeProperty rdf:about="http://www.project-best.eu/owl/aixm-mod/airportheliport#NavaidEquipmentDistance-distanceAccuracy">
        <rdfs:comment xml:lang="en">Accuracy of the measured or calculated distance between a Runway Centreline Point and a Navaid Equipment piece.</rdfs:comment>
        <rdfs:domain rdf:resource="http://www.project-best.eu/owl/aixm-mod/airportheliport#NavaidEquipmentDistance"/>
        <rdfs:range rdf:resource="http://www.w3.org/2001/XMLSchema#decimal"/>
    </owl:DatatypeProperty>
    


    <!-- http://www.project-best.eu/owl/aixm-mod/airportheliport#Ridge-depth -->

    <owl:DatatypeProperty rdf:about="http://www.project-best.eu/owl/aixm-mod/airportheliport#Ridge-depth">
        <rdfs:comment xml:lang="en">Height of the ridges of deposited material.</rdfs:comment>
        <rdfs:domain rdf:resource="http://www.project-best.eu/owl/aixm-mod/airportheliport#Ridge"/>
        <rdfs:range rdf:resource="http://www.w3.org/2001/XMLSchema#decimal"/>
    </owl:DatatypeProperty>
    


    <!-- http://www.project-best.eu/owl/aixm-mod/airportheliport#Ridge-distance -->

    <owl:DatatypeProperty rdf:about="http://www.project-best.eu/owl/aixm-mod/airportheliport#Ridge-distance">
        <rdfs:comment xml:lang="en">Distance from the edge of the movement area.</rdfs:comment>
        <rdfs:domain rdf:resource="http://www.project-best.eu/owl/aixm-mod/airportheliport#Ridge"/>
        <rdfs:range rdf:resource="http://www.w3.org/2001/XMLSchema#decimal"/>
    </owl:DatatypeProperty>
    


    <!-- http://www.project-best.eu/owl/aixm-mod/airportheliport#Road-designator -->

    <owl:DatatypeProperty rdf:about="http://www.project-best.eu/owl/aixm-mod/airportheliport#Road-designator">
        <rdfs:comment xml:lang="en">The designator or name of the service road.</rdfs:comment>
        <rdfs:domain rdf:resource="http://www.project-best.eu/owl/aixm-mod/airportheliport#Road"/>
        <rdfs:range rdf:resource="http://www.w3.org/2001/XMLSchema#string"/>
    </owl:DatatypeProperty>
    


    <!-- http://www.project-best.eu/owl/aixm-mod/airportheliport#Runway-designator -->

    <owl:DatatypeProperty rdf:about="http://www.project-best.eu/owl/aixm-mod/airportheliport#Runway-designator">
        <rdfs:comment xml:lang="en">The full textual designator of the runway, used to uniquely identify it at an aerodrome/heliport which has more than one.</rdfs:comment>
        <rdfs:domain rdf:resource="http://www.project-best.eu/owl/aixm-mod/airportheliport#Runway"/>
        <rdfs:range rdf:resource="http://www.w3.org/2001/XMLSchema#string"/>
    </owl:DatatypeProperty>
    


    <!-- http://www.project-best.eu/owl/aixm-mod/airportheliport#Runway-lengthAccuracy -->

    <owl:DatatypeProperty rdf:about="http://www.project-best.eu/owl/aixm-mod/airportheliport#Runway-lengthAccuracy">
        <rdfs:comment xml:lang="en">Accuracy of the value of the physical length of the runway.</rdfs:comment>
        <rdfs:domain rdf:resource="http://www.project-best.eu/owl/aixm-mod/airportheliport#Runway"/>
        <rdfs:range rdf:resource="http://www.w3.org/2001/XMLSchema#decimal"/>
    </owl:DatatypeProperty>
    


    <!-- http://www.project-best.eu/owl/aixm-mod/airportheliport#Runway-lengthOffset -->

    <owl:DatatypeProperty rdf:about="http://www.project-best.eu/owl/aixm-mod/airportheliport#Runway-lengthOffset">
        <rdfs:comment xml:lang="en">A value specifying the longitudinal offset of the strip, when it is not symmetrically extended beyond the two runway ends.</rdfs:comment>
        <rdfs:domain rdf:resource="http://www.project-best.eu/owl/aixm-mod/airportheliport#Runway"/>
        <rdfs:range rdf:resource="http://www.w3.org/2001/XMLSchema#decimal"/>
    </owl:DatatypeProperty>
    


    <!-- http://www.project-best.eu/owl/aixm-mod/airportheliport#Runway-lengthStrip -->

    <owl:DatatypeProperty rdf:about="http://www.project-best.eu/owl/aixm-mod/airportheliport#Runway-lengthStrip">
        <rdfs:comment xml:lang="en">The value of the physical length of the strip. The runway strip is a defined area including the runway and, if applicable, the stop-way. It is intended (a) to reduce the risk of damage to aircraft running off the runway and (b) to protect aircraft flying over the runway during take-off or landing operations.</rdfs:comment>
        <rdfs:domain rdf:resource="http://www.project-best.eu/owl/aixm-mod/airportheliport#Runway"/>
        <rdfs:range rdf:resource="http://www.w3.org/2001/XMLSchema#decimal"/>
    </owl:DatatypeProperty>
    


    <!-- http://www.project-best.eu/owl/aixm-mod/airportheliport#Runway-nominalLength -->

    <owl:DatatypeProperty rdf:about="http://www.project-best.eu/owl/aixm-mod/airportheliport#Runway-nominalLength">
        <rdfs:comment xml:lang="en">The declared longitudinal extent of the runway for operational (performance) calculations.</rdfs:comment>
        <rdfs:domain rdf:resource="http://www.project-best.eu/owl/aixm-mod/airportheliport#Runway"/>
        <rdfs:range rdf:resource="http://www.w3.org/2001/XMLSchema#decimal"/>
    </owl:DatatypeProperty>
    


    <!-- http://www.project-best.eu/owl/aixm-mod/airportheliport#Runway-nominalWidth -->

    <owl:DatatypeProperty rdf:about="http://www.project-best.eu/owl/aixm-mod/airportheliport#Runway-nominalWidth">
        <rdfs:comment xml:lang="en">The declared transversal extent of the runway for operational (performance) calculations.</rdfs:comment>
        <rdfs:domain rdf:resource="http://www.project-best.eu/owl/aixm-mod/airportheliport#Runway"/>
        <rdfs:range rdf:resource="http://www.w3.org/2001/XMLSchema#decimal"/>
    </owl:DatatypeProperty>
    


    <!-- http://www.project-best.eu/owl/aixm-mod/airportheliport#Runway-widthAccuracy -->

    <owl:DatatypeProperty rdf:about="http://www.project-best.eu/owl/aixm-mod/airportheliport#Runway-widthAccuracy">
        <rdfs:comment xml:lang="en">Accuracy of the value of the physical width of the runway.</rdfs:comment>
        <rdfs:domain rdf:resource="http://www.project-best.eu/owl/aixm-mod/airportheliport#Runway"/>
        <rdfs:range rdf:resource="http://www.w3.org/2001/XMLSchema#decimal"/>
    </owl:DatatypeProperty>
    


    <!-- http://www.project-best.eu/owl/aixm-mod/airportheliport#Runway-widthOffset -->

    <owl:DatatypeProperty rdf:about="http://www.project-best.eu/owl/aixm-mod/airportheliport#Runway-widthOffset">
        <rdfs:comment xml:lang="en">A value specifying the lateral offset of the strip, when it is not symmetrically extended beyond the two runway edges.</rdfs:comment>
        <rdfs:domain rdf:resource="http://www.project-best.eu/owl/aixm-mod/airportheliport#Runway"/>
        <rdfs:range rdf:resource="http://www.w3.org/2001/XMLSchema#decimal"/>
    </owl:DatatypeProperty>
    


    <!-- http://www.project-best.eu/owl/aixm-mod/airportheliport#Runway-widthShoulder -->

    <owl:DatatypeProperty rdf:about="http://www.project-best.eu/owl/aixm-mod/airportheliport#Runway-widthShoulder">
        <rdfs:comment xml:lang="en">The value of the runway shoulder width.</rdfs:comment>
        <rdfs:domain rdf:resource="http://www.project-best.eu/owl/aixm-mod/airportheliport#Runway"/>
        <rdfs:range rdf:resource="http://www.w3.org/2001/XMLSchema#decimal"/>
    </owl:DatatypeProperty>
    


    <!-- http://www.project-best.eu/owl/aixm-mod/airportheliport#Runway-widthStrip -->

    <owl:DatatypeProperty rdf:about="http://www.project-best.eu/owl/aixm-mod/airportheliport#Runway-widthStrip">
        <rdfs:comment xml:lang="en">The value of the physical width of the strip.</rdfs:comment>
        <rdfs:domain rdf:resource="http://www.project-best.eu/owl/aixm-mod/airportheliport#Runway"/>
        <rdfs:range rdf:resource="http://www.w3.org/2001/XMLSchema#decimal"/>
    </owl:DatatypeProperty>
    


    <!-- http://www.project-best.eu/owl/aixm-mod/airportheliport#RunwayBlastPad-length -->

    <owl:DatatypeProperty rdf:about="http://www.project-best.eu/owl/aixm-mod/airportheliport#RunwayBlastPad-length">
        <rdfs:comment xml:lang="en">Overall length of the feature</rdfs:comment>
        <rdfs:domain rdf:resource="http://www.project-best.eu/owl/aixm-mod/airportheliport#RunwayBlastPad"/>
        <rdfs:range rdf:resource="http://www.w3.org/2001/XMLSchema#decimal"/>
    </owl:DatatypeProperty>
    


    <!-- http://www.project-best.eu/owl/aixm-mod/airportheliport#RunwayCentrelinePoint-designator -->

    <owl:DatatypeProperty rdf:about="http://www.project-best.eu/owl/aixm-mod/airportheliport#RunwayCentrelinePoint-designator">
        <rdfs:comment xml:lang="en">A code or name by which the point is identified locally at the airport.</rdfs:comment>
        <rdfs:domain rdf:resource="http://www.project-best.eu/owl/aixm-mod/airportheliport#RunwayCentrelinePoint"/>
        <rdfs:range rdf:resource="http://www.w3.org/2001/XMLSchema#string"/>
    </owl:DatatypeProperty>
    


    <!-- http://www.project-best.eu/owl/aixm-mod/airportheliport#RunwayContamination-clearedLength -->

    <owl:DatatypeProperty rdf:about="http://www.project-best.eu/owl/aixm-mod/airportheliport#RunwayContamination-clearedLength">
        <rdfs:comment xml:lang="en">Length of runway cleared of contamination, if less than the total length.</rdfs:comment>
        <rdfs:domain rdf:resource="http://www.project-best.eu/owl/aixm-mod/airportheliport#RunwayContamination"/>
        <rdfs:range rdf:resource="http://www.w3.org/2001/XMLSchema#decimal"/>
    </owl:DatatypeProperty>
    


    <!-- http://www.project-best.eu/owl/aixm-mod/airportheliport#RunwayContamination-clearedLengthBegin -->

    <owl:DatatypeProperty rdf:about="http://www.project-best.eu/owl/aixm-mod/airportheliport#RunwayContamination-clearedLengthBegin">
        <rdfs:comment xml:lang="en">The distance from the threshold with the lowest designator number to the point where the cleared portion starts, in case of partial clearance.</rdfs:comment>
        <rdfs:domain rdf:resource="http://www.project-best.eu/owl/aixm-mod/airportheliport#RunwayContamination"/>
        <rdfs:range rdf:resource="http://www.w3.org/2001/XMLSchema#decimal"/>
    </owl:DatatypeProperty>
    


    <!-- http://www.project-best.eu/owl/aixm-mod/airportheliport#RunwayContamination-clearedWidth -->

    <owl:DatatypeProperty rdf:about="http://www.project-best.eu/owl/aixm-mod/airportheliport#RunwayContamination-clearedWidth">
        <rdfs:comment xml:lang="en">Width of runway cleared of contamination, if less than the total width.</rdfs:comment>
        <rdfs:domain rdf:resource="http://www.project-best.eu/owl/aixm-mod/airportheliport#RunwayContamination"/>
        <rdfs:range rdf:resource="http://www.w3.org/2001/XMLSchema#decimal"/>
    </owl:DatatypeProperty>
    


    <!-- http://www.project-best.eu/owl/aixm-mod/airportheliport#RunwayContamination-furtherClearanceLength -->

    <owl:DatatypeProperty rdf:about="http://www.project-best.eu/owl/aixm-mod/airportheliport#RunwayContamination-furtherClearanceLength">
        <rdfs:comment xml:lang="en">Length of runway that is expected to be cleared of contamination, if less than the total length.</rdfs:comment>
        <rdfs:domain rdf:resource="http://www.project-best.eu/owl/aixm-mod/airportheliport#RunwayContamination"/>
        <rdfs:range rdf:resource="http://www.w3.org/2001/XMLSchema#decimal"/>
    </owl:DatatypeProperty>
    


    <!-- http://www.project-best.eu/owl/aixm-mod/airportheliport#RunwayContamination-furtherClearanceWidth -->

    <owl:DatatypeProperty rdf:about="http://www.project-best.eu/owl/aixm-mod/airportheliport#RunwayContamination-furtherClearanceWidth">
        <rdfs:comment xml:lang="en">Width of runway that is expected to be cleared of contamination, if less than the total width.</rdfs:comment>
        <rdfs:domain rdf:resource="http://www.project-best.eu/owl/aixm-mod/airportheliport#RunwayContamination"/>
        <rdfs:range rdf:resource="http://www.w3.org/2001/XMLSchema#decimal"/>
    </owl:DatatypeProperty>
    


    <!-- http://www.project-best.eu/owl/aixm-mod/airportheliport#RunwayDeclaredDistanceValue-distance -->

    <owl:DatatypeProperty rdf:about="http://www.project-best.eu/owl/aixm-mod/airportheliport#RunwayDeclaredDistanceValue-distance">
        <rdfs:comment xml:lang="en">The value of the declared distance.</rdfs:comment>
        <rdfs:domain rdf:resource="http://www.project-best.eu/owl/aixm-mod/airportheliport#RunwayDeclaredDistanceValue"/>
        <rdfs:range rdf:resource="http://www.w3.org/2001/XMLSchema#decimal"/>
    </owl:DatatypeProperty>
    


    <!-- http://www.project-best.eu/owl/aixm-mod/airportheliport#RunwayDeclaredDistanceValue-distanceAccuracy -->

    <owl:DatatypeProperty rdf:about="http://www.project-best.eu/owl/aixm-mod/airportheliport#RunwayDeclaredDistanceValue-distanceAccuracy">
        <rdfs:comment xml:lang="en">Accuracy of the value of the declared distance.</rdfs:comment>
        <rdfs:domain rdf:resource="http://www.project-best.eu/owl/aixm-mod/airportheliport#RunwayDeclaredDistanceValue"/>
        <rdfs:range rdf:resource="http://www.w3.org/2001/XMLSchema#decimal"/>
    </owl:DatatypeProperty>
    


    <!-- http://www.project-best.eu/owl/aixm-mod/airportheliport#RunwayDirection-designator -->

    <owl:DatatypeProperty rdf:about="http://www.project-best.eu/owl/aixm-mod/airportheliport#RunwayDirection-designator">
        <rdfs:comment xml:lang="en">The full textual designator of the landing and take-off direction.</rdfs:comment>
        <rdfs:domain rdf:resource="http://www.project-best.eu/owl/aixm-mod/airportheliport#RunwayDirection"/>
        <rdfs:range rdf:resource="http://www.w3.org/2001/XMLSchema#string"/>
    </owl:DatatypeProperty>
    


    <!-- http://www.project-best.eu/owl/aixm-mod/airportheliport#RunwayDirection-elevationTDZ -->

    <owl:DatatypeProperty rdf:about="http://www.project-best.eu/owl/aixm-mod/airportheliport#RunwayDirection-elevationTDZ">
        <rdfs:comment xml:lang="en">Elevation of touch down zone:   The value of the highest elevation of the runway Touch Down Zone (TDZ).  </rdfs:comment>
        <rdfs:domain rdf:resource="http://www.project-best.eu/owl/aixm-mod/airportheliport#RunwayDirection"/>
        <rdfs:range rdf:resource="http://www.w3.org/2001/XMLSchema#decimal"/>
    </owl:DatatypeProperty>
    


    <!-- http://www.project-best.eu/owl/aixm-mod/airportheliport#RunwayDirection-elevationTDZAccuracy -->

    <owl:DatatypeProperty rdf:about="http://www.project-best.eu/owl/aixm-mod/airportheliport#RunwayDirection-elevationTDZAccuracy">
        <rdfs:comment xml:lang="en">The accuracy of the reported Touch Down Zone elevation</rdfs:comment>
        <rdfs:domain rdf:resource="http://www.project-best.eu/owl/aixm-mod/airportheliport#RunwayDirection"/>
        <rdfs:range rdf:resource="http://www.w3.org/2001/XMLSchema#decimal"/>
    </owl:DatatypeProperty>
    


    <!-- http://www.project-best.eu/owl/aixm-mod/airportheliport#RunwayDirection-magneticBearing -->

    <owl:DatatypeProperty rdf:about="http://www.project-best.eu/owl/aixm-mod/airportheliport#RunwayDirection-magneticBearing">
        <rdfs:comment xml:lang="en">The measured angle between the runway direction and Magnetic North at a given position.</rdfs:comment>
        <rdfs:domain rdf:resource="http://www.project-best.eu/owl/aixm-mod/airportheliport#RunwayDirection"/>
        <rdfs:range rdf:resource="http://www.w3.org/2001/XMLSchema#decimal"/>
    </owl:DatatypeProperty>
    


    <!-- http://www.project-best.eu/owl/aixm-mod/airportheliport#RunwayDirection-slopeTDZ -->

    <owl:DatatypeProperty rdf:about="http://www.project-best.eu/owl/aixm-mod/airportheliport#RunwayDirection-slopeTDZ">
        <rdfs:comment xml:lang="en">Touchdown zone longitudinal slope (slope of 1/3 of the runway length from threshold or first 3000 feet for runways longer than 9000 feet)</rdfs:comment>
        <rdfs:domain rdf:resource="http://www.project-best.eu/owl/aixm-mod/airportheliport#RunwayDirection"/>
        <rdfs:range rdf:resource="http://www.w3.org/2001/XMLSchema#decimal"/>
    </owl:DatatypeProperty>
    


    <!-- http://www.project-best.eu/owl/aixm-mod/airportheliport#RunwayDirection-trueBearing -->

    <owl:DatatypeProperty rdf:about="http://www.project-best.eu/owl/aixm-mod/airportheliport#RunwayDirection-trueBearing">
        <rdfs:comment xml:lang="en">The measured angle between the runway direction and True North at a given position. Note : The True North is the north point at which the meridian lines meet.</rdfs:comment>
        <rdfs:domain rdf:resource="http://www.project-best.eu/owl/aixm-mod/airportheliport#RunwayDirection"/>
        <rdfs:range rdf:resource="http://www.w3.org/2001/XMLSchema#decimal"/>
    </owl:DatatypeProperty>
    


    <!-- http://www.project-best.eu/owl/aixm-mod/airportheliport#RunwayDirection-trueBearingAccuracy -->

    <owl:DatatypeProperty rdf:about="http://www.project-best.eu/owl/aixm-mod/airportheliport#RunwayDirection-trueBearingAccuracy">
        <rdfs:comment xml:lang="en">Accuracy of the measured angle between the runway direction and True North at a given position.</rdfs:comment>
        <rdfs:domain rdf:resource="http://www.project-best.eu/owl/aixm-mod/airportheliport#RunwayDirection"/>
        <rdfs:range rdf:resource="http://www.w3.org/2001/XMLSchema#decimal"/>
    </owl:DatatypeProperty>
    


    <!-- http://www.project-best.eu/owl/aixm-mod/airportheliport#RunwayElement-length -->

    <owl:DatatypeProperty rdf:about="http://www.project-best.eu/owl/aixm-mod/airportheliport#RunwayElement-length">
        <rdfs:comment xml:lang="en">The length of the runway element.</rdfs:comment>
        <rdfs:domain rdf:resource="http://www.project-best.eu/owl/aixm-mod/airportheliport#RunwayElement"/>
        <rdfs:range rdf:resource="http://www.w3.org/2001/XMLSchema#decimal"/>
    </owl:DatatypeProperty>
    


    <!-- http://www.project-best.eu/owl/aixm-mod/airportheliport#RunwayElement-width -->

    <owl:DatatypeProperty rdf:about="http://www.project-best.eu/owl/aixm-mod/airportheliport#RunwayElement-width">
        <rdfs:comment xml:lang="en">The width of the runway element.</rdfs:comment>
        <rdfs:domain rdf:resource="http://www.project-best.eu/owl/aixm-mod/airportheliport#RunwayElement"/>
        <rdfs:range rdf:resource="http://www.w3.org/2001/XMLSchema#decimal"/>
    </owl:DatatypeProperty>
    


    <!-- http://www.project-best.eu/owl/aixm-mod/airportheliport#SurfaceCharacteristics-classLCN -->

    <owl:DatatypeProperty rdf:about="http://www.project-best.eu/owl/aixm-mod/airportheliport#SurfaceCharacteristics-classLCN">
        <rdfs:comment xml:lang="en">A value which denotes the peak bearing moment the surface can handle repeatedly without shortening its service life.</rdfs:comment>
        <rdfs:domain rdf:resource="http://www.project-best.eu/owl/aixm-mod/airportheliport#SurfaceCharacteristics"/>
        <rdfs:range rdf:resource="http://www.w3.org/2001/XMLSchema#decimal"/>
    </owl:DatatypeProperty>
    


    <!-- http://www.project-best.eu/owl/aixm-mod/airportheliport#SurfaceCharacteristics-classPCN -->

    <owl:DatatypeProperty rdf:about="http://www.project-best.eu/owl/aixm-mod/airportheliport#SurfaceCharacteristics-classPCN">
        <rdfs:comment xml:lang="en">The bearing strength of a pavement for unrestricted operations.</rdfs:comment>
        <rdfs:domain rdf:resource="http://www.project-best.eu/owl/aixm-mod/airportheliport#SurfaceCharacteristics"/>
        <rdfs:range rdf:resource="http://www.w3.org/2001/XMLSchema#decimal"/>
    </owl:DatatypeProperty>
    


    <!-- http://www.project-best.eu/owl/aixm-mod/airportheliport#SurfaceCharacteristics-tyrePressureSIWL -->

    <owl:DatatypeProperty rdf:about="http://www.project-best.eu/owl/aixm-mod/airportheliport#SurfaceCharacteristics-tyrePressureSIWL">
        <rdfs:comment xml:lang="en">The maximum aircraft tire pressure that a movement area surface can support.</rdfs:comment>
        <rdfs:domain rdf:resource="http://www.project-best.eu/owl/aixm-mod/airportheliport#SurfaceCharacteristics"/>
        <rdfs:range rdf:resource="http://www.w3.org/2001/XMLSchema#decimal"/>
    </owl:DatatypeProperty>
    


    <!-- http://www.project-best.eu/owl/aixm-mod/airportheliport#SurfaceCharacteristics-weightAUW -->

    <owl:DatatypeProperty rdf:about="http://www.project-best.eu/owl/aixm-mod/airportheliport#SurfaceCharacteristics-weightAUW">
        <rdfs:comment xml:lang="en">The maximum total value of the weight of an aircraft that a movement area surface may support, regardless of the landing gear configuration of the aircraft.</rdfs:comment>
        <rdfs:domain rdf:resource="http://www.project-best.eu/owl/aixm-mod/airportheliport#SurfaceCharacteristics"/>
        <rdfs:range rdf:resource="http://www.w3.org/2001/XMLSchema#decimal"/>
    </owl:DatatypeProperty>
    


    <!-- http://www.project-best.eu/owl/aixm-mod/airportheliport#SurfaceCharacteristics-weightSIWL -->

    <owl:DatatypeProperty rdf:about="http://www.project-best.eu/owl/aixm-mod/airportheliport#SurfaceCharacteristics-weightSIWL">
        <rdfs:comment xml:lang="en">The maximum calculated load on each tire of a landing gear assembly that a movement area surface can support.</rdfs:comment>
        <rdfs:domain rdf:resource="http://www.project-best.eu/owl/aixm-mod/airportheliport#SurfaceCharacteristics"/>
        <rdfs:range rdf:resource="http://www.w3.org/2001/XMLSchema#decimal"/>
    </owl:DatatypeProperty>
    


    <!-- http://www.project-best.eu/owl/aixm-mod/airportheliport#SurfaceContamination-depth -->

    <owl:DatatypeProperty rdf:about="http://www.project-best.eu/owl/aixm-mod/airportheliport#SurfaceContamination-depth">
        <rdfs:comment xml:lang="en">The depth of the contamination on the surface.</rdfs:comment>
        <rdfs:domain rdf:resource="http://www.project-best.eu/owl/aixm-mod/airportheliport#SurfaceContamination"/>
        <rdfs:range rdf:resource="http://www.w3.org/2001/XMLSchema#decimal"/>
    </owl:DatatypeProperty>
    


    <!-- http://www.project-best.eu/owl/aixm-mod/airportheliport#SurfaceContamination-frictionCoefficient -->

    <owl:DatatypeProperty rdf:about="http://www.project-best.eu/owl/aixm-mod/airportheliport#SurfaceContamination-frictionCoefficient">
        <rdfs:comment xml:lang="en">The average friction coefficient. </rdfs:comment>
        <rdfs:domain rdf:resource="http://www.project-best.eu/owl/aixm-mod/airportheliport#SurfaceContamination"/>
        <rdfs:range rdf:resource="http://www.w3.org/2001/XMLSchema#decimal"/>
    </owl:DatatypeProperty>
    


    <!-- http://www.project-best.eu/owl/aixm-mod/airportheliport#SurfaceContamination-furtherClearanceTime -->

    <owl:DatatypeProperty rdf:about="http://www.project-best.eu/owl/aixm-mod/airportheliport#SurfaceContamination-furtherClearanceTime">
        <rdfs:comment xml:lang="en">The date and time (UTC) when it is expected to complete further clearance.</rdfs:comment>
        <rdfs:domain rdf:resource="http://www.project-best.eu/owl/aixm-mod/airportheliport#SurfaceContamination"/>
        <rdfs:range rdf:resource="http://www.w3.org/2001/XMLSchema#string"/>
    </owl:DatatypeProperty>
    


    <!-- http://www.project-best.eu/owl/aixm-mod/airportheliport#SurfaceContamination-nextObservationTime -->

    <owl:DatatypeProperty rdf:about="http://www.project-best.eu/owl/aixm-mod/airportheliport#SurfaceContamination-nextObservationTime">
        <rdfs:comment xml:lang="en">The date and time of the next intended measurement report (UTC).</rdfs:comment>
        <rdfs:domain rdf:resource="http://www.project-best.eu/owl/aixm-mod/airportheliport#SurfaceContamination"/>
        <rdfs:range rdf:resource="http://www.w3.org/2001/XMLSchema#string"/>
    </owl:DatatypeProperty>
    


    <!-- http://www.project-best.eu/owl/aixm-mod/airportheliport#SurfaceContamination-observationTime -->

    <owl:DatatypeProperty rdf:about="http://www.project-best.eu/owl/aixm-mod/airportheliport#SurfaceContamination-observationTime">
        <rdfs:comment xml:lang="en">The date and time of the measurement completion (UTC).</rdfs:comment>
        <rdfs:domain rdf:resource="http://www.project-best.eu/owl/aixm-mod/airportheliport#SurfaceContamination"/>
        <rdfs:range rdf:resource="http://www.w3.org/2001/XMLSchema#string"/>
    </owl:DatatypeProperty>
    


    <!-- http://www.project-best.eu/owl/aixm-mod/airportheliport#SurfaceContamination-proportion -->

    <owl:DatatypeProperty rdf:about="http://www.project-best.eu/owl/aixm-mod/airportheliport#SurfaceContamination-proportion">
        <rdfs:comment xml:lang="en">The percentage of the contaminated area from the overall extent of the surface.</rdfs:comment>
        <rdfs:domain rdf:resource="http://www.project-best.eu/owl/aixm-mod/airportheliport#SurfaceContamination"/>
        <rdfs:range rdf:resource="http://www.w3.org/2001/XMLSchema#decimal"/>
    </owl:DatatypeProperty>
    


    <!-- http://www.project-best.eu/owl/aixm-mod/airportheliport#SurfaceContaminationLayer-layerOrder -->

    <owl:DatatypeProperty rdf:about="http://www.project-best.eu/owl/aixm-mod/airportheliport#SurfaceContaminationLayer-layerOrder">
        <rdfs:comment xml:lang="en">The order of the layer, starting from the uppermost (value &quot;1&quot;) towards the movement area surface, in case overlapping contaminants are present.</rdfs:comment>
        <rdfs:domain rdf:resource="http://www.project-best.eu/owl/aixm-mod/airportheliport#SurfaceContaminationLayer"/>
        <rdfs:range rdf:resource="http://www.w3.org/2001/XMLSchema#unsignedInt"/>
    </owl:DatatypeProperty>
    


    <!-- http://www.project-best.eu/owl/aixm-mod/airportheliport#SurveyControlPoint-designator -->

    <owl:DatatypeProperty rdf:about="http://www.project-best.eu/owl/aixm-mod/airportheliport#SurveyControlPoint-designator">
        <rdfs:comment xml:lang="en">The identifier of the control survey point.</rdfs:comment>
        <rdfs:domain rdf:resource="http://www.project-best.eu/owl/aixm-mod/airportheliport#SurveyControlPoint"/>
        <rdfs:range rdf:resource="http://www.w3.org/2001/XMLSchema#string"/>
    </owl:DatatypeProperty>
    


    <!-- http://www.project-best.eu/owl/aixm-mod/airportheliport#Taxiway-designator -->

    <owl:DatatypeProperty rdf:about="http://www.project-best.eu/owl/aixm-mod/airportheliport#Taxiway-designator">
        <rdfs:comment xml:lang="en">The textual designator of the taxiway.</rdfs:comment>
        <rdfs:domain rdf:resource="http://www.project-best.eu/owl/aixm-mod/airportheliport#Taxiway"/>
        <rdfs:range rdf:resource="http://www.w3.org/2001/XMLSchema#string"/>
    </owl:DatatypeProperty>
    


    <!-- http://www.project-best.eu/owl/aixm-mod/airportheliport#Taxiway-length -->

    <owl:DatatypeProperty rdf:about="http://www.project-best.eu/owl/aixm-mod/airportheliport#Taxiway-length">
        <rdfs:comment xml:lang="en">Value for the length of the taxiway</rdfs:comment>
        <rdfs:domain rdf:resource="http://www.project-best.eu/owl/aixm-mod/airportheliport#Taxiway"/>
        <rdfs:range rdf:resource="http://www.w3.org/2001/XMLSchema#decimal"/>
    </owl:DatatypeProperty>
    


    <!-- http://www.project-best.eu/owl/aixm-mod/airportheliport#Taxiway-width -->

    <owl:DatatypeProperty rdf:about="http://www.project-best.eu/owl/aixm-mod/airportheliport#Taxiway-width">
        <rdfs:comment xml:lang="en">The value of the physical width of the taxiway.</rdfs:comment>
        <rdfs:domain rdf:resource="http://www.project-best.eu/owl/aixm-mod/airportheliport#Taxiway"/>
        <rdfs:range rdf:resource="http://www.w3.org/2001/XMLSchema#decimal"/>
    </owl:DatatypeProperty>
    


    <!-- http://www.project-best.eu/owl/aixm-mod/airportheliport#Taxiway-widthShoulder -->

    <owl:DatatypeProperty rdf:about="http://www.project-best.eu/owl/aixm-mod/airportheliport#Taxiway-widthShoulder">
        <rdfs:comment xml:lang="en">The value of the taxiway shoulder width.</rdfs:comment>
        <rdfs:domain rdf:resource="http://www.project-best.eu/owl/aixm-mod/airportheliport#Taxiway"/>
        <rdfs:range rdf:resource="http://www.w3.org/2001/XMLSchema#decimal"/>
    </owl:DatatypeProperty>
    


    <!-- http://www.project-best.eu/owl/aixm-mod/airportheliport#TaxiwayContamination-clearedWidth -->

    <owl:DatatypeProperty rdf:about="http://www.project-best.eu/owl/aixm-mod/airportheliport#TaxiwayContamination-clearedWidth">
        <rdfs:comment xml:lang="en">Width of taxiway cleared of contamination.</rdfs:comment>
        <rdfs:domain rdf:resource="http://www.project-best.eu/owl/aixm-mod/airportheliport#TaxiwayContamination"/>
        <rdfs:range rdf:resource="http://www.w3.org/2001/XMLSchema#decimal"/>
    </owl:DatatypeProperty>
    


    <!-- http://www.project-best.eu/owl/aixm-mod/airportheliport#TaxiwayElement-length -->

    <owl:DatatypeProperty rdf:about="http://www.project-best.eu/owl/aixm-mod/airportheliport#TaxiwayElement-length">
        <rdfs:comment xml:lang="en">The length of the runway element.</rdfs:comment>
        <rdfs:domain rdf:resource="http://www.project-best.eu/owl/aixm-mod/airportheliport#TaxiwayElement"/>
        <rdfs:range rdf:resource="http://www.w3.org/2001/XMLSchema#decimal"/>
    </owl:DatatypeProperty>
    


    <!-- http://www.project-best.eu/owl/aixm-mod/airportheliport#TaxiwayElement-width -->

    <owl:DatatypeProperty rdf:about="http://www.project-best.eu/owl/aixm-mod/airportheliport#TaxiwayElement-width">
        <rdfs:comment xml:lang="en">The width of the runway element.</rdfs:comment>
        <rdfs:domain rdf:resource="http://www.project-best.eu/owl/aixm-mod/airportheliport#TaxiwayElement"/>
        <rdfs:range rdf:resource="http://www.w3.org/2001/XMLSchema#decimal"/>
    </owl:DatatypeProperty>
    


    <!-- http://www.project-best.eu/owl/aixm-mod/airportheliport#TouchDownLiftOff-designator -->

    <owl:DatatypeProperty rdf:about="http://www.project-best.eu/owl/aixm-mod/airportheliport#TouchDownLiftOff-designator">
        <rdfs:comment xml:lang="en">The textual designator of the touch down and lift-off area.</rdfs:comment>
        <rdfs:domain rdf:resource="http://www.project-best.eu/owl/aixm-mod/airportheliport#TouchDownLiftOff"/>
        <rdfs:range rdf:resource="http://www.w3.org/2001/XMLSchema#string"/>
    </owl:DatatypeProperty>
    


    <!-- http://www.project-best.eu/owl/aixm-mod/airportheliport#TouchDownLiftOff-length -->

    <owl:DatatypeProperty rdf:about="http://www.project-best.eu/owl/aixm-mod/airportheliport#TouchDownLiftOff-length">
        <rdfs:comment xml:lang="en">The value of the physical length of the touchdown and lift-off area.</rdfs:comment>
        <rdfs:domain rdf:resource="http://www.project-best.eu/owl/aixm-mod/airportheliport#TouchDownLiftOff"/>
        <rdfs:range rdf:resource="http://www.w3.org/2001/XMLSchema#decimal"/>
    </owl:DatatypeProperty>
    


    <!-- http://www.project-best.eu/owl/aixm-mod/airportheliport#TouchDownLiftOff-slope -->

    <owl:DatatypeProperty rdf:about="http://www.project-best.eu/owl/aixm-mod/airportheliport#TouchDownLiftOff-slope">
        <rdfs:comment xml:lang="en">The slope (rate of upward inclination of the surface from the horizontal) of the surface of a feature.</rdfs:comment>
        <rdfs:domain rdf:resource="http://www.project-best.eu/owl/aixm-mod/airportheliport#TouchDownLiftOff"/>
        <rdfs:range rdf:resource="http://www.w3.org/2001/XMLSchema#decimal"/>
    </owl:DatatypeProperty>
    


    <!-- http://www.project-best.eu/owl/aixm-mod/airportheliport#TouchDownLiftOff-width -->

    <owl:DatatypeProperty rdf:about="http://www.project-best.eu/owl/aixm-mod/airportheliport#TouchDownLiftOff-width">
        <rdfs:comment xml:lang="en">The value of the physical width of the touchdown and lift-off area.</rdfs:comment>
        <rdfs:domain rdf:resource="http://www.project-best.eu/owl/aixm-mod/airportheliport#TouchDownLiftOff"/>
        <rdfs:range rdf:resource="http://www.w3.org/2001/XMLSchema#decimal"/>
    </owl:DatatypeProperty>
    


    <!-- http://www.project-best.eu/owl/aixm-mod/airportheliport#UsageCondition-priorPermission -->

    <owl:DatatypeProperty rdf:about="http://www.project-best.eu/owl/aixm-mod/airportheliport#UsageCondition-priorPermission">
        <rdfs:comment xml:lang="en">For a Conditional Permission, this indicates that a prior permission is required.  Positive values indicate prior permission required before using the airport movement area.</rdfs:comment>
        <rdfs:domain rdf:resource="http://www.project-best.eu/owl/aixm-mod/airportheliport#UsageCondition"/>
        <rdfs:range rdf:resource="http://www.w3.org/2001/XMLSchema#decimal"/>
    </owl:DatatypeProperty>
    


    <!-- http://www.project-best.eu/owl/aixm-mod/airportheliport#VisualGlideSlopeIndicator-minimumEyeHightOverThreshold -->

    <owl:DatatypeProperty rdf:about="http://www.project-best.eu/owl/aixm-mod/airportheliport#VisualGlideSlopeIndicator-minimumEyeHightOverThreshold">
        <rdfs:domain rdf:resource="http://www.project-best.eu/owl/aixm-mod/airportheliport#VisualGlideSlopeIndicator"/>
        <rdfs:range rdf:resource="http://www.w3.org/2001/XMLSchema#decimal"/>
    </owl:DatatypeProperty>
    


    <!-- http://www.project-best.eu/owl/aixm-mod/airportheliport#VisualGlideSlopeIndicator-numberBox -->

    <owl:DatatypeProperty rdf:about="http://www.project-best.eu/owl/aixm-mod/airportheliport#VisualGlideSlopeIndicator-numberBox">
        <rdfs:comment xml:lang="en">The number of boxes that compose the visual approach slope indicator system.</rdfs:comment>
        <rdfs:domain rdf:resource="http://www.project-best.eu/owl/aixm-mod/airportheliport#VisualGlideSlopeIndicator"/>
        <rdfs:range rdf:resource="http://www.w3.org/2001/XMLSchema#decimal"/>
    </owl:DatatypeProperty>
    


    <!-- http://www.project-best.eu/owl/aixm-mod/airportheliport#VisualGlideSlopeIndicator-slopeAngle -->

    <owl:DatatypeProperty rdf:about="http://www.project-best.eu/owl/aixm-mod/airportheliport#VisualGlideSlopeIndicator-slopeAngle">
        <rdfs:comment xml:lang="en">The appropriate approach slope angle to be used by an aircraft using the approach.</rdfs:comment>
        <rdfs:domain rdf:resource="http://www.project-best.eu/owl/aixm-mod/airportheliport#VisualGlideSlopeIndicator"/>
        <rdfs:range rdf:resource="http://www.w3.org/2001/XMLSchema#decimal"/>
    </owl:DatatypeProperty>
    


    <!-- http://www.project-best.eu/owl/aixm-mod/airportheliport#WorkArea-plannedOperational -->

    <owl:DatatypeProperty rdf:about="http://www.project-best.eu/owl/aixm-mod/airportheliport#WorkArea-plannedOperational">
        <rdfs:comment xml:lang="en">Date when the activities in the construction area are expected to be operational.</rdfs:comment>
        <rdfs:domain rdf:resource="http://www.project-best.eu/owl/aixm-mod/airportheliport#WorkArea"/>
        <rdfs:range rdf:resource="http://www.w3.org/2001/XMLSchema#string"/>
    </owl:DatatypeProperty>
    


    <!-- 
    ///////////////////////////////////////////////////////////////////////////////////////
    //
    // Classes
    //
    ///////////////////////////////////////////////////////////////////////////////////////
     -->

    


    <!-- http://www.project-best.eu/owl/aixm-mod/airportheliport#AircraftStand -->

    <owl:Class rdf:about="http://www.project-best.eu/owl/aixm-mod/airportheliport#AircraftStand">
        <rdfs:comment xml:lang="en">A designated area on an apron intended to be used for parking an aircraft.</rdfs:comment>
    </owl:Class>
    


    <!-- http://www.project-best.eu/owl/aixm-mod/airportheliport#AircraftStandContamination -->

    <owl:Class rdf:about="http://www.project-best.eu/owl/aixm-mod/airportheliport#AircraftStandContamination">
        <rdfs:subClassOf rdf:resource="http://www.project-best.eu/owl/aixm-mod/airportheliport#SurfaceContamination"/>
        <rdfs:comment xml:lang="en">The presence or removal of hazardous conditions due to snow, ice, slush, water, etc. at an AircraftStand.</rdfs:comment>
    </owl:Class>
    


    <!-- http://www.project-best.eu/owl/aixm-mod/airportheliport#AirportHeliport -->

    <owl:Class rdf:about="http://www.project-best.eu/owl/aixm-mod/airportheliport#AirportHeliport">
        <rdfs:comment xml:lang="en">A defined area on land or water (including any buildings, installations and equipment) intended to be used either wholly or in part for the arrival, departure and surface movement of aircraft/helicopters.</rdfs:comment>
    </owl:Class>
    


    <!-- http://www.project-best.eu/owl/aixm-mod/airportheliport#AirportHeliportAvailability -->

    <owl:Class rdf:about="http://www.project-best.eu/owl/aixm-mod/airportheliport#AirportHeliportAvailability">
        <rdfs:comment xml:lang="en">Information about the operational status of the airport/heliport.</rdfs:comment>
        <rdfs:comment xml:lang="en">Subclass of Shared::Schedules::PropertiesWithSchedule</rdfs:comment>
    </owl:Class>
    


    <!-- http://www.project-best.eu/owl/aixm-mod/airportheliport#AirportHeliportCollocation -->

    <owl:Class rdf:about="http://www.project-best.eu/owl/aixm-mod/airportheliport#AirportHeliportCollocation">
        <rdfs:comment xml:lang="en">Two aerodromes/heliports may be co-located sharing some or all of their ground facilities.</rdfs:comment>
    </owl:Class>
    


    <!-- http://www.project-best.eu/owl/aixm-mod/airportheliport#AirportHeliportContamination -->

    <owl:Class rdf:about="http://www.project-best.eu/owl/aixm-mod/airportheliport#AirportHeliportContamination">
        <rdfs:subClassOf rdf:resource="http://www.project-best.eu/owl/aixm-mod/airportheliport#SurfaceContamination"/>
        <rdfs:comment xml:lang="en">The presence or removal of hazardous conditions due to snow, ice, slush, water, etc. on the airport surfaces.</rdfs:comment>
    </owl:Class>
    


    <!-- http://www.project-best.eu/owl/aixm-mod/airportheliport#AirportHeliportProtectionArea -->

    <owl:Class rdf:about="http://www.project-best.eu/owl/aixm-mod/airportheliport#AirportHeliportProtectionArea">
        <rdfs:comment xml:lang="en">An area situated in the vicinity of a runway, FATO or TLOF, provided to protect aircraft during manoeuvring, take-off and/or landing operations.</rdfs:comment>
    </owl:Class>
    


    <!-- http://www.project-best.eu/owl/aixm-mod/airportheliport#AirportHeliportResponsibilityOrganisation -->

    <owl:Class rdf:about="http://www.project-best.eu/owl/aixm-mod/airportheliport#AirportHeliportResponsibilityOrganisation">
        <rdfs:comment xml:lang="en">Characterises the role of the organisation or authority which is responsible for the AirportHeliport</rdfs:comment>
        <rdfs:comment xml:lang="en">Subclass of Shared::Schedules::PropertiesWithSchedule</rdfs:comment>
    </owl:Class>
    


    <!-- http://www.project-best.eu/owl/aixm-mod/airportheliport#AirportHeliportUsage -->

    <owl:Class rdf:about="http://www.project-best.eu/owl/aixm-mod/airportheliport#AirportHeliportUsage">
        <rdfs:subClassOf rdf:resource="http://www.project-best.eu/owl/aixm-mod/airportheliport#UsageCondition"/>
        <rdfs:comment xml:lang="en">A rule governing the usage of an AirportHeliport.</rdfs:comment>
    </owl:Class>
    


    <!-- http://www.project-best.eu/owl/aixm-mod/airportheliport#AirportHotSpot -->

    <owl:Class rdf:about="http://www.project-best.eu/owl/aixm-mod/airportheliport#AirportHotSpot">
        <rdfs:comment xml:lang="en">A location on aerodrome movement area with a history or potential risk of collision or runway incursion, and where heightened attention by pilots/drivers is necessary.</rdfs:comment>
    </owl:Class>
    


    <!-- http://www.project-best.eu/owl/aixm-mod/airportheliport#AirportProtectionAreaMarking -->

    <owl:Class rdf:about="http://www.project-best.eu/owl/aixm-mod/airportheliport#AirportProtectionAreaMarking">
        <rdfs:subClassOf rdf:resource="http://www.project-best.eu/owl/aixm-mod/airportheliport#Marking"/>
        <rdfs:comment xml:lang="en">A symbol or group of symbols displayed on the edge of the landing protection area.</rdfs:comment>
    </owl:Class>
    


    <!-- http://www.project-best.eu/owl/aixm-mod/airportheliport#AltimeterSource -->

    <owl:Class rdf:about="http://www.project-best.eu/owl/aixm-mod/airportheliport#AltimeterSource">
        <rdfs:comment xml:lang="en">An instrument that measures and indicates the elevation at which an object, such as an airplane, is located</rdfs:comment>
    </owl:Class>
    


    <!-- http://www.project-best.eu/owl/aixm-mod/airportheliport#AltimeterSourceStatus -->

    <owl:Class rdf:about="http://www.project-best.eu/owl/aixm-mod/airportheliport#AltimeterSourceStatus">
        <rdfs:comment xml:lang="en">Information about the operational status of an Altimeter Source.</rdfs:comment>
        <rdfs:comment xml:lang="en">Subclass of Shared::Schedules::PropertiesWithSchedule</rdfs:comment>
    </owl:Class>
    


    <!-- http://www.project-best.eu/owl/aixm-mod/airportheliport#ApproachLightingSystem -->

    <owl:Class rdf:about="http://www.project-best.eu/owl/aixm-mod/airportheliport#ApproachLightingSystem">
        <rdfs:subClassOf rdf:resource="http://www.project-best.eu/owl/aixm-mod/airportheliport#GroundLightSystem"/>
        <rdfs:comment xml:lang="en">An airport lighting facility which provides visual guidance to landing aircraft by radiating light beams in a directional pattern by which the pilot aligns the aircraft with the final approach path for landing.</rdfs:comment>
    </owl:Class>
    


    <!-- http://www.project-best.eu/owl/aixm-mod/airportheliport#Apron -->

    <owl:Class rdf:about="http://www.project-best.eu/owl/aixm-mod/airportheliport#Apron">
        <rdfs:comment xml:lang="en">A defined area, on a land aerodrome/heliport, intended to accommodate aircraft/helicopters for purposes of loading and unloading passengers, mail or cargo, and for fuelling, parking or maintenance.</rdfs:comment>
    </owl:Class>
    


    <!-- http://www.project-best.eu/owl/aixm-mod/airportheliport#ApronAreaAvailability -->

    <owl:Class rdf:about="http://www.project-best.eu/owl/aixm-mod/airportheliport#ApronAreaAvailability">
        <rdfs:comment xml:lang="en">Information about the operational status of an element situated in the apron area.</rdfs:comment>
        <rdfs:comment xml:lang="en">Subclass of Shared::Schedules::PropertiesWithSchedule</rdfs:comment>
    </owl:Class>
    


    <!-- http://www.project-best.eu/owl/aixm-mod/airportheliport#ApronAreaUsage -->

    <owl:Class rdf:about="http://www.project-best.eu/owl/aixm-mod/airportheliport#ApronAreaUsage">
        <rdfs:subClassOf rdf:resource="http://www.project-best.eu/owl/aixm-mod/airportheliport#UsageCondition"/>
        <rdfs:comment xml:lang="en">A rule governing the usage of an element situated in the apron area.</rdfs:comment>
    </owl:Class>
    


    <!-- http://www.project-best.eu/owl/aixm-mod/airportheliport#ApronContamination -->

    <owl:Class rdf:about="http://www.project-best.eu/owl/aixm-mod/airportheliport#ApronContamination">
        <rdfs:subClassOf rdf:resource="http://www.project-best.eu/owl/aixm-mod/airportheliport#SurfaceContamination"/>
        <rdfs:comment xml:lang="en">The presence or removal of hazardous conditions due to snow, ice, slush, water, etc. on the Apron surface.</rdfs:comment>
    </owl:Class>
    


    <!-- http://www.project-best.eu/owl/aixm-mod/airportheliport#ApronElement -->

    <owl:Class rdf:about="http://www.project-best.eu/owl/aixm-mod/airportheliport#ApronElement">
        <rdfs:comment xml:lang="en">Parts of a defined apron area.  ApronElements may have functional characteristics defined in the ApronElement type.  ApronElements may have jetway, fuel, towing, docking and groundPower services.</rdfs:comment>
    </owl:Class>
    


    <!-- http://www.project-best.eu/owl/aixm-mod/airportheliport#ApronLightSystem -->

    <owl:Class rdf:about="http://www.project-best.eu/owl/aixm-mod/airportheliport#ApronLightSystem">
        <rdfs:subClassOf rdf:resource="http://www.project-best.eu/owl/aixm-mod/airportheliport#GroundLightSystem"/>
        <rdfs:comment xml:lang="en">The lighting system provided for an apron.</rdfs:comment>
    </owl:Class>
    


    <!-- http://www.project-best.eu/owl/aixm-mod/airportheliport#ApronMarking -->

    <owl:Class rdf:about="http://www.project-best.eu/owl/aixm-mod/airportheliport#ApronMarking">
        <rdfs:subClassOf rdf:resource="http://www.project-best.eu/owl/aixm-mod/airportheliport#Marking"/>
        <rdfs:comment xml:lang="en">A symbol or group of symbols displayed on the surface of the apron.</rdfs:comment>
    </owl:Class>
    


    <!-- http://www.project-best.eu/owl/aixm-mod/airportheliport#ArrestingGear -->

    <owl:Class rdf:about="http://www.project-best.eu/owl/aixm-mod/airportheliport#ArrestingGear">
        <rdfs:comment xml:lang="en">A series of devices, namely engaging or catching devices and energy absorption devices used to stop an aircraft by absorbing its momentum in a routine, emergency landing or aborted take-off.</rdfs:comment>
    </owl:Class>
    


    <!-- http://www.project-best.eu/owl/aixm-mod/airportheliport#ArrestingGearExtent -->

    <owl:Class rdf:about="http://www.project-best.eu/owl/aixm-mod/airportheliport#ArrestingGearExtent">
        <rdfs:comment xml:lang="en">A link class that allows selecting between a point, a curve or a surface to define the geometry of an ArrestingGear</rdfs:comment>
    </owl:Class>
    


    <!-- http://www.project-best.eu/owl/aixm-mod/airportheliport#City -->

    <owl:Class rdf:about="http://www.project-best.eu/owl/aixm-mod/airportheliport#City">
        <rdfs:comment xml:lang="en">A city or location that may be served by an airport/heliport.</rdfs:comment>
    </owl:Class>
    


    <!-- http://www.project-best.eu/owl/aixm-mod/airportheliport#CodeAircraftStandType -->

    <owl:Class rdf:about="http://www.project-best.eu/owl/aixm-mod/airportheliport#CodeAircraftStandType">
        <rdfs:comment xml:lang="en">A code indicating the type of stand.</rdfs:comment>
    </owl:Class>
    


    <!-- http://www.project-best.eu/owl/aixm-mod/airportheliport#CodeAirportHeliportCollocationType -->

    <owl:Class rdf:about="http://www.project-best.eu/owl/aixm-mod/airportheliport#CodeAirportHeliportCollocationType">
        <rdfs:comment xml:lang="en">A code indicating the extent of collocation between two airports/heliports. </rdfs:comment>
    </owl:Class>
    


    <!-- http://www.project-best.eu/owl/aixm-mod/airportheliport#CodeAirportHeliportType -->

    <owl:Class rdf:about="http://www.project-best.eu/owl/aixm-mod/airportheliport#CodeAirportHeliportType">
        <rdfs:comment xml:lang="en">A code specifying whether a particular entity occurrence is an Aerodrome or a Heliport. </rdfs:comment>
    </owl:Class>
    


    <!-- http://www.project-best.eu/owl/aixm-mod/airportheliport#CodeAirportWarningType -->

    <owl:Class rdf:about="http://www.project-best.eu/owl/aixm-mod/airportheliport#CodeAirportWarningType">
        <rdfs:comment xml:lang="en">A code indicating a reason for caution in airport operations.  For example, work in progress on a runway.</rdfs:comment>
    </owl:Class>
    


    <!-- http://www.project-best.eu/owl/aixm-mod/airportheliport#CodeApproachGuidanceType -->

    <owl:Class rdf:about="http://www.project-best.eu/owl/aixm-mod/airportheliport#CodeApproachGuidanceType">
        <rdfs:comment xml:lang="en">Degree to which navigation aids provide accurate approach guidance.  Precision approaches utilize both lateral (course) and vertical (glideslope) information</rdfs:comment>
    </owl:Class>
    


    <!-- http://www.project-best.eu/owl/aixm-mod/airportheliport#CodeApproachLightingICAOType -->

    <owl:Class rdf:about="http://www.project-best.eu/owl/aixm-mod/airportheliport#CodeApproachLightingICAOType">
        <rdfs:comment xml:lang="en">Classification of the approach lighting system using as criteria the ICAO Annex 14 standards and recommended practices.</rdfs:comment>
    </owl:Class>
    


    <!-- http://www.project-best.eu/owl/aixm-mod/airportheliport#CodeApproachLightingType -->

    <owl:Class rdf:about="http://www.project-best.eu/owl/aixm-mod/airportheliport#CodeApproachLightingType">
        <rdfs:comment xml:lang="en">A regional or organisation specific classification of the Runway approach lighting system equipment. Could also be a brand name. </rdfs:comment>
    </owl:Class>
    


    <!-- http://www.project-best.eu/owl/aixm-mod/airportheliport#CodeApronElementType -->

    <owl:Class rdf:about="http://www.project-best.eu/owl/aixm-mod/airportheliport#CodeApronElementType">
        <rdfs:comment xml:lang="en">A code indicating the type of Apron.</rdfs:comment>
    </owl:Class>
    


    <!-- http://www.project-best.eu/owl/aixm-mod/airportheliport#CodeApronSectionType -->

    <owl:Class rdf:about="http://www.project-best.eu/owl/aixm-mod/airportheliport#CodeApronSectionType">
        <rdfs:comment xml:lang="en">A code indicating a location on the surface of an apron. For example: apron edge. </rdfs:comment>
    </owl:Class>
    


    <!-- http://www.project-best.eu/owl/aixm-mod/airportheliport#CodeArrestingGearEnergyAbsorbType -->

    <owl:Class rdf:about="http://www.project-best.eu/owl/aixm-mod/airportheliport#CodeArrestingGearEnergyAbsorbType">
        <rdfs:comment xml:lang="en">The type of energy absorber (for example: a rotary brake) by which the arresting gear system rapidly dissipates the kinetic energy of a moving aircraft that engages the arresting system, bringing the aircraft to a stop.</rdfs:comment>
    </owl:Class>
    


    <!-- http://www.project-best.eu/owl/aixm-mod/airportheliport#CodeArrestingGearEngageDeviceType -->

    <owl:Class rdf:about="http://www.project-best.eu/owl/aixm-mod/airportheliport#CodeArrestingGearEngageDeviceType">
        <rdfs:comment xml:lang="en">A code indicating the type of device (for example: a hook) that is used to engage an aircraft upon landing in order to immediately stop it.</rdfs:comment>
    </owl:Class>
    


    <!-- http://www.project-best.eu/owl/aixm-mod/airportheliport#CodeAuthorityRoleType -->

    <owl:Class rdf:about="http://www.project-best.eu/owl/aixm-mod/airportheliport#CodeAuthorityRoleType">
        <rdfs:comment xml:lang="en">A code indicating the role of the OrganisationAuthority for the aeronautical feature.  </rdfs:comment>
    </owl:Class>
    


    <!-- http://www.project-best.eu/owl/aixm-mod/airportheliport#CodeBuoyType -->

    <owl:Class rdf:about="http://www.project-best.eu/owl/aixm-mod/airportheliport#CodeBuoyType">
        <rdfs:comment xml:lang="en">Code indicating the type of Buoy</rdfs:comment>
    </owl:Class>
    


    <!-- http://www.project-best.eu/owl/aixm-mod/airportheliport#CodeColourType -->

    <owl:Class rdf:about="http://www.project-best.eu/owl/aixm-mod/airportheliport#CodeColourType">
        <rdfs:comment xml:lang="en">A code indicating a colour. The list of allowable values comprises &apos;named&apos; colours, not colours being only describable using the RGB or the CYMK or another colour system combination. </rdfs:comment>
    </owl:Class>
    


    <!-- http://www.project-best.eu/owl/aixm-mod/airportheliport#CodeContaminationType -->

    <owl:Class rdf:about="http://www.project-best.eu/owl/aixm-mod/airportheliport#CodeContaminationType">
        <rdfs:comment xml:lang="en">An enumeration of substance types, which can contaminate airport/heliport movement areas.</rdfs:comment>
    </owl:Class>
    


    <!-- http://www.project-best.eu/owl/aixm-mod/airportheliport#CodeDayType -->

    <owl:Class rdf:about="http://www.project-best.eu/owl/aixm-mod/airportheliport#CodeDayType">
        <rdfs:comment xml:lang="en">A code indicating a particular day.</rdfs:comment>
    </owl:Class>
    


    <!-- http://www.project-best.eu/owl/aixm-mod/airportheliport#CodeDeclaredDistanceType -->

    <owl:Class rdf:about="http://www.project-best.eu/owl/aixm-mod/airportheliport#CodeDeclaredDistanceType">
        <rdfs:comment xml:lang="en">A code indicating the type of conventional declared distance for a runway. </rdfs:comment>
    </owl:Class>
    


    <!-- http://www.project-best.eu/owl/aixm-mod/airportheliport#CodeDirectionTurnType -->

    <owl:Class rdf:about="http://www.project-best.eu/owl/aixm-mod/airportheliport#CodeDirectionTurnType">
        <rdfs:comment xml:lang="en">A code indicating the direction of a turn. </rdfs:comment>
    </owl:Class>
    


    <!-- http://www.project-best.eu/owl/aixm-mod/airportheliport#CodeDirectionType -->

    <owl:Class rdf:about="http://www.project-best.eu/owl/aixm-mod/airportheliport#CodeDirectionType">
        <rdfs:comment xml:lang="en">A code indicating a 1-dimensional direction, for example, forward or backward. </rdfs:comment>
    </owl:Class>
    


    <!-- http://www.project-best.eu/owl/aixm-mod/airportheliport#CodeFrictionDeviceType -->

    <owl:Class rdf:about="http://www.project-best.eu/owl/aixm-mod/airportheliport#CodeFrictionDeviceType">
        <rdfs:comment xml:lang="en">An enumeration of equipment types used to determine the friction coefficient on an airport/heliport movement area.</rdfs:comment>
    </owl:Class>
    


    <!-- http://www.project-best.eu/owl/aixm-mod/airportheliport#CodeFrictionEstimateType -->

    <owl:Class rdf:about="http://www.project-best.eu/owl/aixm-mod/airportheliport#CodeFrictionEstimateType">
        <rdfs:comment xml:lang="en">An enumeration of qualitative estimates of the friction on a movement area.</rdfs:comment>
    </owl:Class>
    


    <!-- http://www.project-best.eu/owl/aixm-mod/airportheliport#CodeGradeSeparationType -->

    <owl:Class rdf:about="http://www.project-best.eu/owl/aixm-mod/airportheliport#CodeGradeSeparationType">
        <rdfs:comment xml:lang="en">A list of coded values that indicate the placement of an element at a different height from another element.</rdfs:comment>
    </owl:Class>
    


    <!-- http://www.project-best.eu/owl/aixm-mod/airportheliport#CodeGuidanceLineType -->

    <owl:Class rdf:about="http://www.project-best.eu/owl/aixm-mod/airportheliport#CodeGuidanceLineType">
        <rdfs:comment xml:lang="en">A code indicating the type of guidance line.</rdfs:comment>
    </owl:Class>
    


    <!-- http://www.project-best.eu/owl/aixm-mod/airportheliport#CodeHelicopterPerformanceType -->

    <owl:Class rdf:about="http://www.project-best.eu/owl/aixm-mod/airportheliport#CodeHelicopterPerformanceType">
        <rdfs:comment xml:lang="en">A code indicating the performance class of a helicopter. </rdfs:comment>
    </owl:Class>
    


    <!-- http://www.project-best.eu/owl/aixm-mod/airportheliport#CodeHoldingCategoryType -->

    <owl:Class rdf:about="http://www.project-best.eu/owl/aixm-mod/airportheliport#CodeHoldingCategoryType">
        <rdfs:comment xml:lang="en">A coded list of values that indicates the type of precision approach for which that holding position is designed.</rdfs:comment>
    </owl:Class>
    


    <!-- http://www.project-best.eu/owl/aixm-mod/airportheliport#CodeLightHoldingPositionType -->

    <owl:Class rdf:about="http://www.project-best.eu/owl/aixm-mod/airportheliport#CodeLightHoldingPositionType">
        <rdfs:comment xml:lang="en">A coded list of light signs provided for a taxiway holding position.</rdfs:comment>
    </owl:Class>
    


    <!-- http://www.project-best.eu/owl/aixm-mod/airportheliport#CodeLightIntensityType -->

    <owl:Class rdf:about="http://www.project-best.eu/owl/aixm-mod/airportheliport#CodeLightIntensityType">
        <rdfs:comment xml:lang="en">A code indicating the intensity level of a light source.</rdfs:comment>
    </owl:Class>
    


    <!-- http://www.project-best.eu/owl/aixm-mod/airportheliport#CodeLightSourceType -->

    <owl:Class rdf:about="http://www.project-best.eu/owl/aixm-mod/airportheliport#CodeLightSourceType">
        <rdfs:comment xml:lang="en">A code indicating a type of light source, such as strobe or flood. </rdfs:comment>
    </owl:Class>
    


    <!-- http://www.project-best.eu/owl/aixm-mod/airportheliport#CodeLightingJARType -->

    <owl:Class rdf:about="http://www.project-best.eu/owl/aixm-mod/airportheliport#CodeLightingJARType">
        <rdfs:comment xml:lang="en">Classification of the approach lighting system using as criteria JAR-OPS 1 - Subpart E, Appendix 1 to 1.430]</rdfs:comment>
    </owl:Class>
    


    <!-- http://www.project-best.eu/owl/aixm-mod/airportheliport#CodeLoadingBridgeType -->

    <owl:Class rdf:about="http://www.project-best.eu/owl/aixm-mod/airportheliport#CodeLoadingBridgeType">
        <rdfs:comment xml:lang="en">An coded list of values that indicate types of passenger loading bridges.</rdfs:comment>
    </owl:Class>
    


    <!-- http://www.project-best.eu/owl/aixm-mod/airportheliport#CodeLogicalOperatorType -->

    <owl:Class rdf:about="http://www.project-best.eu/owl/aixm-mod/airportheliport#CodeLogicalOperatorType">
        <rdfs:comment xml:lang="en">A boolean operator.</rdfs:comment>
    </owl:Class>
    


    <!-- http://www.project-best.eu/owl/aixm-mod/airportheliport#CodeMarkingConditionType -->

    <owl:Class rdf:about="http://www.project-best.eu/owl/aixm-mod/airportheliport#CodeMarkingConditionType">
        <rdfs:comment xml:lang="en">A coded list of values that indicate the status of the painted surface marking elements.</rdfs:comment>
    </owl:Class>
    


    <!-- http://www.project-best.eu/owl/aixm-mod/airportheliport#CodeMarkingStyleType -->

    <owl:Class rdf:about="http://www.project-best.eu/owl/aixm-mod/airportheliport#CodeMarkingStyleType">
        <rdfs:comment xml:lang="en">A coded list of values indicating styles of painted lines.</rdfs:comment>
    </owl:Class>
    


    <!-- http://www.project-best.eu/owl/aixm-mod/airportheliport#CodeMeteoConditionsType -->

    <owl:Class rdf:about="http://www.project-best.eu/owl/aixm-mod/airportheliport#CodeMeteoConditionsType">
        <rdfs:comment xml:lang="en">A code indicating whether the meteorological conditions allow visual or instrumental operations.</rdfs:comment>
    </owl:Class>
    


    <!-- http://www.project-best.eu/owl/aixm-mod/airportheliport#CodeMilitaryOperationsType -->

    <owl:Class rdf:about="http://www.project-best.eu/owl/aixm-mod/airportheliport#CodeMilitaryOperationsType">
        <rdfs:comment xml:lang="en">A code indicating in terms of civil or military, the type of operations.</rdfs:comment>
    </owl:Class>
    


    <!-- http://www.project-best.eu/owl/aixm-mod/airportheliport#CodeOperationAirportHeliportType -->

    <owl:Class rdf:about="http://www.project-best.eu/owl/aixm-mod/airportheliport#CodeOperationAirportHeliportType">
        <rdfs:comment xml:lang="en">A coded identifier indicating an operation executed by an aircraft in relation with an airport/heliport. </rdfs:comment>
    </owl:Class>
    


    <!-- http://www.project-best.eu/owl/aixm-mod/airportheliport#CodeOperationManoeuvringAreaType -->

    <owl:Class rdf:about="http://www.project-best.eu/owl/aixm-mod/airportheliport#CodeOperationManoeuvringAreaType">
        <rdfs:comment xml:lang="en">A coded list of values that indicates a type of activity on an airport/heliport manoeuvring area element.</rdfs:comment>
    </owl:Class>
    


    <!-- http://www.project-best.eu/owl/aixm-mod/airportheliport#CodePCNMethodType -->

    <owl:Class rdf:about="http://www.project-best.eu/owl/aixm-mod/airportheliport#CodePCNMethodType">
        <rdfs:comment xml:lang="en">A code indicating the method used in the evaluation of a PCN number. </rdfs:comment>
    </owl:Class>
    


    <!-- http://www.project-best.eu/owl/aixm-mod/airportheliport#CodePCNPavementType -->

    <owl:Class rdf:about="http://www.project-best.eu/owl/aixm-mod/airportheliport#CodePCNPavementType">
        <rdfs:comment xml:lang="en">A code indicating the pavement behaviour (rigid or flexible) used for the ACN determination. </rdfs:comment>
    </owl:Class>
    


    <!-- http://www.project-best.eu/owl/aixm-mod/airportheliport#CodePCNSubgradeType -->

    <owl:Class rdf:about="http://www.project-best.eu/owl/aixm-mod/airportheliport#CodePCNSubgradeType">
        <rdfs:comment xml:lang="en">A code indicating the sub-grade strength category related to a PCN number. </rdfs:comment>
    </owl:Class>
    


    <!-- http://www.project-best.eu/owl/aixm-mod/airportheliport#CodePCNTyrePressureType -->

    <owl:Class rdf:about="http://www.project-best.eu/owl/aixm-mod/airportheliport#CodePCNTyrePressureType">
        <rdfs:comment xml:lang="en">A code indicating the maximum allowable tyre pressure category related to a PCN number. </rdfs:comment>
    </owl:Class>
    


    <!-- http://www.project-best.eu/owl/aixm-mod/airportheliport#CodeProtectAreaSectionType -->

    <owl:Class rdf:about="http://www.project-best.eu/owl/aixm-mod/airportheliport#CodeProtectAreaSectionType">
        <rdfs:comment xml:lang="en">A code indicating the location of the Protect Area lighting.</rdfs:comment>
    </owl:Class>
    


    <!-- http://www.project-best.eu/owl/aixm-mod/airportheliport#CodeRVRReadingType -->

    <owl:Class rdf:about="http://www.project-best.eu/owl/aixm-mod/airportheliport#CodeRVRReadingType">
        <rdfs:comment xml:lang="en">A code indicating the position where the RVR reading is reported.</rdfs:comment>
    </owl:Class>
    


    <!-- http://www.project-best.eu/owl/aixm-mod/airportheliport#CodeRoadType -->

    <owl:Class rdf:about="http://www.project-best.eu/owl/aixm-mod/airportheliport#CodeRoadType">
        <rdfs:comment xml:lang="en">A code indicating the type of a road.</rdfs:comment>
    </owl:Class>
    


    <!-- http://www.project-best.eu/owl/aixm-mod/airportheliport#CodeRunwayElementType -->

    <owl:Class rdf:about="http://www.project-best.eu/owl/aixm-mod/airportheliport#CodeRunwayElementType">
        <rdfs:comment xml:lang="en">A code indicating the type of Runway or Taxiway element.</rdfs:comment>
    </owl:Class>
    


    <!-- http://www.project-best.eu/owl/aixm-mod/airportheliport#CodeRunwayMarkingType -->

    <owl:Class rdf:about="http://www.project-best.eu/owl/aixm-mod/airportheliport#CodeRunwayMarkingType">
        <rdfs:comment xml:lang="en">Type of runway marking related to landing categories such as precision, non-precision and basic.</rdfs:comment>
    </owl:Class>
    


    <!-- http://www.project-best.eu/owl/aixm-mod/airportheliport#CodeRunwayPointRoleType -->

    <owl:Class rdf:about="http://www.project-best.eu/owl/aixm-mod/airportheliport#CodeRunwayPointRoleType">
        <rdfs:comment xml:lang="en">Role of the Runway Centreline Point.</rdfs:comment>
    </owl:Class>
    


    <!-- http://www.project-best.eu/owl/aixm-mod/airportheliport#CodeRunwayProtectionAreaType -->

    <owl:Class rdf:about="http://www.project-best.eu/owl/aixm-mod/airportheliport#CodeRunwayProtectionAreaType">
        <rdfs:comment xml:lang="en">A code indicating the type of protection area for a runway</rdfs:comment>
    </owl:Class>
    


    <!-- http://www.project-best.eu/owl/aixm-mod/airportheliport#CodeRunwaySectionType -->

    <owl:Class rdf:about="http://www.project-best.eu/owl/aixm-mod/airportheliport#CodeRunwaySectionType">
        <rdfs:comment xml:lang="en">A code indicating the position of an item on a surface of a runway.</rdfs:comment>
    </owl:Class>
    


    <!-- http://www.project-best.eu/owl/aixm-mod/airportheliport#CodeRunwayType -->

    <owl:Class rdf:about="http://www.project-best.eu/owl/aixm-mod/airportheliport#CodeRunwayType">
        <rdfs:comment xml:lang="en">A code that makes a distinction between runways for airplanes and FATO for helicopters.</rdfs:comment>
    </owl:Class>
    


    <!-- http://www.project-best.eu/owl/aixm-mod/airportheliport#CodeSideType -->

    <owl:Class rdf:about="http://www.project-best.eu/owl/aixm-mod/airportheliport#CodeSideType">
        <rdfs:comment xml:lang="en">A code describing a position, relative to an axis. For example: left/right of runway centreline.</rdfs:comment>
    </owl:Class>
    


    <!-- http://www.project-best.eu/owl/aixm-mod/airportheliport#CodeStatusAirportType -->

    <owl:Class rdf:about="http://www.project-best.eu/owl/aixm-mod/airportheliport#CodeStatusAirportType">
        <rdfs:comment xml:lang="en">A coded list of values that indicates the availability of an airport/heliport facility for specific flight operations.</rdfs:comment>
    </owl:Class>
    


    <!-- http://www.project-best.eu/owl/aixm-mod/airportheliport#CodeStatusConstructionType -->

    <owl:Class rdf:about="http://www.project-best.eu/owl/aixm-mod/airportheliport#CodeStatusConstructionType">
        <rdfs:comment xml:lang="en">A code indicating the status of the construction of a Vertical Structure.</rdfs:comment>
    </owl:Class>
    


    <!-- http://www.project-best.eu/owl/aixm-mod/airportheliport#CodeStatusOperationsType -->

    <owl:Class rdf:about="http://www.project-best.eu/owl/aixm-mod/airportheliport#CodeStatusOperationsType">
        <rdfs:comment xml:lang="en">Code indicating operational status.</rdfs:comment>
    </owl:Class>
    


    <!-- http://www.project-best.eu/owl/aixm-mod/airportheliport#CodeSurfaceCompositionType -->

    <owl:Class rdf:about="http://www.project-best.eu/owl/aixm-mod/airportheliport#CodeSurfaceCompositionType">
        <rdfs:comment xml:lang="en">A code indicating the composition of a surface.</rdfs:comment>
    </owl:Class>
    


    <!-- http://www.project-best.eu/owl/aixm-mod/airportheliport#CodeSurfaceConditionType -->

    <owl:Class rdf:about="http://www.project-best.eu/owl/aixm-mod/airportheliport#CodeSurfaceConditionType">
        <rdfs:comment xml:lang="en">A code indicating the condition of a surface, such as a runway, taxiway, the marking of a threshold, etc.. </rdfs:comment>
    </owl:Class>
    


    <!-- http://www.project-best.eu/owl/aixm-mod/airportheliport#CodeSurfacePreparationType -->

    <owl:Class rdf:about="http://www.project-best.eu/owl/aixm-mod/airportheliport#CodeSurfacePreparationType">
        <rdfs:comment xml:lang="en">A code indicating the preparation technique for a surface area. </rdfs:comment>
    </owl:Class>
    


    <!-- http://www.project-best.eu/owl/aixm-mod/airportheliport#CodeSystemActivationType -->

    <owl:Class rdf:about="http://www.project-best.eu/owl/aixm-mod/airportheliport#CodeSystemActivationType">
        <rdfs:comment xml:lang="en">A code indicating the activation / deactivation of a system following a specific comand.</rdfs:comment>
    </owl:Class>
    


    <!-- http://www.project-best.eu/owl/aixm-mod/airportheliport#CodeTLOFSectionType -->

    <owl:Class rdf:about="http://www.project-best.eu/owl/aixm-mod/airportheliport#CodeTLOFSectionType">
        <rdfs:comment xml:lang="en">A code indicating the position of an item on the surface of a Touch Down and Lift-off Area. </rdfs:comment>
    </owl:Class>
    


    <!-- http://www.project-best.eu/owl/aixm-mod/airportheliport#CodeTaxiwayElementType -->

    <owl:Class rdf:about="http://www.project-best.eu/owl/aixm-mod/airportheliport#CodeTaxiwayElementType">
        <rdfs:comment xml:lang="en">A code list of values indicating a component of the taxiway surface.</rdfs:comment>
    </owl:Class>
    


    <!-- http://www.project-best.eu/owl/aixm-mod/airportheliport#CodeTaxiwaySectionType -->

    <owl:Class rdf:about="http://www.project-best.eu/owl/aixm-mod/airportheliport#CodeTaxiwaySectionType">
        <rdfs:comment xml:lang="en">A code indicating the position of an item on the surface of a taxiway. </rdfs:comment>
    </owl:Class>
    


    <!-- http://www.project-best.eu/owl/aixm-mod/airportheliport#CodeTaxiwayType -->

    <owl:Class rdf:about="http://www.project-best.eu/owl/aixm-mod/airportheliport#CodeTaxiwayType">
        <rdfs:comment xml:lang="en">A code indicating a type of taxiway.</rdfs:comment>
    </owl:Class>
    


    <!-- http://www.project-best.eu/owl/aixm-mod/airportheliport#CodeTelecomNetworkType -->

    <owl:Class rdf:about="http://www.project-best.eu/owl/aixm-mod/airportheliport#CodeTelecomNetworkType">
        <rdfs:comment xml:lang="en">Codelist containing the Telecom Networks that can be used to address an organisation.</rdfs:comment>
    </owl:Class>
    


    <!-- http://www.project-best.eu/owl/aixm-mod/airportheliport#CodeUsageLimitationType -->

    <owl:Class rdf:about="http://www.project-best.eu/owl/aixm-mod/airportheliport#CodeUsageLimitationType">
        <rdfs:comment xml:lang="en">A code indicating whether a limitation is of type permission, interdiction or exclusive usage. </rdfs:comment>
    </owl:Class>
    


    <!-- http://www.project-best.eu/owl/aixm-mod/airportheliport#CodeVASISType -->

    <owl:Class rdf:about="http://www.project-best.eu/owl/aixm-mod/airportheliport#CodeVASISType">
        <rdfs:comment xml:lang="en">A code indicating a type of visual approach slope indicator system.</rdfs:comment>
    </owl:Class>
    


    <!-- http://www.project-best.eu/owl/aixm-mod/airportheliport#CodeValueInterpretationType -->

    <owl:Class rdf:about="http://www.project-best.eu/owl/aixm-mod/airportheliport#CodeValueInterpretationType">
        <rdfs:comment xml:lang="en">A code indicating how a value needs to be interpreted when used as a filter or condition. For example: above the value or below the value.</rdfs:comment>
    </owl:Class>
    


    <!-- http://www.project-best.eu/owl/aixm-mod/airportheliport#CodeVerticalDatumType -->

    <owl:Class rdf:about="http://www.project-best.eu/owl/aixm-mod/airportheliport#CodeVerticalDatumType">
        <rdfs:comment xml:lang="en">List of vertical datums.</rdfs:comment>
    </owl:Class>
    


    <!-- http://www.project-best.eu/owl/aixm-mod/airportheliport#CodeVisualDockingGuidanceType -->

    <owl:Class rdf:about="http://www.project-best.eu/owl/aixm-mod/airportheliport#CodeVisualDockingGuidanceType">
        <rdfs:comment xml:lang="en">A coded list of values that indicate types of systems used at aircraft stands in order to help the pilot align and position the aircraft.</rdfs:comment>
    </owl:Class>
    


    <!-- http://www.project-best.eu/owl/aixm-mod/airportheliport#CodeWorkAreaType -->

    <owl:Class rdf:about="http://www.project-best.eu/owl/aixm-mod/airportheliport#CodeWorkAreaType">
        <rdfs:comment xml:lang="en">A code indicating the type of work performed in the work area.</rdfs:comment>
    </owl:Class>
    


    <!-- http://www.project-best.eu/owl/aixm-mod/airportheliport#ConditionCombination -->

    <owl:Class rdf:about="http://www.project-best.eu/owl/aixm-mod/airportheliport#ConditionCombination">
        <rdfs:comment xml:lang="en">A set of filter criteria used to determine the subset of flights, environmental conditions and times for which the usage is specified.</rdfs:comment>
        <rdfs:comment xml:lang="en">Subclass of Shared::Schedules::PropertiesWithSchedule</rdfs:comment>
    </owl:Class>
    


    <!-- http://www.project-best.eu/owl/aixm-mod/airportheliport#DeicingArea -->

    <owl:Class rdf:about="http://www.project-best.eu/owl/aixm-mod/airportheliport#DeicingArea">
        <rdfs:comment xml:lang="en">An area comprising an inner area for the parking of an aircraft to receive de-icing treatment and an outer area for the manoeuvring of two or more mobile de-icing equipment.</rdfs:comment>
    </owl:Class>
    


    <!-- http://www.project-best.eu/owl/aixm-mod/airportheliport#DeicingAreaMarking -->

    <owl:Class rdf:about="http://www.project-best.eu/owl/aixm-mod/airportheliport#DeicingAreaMarking">
        <rdfs:subClassOf rdf:resource="http://www.project-best.eu/owl/aixm-mod/airportheliport#Marking"/>
        <rdfs:comment xml:lang="en">A symbol or group of symbols displayed on the surface of a Deicing Area</rdfs:comment>
    </owl:Class>
    


    <!-- http://www.project-best.eu/owl/aixm-mod/airportheliport#FloatingDockSite -->

    <owl:Class rdf:about="http://www.project-best.eu/owl/aixm-mod/airportheliport#FloatingDockSite">
        <rdfs:comment xml:lang="en">Floating facility which can serve as a mooring place for vessels or as a floating dry dock</rdfs:comment>
    </owl:Class>
    


    <!-- http://www.project-best.eu/owl/aixm-mod/airportheliport#GroundLightSystem -->

    <owl:Class rdf:about="http://www.project-best.eu/owl/aixm-mod/airportheliport#GroundLightSystem">
        <rdfs:comment xml:lang="en">One or more light sources located on the ground and that provide visual assistance for air and ground navigation.</rdfs:comment>
    </owl:Class>
    


    <!-- http://www.project-best.eu/owl/aixm-mod/airportheliport#GroundLightingAvailability -->

    <owl:Class rdf:about="http://www.project-best.eu/owl/aixm-mod/airportheliport#GroundLightingAvailability">
        <rdfs:comment xml:lang="en">Information about the operational status of a ground light.</rdfs:comment>
        <rdfs:comment xml:lang="en">Subclass of Shared::Schedules::PropertiesWithSchedule</rdfs:comment>
    </owl:Class>
    


    <!-- http://www.project-best.eu/owl/aixm-mod/airportheliport#GuidanceLine -->

    <owl:Class rdf:about="http://www.project-best.eu/owl/aixm-mod/airportheliport#GuidanceLine">
        <rdfs:comment xml:lang="en">A line used to guide aircraft on and between airport movement areas.</rdfs:comment>
    </owl:Class>
    


    <!-- http://www.project-best.eu/owl/aixm-mod/airportheliport#GuidanceLineLightSystem -->

    <owl:Class rdf:about="http://www.project-best.eu/owl/aixm-mod/airportheliport#GuidanceLineLightSystem">
        <rdfs:subClassOf rdf:resource="http://www.project-best.eu/owl/aixm-mod/airportheliport#GroundLightSystem"/>
        <rdfs:comment xml:lang="en">The lighting system for the centreline guidance line.</rdfs:comment>
    </owl:Class>
    


    <!-- http://www.project-best.eu/owl/aixm-mod/airportheliport#GuidanceLineMarking -->

    <owl:Class rdf:about="http://www.project-best.eu/owl/aixm-mod/airportheliport#GuidanceLineMarking">
        <rdfs:subClassOf rdf:resource="http://www.project-best.eu/owl/aixm-mod/airportheliport#Marking"/>
        <rdfs:comment xml:lang="en">A symbol or group of symbols displayed as the guidance line.</rdfs:comment>
    </owl:Class>
    


    <!-- http://www.project-best.eu/owl/aixm-mod/airportheliport#LightActivation -->

    <owl:Class rdf:about="http://www.project-best.eu/owl/aixm-mod/airportheliport#LightActivation">
        <rdfs:comment xml:lang="en">The result and the intensity of the lighting system when activated by the pilot.</rdfs:comment>
    </owl:Class>
    


    <!-- http://www.project-best.eu/owl/aixm-mod/airportheliport#ManoeuvringAreaAvailability -->

    <owl:Class rdf:about="http://www.project-best.eu/owl/aixm-mod/airportheliport#ManoeuvringAreaAvailability">
        <rdfs:comment xml:lang="en">Information about the operational status of the manoeuvring area elements (runway, taxiway, TLOF, etc.)</rdfs:comment>
        <rdfs:comment xml:lang="en">Subclass of Shared::Schedules::PropertiesWithSchedule</rdfs:comment>
    </owl:Class>
    


    <!-- http://www.project-best.eu/owl/aixm-mod/airportheliport#ManoeuvringAreaUsage -->

    <owl:Class rdf:about="http://www.project-best.eu/owl/aixm-mod/airportheliport#ManoeuvringAreaUsage">
        <rdfs:subClassOf rdf:resource="http://www.project-best.eu/owl/aixm-mod/airportheliport#UsageCondition"/>
        <rdfs:comment xml:lang="en">A rule governing the usage of the manoeuvring area element.</rdfs:comment>
    </owl:Class>
    


    <!-- http://www.project-best.eu/owl/aixm-mod/airportheliport#Marking -->

    <owl:Class rdf:about="http://www.project-best.eu/owl/aixm-mod/airportheliport#Marking">
        <rdfs:comment xml:lang="en">A group of symbols displayed on an aerodrome or heliport surface in order to convey aeronautical information.</rdfs:comment>
    </owl:Class>
    


    <!-- http://www.project-best.eu/owl/aixm-mod/airportheliport#MarkingBuoy -->

    <owl:Class rdf:about="http://www.project-best.eu/owl/aixm-mod/airportheliport#MarkingBuoy">
        <rdfs:comment xml:lang="en">Floating marker which is moored to the bottom at a specific known location, which is used as an aid to navigation or for other special purpose</rdfs:comment>
    </owl:Class>
    


    <!-- http://www.project-best.eu/owl/aixm-mod/airportheliport#MarkingElement -->

    <owl:Class rdf:about="http://www.project-best.eu/owl/aixm-mod/airportheliport#MarkingElement">
        <rdfs:comment xml:lang="en">A symbol displayed on an aerodrome or heliport surface.</rdfs:comment>
    </owl:Class>
    


    <!-- http://www.project-best.eu/owl/aixm-mod/airportheliport#MarkingExtent -->

    <owl:Class rdf:about="http://www.project-best.eu/owl/aixm-mod/airportheliport#MarkingExtent">
        <rdfs:comment xml:lang="en">A link class that allows selecting between a point, a curve or a surface to define the geometry of a Marking Element</rdfs:comment>
    </owl:Class>
    


    <!-- http://www.project-best.eu/owl/aixm-mod/airportheliport#NavaidEquipmentDistance -->

    <owl:Class rdf:about="http://www.project-best.eu/owl/aixm-mod/airportheliport#NavaidEquipmentDistance">
        <rdfs:comment xml:lang="en">Captures the distances between various Runway Centreline Points and Navaid Equipment.</rdfs:comment>
    </owl:Class>
    


    <!-- http://www.project-best.eu/owl/aixm-mod/airportheliport#NonMovementArea -->

    <owl:Class rdf:about="http://www.project-best.eu/owl/aixm-mod/airportheliport#NonMovementArea">
        <rdfs:comment xml:lang="en">Area where aircraft cannot be seen by a control tower and therefore are restricted to move</rdfs:comment>
    </owl:Class>
    


    <!-- http://www.project-best.eu/owl/aixm-mod/airportheliport#PassengerLoadingBridge -->

    <owl:Class rdf:about="http://www.project-best.eu/owl/aixm-mod/airportheliport#PassengerLoadingBridge">
        <rdfs:comment xml:lang="en">Bridge for loading/unloading access to airplanes for passengers and crew.</rdfs:comment>
    </owl:Class>
    


    <!-- http://www.project-best.eu/owl/aixm-mod/airportheliport#Ridge -->

    <owl:Class rdf:about="http://www.project-best.eu/owl/aixm-mod/airportheliport#Ridge">
        <rdfs:comment xml:lang="en">Describes ridges of deposited material (such as a snow-bank) to the left or right of the runway (relative to the runway direction with the lowest designation number).</rdfs:comment>
    </owl:Class>
    


    <!-- http://www.project-best.eu/owl/aixm-mod/airportheliport#Road -->

    <owl:Class rdf:about="http://www.project-best.eu/owl/aixm-mod/airportheliport#Road">
        <rdfs:comment xml:lang="en">An established surface route on the aerodrome meant for the exclusive use of authorized vehicles and personnel.</rdfs:comment>
    </owl:Class>
    


    <!-- http://www.project-best.eu/owl/aixm-mod/airportheliport#Runway -->

    <owl:Class rdf:about="http://www.project-best.eu/owl/aixm-mod/airportheliport#Runway">
        <rdfs:comment xml:lang="en">A defined rectangular area on a land aerodrome/heliport prepared for the landing and take-off of aircraft.</rdfs:comment>
    </owl:Class>
    


    <!-- http://www.project-best.eu/owl/aixm-mod/airportheliport#RunwayBlastPad -->

    <owl:Class rdf:about="http://www.project-best.eu/owl/aixm-mod/airportheliport#RunwayBlastPad">
        <rdfs:comment xml:lang="en">Specially prepared surface placed adjacent to the end of a runway to eliminate the erosive affect of the high wind forces produced by airplanes at the beginning of their takeoff rolls.</rdfs:comment>
    </owl:Class>
    


    <!-- http://www.project-best.eu/owl/aixm-mod/airportheliport#RunwayCentrelinePoint -->

    <owl:Class rdf:about="http://www.project-best.eu/owl/aixm-mod/airportheliport#RunwayCentrelinePoint">
        <rdfs:comment xml:lang="en">An operationally significant position on the centre line of a runway direction. A typical example is the runway threshold.</rdfs:comment>
    </owl:Class>
    


    <!-- http://www.project-best.eu/owl/aixm-mod/airportheliport#RunwayContamination -->

    <owl:Class rdf:about="http://www.project-best.eu/owl/aixm-mod/airportheliport#RunwayContamination">
        <rdfs:subClassOf rdf:resource="http://www.project-best.eu/owl/aixm-mod/airportheliport#SurfaceContamination"/>
        <rdfs:comment xml:lang="en">The presence or removal of hazardous conditions due to snow, ice, slush, water, etc. on the runway surface.</rdfs:comment>
    </owl:Class>
    


    <!-- http://www.project-best.eu/owl/aixm-mod/airportheliport#RunwayDeclaredDistance -->

    <owl:Class rdf:about="http://www.project-best.eu/owl/aixm-mod/airportheliport#RunwayDeclaredDistance">
        <rdfs:comment xml:lang="en">A conventional operational distance declared for a runway direction.</rdfs:comment>
    </owl:Class>
    


    <!-- http://www.project-best.eu/owl/aixm-mod/airportheliport#RunwayDeclaredDistanceValue -->

    <owl:Class rdf:about="http://www.project-best.eu/owl/aixm-mod/airportheliport#RunwayDeclaredDistanceValue">
        <rdfs:comment xml:lang="en">Subclass of Shared::Schedules::PropertiesWithSchedule</rdfs:comment>
        <rdfs:comment xml:lang="en">The value of a conventional operational distance declared for a runway direction.</rdfs:comment>
    </owl:Class>
    


    <!-- http://www.project-best.eu/owl/aixm-mod/airportheliport#RunwayDirection -->

    <owl:Class rdf:about="http://www.project-best.eu/owl/aixm-mod/airportheliport#RunwayDirection">
        <rdfs:comment xml:lang="en">One of the two landing and take-off directions of a runway for which attributes like TORA, TODA, LDA, etc. may be defined.</rdfs:comment>
    </owl:Class>
    


    <!-- http://www.project-best.eu/owl/aixm-mod/airportheliport#RunwayDirectionLightSystem -->

    <owl:Class rdf:about="http://www.project-best.eu/owl/aixm-mod/airportheliport#RunwayDirectionLightSystem">
        <rdfs:subClassOf rdf:resource="http://www.project-best.eu/owl/aixm-mod/airportheliport#GroundLightSystem"/>
        <rdfs:comment xml:lang="en">The lighting system provided for a landing and take-off direction, including the stopway lights.</rdfs:comment>
    </owl:Class>
    


    <!-- http://www.project-best.eu/owl/aixm-mod/airportheliport#RunwayElement -->

    <owl:Class rdf:about="http://www.project-best.eu/owl/aixm-mod/airportheliport#RunwayElement">
        <rdfs:comment xml:lang="en">Runway element may consist of one ore more polygons not defined as other portions of the runway class.</rdfs:comment>
    </owl:Class>
    


    <!-- http://www.project-best.eu/owl/aixm-mod/airportheliport#RunwayMarking -->

    <owl:Class rdf:about="http://www.project-best.eu/owl/aixm-mod/airportheliport#RunwayMarking">
        <rdfs:subClassOf rdf:resource="http://www.project-best.eu/owl/aixm-mod/airportheliport#Marking"/>
        <rdfs:comment xml:lang="en">A symbol or group of symbols displayed on the surface of the runway.</rdfs:comment>
    </owl:Class>
    


    <!-- http://www.project-best.eu/owl/aixm-mod/airportheliport#RunwayProtectArea -->

    <owl:Class rdf:about="http://www.project-best.eu/owl/aixm-mod/airportheliport#RunwayProtectArea">
        <rdfs:subClassOf rdf:resource="http://www.project-best.eu/owl/aixm-mod/airportheliport#AirportHeliportProtectionArea"/>
        <rdfs:comment xml:lang="en">An area situated in the vicinity of a runway or provided to protect aircraft during manoeuvring, take-off and landing operations.</rdfs:comment>
    </owl:Class>
    


    <!-- http://www.project-best.eu/owl/aixm-mod/airportheliport#RunwayProtectAreaLightSystem -->

    <owl:Class rdf:about="http://www.project-best.eu/owl/aixm-mod/airportheliport#RunwayProtectAreaLightSystem">
        <rdfs:subClassOf rdf:resource="http://www.project-best.eu/owl/aixm-mod/airportheliport#GroundLightSystem"/>
        <rdfs:comment xml:lang="en">The lighting for the runway project area.</rdfs:comment>
    </owl:Class>
    


    <!-- http://www.project-best.eu/owl/aixm-mod/airportheliport#RunwaySectionContamination -->

    <owl:Class rdf:about="http://www.project-best.eu/owl/aixm-mod/airportheliport#RunwaySectionContamination">
        <rdfs:subClassOf rdf:resource="http://www.project-best.eu/owl/aixm-mod/airportheliport#SurfaceContamination"/>
        <rdfs:comment xml:lang="en">The presence or removal of hazardous conditions due to snow, ice, slush, water, etc. on a section of the runway surface.</rdfs:comment>
    </owl:Class>
    


    <!-- http://www.project-best.eu/owl/aixm-mod/airportheliport#RunwayVisualRange -->

    <owl:Class rdf:about="http://www.project-best.eu/owl/aixm-mod/airportheliport#RunwayVisualRange">
        <rdfs:comment xml:lang="en">A meteorological equipment providing information about the distance over which the pilot of an aircraft on the centre line of a runway can see the runway surface markings or the lights delineating the runway or identifying its centre line.</rdfs:comment>
    </owl:Class>
    


    <!-- http://www.project-best.eu/owl/aixm-mod/airportheliport#SeaplaneLandingArea -->

    <owl:Class rdf:about="http://www.project-best.eu/owl/aixm-mod/airportheliport#SeaplaneLandingArea">
        <rdfs:comment xml:lang="en">Area specifically designated for take-offs and landings of seaplanes </rdfs:comment>
    </owl:Class>
    


    <!-- http://www.project-best.eu/owl/aixm-mod/airportheliport#SeaplaneRampSite -->

    <owl:Class rdf:about="http://www.project-best.eu/owl/aixm-mod/airportheliport#SeaplaneRampSite">
        <rdfs:comment xml:lang="en">Ramps specifically designed to transit seaplanes from land to water and vice versa</rdfs:comment>
    </owl:Class>
    


    <!-- http://www.project-best.eu/owl/aixm-mod/airportheliport#StandMarking -->

    <owl:Class rdf:about="http://www.project-best.eu/owl/aixm-mod/airportheliport#StandMarking">
        <rdfs:subClassOf rdf:resource="http://www.project-best.eu/owl/aixm-mod/airportheliport#Marking"/>
        <rdfs:comment xml:lang="en">A symbol or group of symbols displayed on the surface of the Aircraft Stand.</rdfs:comment>
    </owl:Class>
    


    <!-- http://www.project-best.eu/owl/aixm-mod/airportheliport#SurfaceCharacteristics -->

    <owl:Class rdf:about="http://www.project-best.eu/owl/aixm-mod/airportheliport#SurfaceCharacteristics">
        <rdfs:comment xml:lang="en">An entity grouping together the attributes that model characteristics of an airport surface, such as strength, material, etc.</rdfs:comment>
    </owl:Class>
    


    <!-- http://www.project-best.eu/owl/aixm-mod/airportheliport#SurfaceContamination -->

    <owl:Class rdf:about="http://www.project-best.eu/owl/aixm-mod/airportheliport#SurfaceContamination">
        <rdfs:comment xml:lang="en">Presence or removal of hazardous conditions on movement areas due to snow, ice, slush, water.  </rdfs:comment>
    </owl:Class>
    


    <!-- http://www.project-best.eu/owl/aixm-mod/airportheliport#SurfaceContaminationLayer -->

    <owl:Class rdf:about="http://www.project-best.eu/owl/aixm-mod/airportheliport#SurfaceContaminationLayer">
        <rdfs:comment xml:lang="en">An operationally significant contaminant of homogeneous type such as snow, ice, slush, water, sand, etc., which is present on a large surface of the airport/heliport area.</rdfs:comment>
    </owl:Class>
    


    <!-- http://www.project-best.eu/owl/aixm-mod/airportheliport#SurveyControlPoint -->

    <owl:Class rdf:about="http://www.project-best.eu/owl/aixm-mod/airportheliport#SurveyControlPoint">
        <rdfs:comment xml:lang="en">A monumented survey control point</rdfs:comment>
    </owl:Class>
    


    <!-- http://www.project-best.eu/owl/aixm-mod/airportheliport#TaxiHoldingPosition -->

    <owl:Class rdf:about="http://www.project-best.eu/owl/aixm-mod/airportheliport#TaxiHoldingPosition">
        <rdfs:comment xml:lang="en">A designated position intended for traffic control at which taxiing aircraft and vehicles shall stop and hold until further cleared to proceed, when so instructed by the aerodrome control tower.</rdfs:comment>
    </owl:Class>
    


    <!-- http://www.project-best.eu/owl/aixm-mod/airportheliport#TaxiHoldingPositionLightSystem -->

    <owl:Class rdf:about="http://www.project-best.eu/owl/aixm-mod/airportheliport#TaxiHoldingPositionLightSystem">
        <rdfs:subClassOf rdf:resource="http://www.project-best.eu/owl/aixm-mod/airportheliport#GroundLightSystem"/>
        <rdfs:comment xml:lang="en">Lighting system for a taxiway hold position.</rdfs:comment>
    </owl:Class>
    


    <!-- http://www.project-best.eu/owl/aixm-mod/airportheliport#TaxiHoldingPositionMarking -->

    <owl:Class rdf:about="http://www.project-best.eu/owl/aixm-mod/airportheliport#TaxiHoldingPositionMarking">
        <rdfs:subClassOf rdf:resource="http://www.project-best.eu/owl/aixm-mod/airportheliport#Marking"/>
        <rdfs:comment xml:lang="en">A symbol or group of symbols displayed on the surface of a Taxiway indicating the location of the TaxiHoldingPosition.</rdfs:comment>
    </owl:Class>
    


    <!-- http://www.project-best.eu/owl/aixm-mod/airportheliport#Taxiway -->

    <owl:Class rdf:about="http://www.project-best.eu/owl/aixm-mod/airportheliport#Taxiway">
        <rdfs:comment xml:lang="en">A defined path at an aerodrome/heliport established for the taxiing of aircraft/helicopters and intended to provide a link between one part of the aerodrome and another, including aircraft/helicopter stand taxi-lines, apron taxiways, rapid exit taxiways, air taxiways etc..</rdfs:comment>
    </owl:Class>
    


    <!-- http://www.project-best.eu/owl/aixm-mod/airportheliport#TaxiwayContamination -->

    <owl:Class rdf:about="http://www.project-best.eu/owl/aixm-mod/airportheliport#TaxiwayContamination">
        <rdfs:subClassOf rdf:resource="http://www.project-best.eu/owl/aixm-mod/airportheliport#SurfaceContamination"/>
        <rdfs:comment xml:lang="en">The presence or removal of hazardous conditions due to snow, ice, slush, water, etc. on the taxiway surface.</rdfs:comment>
    </owl:Class>
    


    <!-- http://www.project-best.eu/owl/aixm-mod/airportheliport#TaxiwayElement -->

    <owl:Class rdf:about="http://www.project-best.eu/owl/aixm-mod/airportheliport#TaxiwayElement">
        <rdfs:comment xml:lang="en">Part of a Taxiway</rdfs:comment>
    </owl:Class>
    


    <!-- http://www.project-best.eu/owl/aixm-mod/airportheliport#TaxiwayLightSystem -->

    <owl:Class rdf:about="http://www.project-best.eu/owl/aixm-mod/airportheliport#TaxiwayLightSystem">
        <rdfs:subClassOf rdf:resource="http://www.project-best.eu/owl/aixm-mod/airportheliport#GroundLightSystem"/>
        <rdfs:comment xml:lang="en">The lighting system provided for a taxiway at an aerodrome/heliport.</rdfs:comment>
    </owl:Class>
    


    <!-- http://www.project-best.eu/owl/aixm-mod/airportheliport#TaxiwayMarking -->

    <owl:Class rdf:about="http://www.project-best.eu/owl/aixm-mod/airportheliport#TaxiwayMarking">
        <rdfs:subClassOf rdf:resource="http://www.project-best.eu/owl/aixm-mod/airportheliport#Marking"/>
        <rdfs:comment xml:lang="en">A symbol or group of symbols displayed on the surface of the taxiway.</rdfs:comment>
    </owl:Class>
    


    <!-- http://www.project-best.eu/owl/aixm-mod/airportheliport#TouchDownLiftOff -->

    <owl:Class rdf:about="http://www.project-best.eu/owl/aixm-mod/airportheliport#TouchDownLiftOff">
        <rdfs:comment xml:lang="en">A load bearing area on which a helicopter may touch down or lift-off.</rdfs:comment>
    </owl:Class>
    


    <!-- http://www.project-best.eu/owl/aixm-mod/airportheliport#TouchDownLiftOffContamination -->

    <owl:Class rdf:about="http://www.project-best.eu/owl/aixm-mod/airportheliport#TouchDownLiftOffContamination">
        <rdfs:subClassOf rdf:resource="http://www.project-best.eu/owl/aixm-mod/airportheliport#SurfaceContamination"/>
        <rdfs:comment xml:lang="en">The presence or removal of hazardous conditions due to snow, ice, slush, water, etc. on the TLOF surface.</rdfs:comment>
    </owl:Class>
    


    <!-- http://www.project-best.eu/owl/aixm-mod/airportheliport#TouchDownLiftOffLightSystem -->

    <owl:Class rdf:about="http://www.project-best.eu/owl/aixm-mod/airportheliport#TouchDownLiftOffLightSystem">
        <rdfs:subClassOf rdf:resource="http://www.project-best.eu/owl/aixm-mod/airportheliport#GroundLightSystem"/>
        <rdfs:comment xml:lang="en">The lighting system provided for a TLOF surface at an aerodrome/heliport.</rdfs:comment>
    </owl:Class>
    


    <!-- http://www.project-best.eu/owl/aixm-mod/airportheliport#TouchDownLiftOffMarking -->

    <owl:Class rdf:about="http://www.project-best.eu/owl/aixm-mod/airportheliport#TouchDownLiftOffMarking">
        <rdfs:subClassOf rdf:resource="http://www.project-best.eu/owl/aixm-mod/airportheliport#Marking"/>
        <rdfs:comment xml:lang="en">A symbol or group of symbols displayed on the surface of the touch down and lift-off area.</rdfs:comment>
    </owl:Class>
    


    <!-- http://www.project-best.eu/owl/aixm-mod/airportheliport#TouchDownLiftOffSafeArea -->

    <owl:Class rdf:about="http://www.project-best.eu/owl/aixm-mod/airportheliport#TouchDownLiftOffSafeArea">
        <rdfs:subClassOf rdf:resource="http://www.project-best.eu/owl/aixm-mod/airportheliport#AirportHeliportProtectionArea"/>
        <rdfs:comment xml:lang="en">An obstacle free zone area situated in the vicinity of a touch down and lift-off area, provided to protect helicopters during manoeuvring, take-off and/or landing operations.</rdfs:comment>
    </owl:Class>
    


    <!-- http://www.project-best.eu/owl/aixm-mod/airportheliport#UsageCondition -->

    <owl:Class rdf:about="http://www.project-best.eu/owl/aixm-mod/airportheliport#UsageCondition">
        <rdfs:comment xml:lang="en">A rule governing the usage of an Airport/Heliport or of one of its surfaces.</rdfs:comment>
    </owl:Class>
    


    <!-- http://www.project-best.eu/owl/aixm-mod/airportheliport#VisualGlideSlopeIndicator -->

    <owl:Class rdf:about="http://www.project-best.eu/owl/aixm-mod/airportheliport#VisualGlideSlopeIndicator">
        <rdfs:subClassOf rdf:resource="http://www.project-best.eu/owl/aixm-mod/airportheliport#GroundLightSystem"/>
        <rdfs:comment xml:lang="en">A visual guidance system that provides &quot;below/above glidepath&quot; information to an aircraft executing an approach to a specific runway direction.</rdfs:comment>
    </owl:Class>
    


    <!-- http://www.project-best.eu/owl/aixm-mod/airportheliport#WorkArea -->

    <owl:Class rdf:about="http://www.project-best.eu/owl/aixm-mod/airportheliport#WorkArea">
        <rdfs:comment xml:lang="en">Part of a movement area under construction</rdfs:comment>
    </owl:Class>
    


    <!-- http://www.project-best.eu/owl/aixm-mod/airportheliport#WorkAreaActivity -->

    <owl:Class rdf:about="http://www.project-best.eu/owl/aixm-mod/airportheliport#WorkAreaActivity">
        <rdfs:comment xml:lang="en">Subclass of Shared::Schedules::PropertiesWithSchedule</rdfs:comment>
    </owl:Class>
    


    <!-- 
    ///////////////////////////////////////////////////////////////////////////////////////
    //
    // Individuals
    //
    ///////////////////////////////////////////////////////////////////////////////////////
     -->

    


    <!-- http://www.project-best.eu/owl/aixm-mod/airportheliport#CodeAircraftStandBaseType-ANG_NI -->

    <owl:NamedIndividual rdf:about="http://www.project-best.eu/owl/aixm-mod/airportheliport#CodeAircraftStandBaseType-ANG_NI">
        <rdf:type rdf:resource="http://www.project-best.eu/owl/aixm-mod/airportheliport#CodeAircraftStandType"/>
        <rdfs:comment xml:lang="en">Angled nose-in parking position.</rdfs:comment>
    </owl:NamedIndividual>
    


    <!-- http://www.project-best.eu/owl/aixm-mod/airportheliport#CodeAircraftStandBaseType-ANG_NO -->

    <owl:NamedIndividual rdf:about="http://www.project-best.eu/owl/aixm-mod/airportheliport#CodeAircraftStandBaseType-ANG_NO">
        <rdf:type rdf:resource="http://www.project-best.eu/owl/aixm-mod/airportheliport#CodeAircraftStandType"/>
        <rdfs:comment xml:lang="en">Angled nose-out parking position.</rdfs:comment>
    </owl:NamedIndividual>
    


    <!-- http://www.project-best.eu/owl/aixm-mod/airportheliport#CodeAircraftStandBaseType-ISOL -->

    <owl:NamedIndividual rdf:about="http://www.project-best.eu/owl/aixm-mod/airportheliport#CodeAircraftStandBaseType-ISOL">
        <rdf:type rdf:resource="http://www.project-best.eu/owl/aixm-mod/airportheliport#CodeAircraftStandType"/>
        <rdfs:comment xml:lang="en">Isolated parking position.</rdfs:comment>
    </owl:NamedIndividual>
    


    <!-- http://www.project-best.eu/owl/aixm-mod/airportheliport#CodeAircraftStandBaseType-NI -->

    <owl:NamedIndividual rdf:about="http://www.project-best.eu/owl/aixm-mod/airportheliport#CodeAircraftStandBaseType-NI">
        <rdf:type rdf:resource="http://www.project-best.eu/owl/aixm-mod/airportheliport#CodeAircraftStandType"/>
        <rdfs:comment xml:lang="en">Nose-in parking position.</rdfs:comment>
    </owl:NamedIndividual>
    


    <!-- http://www.project-best.eu/owl/aixm-mod/airportheliport#CodeAircraftStandBaseType-OTHER -->

    <owl:NamedIndividual rdf:about="http://www.project-best.eu/owl/aixm-mod/airportheliport#CodeAircraftStandBaseType-OTHER">
        <rdf:type rdf:resource="http://www.project-best.eu/owl/aixm-mod/airportheliport#CodeAircraftStandType"/>
        <rdfs:comment xml:lang="en">Other</rdfs:comment>
    </owl:NamedIndividual>
    


    <!-- http://www.project-best.eu/owl/aixm-mod/airportheliport#CodeAircraftStandBaseType-PARL -->

    <owl:NamedIndividual rdf:about="http://www.project-best.eu/owl/aixm-mod/airportheliport#CodeAircraftStandBaseType-PARL">
        <rdf:type rdf:resource="http://www.project-best.eu/owl/aixm-mod/airportheliport#CodeAircraftStandType"/>
        <rdfs:comment xml:lang="en">Parallel (to building) parking position.</rdfs:comment>
    </owl:NamedIndividual>
    


    <!-- http://www.project-best.eu/owl/aixm-mod/airportheliport#CodeAircraftStandBaseType-RMT -->

    <owl:NamedIndividual rdf:about="http://www.project-best.eu/owl/aixm-mod/airportheliport#CodeAircraftStandBaseType-RMT">
        <rdf:type rdf:resource="http://www.project-best.eu/owl/aixm-mod/airportheliport#CodeAircraftStandType"/>
        <rdfs:comment xml:lang="en">Remote parking position.</rdfs:comment>
    </owl:NamedIndividual>
    


    <!-- http://www.project-best.eu/owl/aixm-mod/airportheliport#CodeAirportHeliportBaseType-AD -->

    <owl:NamedIndividual rdf:about="http://www.project-best.eu/owl/aixm-mod/airportheliport#CodeAirportHeliportBaseType-AD">
        <rdf:type rdf:resource="http://www.project-best.eu/owl/aixm-mod/airportheliport#CodeAirportHeliportType"/>
        <rdfs:comment xml:lang="en">Aerodrome only.</rdfs:comment>
    </owl:NamedIndividual>
    


    <!-- http://www.project-best.eu/owl/aixm-mod/airportheliport#CodeAirportHeliportBaseType-AH -->

    <owl:NamedIndividual rdf:about="http://www.project-best.eu/owl/aixm-mod/airportheliport#CodeAirportHeliportBaseType-AH">
        <rdf:type rdf:resource="http://www.project-best.eu/owl/aixm-mod/airportheliport#CodeAirportHeliportType"/>
        <rdfs:comment xml:lang="en">Aerodrome with heliport landing area.</rdfs:comment>
    </owl:NamedIndividual>
    


    <!-- http://www.project-best.eu/owl/aixm-mod/airportheliport#CodeAirportHeliportBaseType-HP -->

    <owl:NamedIndividual rdf:about="http://www.project-best.eu/owl/aixm-mod/airportheliport#CodeAirportHeliportBaseType-HP">
        <rdf:type rdf:resource="http://www.project-best.eu/owl/aixm-mod/airportheliport#CodeAirportHeliportType"/>
        <rdfs:comment xml:lang="en">Heliport only.</rdfs:comment>
    </owl:NamedIndividual>
    


    <!-- http://www.project-best.eu/owl/aixm-mod/airportheliport#CodeAirportHeliportBaseType-LS -->

    <owl:NamedIndividual rdf:about="http://www.project-best.eu/owl/aixm-mod/airportheliport#CodeAirportHeliportBaseType-LS">
        <rdf:type rdf:resource="http://www.project-best.eu/owl/aixm-mod/airportheliport#CodeAirportHeliportType"/>
        <rdfs:comment xml:lang="en">Landing site.</rdfs:comment>
    </owl:NamedIndividual>
    


    <!-- http://www.project-best.eu/owl/aixm-mod/airportheliport#CodeAirportHeliportBaseType-OTHER -->

    <owl:NamedIndividual rdf:about="http://www.project-best.eu/owl/aixm-mod/airportheliport#CodeAirportHeliportBaseType-OTHER">
        <rdf:type rdf:resource="http://www.project-best.eu/owl/aixm-mod/airportheliport#CodeAirportHeliportType"/>
        <rdfs:comment xml:lang="en">Other</rdfs:comment>
    </owl:NamedIndividual>
    


    <!-- http://www.project-best.eu/owl/aixm-mod/airportheliport#CodeAirportHeliportCollocationBaseType-FULL -->

    <owl:NamedIndividual rdf:about="http://www.project-best.eu/owl/aixm-mod/airportheliport#CodeAirportHeliportCollocationBaseType-FULL">
        <rdf:type rdf:resource="http://www.project-best.eu/owl/aixm-mod/airportheliport#CodeAirportHeliportCollocationType"/>
        <rdfs:comment xml:lang="en">Full collocation, there is only one aerodrome/heliport.</rdfs:comment>
    </owl:NamedIndividual>
    


    <!-- http://www.project-best.eu/owl/aixm-mod/airportheliport#CodeAirportHeliportCollocationBaseType-OTHER -->

    <owl:NamedIndividual rdf:about="http://www.project-best.eu/owl/aixm-mod/airportheliport#CodeAirportHeliportCollocationBaseType-OTHER">
        <rdf:type rdf:resource="http://www.project-best.eu/owl/aixm-mod/airportheliport#CodeAirportHeliportCollocationType"/>
        <rdfs:comment xml:lang="en">Other</rdfs:comment>
    </owl:NamedIndividual>
    


    <!-- http://www.project-best.eu/owl/aixm-mod/airportheliport#CodeAirportHeliportCollocationBaseType-PARTIAL -->

    <owl:NamedIndividual rdf:about="http://www.project-best.eu/owl/aixm-mod/airportheliport#CodeAirportHeliportCollocationBaseType-PARTIAL">
        <rdf:type rdf:resource="http://www.project-best.eu/owl/aixm-mod/airportheliport#CodeAirportHeliportCollocationType"/>
        <rdfs:comment xml:lang="en">Partial collocation, the RWYs of the 1st aerodrome are available to the traffic on the 2nd aerodrome..] </rdfs:comment>
    </owl:NamedIndividual>
    


    <!-- http://www.project-best.eu/owl/aixm-mod/airportheliport#CodeAirportHeliportCollocationBaseType-RWY -->

    <owl:NamedIndividual rdf:about="http://www.project-best.eu/owl/aixm-mod/airportheliport#CodeAirportHeliportCollocationBaseType-RWY">
        <rdf:type rdf:resource="http://www.project-best.eu/owl/aixm-mod/airportheliport#CodeAirportHeliportCollocationType"/>
        <rdfs:comment xml:lang="en">The two aerodromes share all their RWYs and TWYs, but not their aprons.</rdfs:comment>
    </owl:NamedIndividual>
    


    <!-- http://www.project-best.eu/owl/aixm-mod/airportheliport#CodeAirportHeliportCollocationBaseType-SEPARATED -->

    <owl:NamedIndividual rdf:about="http://www.project-best.eu/owl/aixm-mod/airportheliport#CodeAirportHeliportCollocationBaseType-SEPARATED">
        <rdf:type rdf:resource="http://www.project-best.eu/owl/aixm-mod/airportheliport#CodeAirportHeliportCollocationType"/>
        <rdfs:comment xml:lang="en">Separated. Even if it is physically possible for an aircraft to taxi between the two aerodrome&apos;s manoeuvring areas, this is not operationally allowed.</rdfs:comment>
    </owl:NamedIndividual>
    


    <!-- http://www.project-best.eu/owl/aixm-mod/airportheliport#CodeAirportHeliportCollocationBaseType-UNILATERAL -->

    <owl:NamedIndividual rdf:about="http://www.project-best.eu/owl/aixm-mod/airportheliport#CodeAirportHeliportCollocationBaseType-UNILATERAL">
        <rdf:type rdf:resource="http://www.project-best.eu/owl/aixm-mod/airportheliport#CodeAirportHeliportCollocationType"/>
        <rdfs:comment xml:lang="en">Unilateral co-location, the RWYs, the TWYs and the aprons of the 1st aerodrome are available to traffic on the 2nd aerodrome.</rdfs:comment>
    </owl:NamedIndividual>
    


    <!-- http://www.project-best.eu/owl/aixm-mod/airportheliport#CodeAirportWarningBaseType-ANIMAL -->

    <owl:NamedIndividual rdf:about="http://www.project-best.eu/owl/aixm-mod/airportheliport#CodeAirportWarningBaseType-ANIMAL">
        <rdf:type rdf:resource="http://www.project-best.eu/owl/aixm-mod/airportheliport#CodeAirportWarningType"/>
        <rdfs:comment xml:lang="en">Animal hazard.</rdfs:comment>
    </owl:NamedIndividual>
    


    <!-- http://www.project-best.eu/owl/aixm-mod/airportheliport#CodeAirportWarningBaseType-BIRD -->

    <owl:NamedIndividual rdf:about="http://www.project-best.eu/owl/aixm-mod/airportheliport#CodeAirportWarningBaseType-BIRD">
        <rdf:type rdf:resource="http://www.project-best.eu/owl/aixm-mod/airportheliport#CodeAirportWarningType"/>
        <rdfs:comment xml:lang="en">Bird hazard</rdfs:comment>
    </owl:NamedIndividual>
    


    <!-- http://www.project-best.eu/owl/aixm-mod/airportheliport#CodeAirportWarningBaseType-CALIBRATION -->

    <owl:NamedIndividual rdf:about="http://www.project-best.eu/owl/aixm-mod/airportheliport#CodeAirportWarningBaseType-CALIBRATION">
        <rdf:type rdf:resource="http://www.project-best.eu/owl/aixm-mod/airportheliport#CodeAirportWarningType"/>
        <rdfs:comment xml:lang="en">Presence of people or equipment due to calibration work for ground facilities.</rdfs:comment>
    </owl:NamedIndividual>
    


    <!-- http://www.project-best.eu/owl/aixm-mod/airportheliport#CodeAirportWarningBaseType-EQUIP -->

    <owl:NamedIndividual rdf:about="http://www.project-best.eu/owl/aixm-mod/airportheliport#CodeAirportWarningBaseType-EQUIP">
        <rdf:type rdf:resource="http://www.project-best.eu/owl/aixm-mod/airportheliport#CodeAirportWarningType"/>
        <rdfs:comment xml:lang="en">Men and Equipment.</rdfs:comment>
    </owl:NamedIndividual>
    


    <!-- http://www.project-best.eu/owl/aixm-mod/airportheliport#CodeAirportWarningBaseType-GRASS_CUTTING -->

    <owl:NamedIndividual rdf:about="http://www.project-best.eu/owl/aixm-mod/airportheliport#CodeAirportWarningBaseType-GRASS_CUTTING">
        <rdf:type rdf:resource="http://www.project-best.eu/owl/aixm-mod/airportheliport#CodeAirportWarningType"/>
        <rdfs:comment xml:lang="en">Presence of people or equipment due to grass cutting work in progress.</rdfs:comment>
    </owl:NamedIndividual>
    


    <!-- http://www.project-best.eu/owl/aixm-mod/airportheliport#CodeAirportWarningBaseType-INSPECTION -->

    <owl:NamedIndividual rdf:about="http://www.project-best.eu/owl/aixm-mod/airportheliport#CodeAirportWarningBaseType-INSPECTION">
        <rdf:type rdf:resource="http://www.project-best.eu/owl/aixm-mod/airportheliport#CodeAirportWarningType"/>
        <rdfs:comment xml:lang="en">Presence of people or equipment due to ground facilities inspection work in progress.</rdfs:comment>
    </owl:NamedIndividual>
    


    <!-- http://www.project-best.eu/owl/aixm-mod/airportheliport#CodeAirportWarningBaseType-OTHER -->

    <owl:NamedIndividual rdf:about="http://www.project-best.eu/owl/aixm-mod/airportheliport#CodeAirportWarningBaseType-OTHER">
        <rdf:type rdf:resource="http://www.project-best.eu/owl/aixm-mod/airportheliport#CodeAirportWarningType"/>
        <rdfs:comment xml:lang="en">Other</rdfs:comment>
    </owl:NamedIndividual>
    


    <!-- http://www.project-best.eu/owl/aixm-mod/airportheliport#CodeAirportWarningBaseType-PAINTING -->

    <owl:NamedIndividual rdf:about="http://www.project-best.eu/owl/aixm-mod/airportheliport#CodeAirportWarningBaseType-PAINTING">
        <rdf:type rdf:resource="http://www.project-best.eu/owl/aixm-mod/airportheliport#CodeAirportWarningType"/>
        <rdfs:comment xml:lang="en">Surface painting work in progress.</rdfs:comment>
    </owl:NamedIndividual>
    


    <!-- http://www.project-best.eu/owl/aixm-mod/airportheliport#CodeAirportWarningBaseType-PARKED_ACFT -->

    <owl:NamedIndividual rdf:about="http://www.project-best.eu/owl/aixm-mod/airportheliport#CodeAirportWarningBaseType-PARKED_ACFT">
        <rdf:type rdf:resource="http://www.project-best.eu/owl/aixm-mod/airportheliport#CodeAirportWarningType"/>
        <rdfs:comment xml:lang="en">Parked or Disabled Aircraft located on the surface.</rdfs:comment>
    </owl:NamedIndividual>
    


    <!-- http://www.project-best.eu/owl/aixm-mod/airportheliport#CodeAirportWarningBaseType-PAVING -->

    <owl:NamedIndividual rdf:about="http://www.project-best.eu/owl/aixm-mod/airportheliport#CodeAirportWarningBaseType-PAVING">
        <rdf:type rdf:resource="http://www.project-best.eu/owl/aixm-mod/airportheliport#CodeAirportWarningType"/>
        <rdfs:comment xml:lang="en">Surface paving work in progress.</rdfs:comment>
    </owl:NamedIndividual>
    


    <!-- http://www.project-best.eu/owl/aixm-mod/airportheliport#CodeAirportWarningBaseType-RESURFACING -->

    <owl:NamedIndividual rdf:about="http://www.project-best.eu/owl/aixm-mod/airportheliport#CodeAirportWarningBaseType-RESURFACING">
        <rdf:type rdf:resource="http://www.project-best.eu/owl/aixm-mod/airportheliport#CodeAirportWarningType"/>
        <rdfs:comment xml:lang="en">Resurfacing work in progress.</rdfs:comment>
    </owl:NamedIndividual>
    


    <!-- http://www.project-best.eu/owl/aixm-mod/airportheliport#CodeAirportWarningBaseType-RUBBER_REMOVAL -->

    <owl:NamedIndividual rdf:about="http://www.project-best.eu/owl/aixm-mod/airportheliport#CodeAirportWarningBaseType-RUBBER_REMOVAL">
        <rdf:type rdf:resource="http://www.project-best.eu/owl/aixm-mod/airportheliport#CodeAirportWarningType"/>
        <rdfs:comment xml:lang="en">Removal of rubber deposits from runways.</rdfs:comment>
    </owl:NamedIndividual>
    


    <!-- http://www.project-best.eu/owl/aixm-mod/airportheliport#CodeAirportWarningBaseType-WIP -->

    <owl:NamedIndividual rdf:about="http://www.project-best.eu/owl/aixm-mod/airportheliport#CodeAirportWarningBaseType-WIP">
        <rdf:type rdf:resource="http://www.project-best.eu/owl/aixm-mod/airportheliport#CodeAirportWarningType"/>
        <rdfs:comment xml:lang="en">Work in progress.</rdfs:comment>
    </owl:NamedIndividual>
    


    <!-- http://www.project-best.eu/owl/aixm-mod/airportheliport#CodeApproachGuidanceBaseType-ILS_PRECISION_CAT_I -->

    <owl:NamedIndividual rdf:about="http://www.project-best.eu/owl/aixm-mod/airportheliport#CodeApproachGuidanceBaseType-ILS_PRECISION_CAT_I">
        <rdf:type rdf:resource="http://www.project-best.eu/owl/aixm-mod/airportheliport#CodeApproachGuidanceType"/>
        <rdfs:comment xml:lang="en"> ILS precision approach runway, category I</rdfs:comment>
    </owl:NamedIndividual>
    


    <!-- http://www.project-best.eu/owl/aixm-mod/airportheliport#CodeApproachGuidanceBaseType-ILS_PRECISION_CAT_II -->

    <owl:NamedIndividual rdf:about="http://www.project-best.eu/owl/aixm-mod/airportheliport#CodeApproachGuidanceBaseType-ILS_PRECISION_CAT_II">
        <rdf:type rdf:resource="http://www.project-best.eu/owl/aixm-mod/airportheliport#CodeApproachGuidanceType"/>
        <rdfs:comment xml:lang="en">ILS precision approach runway, category II</rdfs:comment>
    </owl:NamedIndividual>
    


    <!-- http://www.project-best.eu/owl/aixm-mod/airportheliport#CodeApproachGuidanceBaseType-ILS_PRECISION_CAT_IIIA -->

    <owl:NamedIndividual rdf:about="http://www.project-best.eu/owl/aixm-mod/airportheliport#CodeApproachGuidanceBaseType-ILS_PRECISION_CAT_IIIA">
        <rdf:type rdf:resource="http://www.project-best.eu/owl/aixm-mod/airportheliport#CodeApproachGuidanceType"/>
        <rdfs:comment xml:lang="en">ILS precision approach runway category III A</rdfs:comment>
    </owl:NamedIndividual>
    


    <!-- http://www.project-best.eu/owl/aixm-mod/airportheliport#CodeApproachGuidanceBaseType-ILS_PRECISION_CAT_IIIB -->

    <owl:NamedIndividual rdf:about="http://www.project-best.eu/owl/aixm-mod/airportheliport#CodeApproachGuidanceBaseType-ILS_PRECISION_CAT_IIIB">
        <rdf:type rdf:resource="http://www.project-best.eu/owl/aixm-mod/airportheliport#CodeApproachGuidanceType"/>
        <rdfs:comment xml:lang="en">ILS precision approach runway category III B</rdfs:comment>
    </owl:NamedIndividual>
    


    <!-- http://www.project-best.eu/owl/aixm-mod/airportheliport#CodeApproachGuidanceBaseType-ILS_PRECISION_CAT_IIIC -->

    <owl:NamedIndividual rdf:about="http://www.project-best.eu/owl/aixm-mod/airportheliport#CodeApproachGuidanceBaseType-ILS_PRECISION_CAT_IIIC">
        <rdf:type rdf:resource="http://www.project-best.eu/owl/aixm-mod/airportheliport#CodeApproachGuidanceType"/>
        <rdfs:comment xml:lang="en">ILS precision approach runway category III C</rdfs:comment>
    </owl:NamedIndividual>
    


    <!-- http://www.project-best.eu/owl/aixm-mod/airportheliport#CodeApproachGuidanceBaseType-ILS_PRECISION_CAT_IIID -->

    <owl:NamedIndividual rdf:about="http://www.project-best.eu/owl/aixm-mod/airportheliport#CodeApproachGuidanceBaseType-ILS_PRECISION_CAT_IIID">
        <rdf:type rdf:resource="http://www.project-best.eu/owl/aixm-mod/airportheliport#CodeApproachGuidanceType"/>
        <rdfs:comment xml:lang="en">ILS precision approach runway category III D</rdfs:comment>
    </owl:NamedIndividual>
    


    <!-- http://www.project-best.eu/owl/aixm-mod/airportheliport#CodeApproachGuidanceBaseType-MLS_PRECISION -->

    <owl:NamedIndividual rdf:about="http://www.project-best.eu/owl/aixm-mod/airportheliport#CodeApproachGuidanceBaseType-MLS_PRECISION">
        <rdf:type rdf:resource="http://www.project-best.eu/owl/aixm-mod/airportheliport#CodeApproachGuidanceType"/>
        <rdfs:comment xml:lang="en">Microwave landing system precision approach</rdfs:comment>
    </owl:NamedIndividual>
    


    <!-- http://www.project-best.eu/owl/aixm-mod/airportheliport#CodeApproachGuidanceBaseType-NON_PRECISION -->

    <owl:NamedIndividual rdf:about="http://www.project-best.eu/owl/aixm-mod/airportheliport#CodeApproachGuidanceBaseType-NON_PRECISION">
        <rdf:type rdf:resource="http://www.project-best.eu/owl/aixm-mod/airportheliport#CodeApproachGuidanceType"/>
        <rdfs:comment xml:lang="en">Non-precision approach runway</rdfs:comment>
    </owl:NamedIndividual>
    


    <!-- http://www.project-best.eu/owl/aixm-mod/airportheliport#CodeApproachGuidanceBaseType-OTHER -->

    <owl:NamedIndividual rdf:about="http://www.project-best.eu/owl/aixm-mod/airportheliport#CodeApproachGuidanceBaseType-OTHER">
        <rdf:type rdf:resource="http://www.project-best.eu/owl/aixm-mod/airportheliport#CodeApproachGuidanceType"/>
        <rdfs:comment xml:lang="en">Other</rdfs:comment>
    </owl:NamedIndividual>
    


    <!-- http://www.project-best.eu/owl/aixm-mod/airportheliport#CodeApproachLightingBaseType-AFOVRN -->

    <owl:NamedIndividual rdf:about="http://www.project-best.eu/owl/aixm-mod/airportheliport#CodeApproachLightingBaseType-AFOVRN">
        <rdf:type rdf:resource="http://www.project-best.eu/owl/aixm-mod/airportheliport#CodeApproachLightingType"/>
        <rdfs:comment xml:lang="en">US Air Force Overrun 1000 Foot Standard Approach Lighting System.</rdfs:comment>
    </owl:NamedIndividual>
    


    <!-- http://www.project-best.eu/owl/aixm-mod/airportheliport#CodeApproachLightingBaseType-ALSAF -->

    <owl:NamedIndividual rdf:about="http://www.project-best.eu/owl/aixm-mod/airportheliport#CodeApproachLightingBaseType-ALSAF">
        <rdf:type rdf:resource="http://www.project-best.eu/owl/aixm-mod/airportheliport#CodeApproachLightingType"/>
        <rdfs:comment xml:lang="en">3000 Foot high intensity Approach Lighting System with Sequenced Flashing Lights.</rdfs:comment>
    </owl:NamedIndividual>
    


    <!-- http://www.project-best.eu/owl/aixm-mod/airportheliport#CodeApproachLightingBaseType-CALVERT -->

    <owl:NamedIndividual rdf:about="http://www.project-best.eu/owl/aixm-mod/airportheliport#CodeApproachLightingBaseType-CALVERT">
        <rdf:type rdf:resource="http://www.project-best.eu/owl/aixm-mod/airportheliport#CodeApproachLightingType"/>
        <rdfs:comment xml:lang="en">Calvert Approach Lighting System </rdfs:comment>
    </owl:NamedIndividual>
    


    <!-- http://www.project-best.eu/owl/aixm-mod/airportheliport#CodeApproachLightingBaseType-LDIN -->

    <owl:NamedIndividual rdf:about="http://www.project-best.eu/owl/aixm-mod/airportheliport#CodeApproachLightingBaseType-LDIN">
        <rdf:type rdf:resource="http://www.project-best.eu/owl/aixm-mod/airportheliport#CodeApproachLightingType"/>
        <rdfs:comment xml:lang="en">Lead-In Lighting System.</rdfs:comment>
    </owl:NamedIndividual>
    


    <!-- http://www.project-best.eu/owl/aixm-mod/airportheliport#CodeApproachLightingBaseType-MALS -->

    <owl:NamedIndividual rdf:about="http://www.project-best.eu/owl/aixm-mod/airportheliport#CodeApproachLightingBaseType-MALS">
        <rdf:type rdf:resource="http://www.project-best.eu/owl/aixm-mod/airportheliport#CodeApproachLightingType"/>
        <rdfs:comment xml:lang="en">1400 Foot Medium Intensity Approach Lighting System.</rdfs:comment>
    </owl:NamedIndividual>
    


    <!-- http://www.project-best.eu/owl/aixm-mod/airportheliport#CodeApproachLightingBaseType-MALSR -->

    <owl:NamedIndividual rdf:about="http://www.project-best.eu/owl/aixm-mod/airportheliport#CodeApproachLightingBaseType-MALSR">
        <rdf:type rdf:resource="http://www.project-best.eu/owl/aixm-mod/airportheliport#CodeApproachLightingType"/>
        <rdfs:comment xml:lang="en">1400 Foot Medium Intensity Approach Lighting System with Runway Alignment Indicator Lights.</rdfs:comment>
    </owl:NamedIndividual>
    


    <!-- http://www.project-best.eu/owl/aixm-mod/airportheliport#CodeApproachLightingBaseType-MILOVRN -->

    <owl:NamedIndividual rdf:about="http://www.project-best.eu/owl/aixm-mod/airportheliport#CodeApproachLightingBaseType-MILOVRN">
        <rdf:type rdf:resource="http://www.project-best.eu/owl/aixm-mod/airportheliport#CodeApproachLightingType"/>
        <rdfs:comment xml:lang="en">Military Overrun.</rdfs:comment>
    </owl:NamedIndividual>
    


    <!-- http://www.project-best.eu/owl/aixm-mod/airportheliport#CodeApproachLightingBaseType-ODALS -->

    <owl:NamedIndividual rdf:about="http://www.project-best.eu/owl/aixm-mod/airportheliport#CodeApproachLightingBaseType-ODALS">
        <rdf:type rdf:resource="http://www.project-best.eu/owl/aixm-mod/airportheliport#CodeApproachLightingType"/>
        <rdfs:comment xml:lang="en">Omni Directional Approach Lighting System.</rdfs:comment>
    </owl:NamedIndividual>
    


    <!-- http://www.project-best.eu/owl/aixm-mod/airportheliport#CodeApproachLightingBaseType-OTHER -->

    <owl:NamedIndividual rdf:about="http://www.project-best.eu/owl/aixm-mod/airportheliport#CodeApproachLightingBaseType-OTHER">
        <rdf:type rdf:resource="http://www.project-best.eu/owl/aixm-mod/airportheliport#CodeApproachLightingType"/>
        <rdfs:comment xml:lang="en">Other</rdfs:comment>
    </owl:NamedIndividual>
    


    <!-- http://www.project-best.eu/owl/aixm-mod/airportheliport#CodeApproachLightingBaseType-SALS -->

    <owl:NamedIndividual rdf:about="http://www.project-best.eu/owl/aixm-mod/airportheliport#CodeApproachLightingBaseType-SALS">
        <rdf:type rdf:resource="http://www.project-best.eu/owl/aixm-mod/airportheliport#CodeApproachLightingType"/>
        <rdfs:comment xml:lang="en">Simple Approach Lighting System.</rdfs:comment>
    </owl:NamedIndividual>
    


    <!-- http://www.project-best.eu/owl/aixm-mod/airportheliport#CodeApproachLightingBaseType-SSALR -->

    <owl:NamedIndividual rdf:about="http://www.project-best.eu/owl/aixm-mod/airportheliport#CodeApproachLightingBaseType-SSALR">
        <rdf:type rdf:resource="http://www.project-best.eu/owl/aixm-mod/airportheliport#CodeApproachLightingType"/>
        <rdfs:comment xml:lang="en">Simplified Short Approach Lighting System with Runway Alignment Indicator Lights.</rdfs:comment>
    </owl:NamedIndividual>
    


    <!-- http://www.project-best.eu/owl/aixm-mod/airportheliport#CodeApproachLightingBaseType-SSALS -->

    <owl:NamedIndividual rdf:about="http://www.project-best.eu/owl/aixm-mod/airportheliport#CodeApproachLightingBaseType-SSALS">
        <rdf:type rdf:resource="http://www.project-best.eu/owl/aixm-mod/airportheliport#CodeApproachLightingType"/>
        <rdfs:comment xml:lang="en">Simplified Short Approach Lighting System.</rdfs:comment>
    </owl:NamedIndividual>
    


    <!-- http://www.project-best.eu/owl/aixm-mod/airportheliport#CodeApproachLightingICAOBaseType-CAT1 -->

    <owl:NamedIndividual rdf:about="http://www.project-best.eu/owl/aixm-mod/airportheliport#CodeApproachLightingICAOBaseType-CAT1">
        <rdf:type rdf:resource="http://www.project-best.eu/owl/aixm-mod/airportheliport#CodeApproachLightingICAOType"/>
        <rdfs:comment xml:lang="en">Precision approach category I lighting system (ICAO Annex 14, Vol 1, 5.3.4.10) </rdfs:comment>
    </owl:NamedIndividual>
    


    <!-- http://www.project-best.eu/owl/aixm-mod/airportheliport#CodeApproachLightingICAOBaseType-CAT23 -->

    <owl:NamedIndividual rdf:about="http://www.project-best.eu/owl/aixm-mod/airportheliport#CodeApproachLightingICAOBaseType-CAT23">
        <rdf:type rdf:resource="http://www.project-best.eu/owl/aixm-mod/airportheliport#CodeApproachLightingICAOType"/>
        <rdfs:comment xml:lang="en">Precision approach category II and III lighting system (ICAO Annex 14, Vol 1, 5.3.4.22) </rdfs:comment>
    </owl:NamedIndividual>
    


    <!-- http://www.project-best.eu/owl/aixm-mod/airportheliport#CodeApproachLightingICAOBaseType-CIRCLING -->

    <owl:NamedIndividual rdf:about="http://www.project-best.eu/owl/aixm-mod/airportheliport#CodeApproachLightingICAOBaseType-CIRCLING">
        <rdf:type rdf:resource="http://www.project-best.eu/owl/aixm-mod/airportheliport#CodeApproachLightingICAOType"/>
        <rdfs:comment xml:lang="en">Circling guidance lighting system (ICAO Annex 14, Vol 1, 5.3.6) </rdfs:comment>
    </owl:NamedIndividual>
    


    <!-- http://www.project-best.eu/owl/aixm-mod/airportheliport#CodeApproachLightingICAOBaseType-LEADIN -->

    <owl:NamedIndividual rdf:about="http://www.project-best.eu/owl/aixm-mod/airportheliport#CodeApproachLightingICAOBaseType-LEADIN">
        <rdf:type rdf:resource="http://www.project-best.eu/owl/aixm-mod/airportheliport#CodeApproachLightingICAOType"/>
        <rdfs:comment xml:lang="en">Runway lead-in lighting system (ICAO Annex 14, Vol 1, 5.3.7)</rdfs:comment>
    </owl:NamedIndividual>
    


    <!-- http://www.project-best.eu/owl/aixm-mod/airportheliport#CodeApproachLightingICAOBaseType-NONE -->

    <owl:NamedIndividual rdf:about="http://www.project-best.eu/owl/aixm-mod/airportheliport#CodeApproachLightingICAOBaseType-NONE">
        <rdf:type rdf:resource="http://www.project-best.eu/owl/aixm-mod/airportheliport#CodeApproachLightingICAOType"/>
        <rdfs:comment xml:lang="en"> Does not classify as an ICAO type</rdfs:comment>
    </owl:NamedIndividual>
    


    <!-- http://www.project-best.eu/owl/aixm-mod/airportheliport#CodeApproachLightingICAOBaseType-OTHER -->

    <owl:NamedIndividual rdf:about="http://www.project-best.eu/owl/aixm-mod/airportheliport#CodeApproachLightingICAOBaseType-OTHER">
        <rdf:type rdf:resource="http://www.project-best.eu/owl/aixm-mod/airportheliport#CodeApproachLightingICAOType"/>
        <rdfs:comment xml:lang="en">Other</rdfs:comment>
    </owl:NamedIndividual>
    


    <!-- http://www.project-best.eu/owl/aixm-mod/airportheliport#CodeApproachLightingICAOBaseType-SIMPLE -->

    <owl:NamedIndividual rdf:about="http://www.project-best.eu/owl/aixm-mod/airportheliport#CodeApproachLightingICAOBaseType-SIMPLE">
        <rdf:type rdf:resource="http://www.project-best.eu/owl/aixm-mod/airportheliport#CodeApproachLightingICAOType"/>
        <rdfs:comment xml:lang="en">Simple approach lighting system (ICAO Annex 14, Vol 1, 5.3.4.2) </rdfs:comment>
    </owl:NamedIndividual>
    


    <!-- http://www.project-best.eu/owl/aixm-mod/airportheliport#CodeApronElementBaseType-CARGO -->

    <owl:NamedIndividual rdf:about="http://www.project-best.eu/owl/aixm-mod/airportheliport#CodeApronElementBaseType-CARGO">
        <rdf:type rdf:resource="http://www.project-best.eu/owl/aixm-mod/airportheliport#CodeApronElementType"/>
        <rdfs:comment xml:lang="en">Cargo Loading Area used for loading and unloading cargo. (AirMAT)</rdfs:comment>
    </owl:NamedIndividual>
    


    <!-- http://www.project-best.eu/owl/aixm-mod/airportheliport#CodeApronElementBaseType-FUEL -->

    <owl:NamedIndividual rdf:about="http://www.project-best.eu/owl/aixm-mod/airportheliport#CodeApronElementBaseType-FUEL">
        <rdf:type rdf:resource="http://www.project-best.eu/owl/aixm-mod/airportheliport#CodeApronElementType"/>
        <rdfs:comment xml:lang="en">Area used for aircraft fuelling. (AirMAT)</rdfs:comment>
    </owl:NamedIndividual>
    


    <!-- http://www.project-best.eu/owl/aixm-mod/airportheliport#CodeApronElementBaseType-HARDSTAND -->

    <owl:NamedIndividual rdf:about="http://www.project-best.eu/owl/aixm-mod/airportheliport#CodeApronElementBaseType-HARDSTAND">
        <rdf:type rdf:resource="http://www.project-best.eu/owl/aixm-mod/airportheliport#CodeApronElementType"/>
        <rdfs:comment xml:lang="en">Area for parking a single aircraft more temporary than a parking area (AirMAT)</rdfs:comment>
    </owl:NamedIndividual>
    


    <!-- http://www.project-best.eu/owl/aixm-mod/airportheliport#CodeApronElementBaseType-LOADING -->

    <owl:NamedIndividual rdf:about="http://www.project-best.eu/owl/aixm-mod/airportheliport#CodeApronElementBaseType-LOADING">
        <rdf:type rdf:resource="http://www.project-best.eu/owl/aixm-mod/airportheliport#CodeApronElementType"/>
        <rdfs:comment xml:lang="en">Passenger loading area used for loading/unloading of passengers (AirMAT)</rdfs:comment>
    </owl:NamedIndividual>
    


    <!-- http://www.project-best.eu/owl/aixm-mod/airportheliport#CodeApronElementBaseType-MAINT -->

    <owl:NamedIndividual rdf:about="http://www.project-best.eu/owl/aixm-mod/airportheliport#CodeApronElementBaseType-MAINT">
        <rdf:type rdf:resource="http://www.project-best.eu/owl/aixm-mod/airportheliport#CodeApronElementType"/>
        <rdfs:comment xml:lang="en">Area used for aircraft maintenance. (AirMAT)</rdfs:comment>
    </owl:NamedIndividual>
    


    <!-- http://www.project-best.eu/owl/aixm-mod/airportheliport#CodeApronElementBaseType-MILITARY -->

    <owl:NamedIndividual rdf:about="http://www.project-best.eu/owl/aixm-mod/airportheliport#CodeApronElementBaseType-MILITARY">
        <rdf:type rdf:resource="http://www.project-best.eu/owl/aixm-mod/airportheliport#CodeApronElementType"/>
        <rdfs:comment xml:lang="en">Apron used by military (AirMAT)</rdfs:comment>
    </owl:NamedIndividual>
    


    <!-- http://www.project-best.eu/owl/aixm-mod/airportheliport#CodeApronElementBaseType-NORMAL -->

    <owl:NamedIndividual rdf:about="http://www.project-best.eu/owl/aixm-mod/airportheliport#CodeApronElementBaseType-NORMAL">
        <rdf:type rdf:resource="http://www.project-best.eu/owl/aixm-mod/airportheliport#CodeApronElementType"/>
        <rdfs:comment xml:lang="en">The default type.</rdfs:comment>
    </owl:NamedIndividual>
    


    <!-- http://www.project-best.eu/owl/aixm-mod/airportheliport#CodeApronElementBaseType-OTHER -->

    <owl:NamedIndividual rdf:about="http://www.project-best.eu/owl/aixm-mod/airportheliport#CodeApronElementBaseType-OTHER">
        <rdf:type rdf:resource="http://www.project-best.eu/owl/aixm-mod/airportheliport#CodeApronElementType"/>
        <rdfs:comment xml:lang="en">Other</rdfs:comment>
    </owl:NamedIndividual>
    


    <!-- http://www.project-best.eu/owl/aixm-mod/airportheliport#CodeApronElementBaseType-PARKING -->

    <owl:NamedIndividual rdf:about="http://www.project-best.eu/owl/aixm-mod/airportheliport#CodeApronElementBaseType-PARKING">
        <rdf:type rdf:resource="http://www.project-best.eu/owl/aixm-mod/airportheliport#CodeApronElementType"/>
        <rdfs:comment xml:lang="en">Parking Stand Area (from AMDB)</rdfs:comment>
    </owl:NamedIndividual>
    


    <!-- http://www.project-best.eu/owl/aixm-mod/airportheliport#CodeApronElementBaseType-RAMP -->

    <owl:NamedIndividual rdf:about="http://www.project-best.eu/owl/aixm-mod/airportheliport#CodeApronElementBaseType-RAMP">
        <rdf:type rdf:resource="http://www.project-best.eu/owl/aixm-mod/airportheliport#CodeApronElementType"/>
        <rdfs:comment xml:lang="en">Access pavement between maintenance hangers opening to the apron and the apron edge. (AirMAT)</rdfs:comment>
    </owl:NamedIndividual>
    


    <!-- http://www.project-best.eu/owl/aixm-mod/airportheliport#CodeApronElementBaseType-STAIRS -->

    <owl:NamedIndividual rdf:about="http://www.project-best.eu/owl/aixm-mod/airportheliport#CodeApronElementBaseType-STAIRS">
        <rdf:type rdf:resource="http://www.project-best.eu/owl/aixm-mod/airportheliport#CodeApronElementType"/>
        <rdfs:comment xml:lang="en">Stairs</rdfs:comment>
    </owl:NamedIndividual>
    


    <!-- http://www.project-best.eu/owl/aixm-mod/airportheliport#CodeApronElementBaseType-TAXILANE -->

    <owl:NamedIndividual rdf:about="http://www.project-best.eu/owl/aixm-mod/airportheliport#CodeApronElementBaseType-TAXILANE">
        <rdf:type rdf:resource="http://www.project-best.eu/owl/aixm-mod/airportheliport#CodeApronElementType"/>
        <rdfs:comment xml:lang="en">Area where plane is still under terminal control (airline dispatched) as opposed to tower control. (AirMAT)</rdfs:comment>
    </owl:NamedIndividual>
    


    <!-- http://www.project-best.eu/owl/aixm-mod/airportheliport#CodeApronElementBaseType-TEMPORARY -->

    <owl:NamedIndividual rdf:about="http://www.project-best.eu/owl/aixm-mod/airportheliport#CodeApronElementBaseType-TEMPORARY">
        <rdf:type rdf:resource="http://www.project-best.eu/owl/aixm-mod/airportheliport#CodeApronElementType"/>
        <rdfs:comment xml:lang="en">Temporary</rdfs:comment>
    </owl:NamedIndividual>
    


    <!-- http://www.project-best.eu/owl/aixm-mod/airportheliport#CodeApronElementBaseType-TURNAROUND -->

    <owl:NamedIndividual rdf:about="http://www.project-best.eu/owl/aixm-mod/airportheliport#CodeApronElementBaseType-TURNAROUND">
        <rdf:type rdf:resource="http://www.project-best.eu/owl/aixm-mod/airportheliport#CodeApronElementType"/>
        <rdfs:comment xml:lang="en">Area for aircraft to turn around (AirMAT)</rdfs:comment>
    </owl:NamedIndividual>
    


    <!-- http://www.project-best.eu/owl/aixm-mod/airportheliport#CodeApronSectionBaseType-EDGE -->

    <owl:NamedIndividual rdf:about="http://www.project-best.eu/owl/aixm-mod/airportheliport#CodeApronSectionBaseType-EDGE">
        <rdf:type rdf:resource="http://www.project-best.eu/owl/aixm-mod/airportheliport#CodeApronSectionType"/>
        <rdfs:comment xml:lang="en">Apron edge.</rdfs:comment>
    </owl:NamedIndividual>
    


    <!-- http://www.project-best.eu/owl/aixm-mod/airportheliport#CodeApronSectionBaseType-OTHER -->

    <owl:NamedIndividual rdf:about="http://www.project-best.eu/owl/aixm-mod/airportheliport#CodeApronSectionBaseType-OTHER">
        <rdf:type rdf:resource="http://www.project-best.eu/owl/aixm-mod/airportheliport#CodeApronSectionType"/>
        <rdfs:comment xml:lang="en">Other position on apron.</rdfs:comment>
    </owl:NamedIndividual>
    


    <!-- http://www.project-best.eu/owl/aixm-mod/airportheliport#CodeArrestingGearEnergyAbsorbBaseType-BARRIER_DISK_SAFELAND -->

    <owl:NamedIndividual rdf:about="http://www.project-best.eu/owl/aixm-mod/airportheliport#CodeArrestingGearEnergyAbsorbBaseType-BARRIER_DISK_SAFELAND">
        <rdf:type rdf:resource="http://www.project-best.eu/owl/aixm-mod/airportheliport#CodeArrestingGearEnergyAbsorbType"/>
        <rdfs:comment xml:lang="en">Safe-land Barrier pneumatic disc brake.	Used only with a net engagement device. May be designated as &apos;DJ&apos;.</rdfs:comment>
    </owl:NamedIndividual>
    


    <!-- http://www.project-best.eu/owl/aixm-mod/airportheliport#CodeArrestingGearEnergyAbsorbBaseType-CHAIN_CHAG -->

    <owl:NamedIndividual rdf:about="http://www.project-best.eu/owl/aixm-mod/airportheliport#CodeArrestingGearEnergyAbsorbBaseType-CHAIN_CHAG">
        <rdf:type rdf:resource="http://www.project-best.eu/owl/aixm-mod/airportheliport#CodeArrestingGearEnergyAbsorbType"/>
        <rdfs:comment xml:lang="en">CHAG chain brake.	May be used with any type of engagement device. May be designated as &apos;BS&apos;.</rdfs:comment>
    </owl:NamedIndividual>
    


    <!-- http://www.project-best.eu/owl/aixm-mod/airportheliport#CodeArrestingGearEnergyAbsorbBaseType-CHAIN_E5 -->

    <owl:NamedIndividual rdf:about="http://www.project-best.eu/owl/aixm-mod/airportheliport#CodeArrestingGearEnergyAbsorbBaseType-CHAIN_E5">
        <rdf:type rdf:resource="http://www.project-best.eu/owl/aixm-mod/airportheliport#CodeArrestingGearEnergyAbsorbType"/>
        <rdfs:comment xml:lang="en">E5 chain brake.	Used only with a hook engagement device. May be designated as &apos;BU&apos;.</rdfs:comment>
    </owl:NamedIndividual>
    


    <!-- http://www.project-best.eu/owl/aixm-mod/airportheliport#CodeArrestingGearEnergyAbsorbBaseType-CHAIN_E5_1 -->

    <owl:NamedIndividual rdf:about="http://www.project-best.eu/owl/aixm-mod/airportheliport#CodeArrestingGearEnergyAbsorbBaseType-CHAIN_E5_1">
        <rdf:type rdf:resource="http://www.project-best.eu/owl/aixm-mod/airportheliport#CodeArrestingGearEnergyAbsorbType"/>
        <rdfs:comment xml:lang="en">E5-1 chain brake.	Used only with a hook engagement device. May be designated as &apos;BV&apos;.</rdfs:comment>
    </owl:NamedIndividual>
    


    <!-- http://www.project-best.eu/owl/aixm-mod/airportheliport#CodeArrestingGearEnergyAbsorbBaseType-CHAIN_E5_2 -->

    <owl:NamedIndividual rdf:about="http://www.project-best.eu/owl/aixm-mod/airportheliport#CodeArrestingGearEnergyAbsorbBaseType-CHAIN_E5_2">
        <rdf:type rdf:resource="http://www.project-best.eu/owl/aixm-mod/airportheliport#CodeArrestingGearEnergyAbsorbType"/>
        <rdfs:comment xml:lang="en">E5-2 chain brake.	Used only with a hook engagement device. May be designated as &apos;BW&apos;.</rdfs:comment>
    </owl:NamedIndividual>
    


    <!-- http://www.project-best.eu/owl/aixm-mod/airportheliport#CodeArrestingGearEnergyAbsorbBaseType-CHAIN_E5_3 -->

    <owl:NamedIndividual rdf:about="http://www.project-best.eu/owl/aixm-mod/airportheliport#CodeArrestingGearEnergyAbsorbBaseType-CHAIN_E5_3">
        <rdf:type rdf:resource="http://www.project-best.eu/owl/aixm-mod/airportheliport#CodeArrestingGearEnergyAbsorbType"/>
        <rdfs:comment xml:lang="en">E5-3 chain brake.	Used only with a hook engagement device. May be designated as &apos;CA&apos;.</rdfs:comment>
    </owl:NamedIndividual>
    


    <!-- http://www.project-best.eu/owl/aixm-mod/airportheliport#CodeArrestingGearEnergyAbsorbBaseType-CHAIN_E6 -->

    <owl:NamedIndividual rdf:about="http://www.project-best.eu/owl/aixm-mod/airportheliport#CodeArrestingGearEnergyAbsorbBaseType-CHAIN_E6">
        <rdf:type rdf:resource="http://www.project-best.eu/owl/aixm-mod/airportheliport#CodeArrestingGearEnergyAbsorbType"/>
        <rdfs:comment xml:lang="en">E6 chain brake.	Used only with a hook engagement device. May be designated as &apos;CB&apos;.</rdfs:comment>
    </owl:NamedIndividual>
    


    <!-- http://www.project-best.eu/owl/aixm-mod/airportheliport#CodeArrestingGearEnergyAbsorbBaseType-DISK_BEFAB_12_3 -->

    <owl:NamedIndividual rdf:about="http://www.project-best.eu/owl/aixm-mod/airportheliport#CodeArrestingGearEnergyAbsorbBaseType-DISK_BEFAB_12_3">
        <rdf:type rdf:resource="http://www.project-best.eu/owl/aixm-mod/airportheliport#CodeArrestingGearEnergyAbsorbType"/>
        <rdfs:comment xml:lang="en">BEFAB 12:3 pneumatic disc brake, also known as SAFEBAR or SAFELAND 12:3.	May be used with any type of engagement device. May be designated as &apos;BJ&apos;.</rdfs:comment>
    </owl:NamedIndividual>
    


    <!-- http://www.project-best.eu/owl/aixm-mod/airportheliport#CodeArrestingGearEnergyAbsorbBaseType-DISK_BEFAB_20_4 -->

    <owl:NamedIndividual rdf:about="http://www.project-best.eu/owl/aixm-mod/airportheliport#CodeArrestingGearEnergyAbsorbBaseType-DISK_BEFAB_20_4">
        <rdf:type rdf:resource="http://www.project-best.eu/owl/aixm-mod/airportheliport#CodeArrestingGearEnergyAbsorbType"/>
        <rdfs:comment xml:lang="en">BEFAB 20:4 pneumatic disc brake, also known as SAFEBAR or SAFELAND 20:4.	May be used with any type of engagement device. May be designated as &apos;BN&apos;.</rdfs:comment>
    </owl:NamedIndividual>
    


    <!-- http://www.project-best.eu/owl/aixm-mod/airportheliport#CodeArrestingGearEnergyAbsorbBaseType-DISK_BEFAB_21_2 -->

    <owl:NamedIndividual rdf:about="http://www.project-best.eu/owl/aixm-mod/airportheliport#CodeArrestingGearEnergyAbsorbBaseType-DISK_BEFAB_21_2">
        <rdf:type rdf:resource="http://www.project-best.eu/owl/aixm-mod/airportheliport#CodeArrestingGearEnergyAbsorbType"/>
        <rdfs:comment xml:lang="en">BEFAB 21:2 pneumatic disc brake, also known as SAFEBAR or SAFELAND 21:2.	May be used with any type of engagement device. May be designated as &apos;BO&apos;.</rdfs:comment>
    </owl:NamedIndividual>
    


    <!-- http://www.project-best.eu/owl/aixm-mod/airportheliport#CodeArrestingGearEnergyAbsorbBaseType-DISK_BEFAB_24_4 -->

    <owl:NamedIndividual rdf:about="http://www.project-best.eu/owl/aixm-mod/airportheliport#CodeArrestingGearEnergyAbsorbBaseType-DISK_BEFAB_24_4">
        <rdf:type rdf:resource="http://www.project-best.eu/owl/aixm-mod/airportheliport#CodeArrestingGearEnergyAbsorbType"/>
        <rdfs:comment xml:lang="en">BEFAB 24:4 pneumatic disc brake, also known as SAFEBAR or SAFELAND 24:4.	May be used with any type of engagement device. May be designated as &apos;BP&apos;.</rdfs:comment>
    </owl:NamedIndividual>
    


    <!-- http://www.project-best.eu/owl/aixm-mod/airportheliport#CodeArrestingGearEnergyAbsorbBaseType-DISK_BEFAB_56_2 -->

    <owl:NamedIndividual rdf:about="http://www.project-best.eu/owl/aixm-mod/airportheliport#CodeArrestingGearEnergyAbsorbBaseType-DISK_BEFAB_56_2">
        <rdf:type rdf:resource="http://www.project-best.eu/owl/aixm-mod/airportheliport#CodeArrestingGearEnergyAbsorbType"/>
        <rdfs:comment xml:lang="en">BEFAB 56:2 pneumatic disc brake, also known as SAFEBAR or SAFELAND 56:2.	May be used with any type of engagement device. May be designated as &apos;BQ&apos;.</rdfs:comment>
    </owl:NamedIndividual>
    


    <!-- http://www.project-best.eu/owl/aixm-mod/airportheliport#CodeArrestingGearEnergyAbsorbBaseType-DISK_BEFAB_60_2 -->

    <owl:NamedIndividual rdf:about="http://www.project-best.eu/owl/aixm-mod/airportheliport#CodeArrestingGearEnergyAbsorbBaseType-DISK_BEFAB_60_2">
        <rdf:type rdf:resource="http://www.project-best.eu/owl/aixm-mod/airportheliport#CodeArrestingGearEnergyAbsorbType"/>
        <rdfs:comment xml:lang="en">BEFAB 60:2 pneumatic disc brake, also known as SAFEBAR or SAFELAND 60:2.	May be used with any type of engagement device. May be designated as &apos;BR&apos;.</rdfs:comment>
    </owl:NamedIndividual>
    


    <!-- http://www.project-best.eu/owl/aixm-mod/airportheliport#CodeArrestingGearEnergyAbsorbBaseType-DISK_BEFAB_6_3 -->

    <owl:NamedIndividual rdf:about="http://www.project-best.eu/owl/aixm-mod/airportheliport#CodeArrestingGearEnergyAbsorbBaseType-DISK_BEFAB_6_3">
        <rdf:type rdf:resource="http://www.project-best.eu/owl/aixm-mod/airportheliport#CodeArrestingGearEnergyAbsorbType"/>
        <rdfs:comment xml:lang="en">BEFAB 6:3 pneumatic disc brake, also known as SAFEBAR or SAFELAND 6:2.	May be used with any type of engagement device. May be designated as &apos;BH&apos;.</rdfs:comment>
    </owl:NamedIndividual>
    


    <!-- http://www.project-best.eu/owl/aixm-mod/airportheliport#CodeArrestingGearEnergyAbsorbBaseType-DISK_BEFAB_8_3 -->

    <owl:NamedIndividual rdf:about="http://www.project-best.eu/owl/aixm-mod/airportheliport#CodeArrestingGearEnergyAbsorbBaseType-DISK_BEFAB_8_3">
        <rdf:type rdf:resource="http://www.project-best.eu/owl/aixm-mod/airportheliport#CodeArrestingGearEnergyAbsorbType"/>
        <rdfs:comment xml:lang="en">BEFAB 8:3 pneumatic disc brake, also known as SAFEBAR or SAFELAND 8:3.	May be used with any type of engagement device. May be designated as &apos;BI&apos;.</rdfs:comment>
    </owl:NamedIndividual>
    


    <!-- http://www.project-best.eu/owl/aixm-mod/airportheliport#CodeArrestingGearEnergyAbsorbBaseType-DISK_RAF_MK_12A -->

    <owl:NamedIndividual rdf:about="http://www.project-best.eu/owl/aixm-mod/airportheliport#CodeArrestingGearEnergyAbsorbBaseType-DISK_RAF_MK_12A">
        <rdf:type rdf:resource="http://www.project-best.eu/owl/aixm-mod/airportheliport#CodeArrestingGearEnergyAbsorbType"/>
        <rdfs:comment xml:lang="en">RAF MK-12A pneumatic disc brake.	Used only with a net engagement device. May be designated as &apos;DC&apos;.</rdfs:comment>
    </owl:NamedIndividual>
    


    <!-- http://www.project-best.eu/owl/aixm-mod/airportheliport#CodeArrestingGearEnergyAbsorbBaseType-DISK_RAF_MK_6 -->

    <owl:NamedIndividual rdf:about="http://www.project-best.eu/owl/aixm-mod/airportheliport#CodeArrestingGearEnergyAbsorbBaseType-DISK_RAF_MK_6">
        <rdf:type rdf:resource="http://www.project-best.eu/owl/aixm-mod/airportheliport#CodeArrestingGearEnergyAbsorbType"/>
        <rdfs:comment xml:lang="en">RAF MK-6 pneumatic disc brake.	May be used with any type of engagement device. May be designated as &apos;DF&apos;.</rdfs:comment>
    </owl:NamedIndividual>
    


    <!-- http://www.project-best.eu/owl/aixm-mod/airportheliport#CodeArrestingGearEnergyAbsorbBaseType-DISK_RAF_TYPEA_BEFAB_6_3 -->

    <owl:NamedIndividual rdf:about="http://www.project-best.eu/owl/aixm-mod/airportheliport#CodeArrestingGearEnergyAbsorbBaseType-DISK_RAF_TYPEA_BEFAB_6_3">
        <rdf:type rdf:resource="http://www.project-best.eu/owl/aixm-mod/airportheliport#CodeArrestingGearEnergyAbsorbType"/>
        <rdfs:comment xml:lang="en">RAF Type A BEFAB 6:3 pneumatic disc brake.	Used only with a net engagement device. May be designated as &apos;DG&apos;.</rdfs:comment>
    </owl:NamedIndividual>
    


    <!-- http://www.project-best.eu/owl/aixm-mod/airportheliport#CodeArrestingGearEnergyAbsorbBaseType-DISK_RAF_TYPEB_BEFAB_12_3 -->

    <owl:NamedIndividual rdf:about="http://www.project-best.eu/owl/aixm-mod/airportheliport#CodeArrestingGearEnergyAbsorbBaseType-DISK_RAF_TYPEB_BEFAB_12_3">
        <rdf:type rdf:resource="http://www.project-best.eu/owl/aixm-mod/airportheliport#CodeArrestingGearEnergyAbsorbType"/>
        <rdfs:comment xml:lang="en">RAF Type B BEFAB 12:3 pneumatic disc brake.	Used only with a net engagement device. May be designated as &apos;DH&apos;.</rdfs:comment>
    </owl:NamedIndividual>
    


    <!-- http://www.project-best.eu/owl/aixm-mod/airportheliport#CodeArrestingGearEnergyAbsorbBaseType-LINEAR_BAK_6 -->

    <owl:NamedIndividual rdf:about="http://www.project-best.eu/owl/aixm-mod/airportheliport#CodeArrestingGearEnergyAbsorbBaseType-LINEAR_BAK_6">
        <rdf:type rdf:resource="http://www.project-best.eu/owl/aixm-mod/airportheliport#CodeArrestingGearEnergyAbsorbType"/>
        <rdfs:comment xml:lang="en">BAK-6 linear hydraulic (water squeezer) brake.	Used only with a hook engagement device. May be designated as &apos;BD&apos;.</rdfs:comment>
    </owl:NamedIndividual>
    


    <!-- http://www.project-best.eu/owl/aixm-mod/airportheliport#CodeArrestingGearEnergyAbsorbBaseType-LINEAR_SPRAG_MK_1 -->

    <owl:NamedIndividual rdf:about="http://www.project-best.eu/owl/aixm-mod/airportheliport#CodeArrestingGearEnergyAbsorbBaseType-LINEAR_SPRAG_MK_1">
        <rdf:type rdf:resource="http://www.project-best.eu/owl/aixm-mod/airportheliport#CodeArrestingGearEnergyAbsorbType"/>
        <rdfs:comment xml:lang="en">SPRAG MK-1 linear hydraulic (water squeezer) brake.	Used only with a hook engagement device. May be designated as &apos;DN&apos;.</rdfs:comment>
    </owl:NamedIndividual>
    


    <!-- http://www.project-best.eu/owl/aixm-mod/airportheliport#CodeArrestingGearEnergyAbsorbBaseType-MOBILROTARY_HYDRAULIC_WATER -->

    <owl:NamedIndividual rdf:about="http://www.project-best.eu/owl/aixm-mod/airportheliport#CodeArrestingGearEnergyAbsorbBaseType-MOBILROTARY_HYDRAULIC_WATER">
        <rdf:type rdf:resource="http://www.project-best.eu/owl/aixm-mod/airportheliport#CodeArrestingGearEnergyAbsorbType"/>
        <rdfs:comment xml:lang="en">Water rotary hydraulic mobile arresting gear.</rdfs:comment>
    </owl:NamedIndividual>
    


    <!-- http://www.project-best.eu/owl/aixm-mod/airportheliport#CodeArrestingGearEnergyAbsorbBaseType-MOBILROTARY_M21 -->

    <owl:NamedIndividual rdf:about="http://www.project-best.eu/owl/aixm-mod/airportheliport#CodeArrestingGearEnergyAbsorbBaseType-MOBILROTARY_M21">
        <rdf:type rdf:resource="http://www.project-best.eu/owl/aixm-mod/airportheliport#CodeArrestingGearEnergyAbsorbType"/>
        <rdfs:comment xml:lang="en">M21 rotary hydraulic water brake - mobile	May be used with any type of engagement device. May be designated as &apos;CH&apos;.</rdfs:comment>
    </owl:NamedIndividual>
    


    <!-- http://www.project-best.eu/owl/aixm-mod/airportheliport#CodeArrestingGearEnergyAbsorbBaseType-MOBILROTARY_MAAS -->

    <owl:NamedIndividual rdf:about="http://www.project-best.eu/owl/aixm-mod/airportheliport#CodeArrestingGearEnergyAbsorbBaseType-MOBILROTARY_MAAS">
        <rdf:type rdf:resource="http://www.project-best.eu/owl/aixm-mod/airportheliport#CodeArrestingGearEnergyAbsorbType"/>
        <rdfs:comment xml:lang="en">MAAS, a trailer-mounted rotary friction BAK-12.	Used by the USAF only with a hook engagement device, but may be used with any engagement by others. May be designated as &apos;CI&apos;.</rdfs:comment>
    </owl:NamedIndividual>
    


    <!-- http://www.project-best.eu/owl/aixm-mod/airportheliport#CodeArrestingGearEnergyAbsorbBaseType-MOBILROTARY_MAG_I -->

    <owl:NamedIndividual rdf:about="http://www.project-best.eu/owl/aixm-mod/airportheliport#CodeArrestingGearEnergyAbsorbBaseType-MOBILROTARY_MAG_I">
        <rdf:type rdf:resource="http://www.project-best.eu/owl/aixm-mod/airportheliport#CodeArrestingGearEnergyAbsorbType"/>
        <rdfs:comment xml:lang="en">MAG I rotary hydraulic mobile arresting gear.	Used only with a hook engagement device. May be designated as &apos;CJ&apos;.</rdfs:comment>
    </owl:NamedIndividual>
    


    <!-- http://www.project-best.eu/owl/aixm-mod/airportheliport#CodeArrestingGearEnergyAbsorbBaseType-MOBILROTARY_MAG_II -->

    <owl:NamedIndividual rdf:about="http://www.project-best.eu/owl/aixm-mod/airportheliport#CodeArrestingGearEnergyAbsorbBaseType-MOBILROTARY_MAG_II">
        <rdf:type rdf:resource="http://www.project-best.eu/owl/aixm-mod/airportheliport#CodeArrestingGearEnergyAbsorbType"/>
        <rdfs:comment xml:lang="en">MAG II rotary hydraulic mobile arresting gear.	Used only with a hook engagement device. May be designated as &apos;CN&apos;.</rdfs:comment>
    </owl:NamedIndividual>
    


    <!-- http://www.project-best.eu/owl/aixm-mod/airportheliport#CodeArrestingGearEnergyAbsorbBaseType-MOBILROTARY_MAG_III -->

    <owl:NamedIndividual rdf:about="http://www.project-best.eu/owl/aixm-mod/airportheliport#CodeArrestingGearEnergyAbsorbBaseType-MOBILROTARY_MAG_III">
        <rdf:type rdf:resource="http://www.project-best.eu/owl/aixm-mod/airportheliport#CodeArrestingGearEnergyAbsorbType"/>
        <rdfs:comment xml:lang="en">MAG III rotary hydraulic mobile arresting gear.	Used only with a hook engagement device. May be designated as &apos;CO&apos;.</rdfs:comment>
    </owl:NamedIndividual>
    


    <!-- http://www.project-best.eu/owl/aixm-mod/airportheliport#CodeArrestingGearEnergyAbsorbBaseType-MOBILROTARY_MAG_IV -->

    <owl:NamedIndividual rdf:about="http://www.project-best.eu/owl/aixm-mod/airportheliport#CodeArrestingGearEnergyAbsorbBaseType-MOBILROTARY_MAG_IV">
        <rdf:type rdf:resource="http://www.project-best.eu/owl/aixm-mod/airportheliport#CodeArrestingGearEnergyAbsorbType"/>
        <rdfs:comment xml:lang="en">MAG IV rotary hydraulic mobile arresting gear.	Used only with a hook engagement device. May be designated as &apos;CP&apos;.</rdfs:comment>
    </owl:NamedIndividual>
    


    <!-- http://www.project-best.eu/owl/aixm-mod/airportheliport#CodeArrestingGearEnergyAbsorbBaseType-MOBILROTARY_MAG_IX -->

    <owl:NamedIndividual rdf:about="http://www.project-best.eu/owl/aixm-mod/airportheliport#CodeArrestingGearEnergyAbsorbBaseType-MOBILROTARY_MAG_IX">
        <rdf:type rdf:resource="http://www.project-best.eu/owl/aixm-mod/airportheliport#CodeArrestingGearEnergyAbsorbType"/>
        <rdfs:comment xml:lang="en">MAG IX rotary hydraulic mobile arresting gear.	Used only with a net engagement device. May be designated as &apos;CU&apos;.</rdfs:comment>
    </owl:NamedIndividual>
    


    <!-- http://www.project-best.eu/owl/aixm-mod/airportheliport#CodeArrestingGearEnergyAbsorbBaseType-MOBILROTARY_MAG_VI -->

    <owl:NamedIndividual rdf:about="http://www.project-best.eu/owl/aixm-mod/airportheliport#CodeArrestingGearEnergyAbsorbBaseType-MOBILROTARY_MAG_VI">
        <rdf:type rdf:resource="http://www.project-best.eu/owl/aixm-mod/airportheliport#CodeArrestingGearEnergyAbsorbType"/>
        <rdfs:comment xml:lang="en">MAG VI rotary hydraulic mobile arresting gear.	Used only with a hook engagement device. May be designated as &apos;CR&apos;.</rdfs:comment>
    </owl:NamedIndividual>
    


    <!-- http://www.project-best.eu/owl/aixm-mod/airportheliport#CodeArrestingGearEnergyAbsorbBaseType-MOBILROTARY_MAG_VII -->

    <owl:NamedIndividual rdf:about="http://www.project-best.eu/owl/aixm-mod/airportheliport#CodeArrestingGearEnergyAbsorbBaseType-MOBILROTARY_MAG_VII">
        <rdf:type rdf:resource="http://www.project-best.eu/owl/aixm-mod/airportheliport#CodeArrestingGearEnergyAbsorbType"/>
        <rdfs:comment xml:lang="en">MAG VII rotary hydraulic mobile arresting gear.	Used only with a net engagement device. May be designated as &apos;CS&apos;.</rdfs:comment>
    </owl:NamedIndividual>
    


    <!-- http://www.project-best.eu/owl/aixm-mod/airportheliport#CodeArrestingGearEnergyAbsorbBaseType-MOBILROTARY_MAG_VIII -->

    <owl:NamedIndividual rdf:about="http://www.project-best.eu/owl/aixm-mod/airportheliport#CodeArrestingGearEnergyAbsorbBaseType-MOBILROTARY_MAG_VIII">
        <rdf:type rdf:resource="http://www.project-best.eu/owl/aixm-mod/airportheliport#CodeArrestingGearEnergyAbsorbType"/>
        <rdfs:comment xml:lang="en">MAG VIII rotary hydraulic mobile arresting gear.	Used only with a hook engagement device. May be designated as &apos;CT&apos;.</rdfs:comment>
    </owl:NamedIndividual>
    


    <!-- http://www.project-best.eu/owl/aixm-mod/airportheliport#CodeArrestingGearEnergyAbsorbBaseType-MOBILROTARY_MAG_X -->

    <owl:NamedIndividual rdf:about="http://www.project-best.eu/owl/aixm-mod/airportheliport#CodeArrestingGearEnergyAbsorbBaseType-MOBILROTARY_MAG_X">
        <rdf:type rdf:resource="http://www.project-best.eu/owl/aixm-mod/airportheliport#CodeArrestingGearEnergyAbsorbType"/>
        <rdfs:comment xml:lang="en">MAG X rotary hydraulic mobile arresting gear.	Used only with a hook engagement device. May be designated as &apos;CV&apos;.</rdfs:comment>
    </owl:NamedIndividual>
    


    <!-- http://www.project-best.eu/owl/aixm-mod/airportheliport#CodeArrestingGearEnergyAbsorbBaseType-OTHER -->

    <owl:NamedIndividual rdf:about="http://www.project-best.eu/owl/aixm-mod/airportheliport#CodeArrestingGearEnergyAbsorbBaseType-OTHER">
        <rdf:type rdf:resource="http://www.project-best.eu/owl/aixm-mod/airportheliport#CodeArrestingGearEnergyAbsorbType"/>
        <rdfs:comment xml:lang="en">Other.</rdfs:comment>
    </owl:NamedIndividual>
    


    <!-- http://www.project-best.eu/owl/aixm-mod/airportheliport#CodeArrestingGearEnergyAbsorbBaseType-RAF_PORTABLE_AGEAR -->

    <owl:NamedIndividual rdf:about="http://www.project-best.eu/owl/aixm-mod/airportheliport#CodeArrestingGearEnergyAbsorbBaseType-RAF_PORTABLE_AGEAR">
        <rdf:type rdf:resource="http://www.project-best.eu/owl/aixm-mod/airportheliport#CodeArrestingGearEnergyAbsorbType"/>
        <rdfs:comment xml:lang="en">Portable aircraft arresting gear (British).	Used only with a hook engagement device. May be designated as &apos;CW&apos;.</rdfs:comment>
    </owl:NamedIndividual>
    


    <!-- http://www.project-best.eu/owl/aixm-mod/airportheliport#CodeArrestingGearEnergyAbsorbBaseType-ROTARYTRANS_500S_8 -->

    <owl:NamedIndividual rdf:about="http://www.project-best.eu/owl/aixm-mod/airportheliport#CodeArrestingGearEnergyAbsorbBaseType-ROTARYTRANS_500S_8">
        <rdf:type rdf:resource="http://www.project-best.eu/owl/aixm-mod/airportheliport#CodeArrestingGearEnergyAbsorbType"/>
        <rdfs:comment xml:lang="en">500S-8 rotary friction brake transportable arresting gear that may carry a nameplate showing &apos;Bliss&apos;, &apos;Esco&apos;, or &apos;Gulf+Western&apos; (the &apos;G+W&apos; logo).	May be used with any type of engagement device. May be designated as &apos;AV&apos;.</rdfs:comment>
    </owl:NamedIndividual>
    


    <!-- http://www.project-best.eu/owl/aixm-mod/airportheliport#CodeArrestingGearEnergyAbsorbBaseType-ROTARY_1300 -->

    <owl:NamedIndividual rdf:about="http://www.project-best.eu/owl/aixm-mod/airportheliport#CodeArrestingGearEnergyAbsorbBaseType-ROTARY_1300">
        <rdf:type rdf:resource="http://www.project-best.eu/owl/aixm-mod/airportheliport#CodeArrestingGearEnergyAbsorbType"/>
        <rdfs:comment xml:lang="en">1300 rotary hydraulic water brake.  May be used with any type of engagement device. May be designated as &apos;BA&apos;.</rdfs:comment>
    </owl:NamedIndividual>
    


    <!-- http://www.project-best.eu/owl/aixm-mod/airportheliport#CodeArrestingGearEnergyAbsorbBaseType-ROTARY_2800 -->

    <owl:NamedIndividual rdf:about="http://www.project-best.eu/owl/aixm-mod/airportheliport#CodeArrestingGearEnergyAbsorbBaseType-ROTARY_2800">
        <rdf:type rdf:resource="http://www.project-best.eu/owl/aixm-mod/airportheliport#CodeArrestingGearEnergyAbsorbType"/>
        <rdfs:comment xml:lang="en">2800 rotary hydraulic water brake.  May be used with any type of engagement device. May be designated as &apos;BB&apos;.</rdfs:comment>
    </owl:NamedIndividual>
    


    <!-- http://www.project-best.eu/owl/aixm-mod/airportheliport#CodeArrestingGearEnergyAbsorbBaseType-ROTARY_34B_1A -->

    <owl:NamedIndividual rdf:about="http://www.project-best.eu/owl/aixm-mod/airportheliport#CodeArrestingGearEnergyAbsorbBaseType-ROTARY_34B_1A">
        <rdf:type rdf:resource="http://www.project-best.eu/owl/aixm-mod/airportheliport#CodeArrestingGearEnergyAbsorbType"/>
        <rdfs:comment xml:lang="en">34B-1A rotary hydraulic water brake.  May be used with any type of engagement device. May be designated as &apos;AA&apos;.</rdfs:comment>
    </owl:NamedIndividual>
    


    <!-- http://www.project-best.eu/owl/aixm-mod/airportheliport#CodeArrestingGearEnergyAbsorbBaseType-ROTARY_34B_1B -->

    <owl:NamedIndividual rdf:about="http://www.project-best.eu/owl/aixm-mod/airportheliport#CodeArrestingGearEnergyAbsorbBaseType-ROTARY_34B_1B">
        <rdf:type rdf:resource="http://www.project-best.eu/owl/aixm-mod/airportheliport#CodeArrestingGearEnergyAbsorbType"/>
        <rdfs:comment xml:lang="en">34B-1B rotary hydraulic water brake.  May be used with any type of engagement device. May be designated as &apos;AB&apos;.</rdfs:comment>
    </owl:NamedIndividual>
    


    <!-- http://www.project-best.eu/owl/aixm-mod/airportheliport#CodeArrestingGearEnergyAbsorbBaseType-ROTARY_34B_1C -->

    <owl:NamedIndividual rdf:about="http://www.project-best.eu/owl/aixm-mod/airportheliport#CodeArrestingGearEnergyAbsorbBaseType-ROTARY_34B_1C">
        <rdf:type rdf:resource="http://www.project-best.eu/owl/aixm-mod/airportheliport#CodeArrestingGearEnergyAbsorbType"/>
        <rdfs:comment xml:lang="en">34B-1C rotary hydraulic water brake.  May be used with any type of engagement device. May be designated as &apos;AC&apos;.</rdfs:comment>
    </owl:NamedIndividual>
    


    <!-- http://www.project-best.eu/owl/aixm-mod/airportheliport#CodeArrestingGearEnergyAbsorbBaseType-ROTARY_34D_1F -->

    <owl:NamedIndividual rdf:about="http://www.project-best.eu/owl/aixm-mod/airportheliport#CodeArrestingGearEnergyAbsorbBaseType-ROTARY_34D_1F">
        <rdf:type rdf:resource="http://www.project-best.eu/owl/aixm-mod/airportheliport#CodeArrestingGearEnergyAbsorbType"/>
        <rdfs:comment xml:lang="en">34D-1F rotary hydraulic water brake.  May be used with any type of engagement device. May be designated as &apos;AL&apos;.</rdfs:comment>
    </owl:NamedIndividual>
    


    <!-- http://www.project-best.eu/owl/aixm-mod/airportheliport#CodeArrestingGearEnergyAbsorbBaseType-ROTARY_44B_2C -->

    <owl:NamedIndividual rdf:about="http://www.project-best.eu/owl/aixm-mod/airportheliport#CodeArrestingGearEnergyAbsorbBaseType-ROTARY_44B_2C">
        <rdf:type rdf:resource="http://www.project-best.eu/owl/aixm-mod/airportheliport#CodeArrestingGearEnergyAbsorbType"/>
        <rdfs:comment xml:lang="en">44B-2C rotary hydraulic water brake.	May be used with any type of engagement device. May be designated as &apos;AD&apos;.</rdfs:comment>
    </owl:NamedIndividual>
    


    <!-- http://www.project-best.eu/owl/aixm-mod/airportheliport#CodeArrestingGearEnergyAbsorbBaseType-ROTARY_44B_2D -->

    <owl:NamedIndividual rdf:about="http://www.project-best.eu/owl/aixm-mod/airportheliport#CodeArrestingGearEnergyAbsorbBaseType-ROTARY_44B_2D">
        <rdf:type rdf:resource="http://www.project-best.eu/owl/aixm-mod/airportheliport#CodeArrestingGearEnergyAbsorbType"/>
        <rdfs:comment xml:lang="en">44B-2D rotary hydraulic water brake.	May be used with any type of engagement device. May be designated as &apos;AE&apos;.</rdfs:comment>
    </owl:NamedIndividual>
    


    <!-- http://www.project-best.eu/owl/aixm-mod/airportheliport#CodeArrestingGearEnergyAbsorbBaseType-ROTARY_44B_2E -->

    <owl:NamedIndividual rdf:about="http://www.project-best.eu/owl/aixm-mod/airportheliport#CodeArrestingGearEnergyAbsorbBaseType-ROTARY_44B_2E">
        <rdf:type rdf:resource="http://www.project-best.eu/owl/aixm-mod/airportheliport#CodeArrestingGearEnergyAbsorbType"/>
        <rdfs:comment xml:lang="en">44B-2E rotary hydraulic water brake.	May be used with any type of engagement device. May be designated as &apos;AF&apos;.</rdfs:comment>
    </owl:NamedIndividual>
    


    <!-- http://www.project-best.eu/owl/aixm-mod/airportheliport#CodeArrestingGearEnergyAbsorbBaseType-ROTARY_44B_2F -->

    <owl:NamedIndividual rdf:about="http://www.project-best.eu/owl/aixm-mod/airportheliport#CodeArrestingGearEnergyAbsorbBaseType-ROTARY_44B_2F">
        <rdf:type rdf:resource="http://www.project-best.eu/owl/aixm-mod/airportheliport#CodeArrestingGearEnergyAbsorbType"/>
        <rdfs:comment xml:lang="en">44B-2F rotary hydraulic water brake.	May be used with any type of engagement device. May be designated as &apos;AG&apos;.</rdfs:comment>
    </owl:NamedIndividual>
    


    <!-- http://www.project-best.eu/owl/aixm-mod/airportheliport#CodeArrestingGearEnergyAbsorbBaseType-ROTARY_44B_2H -->

    <owl:NamedIndividual rdf:about="http://www.project-best.eu/owl/aixm-mod/airportheliport#CodeArrestingGearEnergyAbsorbBaseType-ROTARY_44B_2H">
        <rdf:type rdf:resource="http://www.project-best.eu/owl/aixm-mod/airportheliport#CodeArrestingGearEnergyAbsorbType"/>
        <rdfs:comment xml:lang="en">44B-2H rotary hydraulic water brake.	May be used with any type of engagement device. May be designated as &apos;AH&apos;.</rdfs:comment>
    </owl:NamedIndividual>
    


    <!-- http://www.project-best.eu/owl/aixm-mod/airportheliport#CodeArrestingGearEnergyAbsorbBaseType-ROTARY_44B_2I -->

    <owl:NamedIndividual rdf:about="http://www.project-best.eu/owl/aixm-mod/airportheliport#CodeArrestingGearEnergyAbsorbBaseType-ROTARY_44B_2I">
        <rdf:type rdf:resource="http://www.project-best.eu/owl/aixm-mod/airportheliport#CodeArrestingGearEnergyAbsorbType"/>
        <rdfs:comment xml:lang="en">44B-2I rotary hydraulic water brake.	May be used with any type of engagement device. May be designated as &apos;AJ&apos;.</rdfs:comment>
    </owl:NamedIndividual>
    


    <!-- http://www.project-best.eu/owl/aixm-mod/airportheliport#CodeArrestingGearEnergyAbsorbBaseType-ROTARY_44B_2L -->

    <owl:NamedIndividual rdf:about="http://www.project-best.eu/owl/aixm-mod/airportheliport#CodeArrestingGearEnergyAbsorbBaseType-ROTARY_44B_2L">
        <rdf:type rdf:resource="http://www.project-best.eu/owl/aixm-mod/airportheliport#CodeArrestingGearEnergyAbsorbType"/>
        <rdfs:comment xml:lang="en">44B-2L rotary hydraulic water brake.	May be used with any type of engagement device. May be designated as &apos;AI&apos;.</rdfs:comment>
    </owl:NamedIndividual>
    


    <!-- http://www.project-best.eu/owl/aixm-mod/airportheliport#CodeArrestingGearEnergyAbsorbBaseType-ROTARY_44B_3A -->

    <owl:NamedIndividual rdf:about="http://www.project-best.eu/owl/aixm-mod/airportheliport#CodeArrestingGearEnergyAbsorbBaseType-ROTARY_44B_3A">
        <rdf:type rdf:resource="http://www.project-best.eu/owl/aixm-mod/airportheliport#CodeArrestingGearEnergyAbsorbType"/>
        <rdfs:comment xml:lang="en">44B-3A rotary hydraulic water brake.	May be used with any type of engagement device. May be designated as &apos;AN&apos;.</rdfs:comment>
    </owl:NamedIndividual>
    


    <!-- http://www.project-best.eu/owl/aixm-mod/airportheliport#CodeArrestingGearEnergyAbsorbBaseType-ROTARY_44B_3H -->

    <owl:NamedIndividual rdf:about="http://www.project-best.eu/owl/aixm-mod/airportheliport#CodeArrestingGearEnergyAbsorbBaseType-ROTARY_44B_3H">
        <rdf:type rdf:resource="http://www.project-best.eu/owl/aixm-mod/airportheliport#CodeArrestingGearEnergyAbsorbType"/>
        <rdfs:comment xml:lang="en">44B-3H rotary hydraulic water brake.	May be used with any type of engagement device. May be designated as &apos;AO&apos;.</rdfs:comment>
    </owl:NamedIndividual>
    


    <!-- http://www.project-best.eu/owl/aixm-mod/airportheliport#CodeArrestingGearEnergyAbsorbBaseType-ROTARY_44B_3L -->

    <owl:NamedIndividual rdf:about="http://www.project-best.eu/owl/aixm-mod/airportheliport#CodeArrestingGearEnergyAbsorbBaseType-ROTARY_44B_3L">
        <rdf:type rdf:resource="http://www.project-best.eu/owl/aixm-mod/airportheliport#CodeArrestingGearEnergyAbsorbType"/>
        <rdfs:comment xml:lang="en">44B-3L rotary hydraulic water brake.	May be used with any type of engagement device. May be designated as &apos;AK&apos;.</rdfs:comment>
    </owl:NamedIndividual>
    


    <!-- http://www.project-best.eu/owl/aixm-mod/airportheliport#CodeArrestingGearEnergyAbsorbBaseType-ROTARY_44B_4C -->

    <owl:NamedIndividual rdf:about="http://www.project-best.eu/owl/aixm-mod/airportheliport#CodeArrestingGearEnergyAbsorbBaseType-ROTARY_44B_4C">
        <rdf:type rdf:resource="http://www.project-best.eu/owl/aixm-mod/airportheliport#CodeArrestingGearEnergyAbsorbType"/>
        <rdfs:comment xml:lang="en">44B-4C rotary hydraulic water brake.	May be used with any type of engagement device. May be designated as &apos;AP&apos;.</rdfs:comment>
    </owl:NamedIndividual>
    


    <!-- http://www.project-best.eu/owl/aixm-mod/airportheliport#CodeArrestingGearEnergyAbsorbBaseType-ROTARY_44B_4E -->

    <owl:NamedIndividual rdf:about="http://www.project-best.eu/owl/aixm-mod/airportheliport#CodeArrestingGearEnergyAbsorbBaseType-ROTARY_44B_4E">
        <rdf:type rdf:resource="http://www.project-best.eu/owl/aixm-mod/airportheliport#CodeArrestingGearEnergyAbsorbType"/>
        <rdfs:comment xml:lang="en">44B-4E rotary hydraulic water brake.	May be used with any type of engagement device. May be designated as &apos;AQ&apos;.</rdfs:comment>
    </owl:NamedIndividual>
    


    <!-- http://www.project-best.eu/owl/aixm-mod/airportheliport#CodeArrestingGearEnergyAbsorbBaseType-ROTARY_44B_4H -->

    <owl:NamedIndividual rdf:about="http://www.project-best.eu/owl/aixm-mod/airportheliport#CodeArrestingGearEnergyAbsorbBaseType-ROTARY_44B_4H">
        <rdf:type rdf:resource="http://www.project-best.eu/owl/aixm-mod/airportheliport#CodeArrestingGearEnergyAbsorbType"/>
        <rdfs:comment xml:lang="en">44B-4H rotary hydraulic water brake. May be used with any type of engagement device. May be designated as &apos;AR&apos;.</rdfs:comment>
    </owl:NamedIndividual>
    


    <!-- http://www.project-best.eu/owl/aixm-mod/airportheliport#CodeArrestingGearEnergyAbsorbBaseType-ROTARY_500S -->

    <owl:NamedIndividual rdf:about="http://www.project-best.eu/owl/aixm-mod/airportheliport#CodeArrestingGearEnergyAbsorbBaseType-ROTARY_500S">
        <rdf:type rdf:resource="http://www.project-best.eu/owl/aixm-mod/airportheliport#CodeArrestingGearEnergyAbsorbType"/>
        <rdfs:comment xml:lang="en">500S rotary friction brake that may carry a nameplate showing &apos;Bliss&apos;, &apos;Esco&apos;, or &apos;Gulf+Western&apos; (the &apos;G+W&apos; logo).	May be used with any type of engagement device. May be designated as &apos;AS&apos;.</rdfs:comment>
    </owl:NamedIndividual>
    


    <!-- http://www.project-best.eu/owl/aixm-mod/airportheliport#CodeArrestingGearEnergyAbsorbBaseType-ROTARY_500S_4 -->

    <owl:NamedIndividual rdf:about="http://www.project-best.eu/owl/aixm-mod/airportheliport#CodeArrestingGearEnergyAbsorbBaseType-ROTARY_500S_4">
        <rdf:type rdf:resource="http://www.project-best.eu/owl/aixm-mod/airportheliport#CodeArrestingGearEnergyAbsorbType"/>
        <rdfs:comment xml:lang="en">500S-4 rotary friction brake that may carry a nameplate showing &apos;Bliss&apos;, &apos;Esco&apos;, or &apos;Gulf+Western&apos; (the &apos;G+W&apos; logo).	May be used with any type of engagement device. May be designated as &apos;AT&apos;.</rdfs:comment>
    </owl:NamedIndividual>
    


    <!-- http://www.project-best.eu/owl/aixm-mod/airportheliport#CodeArrestingGearEnergyAbsorbBaseType-ROTARY_500S_6 -->

    <owl:NamedIndividual rdf:about="http://www.project-best.eu/owl/aixm-mod/airportheliport#CodeArrestingGearEnergyAbsorbBaseType-ROTARY_500S_6">
        <rdf:type rdf:resource="http://www.project-best.eu/owl/aixm-mod/airportheliport#CodeArrestingGearEnergyAbsorbType"/>
        <rdfs:comment xml:lang="en">500S-6 rotary friction brake that may carry a nameplate showing &apos;Bliss&apos;, &apos;Esco&apos;, or &apos;Gulf+Western&apos; (the &apos;G+W&apos; logo).  May be used with any type of engagement device. May be designated as &apos;AU&apos;.</rdfs:comment>
    </owl:NamedIndividual>
    


    <!-- http://www.project-best.eu/owl/aixm-mod/airportheliport#CodeArrestingGearEnergyAbsorbBaseType-ROTARY_500S_8 -->

    <owl:NamedIndividual rdf:about="http://www.project-best.eu/owl/aixm-mod/airportheliport#CodeArrestingGearEnergyAbsorbBaseType-ROTARY_500S_8">
        <rdf:type rdf:resource="http://www.project-best.eu/owl/aixm-mod/airportheliport#CodeArrestingGearEnergyAbsorbType"/>
        <rdfs:comment xml:lang="en">500S-8 rotary friction brake that may carry a nameplate showing &apos;Bliss&apos;, &apos;Esco&apos;, or &apos;Gulf+Western&apos; (the &apos;G+W&apos; logo).	May be used with any type of engagement device. May be designated as &apos;AW&apos;.</rdfs:comment>
    </owl:NamedIndividual>
    


    <!-- http://www.project-best.eu/owl/aixm-mod/airportheliport#CodeArrestingGearEnergyAbsorbBaseType-ROTARY_AAE_64 -->

    <owl:NamedIndividual rdf:about="http://www.project-best.eu/owl/aixm-mod/airportheliport#CodeArrestingGearEnergyAbsorbBaseType-ROTARY_AAE_64">
        <rdf:type rdf:resource="http://www.project-best.eu/owl/aixm-mod/airportheliport#CodeArrestingGearEnergyAbsorbType"/>
        <rdfs:comment xml:lang="en">AAE-64 rotary hydraulic water brake.	May be used with any type of engagement device. May be designated as &apos;BC&apos;.</rdfs:comment>
    </owl:NamedIndividual>
    


    <!-- http://www.project-best.eu/owl/aixm-mod/airportheliport#CodeArrestingGearEnergyAbsorbBaseType-ROTARY_BAK_12A -->

    <owl:NamedIndividual rdf:about="http://www.project-best.eu/owl/aixm-mod/airportheliport#CodeArrestingGearEnergyAbsorbBaseType-ROTARY_BAK_12A">
        <rdf:type rdf:resource="http://www.project-best.eu/owl/aixm-mod/airportheliport#CodeArrestingGearEnergyAbsorbType"/>
        <rdfs:comment xml:lang="en">BAK-12A rotary friction brake (950 foot run-out; 40,000 pound capacity).	May be used with any type of engagement device. May be designated as &apos;BK&apos;.</rdfs:comment>
    </owl:NamedIndividual>
    


    <!-- http://www.project-best.eu/owl/aixm-mod/airportheliport#CodeArrestingGearEnergyAbsorbBaseType-ROTARY_BAK_12B -->

    <owl:NamedIndividual rdf:about="http://www.project-best.eu/owl/aixm-mod/airportheliport#CodeArrestingGearEnergyAbsorbBaseType-ROTARY_BAK_12B">
        <rdf:type rdf:resource="http://www.project-best.eu/owl/aixm-mod/airportheliport#CodeArrestingGearEnergyAbsorbType"/>
        <rdfs:comment xml:lang="en">BAK-12B rotary friction brake (1,200 foot run-out; 50,000 pound capacity).	May be used with any type of engagement device. May be designated as &apos;BL&apos;.</rdfs:comment>
    </owl:NamedIndividual>
    


    <!-- http://www.project-best.eu/owl/aixm-mod/airportheliport#CodeArrestingGearEnergyAbsorbBaseType-ROTARY_BAK_13 -->

    <owl:NamedIndividual rdf:about="http://www.project-best.eu/owl/aixm-mod/airportheliport#CodeArrestingGearEnergyAbsorbBaseType-ROTARY_BAK_13">
        <rdf:type rdf:resource="http://www.project-best.eu/owl/aixm-mod/airportheliport#CodeArrestingGearEnergyAbsorbType"/>
        <rdfs:comment xml:lang="en">BAK-13 rotary hydraulic water brake.	May be used with any type of engagement device. May be designated as &apos;BG&apos;.</rdfs:comment>
    </owl:NamedIndividual>
    


    <!-- http://www.project-best.eu/owl/aixm-mod/airportheliport#CodeArrestingGearEnergyAbsorbBaseType-ROTARY_BAK_9 -->

    <owl:NamedIndividual rdf:about="http://www.project-best.eu/owl/aixm-mod/airportheliport#CodeArrestingGearEnergyAbsorbBaseType-ROTARY_BAK_9">
        <rdf:type rdf:resource="http://www.project-best.eu/owl/aixm-mod/airportheliport#CodeArrestingGearEnergyAbsorbType"/>
        <rdfs:comment xml:lang="en">BAK-9 rotary friction brake.	May be used with any type of engagement device. May be designated as &apos;BE&apos;.</rdfs:comment>
    </owl:NamedIndividual>
    


    <!-- http://www.project-best.eu/owl/aixm-mod/airportheliport#CodeArrestingGearEnergyAbsorbBaseType-ROTARY_CHAIN_JETSTOP -->

    <owl:NamedIndividual rdf:about="http://www.project-best.eu/owl/aixm-mod/airportheliport#CodeArrestingGearEnergyAbsorbBaseType-ROTARY_CHAIN_JETSTOP">
        <rdf:type rdf:resource="http://www.project-best.eu/owl/aixm-mod/airportheliport#CodeArrestingGearEnergyAbsorbType"/>
        <rdfs:comment xml:lang="en">JET STOP rotary friction chain gear.	May be used with any type of engagement device. May be designated as &apos;CG&apos;.</rdfs:comment>
    </owl:NamedIndividual>
    


    <!-- http://www.project-best.eu/owl/aixm-mod/airportheliport#CodeArrestingGearEnergyAbsorbBaseType-ROTARY_DUAL_BAK_12 -->

    <owl:NamedIndividual rdf:about="http://www.project-best.eu/owl/aixm-mod/airportheliport#CodeArrestingGearEnergyAbsorbBaseType-ROTARY_DUAL_BAK_12">
        <rdf:type rdf:resource="http://www.project-best.eu/owl/aixm-mod/airportheliport#CodeArrestingGearEnergyAbsorbType"/>
        <rdfs:comment xml:lang="en">Dual BAK-12 rotary friction brake.	May be used with any type of engagement device. May be designated as &apos;BT&apos;.</rdfs:comment>
    </owl:NamedIndividual>
    


    <!-- http://www.project-best.eu/owl/aixm-mod/airportheliport#CodeArrestingGearEnergyAbsorbBaseType-ROTARY_E15 -->

    <owl:NamedIndividual rdf:about="http://www.project-best.eu/owl/aixm-mod/airportheliport#CodeArrestingGearEnergyAbsorbBaseType-ROTARY_E15">
        <rdf:type rdf:resource="http://www.project-best.eu/owl/aixm-mod/airportheliport#CodeArrestingGearEnergyAbsorbType"/>
        <rdfs:comment xml:lang="en">E15 rotary friction brake.	Used only with a hook engagement device. May be designated as &apos;CD&apos;.</rdfs:comment>
    </owl:NamedIndividual>
    


    <!-- http://www.project-best.eu/owl/aixm-mod/airportheliport#CodeArrestingGearEnergyAbsorbBaseType-ROTARY_E27 -->

    <owl:NamedIndividual rdf:about="http://www.project-best.eu/owl/aixm-mod/airportheliport#CodeArrestingGearEnergyAbsorbBaseType-ROTARY_E27">
        <rdf:type rdf:resource="http://www.project-best.eu/owl/aixm-mod/airportheliport#CodeArrestingGearEnergyAbsorbType"/>
        <rdfs:comment xml:lang="en">E27 rotary friction brake.	Used only with a hook engagement device. May be designated as &apos;CE&apos;.</rdfs:comment>
    </owl:NamedIndividual>
    


    <!-- http://www.project-best.eu/owl/aixm-mod/airportheliport#CodeArrestingGearEnergyAbsorbBaseType-ROTARY_E28 -->

    <owl:NamedIndividual rdf:about="http://www.project-best.eu/owl/aixm-mod/airportheliport#CodeArrestingGearEnergyAbsorbBaseType-ROTARY_E28">
        <rdf:type rdf:resource="http://www.project-best.eu/owl/aixm-mod/airportheliport#CodeArrestingGearEnergyAbsorbType"/>
        <rdfs:comment xml:lang="en">E28 rotary hydraulic water brake.	May be used with any type of engagement device. May be designated as &apos;CF&apos;.</rdfs:comment>
    </owl:NamedIndividual>
    


    <!-- http://www.project-best.eu/owl/aixm-mod/airportheliport#CodeArrestingGearEnergyAbsorbBaseType-ROTARY_HYDRAULIC_WATER -->

    <owl:NamedIndividual rdf:about="http://www.project-best.eu/owl/aixm-mod/airportheliport#CodeArrestingGearEnergyAbsorbBaseType-ROTARY_HYDRAULIC_WATER">
        <rdf:type rdf:resource="http://www.project-best.eu/owl/aixm-mod/airportheliport#CodeArrestingGearEnergyAbsorbType"/>
        <rdfs:comment xml:lang="en">Water rotary hydraulic arresting gear.</rdfs:comment>
    </owl:NamedIndividual>
    


    <!-- http://www.project-best.eu/owl/aixm-mod/airportheliport#CodeArrestingGearEnergyAbsorbBaseType-ROTARY_PUAG_MK_21 -->

    <owl:NamedIndividual rdf:about="http://www.project-best.eu/owl/aixm-mod/airportheliport#CodeArrestingGearEnergyAbsorbBaseType-ROTARY_PUAG_MK_21">
        <rdf:type rdf:resource="http://www.project-best.eu/owl/aixm-mod/airportheliport#CodeArrestingGearEnergyAbsorbType"/>
        <rdfs:comment xml:lang="en">PUAG MK-21 rotary hydraulic water brake.	Used only with a hook engagement device. May be designated as &apos;DA&apos;.</rdfs:comment>
    </owl:NamedIndividual>
    


    <!-- http://www.project-best.eu/owl/aixm-mod/airportheliport#CodeArrestingGearEnergyAbsorbBaseType-ROTARY_RHAG_MK_1 -->

    <owl:NamedIndividual rdf:about="http://www.project-best.eu/owl/aixm-mod/airportheliport#CodeArrestingGearEnergyAbsorbBaseType-ROTARY_RHAG_MK_1">
        <rdf:type rdf:resource="http://www.project-best.eu/owl/aixm-mod/airportheliport#CodeArrestingGearEnergyAbsorbType"/>
        <rdfs:comment xml:lang="en">RHAG MK-1 rotary hydraulic water brake.	Used only with a hook engagement device. May be designated as &apos;DI&apos;.</rdfs:comment>
    </owl:NamedIndividual>
    


    <!-- http://www.project-best.eu/owl/aixm-mod/airportheliport#CodeArrestingGearEnergyAbsorbBaseType-TEXTILE_MB_100 -->

    <owl:NamedIndividual rdf:about="http://www.project-best.eu/owl/aixm-mod/airportheliport#CodeArrestingGearEnergyAbsorbBaseType-TEXTILE_MB_100">
        <rdf:type rdf:resource="http://www.project-best.eu/owl/aixm-mod/airportheliport#CodeArrestingGearEnergyAbsorbType"/>
        <rdfs:comment xml:lang="en">MB-100 textile brake (bidirectional).	May be designated as &apos;DQ&apos;.</rdfs:comment>
    </owl:NamedIndividual>
    


    <!-- http://www.project-best.eu/owl/aixm-mod/airportheliport#CodeArrestingGearEnergyAbsorbBaseType-TEXTILE_MB_60 -->

    <owl:NamedIndividual rdf:about="http://www.project-best.eu/owl/aixm-mod/airportheliport#CodeArrestingGearEnergyAbsorbBaseType-TEXTILE_MB_60">
        <rdf:type rdf:resource="http://www.project-best.eu/owl/aixm-mod/airportheliport#CodeArrestingGearEnergyAbsorbType"/>
        <rdfs:comment xml:lang="en">MB-60 textile brake (unidirectional).	May be designated as &apos;DP&apos;.</rdfs:comment>
    </owl:NamedIndividual>
    


    <!-- http://www.project-best.eu/owl/aixm-mod/airportheliport#CodeArrestingGearEngageDeviceBaseType-61QSII -->

    <owl:NamedIndividual rdf:about="http://www.project-best.eu/owl/aixm-mod/airportheliport#CodeArrestingGearEngageDeviceBaseType-61QSII">
        <rdf:type rdf:resource="http://www.project-best.eu/owl/aixm-mod/airportheliport#CodeArrestingGearEngageDeviceType"/>
        <rdfs:comment xml:lang="en">61QSII, a barricade net system</rdfs:comment>
    </owl:NamedIndividual>
    


    <!-- http://www.project-best.eu/owl/aixm-mod/airportheliport#CodeArrestingGearEngageDeviceBaseType-62NI -->

    <owl:NamedIndividual rdf:about="http://www.project-best.eu/owl/aixm-mod/airportheliport#CodeArrestingGearEngageDeviceBaseType-62NI">
        <rdf:type rdf:resource="http://www.project-best.eu/owl/aixm-mod/airportheliport#CodeArrestingGearEngageDeviceType"/>
        <rdfs:comment xml:lang="en">62NI, a net barrier with hook cable interconnect</rdfs:comment>
    </owl:NamedIndividual>
    


    <!-- http://www.project-best.eu/owl/aixm-mod/airportheliport#CodeArrestingGearEngageDeviceBaseType-63PI -->

    <owl:NamedIndividual rdf:about="http://www.project-best.eu/owl/aixm-mod/airportheliport#CodeArrestingGearEngageDeviceBaseType-63PI">
        <rdf:type rdf:resource="http://www.project-best.eu/owl/aixm-mod/airportheliport#CodeArrestingGearEngageDeviceType"/>
        <rdfs:comment xml:lang="en">63PI, a dual cable interconnect for hook engagements</rdfs:comment>
    </owl:NamedIndividual>
    


    <!-- http://www.project-best.eu/owl/aixm-mod/airportheliport#CodeArrestingGearEngageDeviceBaseType-BAK_11_STRUT -->

    <owl:NamedIndividual rdf:about="http://www.project-best.eu/owl/aixm-mod/airportheliport#CodeArrestingGearEngageDeviceBaseType-BAK_11_STRUT">
        <rdf:type rdf:resource="http://www.project-best.eu/owl/aixm-mod/airportheliport#CodeArrestingGearEngageDeviceType"/>
        <rdfs:comment xml:lang="en">BAK-11, a main strut engaging device.</rdfs:comment>
    </owl:NamedIndividual>
    


    <!-- http://www.project-best.eu/owl/aixm-mod/airportheliport#CodeArrestingGearEngageDeviceBaseType-BAK_12 -->

    <owl:NamedIndividual rdf:about="http://www.project-best.eu/owl/aixm-mod/airportheliport#CodeArrestingGearEngageDeviceBaseType-BAK_12">
        <rdf:type rdf:resource="http://www.project-best.eu/owl/aixm-mod/airportheliport#CodeArrestingGearEngageDeviceType"/>
        <rdfs:comment xml:lang="en">BAK-12, engaging device.</rdfs:comment>
    </owl:NamedIndividual>
    


    <!-- http://www.project-best.eu/owl/aixm-mod/airportheliport#CodeArrestingGearEngageDeviceBaseType-BAK_14_HOOK -->

    <owl:NamedIndividual rdf:about="http://www.project-best.eu/owl/aixm-mod/airportheliport#CodeArrestingGearEngageDeviceBaseType-BAK_14_HOOK">
        <rdf:type rdf:resource="http://www.project-best.eu/owl/aixm-mod/airportheliport#CodeArrestingGearEngageDeviceType"/>
        <rdfs:comment xml:lang="en">BAK-14, a retractable hook cable engaging device that may be used bi-directionally.  The cable takes 5 seconds to be raised.</rdfs:comment>
    </owl:NamedIndividual>
    


    <!-- http://www.project-best.eu/owl/aixm-mod/airportheliport#CodeArrestingGearEngageDeviceBaseType-BAK_15_HOOK -->

    <owl:NamedIndividual rdf:about="http://www.project-best.eu/owl/aixm-mod/airportheliport#CodeArrestingGearEngageDeviceBaseType-BAK_15_HOOK">
        <rdf:type rdf:resource="http://www.project-best.eu/owl/aixm-mod/airportheliport#CodeArrestingGearEngageDeviceType"/>
        <rdfs:comment xml:lang="en">BAK-15 (NI), a web barrier interconnected with hook pickup cable.</rdfs:comment>
    </owl:NamedIndividual>
    


    <!-- http://www.project-best.eu/owl/aixm-mod/airportheliport#CodeArrestingGearEngageDeviceBaseType-BAK_15_STANCHION_NET -->

    <owl:NamedIndividual rdf:about="http://www.project-best.eu/owl/aixm-mod/airportheliport#CodeArrestingGearEngageDeviceBaseType-BAK_15_STANCHION_NET">
        <rdf:type rdf:resource="http://www.project-best.eu/owl/aixm-mod/airportheliport#CodeArrestingGearEngageDeviceType"/>
        <rdfs:comment xml:lang="en">BAK-15, a 61QSIIM stanchion and net barricade system.</rdfs:comment>
    </owl:NamedIndividual>
    


    <!-- http://www.project-best.eu/owl/aixm-mod/airportheliport#CodeArrestingGearEngageDeviceBaseType-EMAS -->

    <owl:NamedIndividual rdf:about="http://www.project-best.eu/owl/aixm-mod/airportheliport#CodeArrestingGearEngageDeviceBaseType-EMAS">
        <rdf:type rdf:resource="http://www.project-best.eu/owl/aixm-mod/airportheliport#CodeArrestingGearEngageDeviceType"/>
        <rdfs:comment xml:lang="en">Engineered Materials Arresting System.  High-energy-absorbing material located in the runway overrun that is designed to crush under the weight of an aircraft as the material exerts deceleration forces on the aircraft landing gear.</rdfs:comment>
    </owl:NamedIndividual>
    


    <!-- http://www.project-best.eu/owl/aixm-mod/airportheliport#CodeArrestingGearEngageDeviceBaseType-HOOK_CABLE -->

    <owl:NamedIndividual rdf:about="http://www.project-best.eu/owl/aixm-mod/airportheliport#CodeArrestingGearEngageDeviceBaseType-HOOK_CABLE">
        <rdf:type rdf:resource="http://www.project-best.eu/owl/aixm-mod/airportheliport#CodeArrestingGearEngageDeviceType"/>
        <rdfs:comment xml:lang="en">An unspecified type of hook cable (tail hook) engagement.</rdfs:comment>
    </owl:NamedIndividual>
    


    <!-- http://www.project-best.eu/owl/aixm-mod/airportheliport#CodeArrestingGearEngageDeviceBaseType-HOOK_H -->

    <owl:NamedIndividual rdf:about="http://www.project-best.eu/owl/aixm-mod/airportheliport#CodeArrestingGearEngageDeviceBaseType-HOOK_H">
        <rdf:type rdf:resource="http://www.project-best.eu/owl/aixm-mod/airportheliport#CodeArrestingGearEngageDeviceType"/>
        <rdfs:comment xml:lang="en">Type H, a retractable hook cable engaging device that may be used bi-directionally.  The cable takes 1.5 seconds to be raised.</rdfs:comment>
    </owl:NamedIndividual>
    


    <!-- http://www.project-best.eu/owl/aixm-mod/airportheliport#CodeArrestingGearEngageDeviceBaseType-HP_NET -->

    <owl:NamedIndividual rdf:about="http://www.project-best.eu/owl/aixm-mod/airportheliport#CodeArrestingGearEngageDeviceBaseType-HP_NET">
        <rdf:type rdf:resource="http://www.project-best.eu/owl/aixm-mod/airportheliport#CodeArrestingGearEngageDeviceType"/>
        <rdfs:comment xml:lang="en">HP-NET, an ADEC (brand name) high performance net.</rdfs:comment>
    </owl:NamedIndividual>
    


    <!-- http://www.project-best.eu/owl/aixm-mod/airportheliport#CodeArrestingGearEngageDeviceBaseType-JET_BARRIER -->

    <owl:NamedIndividual rdf:about="http://www.project-best.eu/owl/aixm-mod/airportheliport#CodeArrestingGearEngageDeviceBaseType-JET_BARRIER">
        <rdf:type rdf:resource="http://www.project-best.eu/owl/aixm-mod/airportheliport#CodeArrestingGearEngageDeviceType"/>
        <rdfs:comment xml:lang="en">An unspecified barrier used to stop aircraft.</rdfs:comment>
    </owl:NamedIndividual>
    


    <!-- http://www.project-best.eu/owl/aixm-mod/airportheliport#CodeArrestingGearEngageDeviceBaseType-J_BAR -->

    <owl:NamedIndividual rdf:about="http://www.project-best.eu/owl/aixm-mod/airportheliport#CodeArrestingGearEngageDeviceBaseType-J_BAR">
        <rdf:type rdf:resource="http://www.project-best.eu/owl/aixm-mod/airportheliport#CodeArrestingGearEngageDeviceType"/>
        <rdfs:comment xml:lang="en">J-BAR, a generic &apos;barrier&apos; (non-hook cable) engagements.</rdfs:comment>
    </owl:NamedIndividual>
    


    <!-- http://www.project-best.eu/owl/aixm-mod/airportheliport#CodeArrestingGearEngageDeviceBaseType-MA_1A_HOOK_CABLE -->

    <owl:NamedIndividual rdf:about="http://www.project-best.eu/owl/aixm-mod/airportheliport#CodeArrestingGearEngageDeviceBaseType-MA_1A_HOOK_CABLE">
        <rdf:type rdf:resource="http://www.project-best.eu/owl/aixm-mod/airportheliport#CodeArrestingGearEngageDeviceType"/>
        <rdfs:comment xml:lang="en">MA-1A (MOD), an MA-1A main gear cable engagement net barrier with interconnected hook cable.</rdfs:comment>
    </owl:NamedIndividual>
    


    <!-- http://www.project-best.eu/owl/aixm-mod/airportheliport#CodeArrestingGearEngageDeviceBaseType-MA_1_NET -->

    <owl:NamedIndividual rdf:about="http://www.project-best.eu/owl/aixm-mod/airportheliport#CodeArrestingGearEngageDeviceBaseType-MA_1_NET">
        <rdf:type rdf:resource="http://www.project-best.eu/owl/aixm-mod/airportheliport#CodeArrestingGearEngageDeviceType"/>
        <rdfs:comment xml:lang="en">MA-1, a main gear cable engagement net barrier (early MA-1A).</rdfs:comment>
    </owl:NamedIndividual>
    


    <!-- http://www.project-best.eu/owl/aixm-mod/airportheliport#CodeArrestingGearEngageDeviceBaseType-NET -->

    <owl:NamedIndividual rdf:about="http://www.project-best.eu/owl/aixm-mod/airportheliport#CodeArrestingGearEngageDeviceBaseType-NET">
        <rdf:type rdf:resource="http://www.project-best.eu/owl/aixm-mod/airportheliport#CodeArrestingGearEngageDeviceType"/>
        <rdfs:comment xml:lang="en">An unspecified type of net engagement.</rdfs:comment>
    </owl:NamedIndividual>
    


    <!-- http://www.project-best.eu/owl/aixm-mod/airportheliport#CodeArrestingGearEngageDeviceBaseType-NET_A30 -->

    <owl:NamedIndividual rdf:about="http://www.project-best.eu/owl/aixm-mod/airportheliport#CodeArrestingGearEngageDeviceBaseType-NET_A30">
        <rdf:type rdf:resource="http://www.project-best.eu/owl/aixm-mod/airportheliport#CodeArrestingGearEngageDeviceType"/>
        <rdfs:comment xml:lang="en">A30, an AERAZUR (manufacturer name) 30-element net (F30)</rdfs:comment>
    </owl:NamedIndividual>
    


    <!-- http://www.project-best.eu/owl/aixm-mod/airportheliport#CodeArrestingGearEngageDeviceBaseType-NET_A40 -->

    <owl:NamedIndividual rdf:about="http://www.project-best.eu/owl/aixm-mod/airportheliport#CodeArrestingGearEngageDeviceBaseType-NET_A40">
        <rdf:type rdf:resource="http://www.project-best.eu/owl/aixm-mod/airportheliport#CodeArrestingGearEngageDeviceType"/>
        <rdfs:comment xml:lang="en">A40, an AERAZUR (manufacturer name) 40-element net (F40)</rdfs:comment>
    </owl:NamedIndividual>
    


    <!-- http://www.project-best.eu/owl/aixm-mod/airportheliport#CodeArrestingGearEngageDeviceBaseType-OTHER -->

    <owl:NamedIndividual rdf:about="http://www.project-best.eu/owl/aixm-mod/airportheliport#CodeArrestingGearEngageDeviceBaseType-OTHER">
        <rdf:type rdf:resource="http://www.project-best.eu/owl/aixm-mod/airportheliport#CodeArrestingGearEngageDeviceType"/>
        <rdfs:comment xml:lang="en">Other.</rdfs:comment>
    </owl:NamedIndividual>
    


    <!-- http://www.project-best.eu/owl/aixm-mod/airportheliport#CodeAuthorityRoleBaseType-OPERATE -->

    <owl:NamedIndividual rdf:about="http://www.project-best.eu/owl/aixm-mod/airportheliport#CodeAuthorityRoleBaseType-OPERATE">
        <rdf:type rdf:resource="http://www.project-best.eu/owl/aixm-mod/airportheliport#CodeAuthorityRoleType"/>
        <rdfs:comment xml:lang="en">The OrganisationAuthority operates the feature.</rdfs:comment>
    </owl:NamedIndividual>
    


    <!-- http://www.project-best.eu/owl/aixm-mod/airportheliport#CodeAuthorityRoleBaseType-OTHER -->

    <owl:NamedIndividual rdf:about="http://www.project-best.eu/owl/aixm-mod/airportheliport#CodeAuthorityRoleBaseType-OTHER">
        <rdf:type rdf:resource="http://www.project-best.eu/owl/aixm-mod/airportheliport#CodeAuthorityRoleType"/>
        <rdfs:comment xml:lang="en">Other role.</rdfs:comment>
    </owl:NamedIndividual>
    


    <!-- http://www.project-best.eu/owl/aixm-mod/airportheliport#CodeAuthorityRoleBaseType-OWN -->

    <owl:NamedIndividual rdf:about="http://www.project-best.eu/owl/aixm-mod/airportheliport#CodeAuthorityRoleBaseType-OWN">
        <rdf:type rdf:resource="http://www.project-best.eu/owl/aixm-mod/airportheliport#CodeAuthorityRoleType"/>
        <rdfs:comment xml:lang="en">The OrganisationAuthority owns the feature.</rdfs:comment>
    </owl:NamedIndividual>
    


    <!-- http://www.project-best.eu/owl/aixm-mod/airportheliport#CodeAuthorityRoleBaseType-SUPERVISE -->

    <owl:NamedIndividual rdf:about="http://www.project-best.eu/owl/aixm-mod/airportheliport#CodeAuthorityRoleBaseType-SUPERVISE">
        <rdf:type rdf:resource="http://www.project-best.eu/owl/aixm-mod/airportheliport#CodeAuthorityRoleType"/>
        <rdfs:comment xml:lang="en">The OrganisationAuthority exercises regulatory role over the facility.</rdfs:comment>
    </owl:NamedIndividual>
    


    <!-- http://www.project-best.eu/owl/aixm-mod/airportheliport#CodeBuoyBaseType-BLACK_RED_FL2 -->

    <owl:NamedIndividual rdf:about="http://www.project-best.eu/owl/aixm-mod/airportheliport#CodeBuoyBaseType-BLACK_RED_FL2">
        <rdf:type rdf:resource="http://www.project-best.eu/owl/aixm-mod/airportheliport#CodeBuoyType"/>
        <rdfs:comment xml:lang="en">Danger - Black and red alternating horizontal stripes indicates position of isolated danger</rdfs:comment>
    </owl:NamedIndividual>
    


    <!-- http://www.project-best.eu/owl/aixm-mod/airportheliport#CodeBuoyBaseType-GREEN -->

    <owl:NamedIndividual rdf:about="http://www.project-best.eu/owl/aixm-mod/airportheliport#CodeBuoyBaseType-GREEN">
        <rdf:type rdf:resource="http://www.project-best.eu/owl/aixm-mod/airportheliport#CodeBuoyType"/>
        <rdfs:comment xml:lang="en">Lateral buoy - Marks port side of the channel when sailing toward the sea</rdfs:comment>
    </owl:NamedIndividual>
    


    <!-- http://www.project-best.eu/owl/aixm-mod/airportheliport#CodeBuoyBaseType-GREEN_RED_GFL -->

    <owl:NamedIndividual rdf:about="http://www.project-best.eu/owl/aixm-mod/airportheliport#CodeBuoyBaseType-GREEN_RED_GFL">
        <rdf:type rdf:resource="http://www.project-best.eu/owl/aixm-mod/airportheliport#CodeBuoyType"/>
        <rdfs:comment xml:lang="en">Lateral buoy - Preferred channel is to port when a red horizontal stripe is sandwiched between two green horizontal stripes</rdfs:comment>
    </owl:NamedIndividual>
    


    <!-- http://www.project-best.eu/owl/aixm-mod/airportheliport#CodeBuoyBaseType-OTHER -->

    <owl:NamedIndividual rdf:about="http://www.project-best.eu/owl/aixm-mod/airportheliport#CodeBuoyBaseType-OTHER">
        <rdf:type rdf:resource="http://www.project-best.eu/owl/aixm-mod/airportheliport#CodeBuoyType"/>
        <rdfs:comment xml:lang="en">Other</rdfs:comment>
    </owl:NamedIndividual>
    


    <!-- http://www.project-best.eu/owl/aixm-mod/airportheliport#CodeBuoyBaseType-Q3_VQ3 -->

    <owl:NamedIndividual rdf:about="http://www.project-best.eu/owl/aixm-mod/airportheliport#CodeBuoyBaseType-Q3_VQ3">
        <rdf:type rdf:resource="http://www.project-best.eu/owl/aixm-mod/airportheliport#CodeBuoyType"/>
        <rdfs:comment xml:lang="en">Cardinal buoy - Yellow stripe sandwiched between two black stripes and/or two triangles, apex on one pointing up and apex of other pointing down indicates safe water is to the east</rdfs:comment>
    </owl:NamedIndividual>
    


    <!-- http://www.project-best.eu/owl/aixm-mod/airportheliport#CodeBuoyBaseType-Q6_VQ6 -->

    <owl:NamedIndividual rdf:about="http://www.project-best.eu/owl/aixm-mod/airportheliport#CodeBuoyBaseType-Q6_VQ6">
        <rdf:type rdf:resource="http://www.project-best.eu/owl/aixm-mod/airportheliport#CodeBuoyType"/>
        <rdfs:comment xml:lang="en">Cardinal buoy - Yellow stripe is atop a black stripe and/or twp triangles, apex of both pointing down indicates safe water is to the south</rdfs:comment>
    </owl:NamedIndividual>
    


    <!-- http://www.project-best.eu/owl/aixm-mod/airportheliport#CodeBuoyBaseType-Q9_VQ9 -->

    <owl:NamedIndividual rdf:about="http://www.project-best.eu/owl/aixm-mod/airportheliport#CodeBuoyBaseType-Q9_VQ9">
        <rdf:type rdf:resource="http://www.project-best.eu/owl/aixm-mod/airportheliport#CodeBuoyType"/>
        <rdfs:comment xml:lang="en">Cardinal buoy - Black stripe sandwiched between two yellow stripes and/or two triangles apex of both point toward each other indicates safe water is to the west</rdfs:comment>
    </owl:NamedIndividual>
    


    <!-- http://www.project-best.eu/owl/aixm-mod/airportheliport#CodeBuoyBaseType-Q_VQ -->

    <owl:NamedIndividual rdf:about="http://www.project-best.eu/owl/aixm-mod/airportheliport#CodeBuoyBaseType-Q_VQ">
        <rdf:type rdf:resource="http://www.project-best.eu/owl/aixm-mod/airportheliport#CodeBuoyType"/>
        <rdfs:comment xml:lang="en">Cardinal buoy - Black stripe atop a yellow stripe and/or two triangles apex of both point up indicates safe water is to the north</rdfs:comment>
    </owl:NamedIndividual>
    


    <!-- http://www.project-best.eu/owl/aixm-mod/airportheliport#CodeBuoyBaseType-RED -->

    <owl:NamedIndividual rdf:about="http://www.project-best.eu/owl/aixm-mod/airportheliport#CodeBuoyBaseType-RED">
        <rdf:type rdf:resource="http://www.project-best.eu/owl/aixm-mod/airportheliport#CodeBuoyType"/>
        <rdfs:comment xml:lang="en">Lateral buoy - Marks port side of the channel when returning from the sea</rdfs:comment>
    </owl:NamedIndividual>
    


    <!-- http://www.project-best.eu/owl/aixm-mod/airportheliport#CodeBuoyBaseType-RED_GREEN_RFL -->

    <owl:NamedIndividual rdf:about="http://www.project-best.eu/owl/aixm-mod/airportheliport#CodeBuoyBaseType-RED_GREEN_RFL">
        <rdf:type rdf:resource="http://www.project-best.eu/owl/aixm-mod/airportheliport#CodeBuoyType"/>
        <rdfs:comment xml:lang="en">Lateral buoy - Preferred channel to starboard when a green horizontal strips is sandwiched between two red horizontal stripes</rdfs:comment>
    </owl:NamedIndividual>
    


    <!-- http://www.project-best.eu/owl/aixm-mod/airportheliport#CodeBuoyBaseType-RED_WHITE -->

    <owl:NamedIndividual rdf:about="http://www.project-best.eu/owl/aixm-mod/airportheliport#CodeBuoyBaseType-RED_WHITE">
        <rdf:type rdf:resource="http://www.project-best.eu/owl/aixm-mod/airportheliport#CodeBuoyType"/>
        <rdfs:comment xml:lang="en">Safe water buoy - Alternating red and white vertical stripes indicates safe water</rdfs:comment>
    </owl:NamedIndividual>
    


    <!-- http://www.project-best.eu/owl/aixm-mod/airportheliport#CodeBuoyBaseType-WHITE -->

    <owl:NamedIndividual rdf:about="http://www.project-best.eu/owl/aixm-mod/airportheliport#CodeBuoyBaseType-WHITE">
        <rdf:type rdf:resource="http://www.project-best.eu/owl/aixm-mod/airportheliport#CodeBuoyType"/>
        <rdfs:comment xml:lang="en">No colour is stated on the chart </rdfs:comment>
    </owl:NamedIndividual>
    


    <!-- http://www.project-best.eu/owl/aixm-mod/airportheliport#CodeBuoyBaseType-YELLOW -->

    <owl:NamedIndividual rdf:about="http://www.project-best.eu/owl/aixm-mod/airportheliport#CodeBuoyBaseType-YELLOW">
        <rdf:type rdf:resource="http://www.project-best.eu/owl/aixm-mod/airportheliport#CodeBuoyType"/>
        <rdfs:comment xml:lang="en">Special buoy - Area used by navies, pipelines, surfing </rdfs:comment>
    </owl:NamedIndividual>
    


    <!-- http://www.project-best.eu/owl/aixm-mod/airportheliport#CodeColourBaseType-AMBER -->

    <owl:NamedIndividual rdf:about="http://www.project-best.eu/owl/aixm-mod/airportheliport#CodeColourBaseType-AMBER">
        <rdf:type rdf:resource="http://www.project-best.eu/owl/aixm-mod/airportheliport#CodeColourType"/>
        <rdfs:comment xml:lang="en">amber</rdfs:comment>
    </owl:NamedIndividual>
    


    <!-- http://www.project-best.eu/owl/aixm-mod/airportheliport#CodeColourBaseType-BLACK -->

    <owl:NamedIndividual rdf:about="http://www.project-best.eu/owl/aixm-mod/airportheliport#CodeColourBaseType-BLACK">
        <rdf:type rdf:resource="http://www.project-best.eu/owl/aixm-mod/airportheliport#CodeColourType"/>
        <rdfs:comment xml:lang="en">Black</rdfs:comment>
    </owl:NamedIndividual>
    


    <!-- http://www.project-best.eu/owl/aixm-mod/airportheliport#CodeColourBaseType-BLUE -->

    <owl:NamedIndividual rdf:about="http://www.project-best.eu/owl/aixm-mod/airportheliport#CodeColourBaseType-BLUE">
        <rdf:type rdf:resource="http://www.project-best.eu/owl/aixm-mod/airportheliport#CodeColourType"/>
        <rdfs:comment xml:lang="en">Blue.</rdfs:comment>
    </owl:NamedIndividual>
    


    <!-- http://www.project-best.eu/owl/aixm-mod/airportheliport#CodeColourBaseType-BROWN -->

    <owl:NamedIndividual rdf:about="http://www.project-best.eu/owl/aixm-mod/airportheliport#CodeColourBaseType-BROWN">
        <rdf:type rdf:resource="http://www.project-best.eu/owl/aixm-mod/airportheliport#CodeColourType"/>
        <rdfs:comment xml:lang="en">Brown</rdfs:comment>
    </owl:NamedIndividual>
    


    <!-- http://www.project-best.eu/owl/aixm-mod/airportheliport#CodeColourBaseType-GREEN -->

    <owl:NamedIndividual rdf:about="http://www.project-best.eu/owl/aixm-mod/airportheliport#CodeColourBaseType-GREEN">
        <rdf:type rdf:resource="http://www.project-best.eu/owl/aixm-mod/airportheliport#CodeColourType"/>
        <rdfs:comment xml:lang="en">Green.</rdfs:comment>
    </owl:NamedIndividual>
    


    <!-- http://www.project-best.eu/owl/aixm-mod/airportheliport#CodeColourBaseType-GREY -->

    <owl:NamedIndividual rdf:about="http://www.project-best.eu/owl/aixm-mod/airportheliport#CodeColourBaseType-GREY">
        <rdf:type rdf:resource="http://www.project-best.eu/owl/aixm-mod/airportheliport#CodeColourType"/>
        <rdfs:comment xml:lang="en">Grey</rdfs:comment>
    </owl:NamedIndividual>
    


    <!-- http://www.project-best.eu/owl/aixm-mod/airportheliport#CodeColourBaseType-LIGHT_GREY -->

    <owl:NamedIndividual rdf:about="http://www.project-best.eu/owl/aixm-mod/airportheliport#CodeColourBaseType-LIGHT_GREY">
        <rdf:type rdf:resource="http://www.project-best.eu/owl/aixm-mod/airportheliport#CodeColourType"/>
        <rdfs:comment xml:lang="en">Light grey</rdfs:comment>
    </owl:NamedIndividual>
    


    <!-- http://www.project-best.eu/owl/aixm-mod/airportheliport#CodeColourBaseType-MAGENTA -->

    <owl:NamedIndividual rdf:about="http://www.project-best.eu/owl/aixm-mod/airportheliport#CodeColourBaseType-MAGENTA">
        <rdf:type rdf:resource="http://www.project-best.eu/owl/aixm-mod/airportheliport#CodeColourType"/>
        <rdfs:comment xml:lang="en">Magenta</rdfs:comment>
    </owl:NamedIndividual>
    


    <!-- http://www.project-best.eu/owl/aixm-mod/airportheliport#CodeColourBaseType-ORANGE -->

    <owl:NamedIndividual rdf:about="http://www.project-best.eu/owl/aixm-mod/airportheliport#CodeColourBaseType-ORANGE">
        <rdf:type rdf:resource="http://www.project-best.eu/owl/aixm-mod/airportheliport#CodeColourType"/>
        <rdfs:comment xml:lang="en">Orange.</rdfs:comment>
    </owl:NamedIndividual>
    


    <!-- http://www.project-best.eu/owl/aixm-mod/airportheliport#CodeColourBaseType-OTHER -->

    <owl:NamedIndividual rdf:about="http://www.project-best.eu/owl/aixm-mod/airportheliport#CodeColourBaseType-OTHER">
        <rdf:type rdf:resource="http://www.project-best.eu/owl/aixm-mod/airportheliport#CodeColourType"/>
        <rdfs:comment xml:lang="en">Other.</rdfs:comment>
    </owl:NamedIndividual>
    


    <!-- http://www.project-best.eu/owl/aixm-mod/airportheliport#CodeColourBaseType-PINK -->

    <owl:NamedIndividual rdf:about="http://www.project-best.eu/owl/aixm-mod/airportheliport#CodeColourBaseType-PINK">
        <rdf:type rdf:resource="http://www.project-best.eu/owl/aixm-mod/airportheliport#CodeColourType"/>
        <rdfs:comment xml:lang="en">Pink</rdfs:comment>
    </owl:NamedIndividual>
    


    <!-- http://www.project-best.eu/owl/aixm-mod/airportheliport#CodeColourBaseType-PURPLE -->

    <owl:NamedIndividual rdf:about="http://www.project-best.eu/owl/aixm-mod/airportheliport#CodeColourBaseType-PURPLE">
        <rdf:type rdf:resource="http://www.project-best.eu/owl/aixm-mod/airportheliport#CodeColourType"/>
        <rdfs:comment xml:lang="en">Purple.</rdfs:comment>
    </owl:NamedIndividual>
    


    <!-- http://www.project-best.eu/owl/aixm-mod/airportheliport#CodeColourBaseType-RED -->

    <owl:NamedIndividual rdf:about="http://www.project-best.eu/owl/aixm-mod/airportheliport#CodeColourBaseType-RED">
        <rdf:type rdf:resource="http://www.project-best.eu/owl/aixm-mod/airportheliport#CodeColourType"/>
        <rdfs:comment xml:lang="en">Red,</rdfs:comment>
    </owl:NamedIndividual>
    


    <!-- http://www.project-best.eu/owl/aixm-mod/airportheliport#CodeColourBaseType-VIOLET -->

    <owl:NamedIndividual rdf:about="http://www.project-best.eu/owl/aixm-mod/airportheliport#CodeColourBaseType-VIOLET">
        <rdf:type rdf:resource="http://www.project-best.eu/owl/aixm-mod/airportheliport#CodeColourType"/>
        <rdfs:comment xml:lang="en">Violet</rdfs:comment>
    </owl:NamedIndividual>
    


    <!-- http://www.project-best.eu/owl/aixm-mod/airportheliport#CodeColourBaseType-WHITE -->

    <owl:NamedIndividual rdf:about="http://www.project-best.eu/owl/aixm-mod/airportheliport#CodeColourBaseType-WHITE">
        <rdf:type rdf:resource="http://www.project-best.eu/owl/aixm-mod/airportheliport#CodeColourType"/>
        <rdfs:comment xml:lang="en">White.</rdfs:comment>
    </owl:NamedIndividual>
    


    <!-- http://www.project-best.eu/owl/aixm-mod/airportheliport#CodeColourBaseType-YELLOW -->

    <owl:NamedIndividual rdf:about="http://www.project-best.eu/owl/aixm-mod/airportheliport#CodeColourBaseType-YELLOW">
        <rdf:type rdf:resource="http://www.project-best.eu/owl/aixm-mod/airportheliport#CodeColourType"/>
        <rdfs:comment xml:lang="en">Yellow.</rdfs:comment>
    </owl:NamedIndividual>
    


    <!-- http://www.project-best.eu/owl/aixm-mod/airportheliport#CodeContaminationBaseType-ASH -->

    <owl:NamedIndividual rdf:about="http://www.project-best.eu/owl/aixm-mod/airportheliport#CodeContaminationBaseType-ASH">
        <rdf:type rdf:resource="http://www.project-best.eu/owl/aixm-mod/airportheliport#CodeContaminationType"/>
        <rdfs:comment xml:lang="en">Ash from volcanic activity.</rdfs:comment>
    </owl:NamedIndividual>
    


    <!-- http://www.project-best.eu/owl/aixm-mod/airportheliport#CodeContaminationBaseType-COMPACT_SNOW -->

    <owl:NamedIndividual rdf:about="http://www.project-best.eu/owl/aixm-mod/airportheliport#CodeContaminationBaseType-COMPACT_SNOW">
        <rdf:type rdf:resource="http://www.project-best.eu/owl/aixm-mod/airportheliport#CodeContaminationType"/>
        <rdfs:comment xml:lang="en">Snow which has been compressed</rdfs:comment>
    </owl:NamedIndividual>
    


    <!-- http://www.project-best.eu/owl/aixm-mod/airportheliport#CodeContaminationBaseType-DAMP -->

    <owl:NamedIndividual rdf:about="http://www.project-best.eu/owl/aixm-mod/airportheliport#CodeContaminationBaseType-DAMP">
        <rdf:type rdf:resource="http://www.project-best.eu/owl/aixm-mod/airportheliport#CodeContaminationType"/>
        <rdfs:comment xml:lang="en">A wee bit wet.</rdfs:comment>
    </owl:NamedIndividual>
    


    <!-- http://www.project-best.eu/owl/aixm-mod/airportheliport#CodeContaminationBaseType-DRY_SNOW -->

    <owl:NamedIndividual rdf:about="http://www.project-best.eu/owl/aixm-mod/airportheliport#CodeContaminationBaseType-DRY_SNOW">
        <rdf:type rdf:resource="http://www.project-best.eu/owl/aixm-mod/airportheliport#CodeContaminationType"/>
        <rdfs:comment xml:lang="en">Snow which can be blown if loose or, if</rdfs:comment>
    </owl:NamedIndividual>
    


    <!-- http://www.project-best.eu/owl/aixm-mod/airportheliport#CodeContaminationBaseType-FROST -->

    <owl:NamedIndividual rdf:about="http://www.project-best.eu/owl/aixm-mod/airportheliport#CodeContaminationBaseType-FROST">
        <rdf:type rdf:resource="http://www.project-best.eu/owl/aixm-mod/airportheliport#CodeContaminationType"/>
        <rdfs:comment xml:lang="en">Rime or Frost covered (depth less than 1 mm)</rdfs:comment>
    </owl:NamedIndividual>
    


    <!-- http://www.project-best.eu/owl/aixm-mod/airportheliport#CodeContaminationBaseType-GRAS -->

    <owl:NamedIndividual rdf:about="http://www.project-best.eu/owl/aixm-mod/airportheliport#CodeContaminationBaseType-GRAS">
        <rdf:type rdf:resource="http://www.project-best.eu/owl/aixm-mod/airportheliport#CodeContaminationType"/>
        <rdfs:comment xml:lang="en">Overgrown grass</rdfs:comment>
    </owl:NamedIndividual>
    


    <!-- http://www.project-best.eu/owl/aixm-mod/airportheliport#CodeContaminationBaseType-ICE -->

    <owl:NamedIndividual rdf:about="http://www.project-best.eu/owl/aixm-mod/airportheliport#CodeContaminationBaseType-ICE">
        <rdf:type rdf:resource="http://www.project-best.eu/owl/aixm-mod/airportheliport#CodeContaminationType"/>
        <rdfs:comment xml:lang="en">Ice.</rdfs:comment>
    </owl:NamedIndividual>
    


    <!-- http://www.project-best.eu/owl/aixm-mod/airportheliport#CodeContaminationBaseType-NONE -->

    <owl:NamedIndividual rdf:about="http://www.project-best.eu/owl/aixm-mod/airportheliport#CodeContaminationBaseType-NONE">
        <rdf:type rdf:resource="http://www.project-best.eu/owl/aixm-mod/airportheliport#CodeContaminationType"/>
        <rdfs:comment xml:lang="en">Clear and dry.</rdfs:comment>
    </owl:NamedIndividual>
    


    <!-- http://www.project-best.eu/owl/aixm-mod/airportheliport#CodeContaminationBaseType-OIL -->

    <owl:NamedIndividual rdf:about="http://www.project-best.eu/owl/aixm-mod/airportheliport#CodeContaminationBaseType-OIL">
        <rdf:type rdf:resource="http://www.project-best.eu/owl/aixm-mod/airportheliport#CodeContaminationType"/>
        <rdfs:comment xml:lang="en">Oil and gas.</rdfs:comment>
    </owl:NamedIndividual>
    


    <!-- http://www.project-best.eu/owl/aixm-mod/airportheliport#CodeContaminationBaseType-OTHER -->

    <owl:NamedIndividual rdf:about="http://www.project-best.eu/owl/aixm-mod/airportheliport#CodeContaminationBaseType-OTHER">
        <rdf:type rdf:resource="http://www.project-best.eu/owl/aixm-mod/airportheliport#CodeContaminationType"/>
        <rdfs:comment xml:lang="en">Other</rdfs:comment>
    </owl:NamedIndividual>
    


    <!-- http://www.project-best.eu/owl/aixm-mod/airportheliport#CodeContaminationBaseType-RUBBER -->

    <owl:NamedIndividual rdf:about="http://www.project-best.eu/owl/aixm-mod/airportheliport#CodeContaminationBaseType-RUBBER">
        <rdf:type rdf:resource="http://www.project-best.eu/owl/aixm-mod/airportheliport#CodeContaminationType"/>
        <rdfs:comment xml:lang="en">Rubber deposits.</rdfs:comment>
    </owl:NamedIndividual>
    


    <!-- http://www.project-best.eu/owl/aixm-mod/airportheliport#CodeContaminationBaseType-RUT -->

    <owl:NamedIndividual rdf:about="http://www.project-best.eu/owl/aixm-mod/airportheliport#CodeContaminationBaseType-RUT">
        <rdf:type rdf:resource="http://www.project-best.eu/owl/aixm-mod/airportheliport#CodeContaminationType"/>
        <rdfs:comment xml:lang="en">Frozen ruts or ridges.</rdfs:comment>
    </owl:NamedIndividual>
    


    <!-- http://www.project-best.eu/owl/aixm-mod/airportheliport#CodeContaminationBaseType-SAND -->

    <owl:NamedIndividual rdf:about="http://www.project-best.eu/owl/aixm-mod/airportheliport#CodeContaminationBaseType-SAND">
        <rdf:type rdf:resource="http://www.project-best.eu/owl/aixm-mod/airportheliport#CodeContaminationType"/>
        <rdfs:comment xml:lang="en">Sand.</rdfs:comment>
    </owl:NamedIndividual>
    


    <!-- http://www.project-best.eu/owl/aixm-mod/airportheliport#CodeContaminationBaseType-SLUSH -->

    <owl:NamedIndividual rdf:about="http://www.project-best.eu/owl/aixm-mod/airportheliport#CodeContaminationBaseType-SLUSH">
        <rdf:type rdf:resource="http://www.project-best.eu/owl/aixm-mod/airportheliport#CodeContaminationType"/>
        <rdfs:comment xml:lang="en">Water-saturated snow which with a heel-and-toe slapdown</rdfs:comment>
    </owl:NamedIndividual>
    


    <!-- http://www.project-best.eu/owl/aixm-mod/airportheliport#CodeContaminationBaseType-WATER -->

    <owl:NamedIndividual rdf:about="http://www.project-best.eu/owl/aixm-mod/airportheliport#CodeContaminationBaseType-WATER">
        <rdf:type rdf:resource="http://www.project-best.eu/owl/aixm-mod/airportheliport#CodeContaminationType"/>
        <rdfs:comment xml:lang="en">Wet or water patches.</rdfs:comment>
    </owl:NamedIndividual>
    


    <!-- http://www.project-best.eu/owl/aixm-mod/airportheliport#CodeContaminationBaseType-WET_SNOW -->

    <owl:NamedIndividual rdf:about="http://www.project-best.eu/owl/aixm-mod/airportheliport#CodeContaminationBaseType-WET_SNOW">
        <rdf:type rdf:resource="http://www.project-best.eu/owl/aixm-mod/airportheliport#CodeContaminationType"/>
        <rdfs:comment xml:lang="en">Snow which, if compacted by hand, will stick</rdfs:comment>
    </owl:NamedIndividual>
    


    <!-- http://www.project-best.eu/owl/aixm-mod/airportheliport#CodeDayBaseType-AFT_HOL -->

    <owl:NamedIndividual rdf:about="http://www.project-best.eu/owl/aixm-mod/airportheliport#CodeDayBaseType-AFT_HOL">
        <rdf:type rdf:resource="http://www.project-best.eu/owl/aixm-mod/airportheliport#CodeDayType"/>
        <rdfs:comment xml:lang="en">The day after a legal holiday.</rdfs:comment>
    </owl:NamedIndividual>
    


    <!-- http://www.project-best.eu/owl/aixm-mod/airportheliport#CodeDayBaseType-AFT_WORK_DAY -->

    <owl:NamedIndividual rdf:about="http://www.project-best.eu/owl/aixm-mod/airportheliport#CodeDayBaseType-AFT_WORK_DAY">
        <rdf:type rdf:resource="http://www.project-best.eu/owl/aixm-mod/airportheliport#CodeDayType"/>
        <rdfs:comment xml:lang="en">The day after a working day.</rdfs:comment>
    </owl:NamedIndividual>
    


    <!-- http://www.project-best.eu/owl/aixm-mod/airportheliport#CodeDayBaseType-ANY -->

    <owl:NamedIndividual rdf:about="http://www.project-best.eu/owl/aixm-mod/airportheliport#CodeDayBaseType-ANY">
        <rdf:type rdf:resource="http://www.project-best.eu/owl/aixm-mod/airportheliport#CodeDayType"/>
        <rdfs:comment xml:lang="en">Any day.</rdfs:comment>
    </owl:NamedIndividual>
    


    <!-- http://www.project-best.eu/owl/aixm-mod/airportheliport#CodeDayBaseType-BEF_HOL -->

    <owl:NamedIndividual rdf:about="http://www.project-best.eu/owl/aixm-mod/airportheliport#CodeDayBaseType-BEF_HOL">
        <rdf:type rdf:resource="http://www.project-best.eu/owl/aixm-mod/airportheliport#CodeDayType"/>
        <rdfs:comment xml:lang="en">The day preceding a legal holiday.</rdfs:comment>
    </owl:NamedIndividual>
    


    <!-- http://www.project-best.eu/owl/aixm-mod/airportheliport#CodeDayBaseType-BEF_WORK_DAY -->

    <owl:NamedIndividual rdf:about="http://www.project-best.eu/owl/aixm-mod/airportheliport#CodeDayBaseType-BEF_WORK_DAY">
        <rdf:type rdf:resource="http://www.project-best.eu/owl/aixm-mod/airportheliport#CodeDayType"/>
        <rdfs:comment xml:lang="en">The day preceding a working day.</rdfs:comment>
    </owl:NamedIndividual>
    


    <!-- http://www.project-best.eu/owl/aixm-mod/airportheliport#CodeDayBaseType-BUSY_FRI -->

    <owl:NamedIndividual rdf:about="http://www.project-best.eu/owl/aixm-mod/airportheliport#CodeDayBaseType-BUSY_FRI">
        <rdf:type rdf:resource="http://www.project-best.eu/owl/aixm-mod/airportheliport#CodeDayType"/>
        <rdfs:comment xml:lang="en">Formally declared as &apos;Busy Friday&apos; by the authority responsible for aeronautical information provision in the area concerned, in order to activate special traffic management arrangements.</rdfs:comment>
    </owl:NamedIndividual>
    


    <!-- http://www.project-best.eu/owl/aixm-mod/airportheliport#CodeDayBaseType-FRI -->

    <owl:NamedIndividual rdf:about="http://www.project-best.eu/owl/aixm-mod/airportheliport#CodeDayBaseType-FRI">
        <rdf:type rdf:resource="http://www.project-best.eu/owl/aixm-mod/airportheliport#CodeDayType"/>
        <rdfs:comment xml:lang="en">Friday.</rdfs:comment>
    </owl:NamedIndividual>
    


    <!-- http://www.project-best.eu/owl/aixm-mod/airportheliport#CodeDayBaseType-HOL -->

    <owl:NamedIndividual rdf:about="http://www.project-best.eu/owl/aixm-mod/airportheliport#CodeDayBaseType-HOL">
        <rdf:type rdf:resource="http://www.project-best.eu/owl/aixm-mod/airportheliport#CodeDayType"/>
        <rdfs:comment xml:lang="en">Legal Holiday.  The value does not include the weekly non-working days (for example, Saturday and Sunday in most European States).</rdfs:comment>
    </owl:NamedIndividual>
    


    <!-- http://www.project-best.eu/owl/aixm-mod/airportheliport#CodeDayBaseType-MON -->

    <owl:NamedIndividual rdf:about="http://www.project-best.eu/owl/aixm-mod/airportheliport#CodeDayBaseType-MON">
        <rdf:type rdf:resource="http://www.project-best.eu/owl/aixm-mod/airportheliport#CodeDayType"/>
        <rdfs:comment xml:lang="en">Monday.</rdfs:comment>
    </owl:NamedIndividual>
    


    <!-- http://www.project-best.eu/owl/aixm-mod/airportheliport#CodeDayBaseType-OTHER -->

    <owl:NamedIndividual rdf:about="http://www.project-best.eu/owl/aixm-mod/airportheliport#CodeDayBaseType-OTHER">
        <rdf:type rdf:resource="http://www.project-best.eu/owl/aixm-mod/airportheliport#CodeDayType"/>
        <rdfs:comment xml:lang="en">Other</rdfs:comment>
    </owl:NamedIndividual>
    


    <!-- http://www.project-best.eu/owl/aixm-mod/airportheliport#CodeDayBaseType-SAT -->

    <owl:NamedIndividual rdf:about="http://www.project-best.eu/owl/aixm-mod/airportheliport#CodeDayBaseType-SAT">
        <rdf:type rdf:resource="http://www.project-best.eu/owl/aixm-mod/airportheliport#CodeDayType"/>
        <rdfs:comment xml:lang="en">Saturday.</rdfs:comment>
    </owl:NamedIndividual>
    


    <!-- http://www.project-best.eu/owl/aixm-mod/airportheliport#CodeDayBaseType-SUN -->

    <owl:NamedIndividual rdf:about="http://www.project-best.eu/owl/aixm-mod/airportheliport#CodeDayBaseType-SUN">
        <rdf:type rdf:resource="http://www.project-best.eu/owl/aixm-mod/airportheliport#CodeDayType"/>
        <rdfs:comment xml:lang="en">Sunday.</rdfs:comment>
    </owl:NamedIndividual>
    


    <!-- http://www.project-best.eu/owl/aixm-mod/airportheliport#CodeDayBaseType-THU -->

    <owl:NamedIndividual rdf:about="http://www.project-best.eu/owl/aixm-mod/airportheliport#CodeDayBaseType-THU">
        <rdf:type rdf:resource="http://www.project-best.eu/owl/aixm-mod/airportheliport#CodeDayType"/>
        <rdfs:comment xml:lang="en">Thursday.</rdfs:comment>
    </owl:NamedIndividual>
    


    <!-- http://www.project-best.eu/owl/aixm-mod/airportheliport#CodeDayBaseType-TUE -->

    <owl:NamedIndividual rdf:about="http://www.project-best.eu/owl/aixm-mod/airportheliport#CodeDayBaseType-TUE">
        <rdf:type rdf:resource="http://www.project-best.eu/owl/aixm-mod/airportheliport#CodeDayType"/>
        <rdfs:comment xml:lang="en">Tuesday.</rdfs:comment>
    </owl:NamedIndividual>
    


    <!-- http://www.project-best.eu/owl/aixm-mod/airportheliport#CodeDayBaseType-WED -->

    <owl:NamedIndividual rdf:about="http://www.project-best.eu/owl/aixm-mod/airportheliport#CodeDayBaseType-WED">
        <rdf:type rdf:resource="http://www.project-best.eu/owl/aixm-mod/airportheliport#CodeDayType"/>
        <rdfs:comment xml:lang="en">Wednesday.</rdfs:comment>
    </owl:NamedIndividual>
    


    <!-- http://www.project-best.eu/owl/aixm-mod/airportheliport#CodeDayBaseType-WORK_DAY -->

    <owl:NamedIndividual rdf:about="http://www.project-best.eu/owl/aixm-mod/airportheliport#CodeDayBaseType-WORK_DAY">
        <rdf:type rdf:resource="http://www.project-best.eu/owl/aixm-mod/airportheliport#CodeDayType"/>
        <rdfs:comment xml:lang="en">Working Day.  This value indicates any day which is neither a Legal Holiday nor a weekly non-working day.</rdfs:comment>
    </owl:NamedIndividual>
    


    <!-- http://www.project-best.eu/owl/aixm-mod/airportheliport#CodeDeclaredDistanceBaseType-ASDA -->

    <owl:NamedIndividual rdf:about="http://www.project-best.eu/owl/aixm-mod/airportheliport#CodeDeclaredDistanceBaseType-ASDA">
        <rdf:type rdf:resource="http://www.project-best.eu/owl/aixm-mod/airportheliport#CodeDeclaredDistanceType"/>
        <rdfs:comment xml:lang="en">Accelerate-stop distance available</rdfs:comment>
    </owl:NamedIndividual>
    


    <!-- http://www.project-best.eu/owl/aixm-mod/airportheliport#CodeDeclaredDistanceBaseType-DTHR -->

    <owl:NamedIndividual rdf:about="http://www.project-best.eu/owl/aixm-mod/airportheliport#CodeDeclaredDistanceBaseType-DTHR">
        <rdf:type rdf:resource="http://www.project-best.eu/owl/aixm-mod/airportheliport#CodeDeclaredDistanceType"/>
        <rdfs:comment xml:lang="en">Threshold displacement (from the physical start of the runway direction).</rdfs:comment>
    </owl:NamedIndividual>
    


    <!-- http://www.project-best.eu/owl/aixm-mod/airportheliport#CodeDeclaredDistanceBaseType-LDA -->

    <owl:NamedIndividual rdf:about="http://www.project-best.eu/owl/aixm-mod/airportheliport#CodeDeclaredDistanceBaseType-LDA">
        <rdf:type rdf:resource="http://www.project-best.eu/owl/aixm-mod/airportheliport#CodeDeclaredDistanceType"/>
        <rdfs:comment xml:lang="en">Landing distance available</rdfs:comment>
    </owl:NamedIndividual>
    


    <!-- http://www.project-best.eu/owl/aixm-mod/airportheliport#CodeDeclaredDistanceBaseType-LDAH -->

    <owl:NamedIndividual rdf:about="http://www.project-best.eu/owl/aixm-mod/airportheliport#CodeDeclaredDistanceBaseType-LDAH">
        <rdf:type rdf:resource="http://www.project-best.eu/owl/aixm-mod/airportheliport#CodeDeclaredDistanceType"/>
        <rdfs:comment xml:lang="en">LDA for Helicopters</rdfs:comment>
    </owl:NamedIndividual>
    


    <!-- http://www.project-best.eu/owl/aixm-mod/airportheliport#CodeDeclaredDistanceBaseType-OTHER -->

    <owl:NamedIndividual rdf:about="http://www.project-best.eu/owl/aixm-mod/airportheliport#CodeDeclaredDistanceBaseType-OTHER">
        <rdf:type rdf:resource="http://www.project-best.eu/owl/aixm-mod/airportheliport#CodeDeclaredDistanceType"/>
        <rdfs:comment xml:lang="en">Other</rdfs:comment>
    </owl:NamedIndividual>
    


    <!-- http://www.project-best.eu/owl/aixm-mod/airportheliport#CodeDeclaredDistanceBaseType-RTODAH -->

    <owl:NamedIndividual rdf:about="http://www.project-best.eu/owl/aixm-mod/airportheliport#CodeDeclaredDistanceBaseType-RTODAH">
        <rdf:type rdf:resource="http://www.project-best.eu/owl/aixm-mod/airportheliport#CodeDeclaredDistanceType"/>
        <rdfs:comment xml:lang="en">Rejected TODA for Helicopters</rdfs:comment>
    </owl:NamedIndividual>
    


    <!-- http://www.project-best.eu/owl/aixm-mod/airportheliport#CodeDeclaredDistanceBaseType-TODA -->

    <owl:NamedIndividual rdf:about="http://www.project-best.eu/owl/aixm-mod/airportheliport#CodeDeclaredDistanceBaseType-TODA">
        <rdf:type rdf:resource="http://www.project-best.eu/owl/aixm-mod/airportheliport#CodeDeclaredDistanceType"/>
        <rdfs:comment xml:lang="en">Take-off distance available</rdfs:comment>
    </owl:NamedIndividual>
    


    <!-- http://www.project-best.eu/owl/aixm-mod/airportheliport#CodeDeclaredDistanceBaseType-TODAH -->

    <owl:NamedIndividual rdf:about="http://www.project-best.eu/owl/aixm-mod/airportheliport#CodeDeclaredDistanceBaseType-TODAH">
        <rdf:type rdf:resource="http://www.project-best.eu/owl/aixm-mod/airportheliport#CodeDeclaredDistanceType"/>
        <rdfs:comment xml:lang="en">Take-Off Distance Available for Helicopters</rdfs:comment>
    </owl:NamedIndividual>
    


    <!-- http://www.project-best.eu/owl/aixm-mod/airportheliport#CodeDeclaredDistanceBaseType-TORA -->

    <owl:NamedIndividual rdf:about="http://www.project-best.eu/owl/aixm-mod/airportheliport#CodeDeclaredDistanceBaseType-TORA">
        <rdf:type rdf:resource="http://www.project-best.eu/owl/aixm-mod/airportheliport#CodeDeclaredDistanceType"/>
        <rdfs:comment xml:lang="en">Take-off run available</rdfs:comment>
    </owl:NamedIndividual>
    


    <!-- http://www.project-best.eu/owl/aixm-mod/airportheliport#CodeDirectionBaseType-BACKWARD -->

    <owl:NamedIndividual rdf:about="http://www.project-best.eu/owl/aixm-mod/airportheliport#CodeDirectionBaseType-BACKWARD">
        <rdf:type rdf:resource="http://www.project-best.eu/owl/aixm-mod/airportheliport#CodeDirectionType"/>
        <rdfs:comment xml:lang="en">Backward.</rdfs:comment>
    </owl:NamedIndividual>
    


    <!-- http://www.project-best.eu/owl/aixm-mod/airportheliport#CodeDirectionBaseType-BOTH -->

    <owl:NamedIndividual rdf:about="http://www.project-best.eu/owl/aixm-mod/airportheliport#CodeDirectionBaseType-BOTH">
        <rdf:type rdf:resource="http://www.project-best.eu/owl/aixm-mod/airportheliport#CodeDirectionType"/>
        <rdfs:comment xml:lang="en">Both</rdfs:comment>
    </owl:NamedIndividual>
    


    <!-- http://www.project-best.eu/owl/aixm-mod/airportheliport#CodeDirectionBaseType-FORWARD -->

    <owl:NamedIndividual rdf:about="http://www.project-best.eu/owl/aixm-mod/airportheliport#CodeDirectionBaseType-FORWARD">
        <rdf:type rdf:resource="http://www.project-best.eu/owl/aixm-mod/airportheliport#CodeDirectionType"/>
        <rdfs:comment xml:lang="en">Forward.</rdfs:comment>
    </owl:NamedIndividual>
    


    <!-- http://www.project-best.eu/owl/aixm-mod/airportheliport#CodeDirectionBaseType-OTHER -->

    <owl:NamedIndividual rdf:about="http://www.project-best.eu/owl/aixm-mod/airportheliport#CodeDirectionBaseType-OTHER">
        <rdf:type rdf:resource="http://www.project-best.eu/owl/aixm-mod/airportheliport#CodeDirectionType"/>
        <rdfs:comment xml:lang="en">Other</rdfs:comment>
    </owl:NamedIndividual>
    


    <!-- http://www.project-best.eu/owl/aixm-mod/airportheliport#CodeDirectionTurnBaseType-EITHER -->

    <owl:NamedIndividual rdf:about="http://www.project-best.eu/owl/aixm-mod/airportheliport#CodeDirectionTurnBaseType-EITHER">
        <rdf:type rdf:resource="http://www.project-best.eu/owl/aixm-mod/airportheliport#CodeDirectionTurnType"/>
        <rdfs:comment xml:lang="en">Either left or right.</rdfs:comment>
    </owl:NamedIndividual>
    


    <!-- http://www.project-best.eu/owl/aixm-mod/airportheliport#CodeDirectionTurnBaseType-LEFT -->

    <owl:NamedIndividual rdf:about="http://www.project-best.eu/owl/aixm-mod/airportheliport#CodeDirectionTurnBaseType-LEFT">
        <rdf:type rdf:resource="http://www.project-best.eu/owl/aixm-mod/airportheliport#CodeDirectionTurnType"/>
        <rdfs:comment xml:lang="en">Left.</rdfs:comment>
    </owl:NamedIndividual>
    


    <!-- http://www.project-best.eu/owl/aixm-mod/airportheliport#CodeDirectionTurnBaseType-OTHER -->

    <owl:NamedIndividual rdf:about="http://www.project-best.eu/owl/aixm-mod/airportheliport#CodeDirectionTurnBaseType-OTHER">
        <rdf:type rdf:resource="http://www.project-best.eu/owl/aixm-mod/airportheliport#CodeDirectionTurnType"/>
        <rdfs:comment xml:lang="en">Other</rdfs:comment>
    </owl:NamedIndividual>
    


    <!-- http://www.project-best.eu/owl/aixm-mod/airportheliport#CodeDirectionTurnBaseType-RIGHT -->

    <owl:NamedIndividual rdf:about="http://www.project-best.eu/owl/aixm-mod/airportheliport#CodeDirectionTurnBaseType-RIGHT">
        <rdf:type rdf:resource="http://www.project-best.eu/owl/aixm-mod/airportheliport#CodeDirectionTurnType"/>
        <rdfs:comment xml:lang="en">Right.</rdfs:comment>
    </owl:NamedIndividual>
    


    <!-- http://www.project-best.eu/owl/aixm-mod/airportheliport#CodeFrictionDeviceBaseType-BRD -->

    <owl:NamedIndividual rdf:about="http://www.project-best.eu/owl/aixm-mod/airportheliport#CodeFrictionDeviceBaseType-BRD">
        <rdf:type rdf:resource="http://www.project-best.eu/owl/aixm-mod/airportheliport#CodeFrictionDeviceType"/>
        <rdfs:comment xml:lang="en">Brakemeter-Dynometer.</rdfs:comment>
    </owl:NamedIndividual>
    


    <!-- http://www.project-best.eu/owl/aixm-mod/airportheliport#CodeFrictionDeviceBaseType-GRT -->

    <owl:NamedIndividual rdf:about="http://www.project-best.eu/owl/aixm-mod/airportheliport#CodeFrictionDeviceBaseType-GRT">
        <rdf:type rdf:resource="http://www.project-best.eu/owl/aixm-mod/airportheliport#CodeFrictionDeviceType"/>
        <rdfs:comment xml:lang="en">Grip tester.</rdfs:comment>
    </owl:NamedIndividual>
    


    <!-- http://www.project-best.eu/owl/aixm-mod/airportheliport#CodeFrictionDeviceBaseType-MUM -->

    <owl:NamedIndividual rdf:about="http://www.project-best.eu/owl/aixm-mod/airportheliport#CodeFrictionDeviceBaseType-MUM">
        <rdf:type rdf:resource="http://www.project-best.eu/owl/aixm-mod/airportheliport#CodeFrictionDeviceType"/>
        <rdfs:comment xml:lang="en">Mu-meter.</rdfs:comment>
    </owl:NamedIndividual>
    


    <!-- http://www.project-best.eu/owl/aixm-mod/airportheliport#CodeFrictionDeviceBaseType-OTHER -->

    <owl:NamedIndividual rdf:about="http://www.project-best.eu/owl/aixm-mod/airportheliport#CodeFrictionDeviceBaseType-OTHER">
        <rdf:type rdf:resource="http://www.project-best.eu/owl/aixm-mod/airportheliport#CodeFrictionDeviceType"/>
        <rdfs:comment xml:lang="en">Other friction device.</rdfs:comment>
    </owl:NamedIndividual>
    


    <!-- http://www.project-best.eu/owl/aixm-mod/airportheliport#CodeFrictionDeviceBaseType-RFT -->

    <owl:NamedIndividual rdf:about="http://www.project-best.eu/owl/aixm-mod/airportheliport#CodeFrictionDeviceBaseType-RFT">
        <rdf:type rdf:resource="http://www.project-best.eu/owl/aixm-mod/airportheliport#CodeFrictionDeviceType"/>
        <rdfs:comment xml:lang="en">Runway friction tester.</rdfs:comment>
    </owl:NamedIndividual>
    


    <!-- http://www.project-best.eu/owl/aixm-mod/airportheliport#CodeFrictionDeviceBaseType-SFH -->

    <owl:NamedIndividual rdf:about="http://www.project-best.eu/owl/aixm-mod/airportheliport#CodeFrictionDeviceBaseType-SFH">
        <rdf:type rdf:resource="http://www.project-best.eu/owl/aixm-mod/airportheliport#CodeFrictionDeviceType"/>
        <rdfs:comment xml:lang="en">Surface friction tester (high-pressure tire).</rdfs:comment>
    </owl:NamedIndividual>
    


    <!-- http://www.project-best.eu/owl/aixm-mod/airportheliport#CodeFrictionDeviceBaseType-SFL -->

    <owl:NamedIndividual rdf:about="http://www.project-best.eu/owl/aixm-mod/airportheliport#CodeFrictionDeviceBaseType-SFL">
        <rdf:type rdf:resource="http://www.project-best.eu/owl/aixm-mod/airportheliport#CodeFrictionDeviceType"/>
        <rdfs:comment xml:lang="en">Surface friction tester (low-pressure tire).</rdfs:comment>
    </owl:NamedIndividual>
    


    <!-- http://www.project-best.eu/owl/aixm-mod/airportheliport#CodeFrictionDeviceBaseType-SKH -->

    <owl:NamedIndividual rdf:about="http://www.project-best.eu/owl/aixm-mod/airportheliport#CodeFrictionDeviceBaseType-SKH">
        <rdf:type rdf:resource="http://www.project-best.eu/owl/aixm-mod/airportheliport#CodeFrictionDeviceType"/>
        <rdfs:comment xml:lang="en">Skiddometer (high-pressure tire).</rdfs:comment>
    </owl:NamedIndividual>
    


    <!-- http://www.project-best.eu/owl/aixm-mod/airportheliport#CodeFrictionDeviceBaseType-SKL -->

    <owl:NamedIndividual rdf:about="http://www.project-best.eu/owl/aixm-mod/airportheliport#CodeFrictionDeviceBaseType-SKL">
        <rdf:type rdf:resource="http://www.project-best.eu/owl/aixm-mod/airportheliport#CodeFrictionDeviceType"/>
        <rdfs:comment xml:lang="en">Skiddometer (low-pressure tire).</rdfs:comment>
    </owl:NamedIndividual>
    


    <!-- http://www.project-best.eu/owl/aixm-mod/airportheliport#CodeFrictionDeviceBaseType-TAP -->

    <owl:NamedIndividual rdf:about="http://www.project-best.eu/owl/aixm-mod/airportheliport#CodeFrictionDeviceBaseType-TAP">
        <rdf:type rdf:resource="http://www.project-best.eu/owl/aixm-mod/airportheliport#CodeFrictionDeviceType"/>
        <rdfs:comment xml:lang="en">Tapley meter.</rdfs:comment>
    </owl:NamedIndividual>
    


    <!-- http://www.project-best.eu/owl/aixm-mod/airportheliport#CodeFrictionEstimateBaseType-GOOD -->

    <owl:NamedIndividual rdf:about="http://www.project-best.eu/owl/aixm-mod/airportheliport#CodeFrictionEstimateBaseType-GOOD">
        <rdf:type rdf:resource="http://www.project-best.eu/owl/aixm-mod/airportheliport#CodeFrictionEstimateType"/>
        <rdfs:comment xml:lang="en">Good.</rdfs:comment>
    </owl:NamedIndividual>
    


    <!-- http://www.project-best.eu/owl/aixm-mod/airportheliport#CodeFrictionEstimateBaseType-MEDIUM -->

    <owl:NamedIndividual rdf:about="http://www.project-best.eu/owl/aixm-mod/airportheliport#CodeFrictionEstimateBaseType-MEDIUM">
        <rdf:type rdf:resource="http://www.project-best.eu/owl/aixm-mod/airportheliport#CodeFrictionEstimateType"/>
        <rdfs:comment xml:lang="en">Medium.</rdfs:comment>
    </owl:NamedIndividual>
    


    <!-- http://www.project-best.eu/owl/aixm-mod/airportheliport#CodeFrictionEstimateBaseType-MEDIUM_GOOD -->

    <owl:NamedIndividual rdf:about="http://www.project-best.eu/owl/aixm-mod/airportheliport#CodeFrictionEstimateBaseType-MEDIUM_GOOD">
        <rdf:type rdf:resource="http://www.project-best.eu/owl/aixm-mod/airportheliport#CodeFrictionEstimateType"/>
        <rdfs:comment xml:lang="en">Medium to good.</rdfs:comment>
    </owl:NamedIndividual>
    


    <!-- http://www.project-best.eu/owl/aixm-mod/airportheliport#CodeFrictionEstimateBaseType-MEDIUM_POOR -->

    <owl:NamedIndividual rdf:about="http://www.project-best.eu/owl/aixm-mod/airportheliport#CodeFrictionEstimateBaseType-MEDIUM_POOR">
        <rdf:type rdf:resource="http://www.project-best.eu/owl/aixm-mod/airportheliport#CodeFrictionEstimateType"/>
        <rdfs:comment xml:lang="en">Medium to poor.</rdfs:comment>
    </owl:NamedIndividual>
    


    <!-- http://www.project-best.eu/owl/aixm-mod/airportheliport#CodeFrictionEstimateBaseType-OTHER -->

    <owl:NamedIndividual rdf:about="http://www.project-best.eu/owl/aixm-mod/airportheliport#CodeFrictionEstimateBaseType-OTHER">
        <rdf:type rdf:resource="http://www.project-best.eu/owl/aixm-mod/airportheliport#CodeFrictionEstimateType"/>
        <rdfs:comment xml:lang="en">Other</rdfs:comment>
    </owl:NamedIndividual>
    


    <!-- http://www.project-best.eu/owl/aixm-mod/airportheliport#CodeFrictionEstimateBaseType-POOR -->

    <owl:NamedIndividual rdf:about="http://www.project-best.eu/owl/aixm-mod/airportheliport#CodeFrictionEstimateBaseType-POOR">
        <rdf:type rdf:resource="http://www.project-best.eu/owl/aixm-mod/airportheliport#CodeFrictionEstimateType"/>
        <rdfs:comment xml:lang="en">Poor.</rdfs:comment>
    </owl:NamedIndividual>
    


    <!-- http://www.project-best.eu/owl/aixm-mod/airportheliport#CodeFrictionEstimateBaseType-UNRELIABLE -->

    <owl:NamedIndividual rdf:about="http://www.project-best.eu/owl/aixm-mod/airportheliport#CodeFrictionEstimateBaseType-UNRELIABLE">
        <rdf:type rdf:resource="http://www.project-best.eu/owl/aixm-mod/airportheliport#CodeFrictionEstimateType"/>
        <rdfs:comment xml:lang="en">The surface conditions or available friction measuring device do not permit a reliable surface friction measurement to be made.</rdfs:comment>
    </owl:NamedIndividual>
    


    <!-- http://www.project-best.eu/owl/aixm-mod/airportheliport#CodeGradeSeparationBaseType-OTHER -->

    <owl:NamedIndividual rdf:about="http://www.project-best.eu/owl/aixm-mod/airportheliport#CodeGradeSeparationBaseType-OTHER">
        <rdf:type rdf:resource="http://www.project-best.eu/owl/aixm-mod/airportheliport#CodeGradeSeparationType"/>
        <rdfs:comment xml:lang="en">Other.</rdfs:comment>
    </owl:NamedIndividual>
    


    <!-- http://www.project-best.eu/owl/aixm-mod/airportheliport#CodeGradeSeparationBaseType-OVERPASS -->

    <owl:NamedIndividual rdf:about="http://www.project-best.eu/owl/aixm-mod/airportheliport#CodeGradeSeparationBaseType-OVERPASS">
        <rdf:type rdf:resource="http://www.project-best.eu/owl/aixm-mod/airportheliport#CodeGradeSeparationType"/>
        <rdfs:comment xml:lang="en">The current element is on a bridge above another element.</rdfs:comment>
    </owl:NamedIndividual>
    


    <!-- http://www.project-best.eu/owl/aixm-mod/airportheliport#CodeGradeSeparationBaseType-UNDERPASS -->

    <owl:NamedIndividual rdf:about="http://www.project-best.eu/owl/aixm-mod/airportheliport#CodeGradeSeparationBaseType-UNDERPASS">
        <rdf:type rdf:resource="http://www.project-best.eu/owl/aixm-mod/airportheliport#CodeGradeSeparationType"/>
        <rdfs:comment xml:lang="en">The current element is in a tunnel below another element.</rdfs:comment>
    </owl:NamedIndividual>
    


    <!-- http://www.project-best.eu/owl/aixm-mod/airportheliport#CodeGuidanceLineBaseType-AIR_TLANE -->

    <owl:NamedIndividual rdf:about="http://www.project-best.eu/owl/aixm-mod/airportheliport#CodeGuidanceLineBaseType-AIR_TLANE">
        <rdf:type rdf:resource="http://www.project-best.eu/owl/aixm-mod/airportheliport#CodeGuidanceLineType"/>
        <rdfs:comment xml:lang="en">A virtual taxi line in the air, used by helicopters.</rdfs:comment>
    </owl:NamedIndividual>
    


    <!-- http://www.project-best.eu/owl/aixm-mod/airportheliport#CodeGuidanceLineBaseType-APRON -->

    <owl:NamedIndividual rdf:about="http://www.project-best.eu/owl/aixm-mod/airportheliport#CodeGuidanceLineBaseType-APRON">
        <rdf:type rdf:resource="http://www.project-best.eu/owl/aixm-mod/airportheliport#CodeGuidanceLineType"/>
        <rdfs:comment xml:lang="en">Taxi line on the apron surface.</rdfs:comment>
    </owl:NamedIndividual>
    


    <!-- http://www.project-best.eu/owl/aixm-mod/airportheliport#CodeGuidanceLineBaseType-GATE_TLANE -->

    <owl:NamedIndividual rdf:about="http://www.project-best.eu/owl/aixm-mod/airportheliport#CodeGuidanceLineBaseType-GATE_TLANE">
        <rdf:type rdf:resource="http://www.project-best.eu/owl/aixm-mod/airportheliport#CodeGuidanceLineType"/>
        <rdfs:comment xml:lang="en">Taxi line on the apron surface, leading to a gate/stand.</rdfs:comment>
    </owl:NamedIndividual>
    


    <!-- http://www.project-best.eu/owl/aixm-mod/airportheliport#CodeGuidanceLineBaseType-LI_TLANE -->

    <owl:NamedIndividual rdf:about="http://www.project-best.eu/owl/aixm-mod/airportheliport#CodeGuidanceLineBaseType-LI_TLANE">
        <rdf:type rdf:resource="http://www.project-best.eu/owl/aixm-mod/airportheliport#CodeGuidanceLineType"/>
        <rdfs:comment xml:lang="en">Lead-in taxi line.</rdfs:comment>
    </owl:NamedIndividual>
    


    <!-- http://www.project-best.eu/owl/aixm-mod/airportheliport#CodeGuidanceLineBaseType-LO_TLANE -->

    <owl:NamedIndividual rdf:about="http://www.project-best.eu/owl/aixm-mod/airportheliport#CodeGuidanceLineBaseType-LO_TLANE">
        <rdf:type rdf:resource="http://www.project-best.eu/owl/aixm-mod/airportheliport#CodeGuidanceLineType"/>
        <rdfs:comment xml:lang="en">Lead-out taxi line.</rdfs:comment>
    </owl:NamedIndividual>
    


    <!-- http://www.project-best.eu/owl/aixm-mod/airportheliport#CodeGuidanceLineBaseType-OTHER -->

    <owl:NamedIndividual rdf:about="http://www.project-best.eu/owl/aixm-mod/airportheliport#CodeGuidanceLineBaseType-OTHER">
        <rdf:type rdf:resource="http://www.project-best.eu/owl/aixm-mod/airportheliport#CodeGuidanceLineType"/>
        <rdfs:comment xml:lang="en">Other.</rdfs:comment>
    </owl:NamedIndividual>
    


    <!-- http://www.project-best.eu/owl/aixm-mod/airportheliport#CodeGuidanceLineBaseType-RWY -->

    <owl:NamedIndividual rdf:about="http://www.project-best.eu/owl/aixm-mod/airportheliport#CodeGuidanceLineBaseType-RWY">
        <rdf:type rdf:resource="http://www.project-best.eu/owl/aixm-mod/airportheliport#CodeGuidanceLineType"/>
        <rdfs:comment xml:lang="en">Taxi line on a runway surface, leading between the runway and other airport surfaces.</rdfs:comment>
    </owl:NamedIndividual>
    


    <!-- http://www.project-best.eu/owl/aixm-mod/airportheliport#CodeGuidanceLineBaseType-TWY -->

    <owl:NamedIndividual rdf:about="http://www.project-best.eu/owl/aixm-mod/airportheliport#CodeGuidanceLineBaseType-TWY">
        <rdf:type rdf:resource="http://www.project-best.eu/owl/aixm-mod/airportheliport#CodeGuidanceLineType"/>
        <rdfs:comment xml:lang="en">Taxi line on a taxiway surface, leading between the taxiway and other airport surfaces.</rdfs:comment>
    </owl:NamedIndividual>
    


    <!-- http://www.project-best.eu/owl/aixm-mod/airportheliport#CodeHelicopterPerformanceBaseType-1 -->

    <owl:NamedIndividual rdf:about="http://www.project-best.eu/owl/aixm-mod/airportheliport#CodeHelicopterPerformanceBaseType-1">
        <rdf:type rdf:resource="http://www.project-best.eu/owl/aixm-mod/airportheliport#CodeHelicopterPerformanceType"/>
        <rdfs:comment xml:lang="en">Helicopter class 1.</rdfs:comment>
    </owl:NamedIndividual>
    


    <!-- http://www.project-best.eu/owl/aixm-mod/airportheliport#CodeHelicopterPerformanceBaseType-2 -->

    <owl:NamedIndividual rdf:about="http://www.project-best.eu/owl/aixm-mod/airportheliport#CodeHelicopterPerformanceBaseType-2">
        <rdf:type rdf:resource="http://www.project-best.eu/owl/aixm-mod/airportheliport#CodeHelicopterPerformanceType"/>
        <rdfs:comment xml:lang="en">Helicopter class 2.</rdfs:comment>
    </owl:NamedIndividual>
    


    <!-- http://www.project-best.eu/owl/aixm-mod/airportheliport#CodeHelicopterPerformanceBaseType-3 -->

    <owl:NamedIndividual rdf:about="http://www.project-best.eu/owl/aixm-mod/airportheliport#CodeHelicopterPerformanceBaseType-3">
        <rdf:type rdf:resource="http://www.project-best.eu/owl/aixm-mod/airportheliport#CodeHelicopterPerformanceType"/>
        <rdfs:comment xml:lang="en">Helicopter class 3.</rdfs:comment>
    </owl:NamedIndividual>
    


    <!-- http://www.project-best.eu/owl/aixm-mod/airportheliport#CodeHelicopterPerformanceBaseType-OTHER -->

    <owl:NamedIndividual rdf:about="http://www.project-best.eu/owl/aixm-mod/airportheliport#CodeHelicopterPerformanceBaseType-OTHER">
        <rdf:type rdf:resource="http://www.project-best.eu/owl/aixm-mod/airportheliport#CodeHelicopterPerformanceType"/>
        <rdfs:comment xml:lang="en">Other.</rdfs:comment>
    </owl:NamedIndividual>
    


    <!-- http://www.project-best.eu/owl/aixm-mod/airportheliport#CodeHoldingCategoryBaseType-CAT_I -->

    <owl:NamedIndividual rdf:about="http://www.project-best.eu/owl/aixm-mod/airportheliport#CodeHoldingCategoryBaseType-CAT_I">
        <rdf:type rdf:resource="http://www.project-best.eu/owl/aixm-mod/airportheliport#CodeHoldingCategoryType"/>
        <rdfs:comment xml:lang="en">Precision approaches cat I.</rdfs:comment>
    </owl:NamedIndividual>
    


    <!-- http://www.project-best.eu/owl/aixm-mod/airportheliport#CodeHoldingCategoryBaseType-CAT_II_III -->

    <owl:NamedIndividual rdf:about="http://www.project-best.eu/owl/aixm-mod/airportheliport#CodeHoldingCategoryBaseType-CAT_II_III">
        <rdf:type rdf:resource="http://www.project-best.eu/owl/aixm-mod/airportheliport#CodeHoldingCategoryType"/>
        <rdfs:comment xml:lang="en">Precision approaches cat II/III.</rdfs:comment>
    </owl:NamedIndividual>
    


    <!-- http://www.project-best.eu/owl/aixm-mod/airportheliport#CodeHoldingCategoryBaseType-NON_PRECISION -->

    <owl:NamedIndividual rdf:about="http://www.project-best.eu/owl/aixm-mod/airportheliport#CodeHoldingCategoryBaseType-NON_PRECISION">
        <rdf:type rdf:resource="http://www.project-best.eu/owl/aixm-mod/airportheliport#CodeHoldingCategoryType"/>
        <rdfs:comment xml:lang="en">Non precision approaches.</rdfs:comment>
    </owl:NamedIndividual>
    


    <!-- http://www.project-best.eu/owl/aixm-mod/airportheliport#CodeHoldingCategoryBaseType-OTHER -->

    <owl:NamedIndividual rdf:about="http://www.project-best.eu/owl/aixm-mod/airportheliport#CodeHoldingCategoryBaseType-OTHER">
        <rdf:type rdf:resource="http://www.project-best.eu/owl/aixm-mod/airportheliport#CodeHoldingCategoryType"/>
        <rdfs:comment xml:lang="en">Other.</rdfs:comment>
    </owl:NamedIndividual>
    


    <!-- http://www.project-best.eu/owl/aixm-mod/airportheliport#CodeLightHoldingPositionBaseType-OTHER -->

    <owl:NamedIndividual rdf:about="http://www.project-best.eu/owl/aixm-mod/airportheliport#CodeLightHoldingPositionBaseType-OTHER">
        <rdf:type rdf:resource="http://www.project-best.eu/owl/aixm-mod/airportheliport#CodeLightHoldingPositionType"/>
        <rdfs:comment xml:lang="en">Other</rdfs:comment>
    </owl:NamedIndividual>
    


    <!-- http://www.project-best.eu/owl/aixm-mod/airportheliport#CodeLightHoldingPositionBaseType-SIGN -->

    <owl:NamedIndividual rdf:about="http://www.project-best.eu/owl/aixm-mod/airportheliport#CodeLightHoldingPositionBaseType-SIGN">
        <rdf:type rdf:resource="http://www.project-best.eu/owl/aixm-mod/airportheliport#CodeLightHoldingPositionType"/>
        <rdfs:comment xml:lang="en">Lighted sign on the side of the holding position.</rdfs:comment>
    </owl:NamedIndividual>
    


    <!-- http://www.project-best.eu/owl/aixm-mod/airportheliport#CodeLightHoldingPositionBaseType-STOP_BAR -->

    <owl:NamedIndividual rdf:about="http://www.project-best.eu/owl/aixm-mod/airportheliport#CodeLightHoldingPositionBaseType-STOP_BAR">
        <rdf:type rdf:resource="http://www.project-best.eu/owl/aixm-mod/airportheliport#CodeLightHoldingPositionType"/>
        <rdfs:comment xml:lang="en">Stop-bar (on the surface of the taxiway).</rdfs:comment>
    </owl:NamedIndividual>
    


    <!-- http://www.project-best.eu/owl/aixm-mod/airportheliport#CodeLightIntensityBaseType-LIH -->

    <owl:NamedIndividual rdf:about="http://www.project-best.eu/owl/aixm-mod/airportheliport#CodeLightIntensityBaseType-LIH">
        <rdf:type rdf:resource="http://www.project-best.eu/owl/aixm-mod/airportheliport#CodeLightIntensityType"/>
        <rdfs:comment xml:lang="en">Light intensity high.</rdfs:comment>
    </owl:NamedIndividual>
    


    <!-- http://www.project-best.eu/owl/aixm-mod/airportheliport#CodeLightIntensityBaseType-LIL -->

    <owl:NamedIndividual rdf:about="http://www.project-best.eu/owl/aixm-mod/airportheliport#CodeLightIntensityBaseType-LIL">
        <rdf:type rdf:resource="http://www.project-best.eu/owl/aixm-mod/airportheliport#CodeLightIntensityType"/>
        <rdfs:comment xml:lang="en">Light intensity low.</rdfs:comment>
    </owl:NamedIndividual>
    


    <!-- http://www.project-best.eu/owl/aixm-mod/airportheliport#CodeLightIntensityBaseType-LIL_LIH -->

    <owl:NamedIndividual rdf:about="http://www.project-best.eu/owl/aixm-mod/airportheliport#CodeLightIntensityBaseType-LIL_LIH">
        <rdf:type rdf:resource="http://www.project-best.eu/owl/aixm-mod/airportheliport#CodeLightIntensityType"/>
        <rdfs:comment xml:lang="en">Low intensity for night use; high intensity for day use, as determined by a photo-cell.</rdfs:comment>
    </owl:NamedIndividual>
    


    <!-- http://www.project-best.eu/owl/aixm-mod/airportheliport#CodeLightIntensityBaseType-LIM -->

    <owl:NamedIndividual rdf:about="http://www.project-best.eu/owl/aixm-mod/airportheliport#CodeLightIntensityBaseType-LIM">
        <rdf:type rdf:resource="http://www.project-best.eu/owl/aixm-mod/airportheliport#CodeLightIntensityType"/>
        <rdfs:comment xml:lang="en">Light intensity medium.</rdfs:comment>
    </owl:NamedIndividual>
    


    <!-- http://www.project-best.eu/owl/aixm-mod/airportheliport#CodeLightIntensityBaseType-OTHER -->

    <owl:NamedIndividual rdf:about="http://www.project-best.eu/owl/aixm-mod/airportheliport#CodeLightIntensityBaseType-OTHER">
        <rdf:type rdf:resource="http://www.project-best.eu/owl/aixm-mod/airportheliport#CodeLightIntensityType"/>
        <rdfs:comment xml:lang="en">Other.</rdfs:comment>
    </owl:NamedIndividual>
    


    <!-- http://www.project-best.eu/owl/aixm-mod/airportheliport#CodeLightIntensityBaseType-PREDETERMINED -->

    <owl:NamedIndividual rdf:about="http://www.project-best.eu/owl/aixm-mod/airportheliport#CodeLightIntensityBaseType-PREDETERMINED">
        <rdf:type rdf:resource="http://www.project-best.eu/owl/aixm-mod/airportheliport#CodeLightIntensityType"/>
        <rdfs:comment xml:lang="en">A predetermined intensity step, in the approach lighting system that takes precedence for air-to-ground radio control over the runway lighting system which is set, based on expected visibility conditions.</rdfs:comment>
    </owl:NamedIndividual>
    


    <!-- http://www.project-best.eu/owl/aixm-mod/airportheliport#CodeLightSourceBaseType-FLOOD -->

    <owl:NamedIndividual rdf:about="http://www.project-best.eu/owl/aixm-mod/airportheliport#CodeLightSourceBaseType-FLOOD">
        <rdf:type rdf:resource="http://www.project-best.eu/owl/aixm-mod/airportheliport#CodeLightSourceType"/>
        <rdfs:comment xml:lang="en">Flood light.</rdfs:comment>
    </owl:NamedIndividual>
    


    <!-- http://www.project-best.eu/owl/aixm-mod/airportheliport#CodeLightSourceBaseType-OTHER -->

    <owl:NamedIndividual rdf:about="http://www.project-best.eu/owl/aixm-mod/airportheliport#CodeLightSourceBaseType-OTHER">
        <rdf:type rdf:resource="http://www.project-best.eu/owl/aixm-mod/airportheliport#CodeLightSourceType"/>
        <rdfs:comment xml:lang="en">Another type of light source.</rdfs:comment>
    </owl:NamedIndividual>
    


    <!-- http://www.project-best.eu/owl/aixm-mod/airportheliport#CodeLightSourceBaseType-STROBE -->

    <owl:NamedIndividual rdf:about="http://www.project-best.eu/owl/aixm-mod/airportheliport#CodeLightSourceBaseType-STROBE">
        <rdf:type rdf:resource="http://www.project-best.eu/owl/aixm-mod/airportheliport#CodeLightSourceType"/>
        <rdfs:comment xml:lang="en">Strobe light.</rdfs:comment>
    </owl:NamedIndividual>
    


    <!-- http://www.project-best.eu/owl/aixm-mod/airportheliport#CodeLightingJARBaseType-BALS -->

    <owl:NamedIndividual rdf:about="http://www.project-best.eu/owl/aixm-mod/airportheliport#CodeLightingJARBaseType-BALS">
        <rdf:type rdf:resource="http://www.project-best.eu/owl/aixm-mod/airportheliport#CodeLightingJARType"/>
        <rdfs:comment xml:lang="en">Basic approach light facilities; comprise runway markings, less than 420 m of high/medium intensity approach lights (or any length of low intensity approach lights), runway edge lights, threshold lights and runway end lights. </rdfs:comment>
    </owl:NamedIndividual>
    


    <!-- http://www.project-best.eu/owl/aixm-mod/airportheliport#CodeLightingJARBaseType-FALS -->

    <owl:NamedIndividual rdf:about="http://www.project-best.eu/owl/aixm-mod/airportheliport#CodeLightingJARBaseType-FALS">
        <rdf:type rdf:resource="http://www.project-best.eu/owl/aixm-mod/airportheliport#CodeLightingJARType"/>
        <rdfs:comment xml:lang="en">Full approach light facilities; comprise runway markings, 720 m or more of high/medium intensity approach lights, runway edge lights, threshold lights and runway end lights. </rdfs:comment>
    </owl:NamedIndividual>
    


    <!-- http://www.project-best.eu/owl/aixm-mod/airportheliport#CodeLightingJARBaseType-IALS -->

    <owl:NamedIndividual rdf:about="http://www.project-best.eu/owl/aixm-mod/airportheliport#CodeLightingJARBaseType-IALS">
        <rdf:type rdf:resource="http://www.project-best.eu/owl/aixm-mod/airportheliport#CodeLightingJARType"/>
        <rdfs:comment xml:lang="en">Intermediate approach light facilities; comprise runway markings, 420 to 720 m of high/medium intensity approach lights, runway edge lights, threshold lights and runway end lights. </rdfs:comment>
    </owl:NamedIndividual>
    


    <!-- http://www.project-best.eu/owl/aixm-mod/airportheliport#CodeLightingJARBaseType-NALS -->

    <owl:NamedIndividual rdf:about="http://www.project-best.eu/owl/aixm-mod/airportheliport#CodeLightingJARBaseType-NALS">
        <rdf:type rdf:resource="http://www.project-best.eu/owl/aixm-mod/airportheliport#CodeLightingJARType"/>
        <rdfs:comment xml:lang="en">None or insufficient approach light facilities; comprise runway markings, runway edge lights, threshold lights, runway end lights or no lights at all.</rdfs:comment>
    </owl:NamedIndividual>
    


    <!-- http://www.project-best.eu/owl/aixm-mod/airportheliport#CodeLightingJARBaseType-OTHER -->

    <owl:NamedIndividual rdf:about="http://www.project-best.eu/owl/aixm-mod/airportheliport#CodeLightingJARBaseType-OTHER">
        <rdf:type rdf:resource="http://www.project-best.eu/owl/aixm-mod/airportheliport#CodeLightingJARType"/>
        <rdfs:comment xml:lang="en">Other</rdfs:comment>
    </owl:NamedIndividual>
    


    <!-- http://www.project-best.eu/owl/aixm-mod/airportheliport#CodeLoadingBridgeBaseType-ARM -->

    <owl:NamedIndividual rdf:about="http://www.project-best.eu/owl/aixm-mod/airportheliport#CodeLoadingBridgeBaseType-ARM">
        <rdf:type rdf:resource="http://www.project-best.eu/owl/aixm-mod/airportheliport#CodeLoadingBridgeType"/>
        <rdfs:comment xml:lang="en">Arm</rdfs:comment>
    </owl:NamedIndividual>
    


    <!-- http://www.project-best.eu/owl/aixm-mod/airportheliport#CodeLoadingBridgeBaseType-MOVABLE_ARM -->

    <owl:NamedIndividual rdf:about="http://www.project-best.eu/owl/aixm-mod/airportheliport#CodeLoadingBridgeBaseType-MOVABLE_ARM">
        <rdf:type rdf:resource="http://www.project-best.eu/owl/aixm-mod/airportheliport#CodeLoadingBridgeType"/>
        <rdfs:comment xml:lang="en">Movable arm</rdfs:comment>
    </owl:NamedIndividual>
    


    <!-- http://www.project-best.eu/owl/aixm-mod/airportheliport#CodeLoadingBridgeBaseType-OTHER -->

    <owl:NamedIndividual rdf:about="http://www.project-best.eu/owl/aixm-mod/airportheliport#CodeLoadingBridgeBaseType-OTHER">
        <rdf:type rdf:resource="http://www.project-best.eu/owl/aixm-mod/airportheliport#CodeLoadingBridgeType"/>
        <rdfs:comment xml:lang="en">Other</rdfs:comment>
    </owl:NamedIndividual>
    


    <!-- http://www.project-best.eu/owl/aixm-mod/airportheliport#CodeLoadingBridgeBaseType-PORTABLE_RAMP -->

    <owl:NamedIndividual rdf:about="http://www.project-best.eu/owl/aixm-mod/airportheliport#CodeLoadingBridgeBaseType-PORTABLE_RAMP">
        <rdf:type rdf:resource="http://www.project-best.eu/owl/aixm-mod/airportheliport#CodeLoadingBridgeType"/>
        <rdfs:comment xml:lang="en">Portable ramp</rdfs:comment>
    </owl:NamedIndividual>
    


    <!-- http://www.project-best.eu/owl/aixm-mod/airportheliport#CodeLoadingBridgeBaseType-PORTABLE_STAIRS -->

    <owl:NamedIndividual rdf:about="http://www.project-best.eu/owl/aixm-mod/airportheliport#CodeLoadingBridgeBaseType-PORTABLE_STAIRS">
        <rdf:type rdf:resource="http://www.project-best.eu/owl/aixm-mod/airportheliport#CodeLoadingBridgeType"/>
        <rdfs:comment xml:lang="en">Portable stairs</rdfs:comment>
    </owl:NamedIndividual>
    


    <!-- http://www.project-best.eu/owl/aixm-mod/airportheliport#CodeLogicalOperatorBaseType-AND -->

    <owl:NamedIndividual rdf:about="http://www.project-best.eu/owl/aixm-mod/airportheliport#CodeLogicalOperatorBaseType-AND">
        <rdf:type rdf:resource="http://www.project-best.eu/owl/aixm-mod/airportheliport#CodeLogicalOperatorType"/>
        <rdfs:comment xml:lang="en">The result is true only when all operands are true.</rdfs:comment>
    </owl:NamedIndividual>
    


    <!-- http://www.project-best.eu/owl/aixm-mod/airportheliport#CodeLogicalOperatorBaseType-NONE -->

    <owl:NamedIndividual rdf:about="http://www.project-best.eu/owl/aixm-mod/airportheliport#CodeLogicalOperatorBaseType-NONE">
        <rdf:type rdf:resource="http://www.project-best.eu/owl/aixm-mod/airportheliport#CodeLogicalOperatorType"/>
        <rdfs:comment xml:lang="en">No operation (used for single conditions).</rdfs:comment>
    </owl:NamedIndividual>
    


    <!-- http://www.project-best.eu/owl/aixm-mod/airportheliport#CodeLogicalOperatorBaseType-NOT -->

    <owl:NamedIndividual rdf:about="http://www.project-best.eu/owl/aixm-mod/airportheliport#CodeLogicalOperatorBaseType-NOT">
        <rdf:type rdf:resource="http://www.project-best.eu/owl/aixm-mod/airportheliport#CodeLogicalOperatorType"/>
        <rdfs:comment xml:lang="en">The result is the opposite of the operands true/false state (it applies to a single operand).</rdfs:comment>
    </owl:NamedIndividual>
    


    <!-- http://www.project-best.eu/owl/aixm-mod/airportheliport#CodeLogicalOperatorBaseType-OR -->

    <owl:NamedIndividual rdf:about="http://www.project-best.eu/owl/aixm-mod/airportheliport#CodeLogicalOperatorBaseType-OR">
        <rdf:type rdf:resource="http://www.project-best.eu/owl/aixm-mod/airportheliport#CodeLogicalOperatorType"/>
        <rdfs:comment xml:lang="en">The result is true if any operand is true.</rdfs:comment>
    </owl:NamedIndividual>
    


    <!-- http://www.project-best.eu/owl/aixm-mod/airportheliport#CodeLogicalOperatorBaseType-OTHER -->

    <owl:NamedIndividual rdf:about="http://www.project-best.eu/owl/aixm-mod/airportheliport#CodeLogicalOperatorBaseType-OTHER">
        <rdf:type rdf:resource="http://www.project-best.eu/owl/aixm-mod/airportheliport#CodeLogicalOperatorType"/>
        <rdfs:comment xml:lang="en">Other</rdfs:comment>
    </owl:NamedIndividual>
    


    <!-- http://www.project-best.eu/owl/aixm-mod/airportheliport#CodeMarkingConditionBaseType-EXCELLENT -->

    <owl:NamedIndividual rdf:about="http://www.project-best.eu/owl/aixm-mod/airportheliport#CodeMarkingConditionBaseType-EXCELLENT">
        <rdf:type rdf:resource="http://www.project-best.eu/owl/aixm-mod/airportheliport#CodeMarkingConditionType"/>
        <rdfs:comment xml:lang="en">Marking is in perfect condition.</rdfs:comment>
    </owl:NamedIndividual>
    


    <!-- http://www.project-best.eu/owl/aixm-mod/airportheliport#CodeMarkingConditionBaseType-FAIR -->

    <owl:NamedIndividual rdf:about="http://www.project-best.eu/owl/aixm-mod/airportheliport#CodeMarkingConditionBaseType-FAIR">
        <rdf:type rdf:resource="http://www.project-best.eu/owl/aixm-mod/airportheliport#CodeMarkingConditionType"/>
        <rdfs:comment xml:lang="en">Marking is in fair condition.</rdfs:comment>
    </owl:NamedIndividual>
    


    <!-- http://www.project-best.eu/owl/aixm-mod/airportheliport#CodeMarkingConditionBaseType-GOOD -->

    <owl:NamedIndividual rdf:about="http://www.project-best.eu/owl/aixm-mod/airportheliport#CodeMarkingConditionBaseType-GOOD">
        <rdf:type rdf:resource="http://www.project-best.eu/owl/aixm-mod/airportheliport#CodeMarkingConditionType"/>
        <rdfs:comment xml:lang="en">Marking is in good condition.</rdfs:comment>
    </owl:NamedIndividual>
    


    <!-- http://www.project-best.eu/owl/aixm-mod/airportheliport#CodeMarkingConditionBaseType-OTHER -->

    <owl:NamedIndividual rdf:about="http://www.project-best.eu/owl/aixm-mod/airportheliport#CodeMarkingConditionBaseType-OTHER">
        <rdf:type rdf:resource="http://www.project-best.eu/owl/aixm-mod/airportheliport#CodeMarkingConditionType"/>
        <rdfs:comment xml:lang="en">Other.</rdfs:comment>
    </owl:NamedIndividual>
    


    <!-- http://www.project-best.eu/owl/aixm-mod/airportheliport#CodeMarkingConditionBaseType-POOR -->

    <owl:NamedIndividual rdf:about="http://www.project-best.eu/owl/aixm-mod/airportheliport#CodeMarkingConditionBaseType-POOR">
        <rdf:type rdf:resource="http://www.project-best.eu/owl/aixm-mod/airportheliport#CodeMarkingConditionType"/>
        <rdfs:comment xml:lang="en">Marking is in poor condition.</rdfs:comment>
    </owl:NamedIndividual>
    


    <!-- http://www.project-best.eu/owl/aixm-mod/airportheliport#CodeMarkingStyleBaseType-DASHED -->

    <owl:NamedIndividual rdf:about="http://www.project-best.eu/owl/aixm-mod/airportheliport#CodeMarkingStyleBaseType-DASHED">
        <rdf:type rdf:resource="http://www.project-best.eu/owl/aixm-mod/airportheliport#CodeMarkingStyleType"/>
        <rdfs:comment xml:lang="en">Dashed line.</rdfs:comment>
    </owl:NamedIndividual>
    


    <!-- http://www.project-best.eu/owl/aixm-mod/airportheliport#CodeMarkingStyleBaseType-DOTTED -->

    <owl:NamedIndividual rdf:about="http://www.project-best.eu/owl/aixm-mod/airportheliport#CodeMarkingStyleBaseType-DOTTED">
        <rdf:type rdf:resource="http://www.project-best.eu/owl/aixm-mod/airportheliport#CodeMarkingStyleType"/>
        <rdfs:comment xml:lang="en">Dotted line.</rdfs:comment>
    </owl:NamedIndividual>
    


    <!-- http://www.project-best.eu/owl/aixm-mod/airportheliport#CodeMarkingStyleBaseType-OTHER -->

    <owl:NamedIndividual rdf:about="http://www.project-best.eu/owl/aixm-mod/airportheliport#CodeMarkingStyleBaseType-OTHER">
        <rdf:type rdf:resource="http://www.project-best.eu/owl/aixm-mod/airportheliport#CodeMarkingStyleType"/>
        <rdfs:comment xml:lang="en">Other</rdfs:comment>
    </owl:NamedIndividual>
    


    <!-- http://www.project-best.eu/owl/aixm-mod/airportheliport#CodeMarkingStyleBaseType-SOLID -->

    <owl:NamedIndividual rdf:about="http://www.project-best.eu/owl/aixm-mod/airportheliport#CodeMarkingStyleBaseType-SOLID">
        <rdf:type rdf:resource="http://www.project-best.eu/owl/aixm-mod/airportheliport#CodeMarkingStyleType"/>
        <rdfs:comment xml:lang="en">solid line.</rdfs:comment>
    </owl:NamedIndividual>
    


    <!-- http://www.project-best.eu/owl/aixm-mod/airportheliport#CodeMeteoConditionsBaseType-ALL -->

    <owl:NamedIndividual rdf:about="http://www.project-best.eu/owl/aixm-mod/airportheliport#CodeMeteoConditionsBaseType-ALL">
        <rdf:type rdf:resource="http://www.project-best.eu/owl/aixm-mod/airportheliport#CodeMeteoConditionsType"/>
        <rdfs:comment xml:lang="en">Both IMC and VMC.</rdfs:comment>
    </owl:NamedIndividual>
    


    <!-- http://www.project-best.eu/owl/aixm-mod/airportheliport#CodeMeteoConditionsBaseType-IMC -->

    <owl:NamedIndividual rdf:about="http://www.project-best.eu/owl/aixm-mod/airportheliport#CodeMeteoConditionsBaseType-IMC">
        <rdf:type rdf:resource="http://www.project-best.eu/owl/aixm-mod/airportheliport#CodeMeteoConditionsType"/>
        <rdfs:comment xml:lang="en">[Instrument Meteorological Conditions] Weather conditions that normally require pilots to fly primarily by reference to instruments, and therefore under Instrument Flight Rules (IFR).</rdfs:comment>
    </owl:NamedIndividual>
    


    <!-- http://www.project-best.eu/owl/aixm-mod/airportheliport#CodeMeteoConditionsBaseType-OTHER -->

    <owl:NamedIndividual rdf:about="http://www.project-best.eu/owl/aixm-mod/airportheliport#CodeMeteoConditionsBaseType-OTHER">
        <rdf:type rdf:resource="http://www.project-best.eu/owl/aixm-mod/airportheliport#CodeMeteoConditionsType"/>
        <rdfs:comment xml:lang="en">Other</rdfs:comment>
    </owl:NamedIndividual>
    


    <!-- http://www.project-best.eu/owl/aixm-mod/airportheliport#CodeMeteoConditionsBaseType-VMC -->

    <owl:NamedIndividual rdf:about="http://www.project-best.eu/owl/aixm-mod/airportheliport#CodeMeteoConditionsBaseType-VMC">
        <rdf:type rdf:resource="http://www.project-best.eu/owl/aixm-mod/airportheliport#CodeMeteoConditionsType"/>
        <rdfs:comment xml:lang="en">[Visual Meteorological Conditions] Weather conditions in which visual flight rules (VFR) flight is permitted. That is, conditions in which pilots have sufficient visibility to fly the aircraft maintaining visual separation from terrain and other aircraft.</rdfs:comment>
    </owl:NamedIndividual>
    


    <!-- http://www.project-best.eu/owl/aixm-mod/airportheliport#CodeMilitaryOperationsBaseType-CIVIL -->

    <owl:NamedIndividual rdf:about="http://www.project-best.eu/owl/aixm-mod/airportheliport#CodeMilitaryOperationsBaseType-CIVIL">
        <rdf:type rdf:resource="http://www.project-best.eu/owl/aixm-mod/airportheliport#CodeMilitaryOperationsType"/>
        <rdfs:comment xml:lang="en">Only Civil Air traffic is concerned.</rdfs:comment>
    </owl:NamedIndividual>
    


    <!-- http://www.project-best.eu/owl/aixm-mod/airportheliport#CodeMilitaryOperationsBaseType-JOINT -->

    <owl:NamedIndividual rdf:about="http://www.project-best.eu/owl/aixm-mod/airportheliport#CodeMilitaryOperationsBaseType-JOINT">
        <rdf:type rdf:resource="http://www.project-best.eu/owl/aixm-mod/airportheliport#CodeMilitaryOperationsType"/>
        <rdfs:comment xml:lang="en">Both Civil and Military air traffic are concerned.</rdfs:comment>
    </owl:NamedIndividual>
    


    <!-- http://www.project-best.eu/owl/aixm-mod/airportheliport#CodeMilitaryOperationsBaseType-MIL -->

    <owl:NamedIndividual rdf:about="http://www.project-best.eu/owl/aixm-mod/airportheliport#CodeMilitaryOperationsBaseType-MIL">
        <rdf:type rdf:resource="http://www.project-best.eu/owl/aixm-mod/airportheliport#CodeMilitaryOperationsType"/>
        <rdfs:comment xml:lang="en">Only Military Air traffic is concerned.</rdfs:comment>
    </owl:NamedIndividual>
    


    <!-- http://www.project-best.eu/owl/aixm-mod/airportheliport#CodeMilitaryOperationsBaseType-OTHER -->

    <owl:NamedIndividual rdf:about="http://www.project-best.eu/owl/aixm-mod/airportheliport#CodeMilitaryOperationsBaseType-OTHER">
        <rdf:type rdf:resource="http://www.project-best.eu/owl/aixm-mod/airportheliport#CodeMilitaryOperationsType"/>
        <rdfs:comment xml:lang="en">Other</rdfs:comment>
    </owl:NamedIndividual>
    


    <!-- http://www.project-best.eu/owl/aixm-mod/airportheliport#CodeOperationAirportHeliportBaseType-AIRSHOW -->

    <owl:NamedIndividual rdf:about="http://www.project-best.eu/owl/aixm-mod/airportheliport#CodeOperationAirportHeliportBaseType-AIRSHOW">
        <rdf:type rdf:resource="http://www.project-best.eu/owl/aixm-mod/airportheliport#CodeOperationAirportHeliportType"/>
        <rdfs:comment xml:lang="en">Air show</rdfs:comment>
    </owl:NamedIndividual>
    


    <!-- http://www.project-best.eu/owl/aixm-mod/airportheliport#CodeOperationAirportHeliportBaseType-ALL -->

    <owl:NamedIndividual rdf:about="http://www.project-best.eu/owl/aixm-mod/airportheliport#CodeOperationAirportHeliportBaseType-ALL">
        <rdf:type rdf:resource="http://www.project-best.eu/owl/aixm-mod/airportheliport#CodeOperationAirportHeliportType"/>
        <rdfs:comment xml:lang="en">All operation types.</rdfs:comment>
    </owl:NamedIndividual>
    


    <!-- http://www.project-best.eu/owl/aixm-mod/airportheliport#CodeOperationAirportHeliportBaseType-ALTN_LANDING -->

    <owl:NamedIndividual rdf:about="http://www.project-best.eu/owl/aixm-mod/airportheliport#CodeOperationAirportHeliportBaseType-ALTN_LANDING">
        <rdf:type rdf:resource="http://www.project-best.eu/owl/aixm-mod/airportheliport#CodeOperationAirportHeliportType"/>
        <rdfs:comment xml:lang="en">Landing at an Alternate Airport/Heliport.</rdfs:comment>
    </owl:NamedIndividual>
    


    <!-- http://www.project-best.eu/owl/aixm-mod/airportheliport#CodeOperationAirportHeliportBaseType-LANDING -->

    <owl:NamedIndividual rdf:about="http://www.project-best.eu/owl/aixm-mod/airportheliport#CodeOperationAirportHeliportBaseType-LANDING">
        <rdf:type rdf:resource="http://www.project-best.eu/owl/aixm-mod/airportheliport#CodeOperationAirportHeliportType"/>
        <rdfs:comment xml:lang="en">Landing</rdfs:comment>
    </owl:NamedIndividual>
    


    <!-- http://www.project-best.eu/owl/aixm-mod/airportheliport#CodeOperationAirportHeliportBaseType-OTHER -->

    <owl:NamedIndividual rdf:about="http://www.project-best.eu/owl/aixm-mod/airportheliport#CodeOperationAirportHeliportBaseType-OTHER">
        <rdf:type rdf:resource="http://www.project-best.eu/owl/aixm-mod/airportheliport#CodeOperationAirportHeliportType"/>
        <rdfs:comment xml:lang="en">Other.</rdfs:comment>
    </owl:NamedIndividual>
    


    <!-- http://www.project-best.eu/owl/aixm-mod/airportheliport#CodeOperationAirportHeliportBaseType-TAKEOFF -->

    <owl:NamedIndividual rdf:about="http://www.project-best.eu/owl/aixm-mod/airportheliport#CodeOperationAirportHeliportBaseType-TAKEOFF">
        <rdf:type rdf:resource="http://www.project-best.eu/owl/aixm-mod/airportheliport#CodeOperationAirportHeliportType"/>
        <rdfs:comment xml:lang="en">Take off</rdfs:comment>
    </owl:NamedIndividual>
    


    <!-- http://www.project-best.eu/owl/aixm-mod/airportheliport#CodeOperationAirportHeliportBaseType-TOUCHGO -->

    <owl:NamedIndividual rdf:about="http://www.project-best.eu/owl/aixm-mod/airportheliport#CodeOperationAirportHeliportBaseType-TOUCHGO">
        <rdf:type rdf:resource="http://www.project-best.eu/owl/aixm-mod/airportheliport#CodeOperationAirportHeliportType"/>
        <rdfs:comment xml:lang="en">Touch and go</rdfs:comment>
    </owl:NamedIndividual>
    


    <!-- http://www.project-best.eu/owl/aixm-mod/airportheliport#CodeOperationAirportHeliportBaseType-TRAIN_APPROACH -->

    <owl:NamedIndividual rdf:about="http://www.project-best.eu/owl/aixm-mod/airportheliport#CodeOperationAirportHeliportBaseType-TRAIN_APPROACH">
        <rdf:type rdf:resource="http://www.project-best.eu/owl/aixm-mod/airportheliport#CodeOperationAirportHeliportType"/>
        <rdfs:comment xml:lang="en">Practice low approaches.</rdfs:comment>
    </owl:NamedIndividual>
    


    <!-- http://www.project-best.eu/owl/aixm-mod/airportheliport#CodeOperationManoeuvringAreaBaseType-AIRSHOW -->

    <owl:NamedIndividual rdf:about="http://www.project-best.eu/owl/aixm-mod/airportheliport#CodeOperationManoeuvringAreaBaseType-AIRSHOW">
        <rdf:type rdf:resource="http://www.project-best.eu/owl/aixm-mod/airportheliport#CodeOperationManoeuvringAreaType"/>
        <rdfs:comment xml:lang="en">Air show and aircraft display activities.</rdfs:comment>
    </owl:NamedIndividual>
    


    <!-- http://www.project-best.eu/owl/aixm-mod/airportheliport#CodeOperationManoeuvringAreaBaseType-ALL -->

    <owl:NamedIndividual rdf:about="http://www.project-best.eu/owl/aixm-mod/airportheliport#CodeOperationManoeuvringAreaBaseType-ALL">
        <rdf:type rdf:resource="http://www.project-best.eu/owl/aixm-mod/airportheliport#CodeOperationManoeuvringAreaType"/>
        <rdfs:comment xml:lang="en">All operation types.</rdfs:comment>
    </owl:NamedIndividual>
    


    <!-- http://www.project-best.eu/owl/aixm-mod/airportheliport#CodeOperationManoeuvringAreaBaseType-CROSSING -->

    <owl:NamedIndividual rdf:about="http://www.project-best.eu/owl/aixm-mod/airportheliport#CodeOperationManoeuvringAreaBaseType-CROSSING">
        <rdf:type rdf:resource="http://www.project-best.eu/owl/aixm-mod/airportheliport#CodeOperationManoeuvringAreaType"/>
        <rdfs:comment xml:lang="en">Crossing an element of the airport/heliport manoeuvring area, as opposed to taxiing along that element.</rdfs:comment>
    </owl:NamedIndividual>
    


    <!-- http://www.project-best.eu/owl/aixm-mod/airportheliport#CodeOperationManoeuvringAreaBaseType-LANDING -->

    <owl:NamedIndividual rdf:about="http://www.project-best.eu/owl/aixm-mod/airportheliport#CodeOperationManoeuvringAreaBaseType-LANDING">
        <rdf:type rdf:resource="http://www.project-best.eu/owl/aixm-mod/airportheliport#CodeOperationManoeuvringAreaType"/>
        <rdfs:comment xml:lang="en">Aircraft landing.</rdfs:comment>
    </owl:NamedIndividual>
    


    <!-- http://www.project-best.eu/owl/aixm-mod/airportheliport#CodeOperationManoeuvringAreaBaseType-OTHER -->

    <owl:NamedIndividual rdf:about="http://www.project-best.eu/owl/aixm-mod/airportheliport#CodeOperationManoeuvringAreaBaseType-OTHER">
        <rdf:type rdf:resource="http://www.project-best.eu/owl/aixm-mod/airportheliport#CodeOperationManoeuvringAreaType"/>
        <rdfs:comment xml:lang="en">Other.</rdfs:comment>
    </owl:NamedIndividual>
    


    <!-- http://www.project-best.eu/owl/aixm-mod/airportheliport#CodeOperationManoeuvringAreaBaseType-TAKEOFF -->

    <owl:NamedIndividual rdf:about="http://www.project-best.eu/owl/aixm-mod/airportheliport#CodeOperationManoeuvringAreaBaseType-TAKEOFF">
        <rdf:type rdf:resource="http://www.project-best.eu/owl/aixm-mod/airportheliport#CodeOperationManoeuvringAreaType"/>
        <rdfs:comment xml:lang="en">Aircraft take off.</rdfs:comment>
    </owl:NamedIndividual>
    


    <!-- http://www.project-best.eu/owl/aixm-mod/airportheliport#CodeOperationManoeuvringAreaBaseType-TAXIING -->

    <owl:NamedIndividual rdf:about="http://www.project-best.eu/owl/aixm-mod/airportheliport#CodeOperationManoeuvringAreaBaseType-TAXIING">
        <rdf:type rdf:resource="http://www.project-best.eu/owl/aixm-mod/airportheliport#CodeOperationManoeuvringAreaType"/>
        <rdfs:comment xml:lang="en">Aircraft taxiing along an element of the airport/heliport movement area.</rdfs:comment>
    </owl:NamedIndividual>
    


    <!-- http://www.project-best.eu/owl/aixm-mod/airportheliport#CodeOperationManoeuvringAreaBaseType-TOUCHGO -->

    <owl:NamedIndividual rdf:about="http://www.project-best.eu/owl/aixm-mod/airportheliport#CodeOperationManoeuvringAreaBaseType-TOUCHGO">
        <rdf:type rdf:resource="http://www.project-best.eu/owl/aixm-mod/airportheliport#CodeOperationManoeuvringAreaType"/>
        <rdfs:comment xml:lang="en">Aircraft landing followed by an immediate take-off, without deceleration.</rdfs:comment>
    </owl:NamedIndividual>
    


    <!-- http://www.project-best.eu/owl/aixm-mod/airportheliport#CodeOperationManoeuvringAreaBaseType-TRAIN_APPROACH -->

    <owl:NamedIndividual rdf:about="http://www.project-best.eu/owl/aixm-mod/airportheliport#CodeOperationManoeuvringAreaBaseType-TRAIN_APPROACH">
        <rdf:type rdf:resource="http://www.project-best.eu/owl/aixm-mod/airportheliport#CodeOperationManoeuvringAreaType"/>
        <rdfs:comment xml:lang="en">Aircraft practices low approaches.</rdfs:comment>
    </owl:NamedIndividual>
    


    <!-- http://www.project-best.eu/owl/aixm-mod/airportheliport#CodePCNMethodBaseType-ACFT -->

    <owl:NamedIndividual rdf:about="http://www.project-best.eu/owl/aixm-mod/airportheliport#CodePCNMethodBaseType-ACFT">
        <rdf:type rdf:resource="http://www.project-best.eu/owl/aixm-mod/airportheliport#CodePCNMethodType"/>
        <rdfs:comment xml:lang="en">[U] Based on aircraft experience.</rdfs:comment>
    </owl:NamedIndividual>
    


    <!-- http://www.project-best.eu/owl/aixm-mod/airportheliport#CodePCNMethodBaseType-OTHER -->

    <owl:NamedIndividual rdf:about="http://www.project-best.eu/owl/aixm-mod/airportheliport#CodePCNMethodBaseType-OTHER">
        <rdf:type rdf:resource="http://www.project-best.eu/owl/aixm-mod/airportheliport#CodePCNMethodType"/>
        <rdfs:comment xml:lang="en">Other</rdfs:comment>
    </owl:NamedIndividual>
    


    <!-- http://www.project-best.eu/owl/aixm-mod/airportheliport#CodePCNMethodBaseType-TECH -->

    <owl:NamedIndividual rdf:about="http://www.project-best.eu/owl/aixm-mod/airportheliport#CodePCNMethodBaseType-TECH">
        <rdf:type rdf:resource="http://www.project-best.eu/owl/aixm-mod/airportheliport#CodePCNMethodType"/>
        <rdfs:comment xml:lang="en">[T] Technical evaluation.</rdfs:comment>
    </owl:NamedIndividual>
    


    <!-- http://www.project-best.eu/owl/aixm-mod/airportheliport#CodePCNPavementBaseType-FLEXIBLE -->

    <owl:NamedIndividual rdf:about="http://www.project-best.eu/owl/aixm-mod/airportheliport#CodePCNPavementBaseType-FLEXIBLE">
        <rdf:type rdf:resource="http://www.project-best.eu/owl/aixm-mod/airportheliport#CodePCNPavementType"/>
        <rdfs:comment xml:lang="en">[F] Flexible pavement.</rdfs:comment>
    </owl:NamedIndividual>
    


    <!-- http://www.project-best.eu/owl/aixm-mod/airportheliport#CodePCNPavementBaseType-OTHER -->

    <owl:NamedIndividual rdf:about="http://www.project-best.eu/owl/aixm-mod/airportheliport#CodePCNPavementBaseType-OTHER">
        <rdf:type rdf:resource="http://www.project-best.eu/owl/aixm-mod/airportheliport#CodePCNPavementType"/>
        <rdfs:comment xml:lang="en">Other</rdfs:comment>
    </owl:NamedIndividual>
    


    <!-- http://www.project-best.eu/owl/aixm-mod/airportheliport#CodePCNPavementBaseType-RIGID -->

    <owl:NamedIndividual rdf:about="http://www.project-best.eu/owl/aixm-mod/airportheliport#CodePCNPavementBaseType-RIGID">
        <rdf:type rdf:resource="http://www.project-best.eu/owl/aixm-mod/airportheliport#CodePCNPavementType"/>
        <rdfs:comment xml:lang="en">[R] Rigid pavement.</rdfs:comment>
    </owl:NamedIndividual>
    


    <!-- http://www.project-best.eu/owl/aixm-mod/airportheliport#CodePCNSubgradeBaseType-A -->

    <owl:NamedIndividual rdf:about="http://www.project-best.eu/owl/aixm-mod/airportheliport#CodePCNSubgradeBaseType-A">
        <rdf:type rdf:resource="http://www.project-best.eu/owl/aixm-mod/airportheliport#CodePCNSubgradeType"/>
        <rdfs:comment xml:lang="en">High strength sub-grade.</rdfs:comment>
    </owl:NamedIndividual>
    


    <!-- http://www.project-best.eu/owl/aixm-mod/airportheliport#CodePCNSubgradeBaseType-B -->

    <owl:NamedIndividual rdf:about="http://www.project-best.eu/owl/aixm-mod/airportheliport#CodePCNSubgradeBaseType-B">
        <rdf:type rdf:resource="http://www.project-best.eu/owl/aixm-mod/airportheliport#CodePCNSubgradeType"/>
        <rdfs:comment xml:lang="en">Medium strength sub-grade.</rdfs:comment>
    </owl:NamedIndividual>
    


    <!-- http://www.project-best.eu/owl/aixm-mod/airportheliport#CodePCNSubgradeBaseType-C -->

    <owl:NamedIndividual rdf:about="http://www.project-best.eu/owl/aixm-mod/airportheliport#CodePCNSubgradeBaseType-C">
        <rdf:type rdf:resource="http://www.project-best.eu/owl/aixm-mod/airportheliport#CodePCNSubgradeType"/>
        <rdfs:comment xml:lang="en">Low strength sub-grade.</rdfs:comment>
    </owl:NamedIndividual>
    


    <!-- http://www.project-best.eu/owl/aixm-mod/airportheliport#CodePCNSubgradeBaseType-D -->

    <owl:NamedIndividual rdf:about="http://www.project-best.eu/owl/aixm-mod/airportheliport#CodePCNSubgradeBaseType-D">
        <rdf:type rdf:resource="http://www.project-best.eu/owl/aixm-mod/airportheliport#CodePCNSubgradeType"/>
        <rdfs:comment xml:lang="en">Ultra-low strength sub-grade.</rdfs:comment>
    </owl:NamedIndividual>
    


    <!-- http://www.project-best.eu/owl/aixm-mod/airportheliport#CodePCNSubgradeBaseType-OTHER -->

    <owl:NamedIndividual rdf:about="http://www.project-best.eu/owl/aixm-mod/airportheliport#CodePCNSubgradeBaseType-OTHER">
        <rdf:type rdf:resource="http://www.project-best.eu/owl/aixm-mod/airportheliport#CodePCNSubgradeType"/>
        <rdfs:comment xml:lang="en">Other</rdfs:comment>
    </owl:NamedIndividual>
    


    <!-- http://www.project-best.eu/owl/aixm-mod/airportheliport#CodePCNTyrePressureBaseType-OTHER -->

    <owl:NamedIndividual rdf:about="http://www.project-best.eu/owl/aixm-mod/airportheliport#CodePCNTyrePressureBaseType-OTHER">
        <rdf:type rdf:resource="http://www.project-best.eu/owl/aixm-mod/airportheliport#CodePCNTyrePressureType"/>
        <rdfs:comment xml:lang="en">Other</rdfs:comment>
    </owl:NamedIndividual>
    


    <!-- http://www.project-best.eu/owl/aixm-mod/airportheliport#CodePCNTyrePressureBaseType-W -->

    <owl:NamedIndividual rdf:about="http://www.project-best.eu/owl/aixm-mod/airportheliport#CodePCNTyrePressureBaseType-W">
        <rdf:type rdf:resource="http://www.project-best.eu/owl/aixm-mod/airportheliport#CodePCNTyrePressureType"/>
        <rdfs:comment xml:lang="en">High: No pressure limit.</rdfs:comment>
    </owl:NamedIndividual>
    


    <!-- http://www.project-best.eu/owl/aixm-mod/airportheliport#CodePCNTyrePressureBaseType-X -->

    <owl:NamedIndividual rdf:about="http://www.project-best.eu/owl/aixm-mod/airportheliport#CodePCNTyrePressureBaseType-X">
        <rdf:type rdf:resource="http://www.project-best.eu/owl/aixm-mod/airportheliport#CodePCNTyrePressureType"/>
        <rdfs:comment xml:lang="en">Medium: Pressure limited to 1.5 MPa (217 psi).</rdfs:comment>
    </owl:NamedIndividual>
    


    <!-- http://www.project-best.eu/owl/aixm-mod/airportheliport#CodePCNTyrePressureBaseType-Y -->

    <owl:NamedIndividual rdf:about="http://www.project-best.eu/owl/aixm-mod/airportheliport#CodePCNTyrePressureBaseType-Y">
        <rdf:type rdf:resource="http://www.project-best.eu/owl/aixm-mod/airportheliport#CodePCNTyrePressureType"/>
        <rdfs:comment xml:lang="en">Low: Pressure limited to 1.00 MPa (145 psi).</rdfs:comment>
    </owl:NamedIndividual>
    


    <!-- http://www.project-best.eu/owl/aixm-mod/airportheliport#CodePCNTyrePressureBaseType-Z -->

    <owl:NamedIndividual rdf:about="http://www.project-best.eu/owl/aixm-mod/airportheliport#CodePCNTyrePressureBaseType-Z">
        <rdf:type rdf:resource="http://www.project-best.eu/owl/aixm-mod/airportheliport#CodePCNTyrePressureType"/>
        <rdfs:comment xml:lang="en">Very low: Pressure limited to 0.50 MPa (73 psi).</rdfs:comment>
    </owl:NamedIndividual>
    


    <!-- http://www.project-best.eu/owl/aixm-mod/airportheliport#CodeProtectAreaSectionBaseType-CL -->

    <owl:NamedIndividual rdf:about="http://www.project-best.eu/owl/aixm-mod/airportheliport#CodeProtectAreaSectionBaseType-CL">
        <rdf:type rdf:resource="http://www.project-best.eu/owl/aixm-mod/airportheliport#CodeProtectAreaSectionType"/>
        <rdfs:comment xml:lang="en">Area centreline</rdfs:comment>
    </owl:NamedIndividual>
    


    <!-- http://www.project-best.eu/owl/aixm-mod/airportheliport#CodeProtectAreaSectionBaseType-EDGE -->

    <owl:NamedIndividual rdf:about="http://www.project-best.eu/owl/aixm-mod/airportheliport#CodeProtectAreaSectionBaseType-EDGE">
        <rdf:type rdf:resource="http://www.project-best.eu/owl/aixm-mod/airportheliport#CodeProtectAreaSectionType"/>
        <rdfs:comment xml:lang="en">Area edge.</rdfs:comment>
    </owl:NamedIndividual>
    


    <!-- http://www.project-best.eu/owl/aixm-mod/airportheliport#CodeProtectAreaSectionBaseType-END -->

    <owl:NamedIndividual rdf:about="http://www.project-best.eu/owl/aixm-mod/airportheliport#CodeProtectAreaSectionBaseType-END">
        <rdf:type rdf:resource="http://www.project-best.eu/owl/aixm-mod/airportheliport#CodeProtectAreaSectionType"/>
        <rdfs:comment xml:lang="en">Area end.</rdfs:comment>
    </owl:NamedIndividual>
    


    <!-- http://www.project-best.eu/owl/aixm-mod/airportheliport#CodeProtectAreaSectionBaseType-OTHER -->

    <owl:NamedIndividual rdf:about="http://www.project-best.eu/owl/aixm-mod/airportheliport#CodeProtectAreaSectionBaseType-OTHER">
        <rdf:type rdf:resource="http://www.project-best.eu/owl/aixm-mod/airportheliport#CodeProtectAreaSectionType"/>
        <rdfs:comment xml:lang="en">Other.</rdfs:comment>
    </owl:NamedIndividual>
    


    <!-- http://www.project-best.eu/owl/aixm-mod/airportheliport#CodeRVRReadingBaseType-MID -->

    <owl:NamedIndividual rdf:about="http://www.project-best.eu/owl/aixm-mod/airportheliport#CodeRVRReadingBaseType-MID">
        <rdf:type rdf:resource="http://www.project-best.eu/owl/aixm-mod/airportheliport#CodeRVRReadingType"/>
        <rdfs:comment xml:lang="en">Middle or centre of runway</rdfs:comment>
    </owl:NamedIndividual>
    


    <!-- http://www.project-best.eu/owl/aixm-mod/airportheliport#CodeRVRReadingBaseType-OTHER -->

    <owl:NamedIndividual rdf:about="http://www.project-best.eu/owl/aixm-mod/airportheliport#CodeRVRReadingBaseType-OTHER">
        <rdf:type rdf:resource="http://www.project-best.eu/owl/aixm-mod/airportheliport#CodeRVRReadingType"/>
        <rdfs:comment xml:lang="en">Other</rdfs:comment>
    </owl:NamedIndividual>
    


    <!-- http://www.project-best.eu/owl/aixm-mod/airportheliport#CodeRVRReadingBaseType-TDZ -->

    <owl:NamedIndividual rdf:about="http://www.project-best.eu/owl/aixm-mod/airportheliport#CodeRVRReadingBaseType-TDZ">
        <rdf:type rdf:resource="http://www.project-best.eu/owl/aixm-mod/airportheliport#CodeRVRReadingType"/>
        <rdfs:comment xml:lang="en">Touchdown</rdfs:comment>
    </owl:NamedIndividual>
    


    <!-- http://www.project-best.eu/owl/aixm-mod/airportheliport#CodeRVRReadingBaseType-TO -->

    <owl:NamedIndividual rdf:about="http://www.project-best.eu/owl/aixm-mod/airportheliport#CodeRVRReadingBaseType-TO">
        <rdf:type rdf:resource="http://www.project-best.eu/owl/aixm-mod/airportheliport#CodeRVRReadingType"/>
        <rdfs:comment xml:lang="en">Takeoff or rollout point.</rdfs:comment>
    </owl:NamedIndividual>
    


    <!-- http://www.project-best.eu/owl/aixm-mod/airportheliport#CodeRoadBaseType-OTHER -->

    <owl:NamedIndividual rdf:about="http://www.project-best.eu/owl/aixm-mod/airportheliport#CodeRoadBaseType-OTHER">
        <rdf:type rdf:resource="http://www.project-best.eu/owl/aixm-mod/airportheliport#CodeRoadType"/>
        <rdfs:comment xml:lang="en">Other</rdfs:comment>
    </owl:NamedIndividual>
    


    <!-- http://www.project-best.eu/owl/aixm-mod/airportheliport#CodeRoadBaseType-PUBLIC -->

    <owl:NamedIndividual rdf:about="http://www.project-best.eu/owl/aixm-mod/airportheliport#CodeRoadBaseType-PUBLIC">
        <rdf:type rdf:resource="http://www.project-best.eu/owl/aixm-mod/airportheliport#CodeRoadType"/>
        <rdfs:comment xml:lang="en">Public road</rdfs:comment>
    </owl:NamedIndividual>
    


    <!-- http://www.project-best.eu/owl/aixm-mod/airportheliport#CodeRoadBaseType-SERVICE -->

    <owl:NamedIndividual rdf:about="http://www.project-best.eu/owl/aixm-mod/airportheliport#CodeRoadBaseType-SERVICE">
        <rdf:type rdf:resource="http://www.project-best.eu/owl/aixm-mod/airportheliport#CodeRoadType"/>
        <rdfs:comment xml:lang="en">Service road</rdfs:comment>
    </owl:NamedIndividual>
    


    <!-- http://www.project-best.eu/owl/aixm-mod/airportheliport#CodeRunwayBaseType-FATO -->

    <owl:NamedIndividual rdf:about="http://www.project-best.eu/owl/aixm-mod/airportheliport#CodeRunwayBaseType-FATO">
        <rdf:type rdf:resource="http://www.project-best.eu/owl/aixm-mod/airportheliport#CodeRunwayType"/>
        <rdfs:comment xml:lang="en">Final Approach and Take Off Area for helicopters</rdfs:comment>
    </owl:NamedIndividual>
    


    <!-- http://www.project-best.eu/owl/aixm-mod/airportheliport#CodeRunwayBaseType-OTHER -->

    <owl:NamedIndividual rdf:about="http://www.project-best.eu/owl/aixm-mod/airportheliport#CodeRunwayBaseType-OTHER">
        <rdf:type rdf:resource="http://www.project-best.eu/owl/aixm-mod/airportheliport#CodeRunwayType"/>
        <rdfs:comment xml:lang="en">Other</rdfs:comment>
    </owl:NamedIndividual>
    


    <!-- http://www.project-best.eu/owl/aixm-mod/airportheliport#CodeRunwayBaseType-RWY -->

    <owl:NamedIndividual rdf:about="http://www.project-best.eu/owl/aixm-mod/airportheliport#CodeRunwayBaseType-RWY">
        <rdf:type rdf:resource="http://www.project-best.eu/owl/aixm-mod/airportheliport#CodeRunwayType"/>
        <rdfs:comment xml:lang="en">Runway for airplanes</rdfs:comment>
    </owl:NamedIndividual>
    


    <!-- http://www.project-best.eu/owl/aixm-mod/airportheliport#CodeRunwayElementBaseType-DISPLACED -->

    <owl:NamedIndividual rdf:about="http://www.project-best.eu/owl/aixm-mod/airportheliport#CodeRunwayElementBaseType-DISPLACED">
        <rdf:type rdf:resource="http://www.project-best.eu/owl/aixm-mod/airportheliport#CodeRunwayElementType"/>
        <rdfs:comment xml:lang="en">The element between the start of the runway and the position of the displaced threshold.</rdfs:comment>
    </owl:NamedIndividual>
    


    <!-- http://www.project-best.eu/owl/aixm-mod/airportheliport#CodeRunwayElementBaseType-INTERSECTION -->

    <owl:NamedIndividual rdf:about="http://www.project-best.eu/owl/aixm-mod/airportheliport#CodeRunwayElementBaseType-INTERSECTION">
        <rdf:type rdf:resource="http://www.project-best.eu/owl/aixm-mod/airportheliport#CodeRunwayElementType"/>
        <rdfs:comment xml:lang="en">Intersection element - with a runway or with a taxiway.</rdfs:comment>
    </owl:NamedIndividual>
    


    <!-- http://www.project-best.eu/owl/aixm-mod/airportheliport#CodeRunwayElementBaseType-NORMAL -->

    <owl:NamedIndividual rdf:about="http://www.project-best.eu/owl/aixm-mod/airportheliport#CodeRunwayElementBaseType-NORMAL">
        <rdf:type rdf:resource="http://www.project-best.eu/owl/aixm-mod/airportheliport#CodeRunwayElementType"/>
        <rdfs:comment xml:lang="en">The default type.</rdfs:comment>
    </owl:NamedIndividual>
    


    <!-- http://www.project-best.eu/owl/aixm-mod/airportheliport#CodeRunwayElementBaseType-OTHER -->

    <owl:NamedIndividual rdf:about="http://www.project-best.eu/owl/aixm-mod/airportheliport#CodeRunwayElementBaseType-OTHER">
        <rdf:type rdf:resource="http://www.project-best.eu/owl/aixm-mod/airportheliport#CodeRunwayElementType"/>
        <rdfs:comment xml:lang="en">Other.</rdfs:comment>
    </owl:NamedIndividual>
    


    <!-- http://www.project-best.eu/owl/aixm-mod/airportheliport#CodeRunwayElementBaseType-SHOULDER -->

    <owl:NamedIndividual rdf:about="http://www.project-best.eu/owl/aixm-mod/airportheliport#CodeRunwayElementBaseType-SHOULDER">
        <rdf:type rdf:resource="http://www.project-best.eu/owl/aixm-mod/airportheliport#CodeRunwayElementType"/>
        <rdfs:comment xml:lang="en">Runway or taxiway shoulder element.</rdfs:comment>
    </owl:NamedIndividual>
    


    <!-- http://www.project-best.eu/owl/aixm-mod/airportheliport#CodeRunwayMarkingBaseType-BASIC -->

    <owl:NamedIndividual rdf:about="http://www.project-best.eu/owl/aixm-mod/airportheliport#CodeRunwayMarkingBaseType-BASIC">
        <rdf:type rdf:resource="http://www.project-best.eu/owl/aixm-mod/airportheliport#CodeRunwayMarkingType"/>
        <rdfs:comment xml:lang="en">Basic (or Visual) runway marking elements include markings for Runway Designation, Centreline, Threshold (On runways sued or intended to be used by international commercial transports) and Aiming Point (On runways 4000 ft (1200M) or longer used by jet aircraft).</rdfs:comment>
    </owl:NamedIndividual>
    


    <!-- http://www.project-best.eu/owl/aixm-mod/airportheliport#CodeRunwayMarkingBaseType-HELIPORT -->

    <owl:NamedIndividual rdf:about="http://www.project-best.eu/owl/aixm-mod/airportheliport#CodeRunwayMarkingBaseType-HELIPORT">
        <rdf:type rdf:resource="http://www.project-best.eu/owl/aixm-mod/airportheliport#CodeRunwayMarkingType"/>
        <rdfs:comment xml:lang="en">Heliport specific marking elements are present.</rdfs:comment>
    </owl:NamedIndividual>
    


    <!-- http://www.project-best.eu/owl/aixm-mod/airportheliport#CodeRunwayMarkingBaseType-NONE -->

    <owl:NamedIndividual rdf:about="http://www.project-best.eu/owl/aixm-mod/airportheliport#CodeRunwayMarkingBaseType-NONE">
        <rdf:type rdf:resource="http://www.project-best.eu/owl/aixm-mod/airportheliport#CodeRunwayMarkingType"/>
        <rdfs:comment xml:lang="en">No runway markings present.</rdfs:comment>
    </owl:NamedIndividual>
    


    <!-- http://www.project-best.eu/owl/aixm-mod/airportheliport#CodeRunwayMarkingBaseType-NONPRECISION -->

    <owl:NamedIndividual rdf:about="http://www.project-best.eu/owl/aixm-mod/airportheliport#CodeRunwayMarkingBaseType-NONPRECISION">
        <rdf:type rdf:resource="http://www.project-best.eu/owl/aixm-mod/airportheliport#CodeRunwayMarkingType"/>
        <rdfs:comment xml:lang="en">Markings appropriate for non-precision approach  runway.  Non-Precision Instrument runway marking elements include markings for Runway designation, Centreline, threshold and Aiming Point.</rdfs:comment>
    </owl:NamedIndividual>
    


    <!-- http://www.project-best.eu/owl/aixm-mod/airportheliport#CodeRunwayMarkingBaseType-NON_STANDARD -->

    <owl:NamedIndividual rdf:about="http://www.project-best.eu/owl/aixm-mod/airportheliport#CodeRunwayMarkingBaseType-NON_STANDARD">
        <rdf:type rdf:resource="http://www.project-best.eu/owl/aixm-mod/airportheliport#CodeRunwayMarkingType"/>
        <rdfs:comment xml:lang="en">Runway marking elements such as Runway Designation, Centreline, Threshold and Aiming Point may be present, but they are Not standard markings.</rdfs:comment>
    </owl:NamedIndividual>
    


    <!-- http://www.project-best.eu/owl/aixm-mod/airportheliport#CodeRunwayMarkingBaseType-OTHER -->

    <owl:NamedIndividual rdf:about="http://www.project-best.eu/owl/aixm-mod/airportheliport#CodeRunwayMarkingBaseType-OTHER">
        <rdf:type rdf:resource="http://www.project-best.eu/owl/aixm-mod/airportheliport#CodeRunwayMarkingType"/>
        <rdfs:comment xml:lang="en">Other runway markings.</rdfs:comment>
    </owl:NamedIndividual>
    


    <!-- http://www.project-best.eu/owl/aixm-mod/airportheliport#CodeRunwayMarkingBaseType-PRECISION -->

    <owl:NamedIndividual rdf:about="http://www.project-best.eu/owl/aixm-mod/airportheliport#CodeRunwayMarkingBaseType-PRECISION">
        <rdf:type rdf:resource="http://www.project-best.eu/owl/aixm-mod/airportheliport#CodeRunwayMarkingType"/>
        <rdfs:comment xml:lang="en">Markings appropriate for precision approach  runway.</rdfs:comment>
    </owl:NamedIndividual>
    


    <!-- http://www.project-best.eu/owl/aixm-mod/airportheliport#CodeRunwayMarkingBaseType-RUNWAY_NUMBERS -->

    <owl:NamedIndividual rdf:about="http://www.project-best.eu/owl/aixm-mod/airportheliport#CodeRunwayMarkingBaseType-RUNWAY_NUMBERS">
        <rdf:type rdf:resource="http://www.project-best.eu/owl/aixm-mod/airportheliport#CodeRunwayMarkingType"/>
        <rdfs:comment xml:lang="en">The only runway marking element present is the Runway Designation.</rdfs:comment>
    </owl:NamedIndividual>
    


    <!-- http://www.project-best.eu/owl/aixm-mod/airportheliport#CodeRunwayPointRoleBaseType-ABEAM_ELEVATION -->

    <owl:NamedIndividual rdf:about="http://www.project-best.eu/owl/aixm-mod/airportheliport#CodeRunwayPointRoleBaseType-ABEAM_ELEVATION">
        <rdf:type rdf:resource="http://www.project-best.eu/owl/aixm-mod/airportheliport#CodeRunwayPointRoleType"/>
        <rdfs:comment xml:lang="en">The point perpendicular to the Elevation Antenna on the Runway Centreline. </rdfs:comment>
    </owl:NamedIndividual>
    


    <!-- http://www.project-best.eu/owl/aixm-mod/airportheliport#CodeRunwayPointRoleBaseType-ABEAM_GLIDESLOPE -->

    <owl:NamedIndividual rdf:about="http://www.project-best.eu/owl/aixm-mod/airportheliport#CodeRunwayPointRoleBaseType-ABEAM_GLIDESLOPE">
        <rdf:type rdf:resource="http://www.project-best.eu/owl/aixm-mod/airportheliport#CodeRunwayPointRoleType"/>
        <rdfs:comment xml:lang="en">The point perpendicular to the Glideslope Antenna on the Runway Centreline.  Also known as the Aiming Point.</rdfs:comment>
    </owl:NamedIndividual>
    


    <!-- http://www.project-best.eu/owl/aixm-mod/airportheliport#CodeRunwayPointRoleBaseType-ABEAM_PAR -->

    <owl:NamedIndividual rdf:about="http://www.project-best.eu/owl/aixm-mod/airportheliport#CodeRunwayPointRoleBaseType-ABEAM_PAR">
        <rdf:type rdf:resource="http://www.project-best.eu/owl/aixm-mod/airportheliport#CodeRunwayPointRoleType"/>
        <rdfs:comment xml:lang="en">The point perpendicular to the Precision Approach Radar (PAR) Antenna on the Runway Centreline. </rdfs:comment>
    </owl:NamedIndividual>
    


    <!-- http://www.project-best.eu/owl/aixm-mod/airportheliport#CodeRunwayPointRoleBaseType-ABEAM_RER -->

    <owl:NamedIndividual rdf:about="http://www.project-best.eu/owl/aixm-mod/airportheliport#CodeRunwayPointRoleBaseType-ABEAM_RER">
        <rdf:type rdf:resource="http://www.project-best.eu/owl/aixm-mod/airportheliport#CodeRunwayPointRoleType"/>
        <rdfs:comment xml:lang="en">The point perpendicular to the Runway End Reflector (RER) on the Runway Centreline. </rdfs:comment>
    </owl:NamedIndividual>
    


    <!-- http://www.project-best.eu/owl/aixm-mod/airportheliport#CodeRunwayPointRoleBaseType-ABEAM_TDR -->

    <owl:NamedIndividual rdf:about="http://www.project-best.eu/owl/aixm-mod/airportheliport#CodeRunwayPointRoleBaseType-ABEAM_TDR">
        <rdf:type rdf:resource="http://www.project-best.eu/owl/aixm-mod/airportheliport#CodeRunwayPointRoleType"/>
        <rdfs:comment xml:lang="en">The point perpendicular to the Touchdown Reflector (TDR) on the Runway Centreline. </rdfs:comment>
    </owl:NamedIndividual>
    


    <!-- http://www.project-best.eu/owl/aixm-mod/airportheliport#CodeRunwayPointRoleBaseType-DISTHR -->

    <owl:NamedIndividual rdf:about="http://www.project-best.eu/owl/aixm-mod/airportheliport#CodeRunwayPointRoleBaseType-DISTHR">
        <rdf:type rdf:resource="http://www.project-best.eu/owl/aixm-mod/airportheliport#CodeRunwayPointRoleType"/>
        <rdfs:comment xml:lang="en">Displaced threshold.</rdfs:comment>
    </owl:NamedIndividual>
    


    <!-- http://www.project-best.eu/owl/aixm-mod/airportheliport#CodeRunwayPointRoleBaseType-END -->

    <owl:NamedIndividual rdf:about="http://www.project-best.eu/owl/aixm-mod/airportheliport#CodeRunwayPointRoleBaseType-END">
        <rdf:type rdf:resource="http://www.project-best.eu/owl/aixm-mod/airportheliport#CodeRunwayPointRoleType"/>
        <rdfs:comment xml:lang="en">Physical end of a runway direction</rdfs:comment>
    </owl:NamedIndividual>
    


    <!-- http://www.project-best.eu/owl/aixm-mod/airportheliport#CodeRunwayPointRoleBaseType-LAHSO -->

    <owl:NamedIndividual rdf:about="http://www.project-best.eu/owl/aixm-mod/airportheliport#CodeRunwayPointRoleBaseType-LAHSO">
        <rdf:type rdf:resource="http://www.project-best.eu/owl/aixm-mod/airportheliport#CodeRunwayPointRoleType"/>
        <rdfs:comment xml:lang="en">Point indicating Land And Hold Short Operation location</rdfs:comment>
    </owl:NamedIndividual>
    


    <!-- http://www.project-best.eu/owl/aixm-mod/airportheliport#CodeRunwayPointRoleBaseType-MID -->

    <owl:NamedIndividual rdf:about="http://www.project-best.eu/owl/aixm-mod/airportheliport#CodeRunwayPointRoleBaseType-MID">
        <rdf:type rdf:resource="http://www.project-best.eu/owl/aixm-mod/airportheliport#CodeRunwayPointRoleType"/>
        <rdfs:comment xml:lang="en">The mid point of the runway</rdfs:comment>
    </owl:NamedIndividual>
    


    <!-- http://www.project-best.eu/owl/aixm-mod/airportheliport#CodeRunwayPointRoleBaseType-OTHER -->

    <owl:NamedIndividual rdf:about="http://www.project-best.eu/owl/aixm-mod/airportheliport#CodeRunwayPointRoleBaseType-OTHER">
        <rdf:type rdf:resource="http://www.project-best.eu/owl/aixm-mod/airportheliport#CodeRunwayPointRoleType"/>
        <rdfs:comment xml:lang="en">Other.</rdfs:comment>
    </owl:NamedIndividual>
    


    <!-- http://www.project-best.eu/owl/aixm-mod/airportheliport#CodeRunwayPointRoleBaseType-START -->

    <owl:NamedIndividual rdf:about="http://www.project-best.eu/owl/aixm-mod/airportheliport#CodeRunwayPointRoleBaseType-START">
        <rdf:type rdf:resource="http://www.project-best.eu/owl/aixm-mod/airportheliport#CodeRunwayPointRoleType"/>
        <rdfs:comment xml:lang="en">Physical start of a runway direction.</rdfs:comment>
    </owl:NamedIndividual>
    


    <!-- http://www.project-best.eu/owl/aixm-mod/airportheliport#CodeRunwayPointRoleBaseType-START_RUN -->

    <owl:NamedIndividual rdf:about="http://www.project-best.eu/owl/aixm-mod/airportheliport#CodeRunwayPointRoleBaseType-START_RUN">
        <rdf:type rdf:resource="http://www.project-best.eu/owl/aixm-mod/airportheliport#CodeRunwayPointRoleType"/>
        <rdfs:comment xml:lang="en">Start of take off run</rdfs:comment>
    </owl:NamedIndividual>
    


    <!-- http://www.project-best.eu/owl/aixm-mod/airportheliport#CodeRunwayPointRoleBaseType-TDZ -->

    <owl:NamedIndividual rdf:about="http://www.project-best.eu/owl/aixm-mod/airportheliport#CodeRunwayPointRoleBaseType-TDZ">
        <rdf:type rdf:resource="http://www.project-best.eu/owl/aixm-mod/airportheliport#CodeRunwayPointRoleType"/>
        <rdfs:comment xml:lang="en">Touchdown Zone</rdfs:comment>
    </owl:NamedIndividual>
    


    <!-- http://www.project-best.eu/owl/aixm-mod/airportheliport#CodeRunwayPointRoleBaseType-THR -->

    <owl:NamedIndividual rdf:about="http://www.project-best.eu/owl/aixm-mod/airportheliport#CodeRunwayPointRoleBaseType-THR">
        <rdf:type rdf:resource="http://www.project-best.eu/owl/aixm-mod/airportheliport#CodeRunwayPointRoleType"/>
        <rdfs:comment xml:lang="en">Threshold</rdfs:comment>
    </owl:NamedIndividual>
    


    <!-- http://www.project-best.eu/owl/aixm-mod/airportheliport#CodeRunwayProtectionAreaBaseType-CWY -->

    <owl:NamedIndividual rdf:about="http://www.project-best.eu/owl/aixm-mod/airportheliport#CodeRunwayProtectionAreaBaseType-CWY">
        <rdf:type rdf:resource="http://www.project-best.eu/owl/aixm-mod/airportheliport#CodeRunwayProtectionAreaType"/>
        <rdfs:comment xml:lang="en">Clearway.</rdfs:comment>
    </owl:NamedIndividual>
    


    <!-- http://www.project-best.eu/owl/aixm-mod/airportheliport#CodeRunwayProtectionAreaBaseType-ILS -->

    <owl:NamedIndividual rdf:about="http://www.project-best.eu/owl/aixm-mod/airportheliport#CodeRunwayProtectionAreaBaseType-ILS">
        <rdf:type rdf:resource="http://www.project-best.eu/owl/aixm-mod/airportheliport#CodeRunwayProtectionAreaType"/>
        <rdfs:comment xml:lang="en">ILS protection area.  Protects ILS signal distortion by forbidding large objects in the area.</rdfs:comment>
    </owl:NamedIndividual>
    


    <!-- http://www.project-best.eu/owl/aixm-mod/airportheliport#CodeRunwayProtectionAreaBaseType-IOFZ -->

    <owl:NamedIndividual rdf:about="http://www.project-best.eu/owl/aixm-mod/airportheliport#CodeRunwayProtectionAreaBaseType-IOFZ">
        <rdf:type rdf:resource="http://www.project-best.eu/owl/aixm-mod/airportheliport#CodeRunwayProtectionAreaType"/>
        <rdfs:comment xml:lang="en">Inner Obstacle free zone or surface  </rdfs:comment>
    </owl:NamedIndividual>
    


    <!-- http://www.project-best.eu/owl/aixm-mod/airportheliport#CodeRunwayProtectionAreaBaseType-OFZ -->

    <owl:NamedIndividual rdf:about="http://www.project-best.eu/owl/aixm-mod/airportheliport#CodeRunwayProtectionAreaBaseType-OFZ">
        <rdf:type rdf:resource="http://www.project-best.eu/owl/aixm-mod/airportheliport#CodeRunwayProtectionAreaType"/>
        <rdfs:comment xml:lang="en">Obstacle free zone or surface</rdfs:comment>
    </owl:NamedIndividual>
    


    <!-- http://www.project-best.eu/owl/aixm-mod/airportheliport#CodeRunwayProtectionAreaBaseType-OTHER -->

    <owl:NamedIndividual rdf:about="http://www.project-best.eu/owl/aixm-mod/airportheliport#CodeRunwayProtectionAreaBaseType-OTHER">
        <rdf:type rdf:resource="http://www.project-best.eu/owl/aixm-mod/airportheliport#CodeRunwayProtectionAreaType"/>
        <rdfs:comment xml:lang="en">Other.</rdfs:comment>
    </owl:NamedIndividual>
    


    <!-- http://www.project-best.eu/owl/aixm-mod/airportheliport#CodeRunwayProtectionAreaBaseType-POFZ -->

    <owl:NamedIndividual rdf:about="http://www.project-best.eu/owl/aixm-mod/airportheliport#CodeRunwayProtectionAreaBaseType-POFZ">
        <rdf:type rdf:resource="http://www.project-best.eu/owl/aixm-mod/airportheliport#CodeRunwayProtectionAreaType"/>
        <rdfs:comment xml:lang="en">Precision Obstacle Free Zone</rdfs:comment>
    </owl:NamedIndividual>
    


    <!-- http://www.project-best.eu/owl/aixm-mod/airportheliport#CodeRunwayProtectionAreaBaseType-RESA -->

    <owl:NamedIndividual rdf:about="http://www.project-best.eu/owl/aixm-mod/airportheliport#CodeRunwayProtectionAreaBaseType-RESA">
        <rdf:type rdf:resource="http://www.project-best.eu/owl/aixm-mod/airportheliport#CodeRunwayProtectionAreaType"/>
        <rdfs:comment xml:lang="en">Runway end safety area.</rdfs:comment>
    </owl:NamedIndividual>
    


    <!-- http://www.project-best.eu/owl/aixm-mod/airportheliport#CodeRunwayProtectionAreaBaseType-STOPWAY -->

    <owl:NamedIndividual rdf:about="http://www.project-best.eu/owl/aixm-mod/airportheliport#CodeRunwayProtectionAreaBaseType-STOPWAY">
        <rdf:type rdf:resource="http://www.project-best.eu/owl/aixm-mod/airportheliport#CodeRunwayProtectionAreaType"/>
        <rdfs:comment xml:lang="en">A defined rectangular area on the ground at the end of take-off run available prepared as a suitable area in which an aircraft can be stopped in the case of an abandoned take-off.</rdfs:comment>
    </owl:NamedIndividual>
    


    <!-- http://www.project-best.eu/owl/aixm-mod/airportheliport#CodeRunwayProtectionAreaBaseType-VGSI -->

    <owl:NamedIndividual rdf:about="http://www.project-best.eu/owl/aixm-mod/airportheliport#CodeRunwayProtectionAreaBaseType-VGSI">
        <rdf:type rdf:resource="http://www.project-best.eu/owl/aixm-mod/airportheliport#CodeRunwayProtectionAreaType"/>
        <rdfs:comment xml:lang="en">Visual Glide Slope Indicator (VGSI) protection area.  Protects VGSI signal coverage by forbidding objects in the area.</rdfs:comment>
    </owl:NamedIndividual>
    


    <!-- http://www.project-best.eu/owl/aixm-mod/airportheliport#CodeRunwaySectionBaseType-1_THIRD -->

    <owl:NamedIndividual rdf:about="http://www.project-best.eu/owl/aixm-mod/airportheliport#CodeRunwaySectionBaseType-1_THIRD">
        <rdf:type rdf:resource="http://www.project-best.eu/owl/aixm-mod/airportheliport#CodeRunwaySectionType"/>
        <rdfs:comment xml:lang="en">The first third of the runway, starting from the threshold with the lower designation number.</rdfs:comment>
    </owl:NamedIndividual>
    


    <!-- http://www.project-best.eu/owl/aixm-mod/airportheliport#CodeRunwaySectionBaseType-2_THIRD -->

    <owl:NamedIndividual rdf:about="http://www.project-best.eu/owl/aixm-mod/airportheliport#CodeRunwaySectionBaseType-2_THIRD">
        <rdf:type rdf:resource="http://www.project-best.eu/owl/aixm-mod/airportheliport#CodeRunwaySectionType"/>
        <rdfs:comment xml:lang="en">The second third of the runway, starting from the threshold with the lower designation number.</rdfs:comment>
    </owl:NamedIndividual>
    


    <!-- http://www.project-best.eu/owl/aixm-mod/airportheliport#CodeRunwaySectionBaseType-3_THIRD -->

    <owl:NamedIndividual rdf:about="http://www.project-best.eu/owl/aixm-mod/airportheliport#CodeRunwaySectionBaseType-3_THIRD">
        <rdf:type rdf:resource="http://www.project-best.eu/owl/aixm-mod/airportheliport#CodeRunwaySectionType"/>
        <rdfs:comment xml:lang="en">The last third of the runway, starting from the threshold with the lower designation number.</rdfs:comment>
    </owl:NamedIndividual>
    


    <!-- http://www.project-best.eu/owl/aixm-mod/airportheliport#CodeRunwaySectionBaseType-AFT_THR -->

    <owl:NamedIndividual rdf:about="http://www.project-best.eu/owl/aixm-mod/airportheliport#CodeRunwaySectionBaseType-AFT_THR">
        <rdf:type rdf:resource="http://www.project-best.eu/owl/aixm-mod/airportheliport#CodeRunwaySectionType"/>
        <rdfs:comment xml:lang="en">After threshold (for fixed distance markings.)</rdfs:comment>
    </owl:NamedIndividual>
    


    <!-- http://www.project-best.eu/owl/aixm-mod/airportheliport#CodeRunwaySectionBaseType-AIM -->

    <owl:NamedIndividual rdf:about="http://www.project-best.eu/owl/aixm-mod/airportheliport#CodeRunwaySectionBaseType-AIM">
        <rdf:type rdf:resource="http://www.project-best.eu/owl/aixm-mod/airportheliport#CodeRunwaySectionType"/>
        <rdfs:comment xml:lang="en">Aiming point.</rdfs:comment>
    </owl:NamedIndividual>
    


    <!-- http://www.project-best.eu/owl/aixm-mod/airportheliport#CodeRunwaySectionBaseType-CL -->

    <owl:NamedIndividual rdf:about="http://www.project-best.eu/owl/aixm-mod/airportheliport#CodeRunwaySectionBaseType-CL">
        <rdf:type rdf:resource="http://www.project-best.eu/owl/aixm-mod/airportheliport#CodeRunwaySectionType"/>
        <rdfs:comment xml:lang="en">Centre line.</rdfs:comment>
    </owl:NamedIndividual>
    


    <!-- http://www.project-best.eu/owl/aixm-mod/airportheliport#CodeRunwaySectionBaseType-DESIG -->

    <owl:NamedIndividual rdf:about="http://www.project-best.eu/owl/aixm-mod/airportheliport#CodeRunwaySectionBaseType-DESIG">
        <rdf:type rdf:resource="http://www.project-best.eu/owl/aixm-mod/airportheliport#CodeRunwaySectionType"/>
        <rdfs:comment xml:lang="en">Runway designation.</rdfs:comment>
    </owl:NamedIndividual>
    


    <!-- http://www.project-best.eu/owl/aixm-mod/airportheliport#CodeRunwaySectionBaseType-DTHR -->

    <owl:NamedIndividual rdf:about="http://www.project-best.eu/owl/aixm-mod/airportheliport#CodeRunwaySectionBaseType-DTHR">
        <rdf:type rdf:resource="http://www.project-best.eu/owl/aixm-mod/airportheliport#CodeRunwaySectionType"/>
        <rdfs:comment xml:lang="en">Displaced threshold.</rdfs:comment>
    </owl:NamedIndividual>
    


    <!-- http://www.project-best.eu/owl/aixm-mod/airportheliport#CodeRunwaySectionBaseType-EDGE -->

    <owl:NamedIndividual rdf:about="http://www.project-best.eu/owl/aixm-mod/airportheliport#CodeRunwaySectionBaseType-EDGE">
        <rdf:type rdf:resource="http://www.project-best.eu/owl/aixm-mod/airportheliport#CodeRunwaySectionType"/>
        <rdfs:comment xml:lang="en">Edge.</rdfs:comment>
    </owl:NamedIndividual>
    


    <!-- http://www.project-best.eu/owl/aixm-mod/airportheliport#CodeRunwaySectionBaseType-END -->

    <owl:NamedIndividual rdf:about="http://www.project-best.eu/owl/aixm-mod/airportheliport#CodeRunwaySectionBaseType-END">
        <rdf:type rdf:resource="http://www.project-best.eu/owl/aixm-mod/airportheliport#CodeRunwaySectionType"/>
        <rdfs:comment xml:lang="en">Runway end.</rdfs:comment>
    </owl:NamedIndividual>
    


    <!-- http://www.project-best.eu/owl/aixm-mod/airportheliport#CodeRunwaySectionBaseType-OTHER -->

    <owl:NamedIndividual rdf:about="http://www.project-best.eu/owl/aixm-mod/airportheliport#CodeRunwaySectionBaseType-OTHER">
        <rdf:type rdf:resource="http://www.project-best.eu/owl/aixm-mod/airportheliport#CodeRunwaySectionType"/>
        <rdfs:comment xml:lang="en">Other.</rdfs:comment>
    </owl:NamedIndividual>
    


    <!-- http://www.project-best.eu/owl/aixm-mod/airportheliport#CodeRunwaySectionBaseType-RPD_TWY_INT -->

    <owl:NamedIndividual rdf:about="http://www.project-best.eu/owl/aixm-mod/airportheliport#CodeRunwaySectionBaseType-RPD_TWY_INT">
        <rdf:type rdf:resource="http://www.project-best.eu/owl/aixm-mod/airportheliport#CodeRunwaySectionType"/>
        <rdfs:comment xml:lang="en">Rapid taxiway intersection.</rdfs:comment>
    </owl:NamedIndividual>
    


    <!-- http://www.project-best.eu/owl/aixm-mod/airportheliport#CodeRunwaySectionBaseType-TDZ -->

    <owl:NamedIndividual rdf:about="http://www.project-best.eu/owl/aixm-mod/airportheliport#CodeRunwaySectionBaseType-TDZ">
        <rdf:type rdf:resource="http://www.project-best.eu/owl/aixm-mod/airportheliport#CodeRunwaySectionType"/>
        <rdfs:comment xml:lang="en">Touch down zone.</rdfs:comment>
    </owl:NamedIndividual>
    


    <!-- http://www.project-best.eu/owl/aixm-mod/airportheliport#CodeRunwaySectionBaseType-THR -->

    <owl:NamedIndividual rdf:about="http://www.project-best.eu/owl/aixm-mod/airportheliport#CodeRunwaySectionBaseType-THR">
        <rdf:type rdf:resource="http://www.project-best.eu/owl/aixm-mod/airportheliport#CodeRunwaySectionType"/>
        <rdfs:comment xml:lang="en">Threshold.</rdfs:comment>
    </owl:NamedIndividual>
    


    <!-- http://www.project-best.eu/owl/aixm-mod/airportheliport#CodeRunwaySectionBaseType-TWY_INT -->

    <owl:NamedIndividual rdf:about="http://www.project-best.eu/owl/aixm-mod/airportheliport#CodeRunwaySectionBaseType-TWY_INT">
        <rdf:type rdf:resource="http://www.project-best.eu/owl/aixm-mod/airportheliport#CodeRunwaySectionType"/>
        <rdfs:comment xml:lang="en">Taxiway intersection.</rdfs:comment>
    </owl:NamedIndividual>
    


    <!-- http://www.project-best.eu/owl/aixm-mod/airportheliport#CodeSideBaseType-BOTH -->

    <owl:NamedIndividual rdf:about="http://www.project-best.eu/owl/aixm-mod/airportheliport#CodeSideBaseType-BOTH">
        <rdf:type rdf:resource="http://www.project-best.eu/owl/aixm-mod/airportheliport#CodeSideType"/>
        <rdfs:comment xml:lang="en">Distributed on both sides of the axis.</rdfs:comment>
    </owl:NamedIndividual>
    


    <!-- http://www.project-best.eu/owl/aixm-mod/airportheliport#CodeSideBaseType-LEFT -->

    <owl:NamedIndividual rdf:about="http://www.project-best.eu/owl/aixm-mod/airportheliport#CodeSideBaseType-LEFT">
        <rdf:type rdf:resource="http://www.project-best.eu/owl/aixm-mod/airportheliport#CodeSideType"/>
        <rdfs:comment xml:lang="en">On the left side of the axis.</rdfs:comment>
    </owl:NamedIndividual>
    


    <!-- http://www.project-best.eu/owl/aixm-mod/airportheliport#CodeSideBaseType-OTHER -->

    <owl:NamedIndividual rdf:about="http://www.project-best.eu/owl/aixm-mod/airportheliport#CodeSideBaseType-OTHER">
        <rdf:type rdf:resource="http://www.project-best.eu/owl/aixm-mod/airportheliport#CodeSideType"/>
        <rdfs:comment xml:lang="en">Another position.</rdfs:comment>
    </owl:NamedIndividual>
    


    <!-- http://www.project-best.eu/owl/aixm-mod/airportheliport#CodeSideBaseType-RIGHT -->

    <owl:NamedIndividual rdf:about="http://www.project-best.eu/owl/aixm-mod/airportheliport#CodeSideBaseType-RIGHT">
        <rdf:type rdf:resource="http://www.project-best.eu/owl/aixm-mod/airportheliport#CodeSideType"/>
        <rdfs:comment xml:lang="en">On the right side of the axis.</rdfs:comment>
    </owl:NamedIndividual>
    


    <!-- http://www.project-best.eu/owl/aixm-mod/airportheliport#CodeStatusAirportBaseType-CLOSED -->

    <owl:NamedIndividual rdf:about="http://www.project-best.eu/owl/aixm-mod/airportheliport#CodeStatusAirportBaseType-CLOSED">
        <rdf:type rdf:resource="http://www.project-best.eu/owl/aixm-mod/airportheliport#CodeStatusAirportType"/>
        <rdfs:comment xml:lang="en">The facility is not operational.</rdfs:comment>
    </owl:NamedIndividual>
    


    <!-- http://www.project-best.eu/owl/aixm-mod/airportheliport#CodeStatusAirportBaseType-LIMITED -->

    <owl:NamedIndividual rdf:about="http://www.project-best.eu/owl/aixm-mod/airportheliport#CodeStatusAirportBaseType-LIMITED">
        <rdf:type rdf:resource="http://www.project-best.eu/owl/aixm-mod/airportheliport#CodeStatusAirportType"/>
        <rdfs:comment xml:lang="en">The facility operates below its nominal parameters, with additional usage restrictions.</rdfs:comment>
    </owl:NamedIndividual>
    


    <!-- http://www.project-best.eu/owl/aixm-mod/airportheliport#CodeStatusAirportBaseType-NORMAL -->

    <owl:NamedIndividual rdf:about="http://www.project-best.eu/owl/aixm-mod/airportheliport#CodeStatusAirportBaseType-NORMAL">
        <rdf:type rdf:resource="http://www.project-best.eu/owl/aixm-mod/airportheliport#CodeStatusAirportType"/>
        <rdfs:comment xml:lang="en">The facility operates with nominal parameters.</rdfs:comment>
    </owl:NamedIndividual>
    


    <!-- http://www.project-best.eu/owl/aixm-mod/airportheliport#CodeStatusAirportBaseType-OTHER -->

    <owl:NamedIndividual rdf:about="http://www.project-best.eu/owl/aixm-mod/airportheliport#CodeStatusAirportBaseType-OTHER">
        <rdf:type rdf:resource="http://www.project-best.eu/owl/aixm-mod/airportheliport#CodeStatusAirportType"/>
        <rdfs:comment xml:lang="en">Other.</rdfs:comment>
    </owl:NamedIndividual>
    


    <!-- http://www.project-best.eu/owl/aixm-mod/airportheliport#CodeStatusConstructionBaseType-COMPLETED -->

    <owl:NamedIndividual rdf:about="http://www.project-best.eu/owl/aixm-mod/airportheliport#CodeStatusConstructionBaseType-COMPLETED">
        <rdf:type rdf:resource="http://www.project-best.eu/owl/aixm-mod/airportheliport#CodeStatusConstructionType"/>
        <rdfs:comment xml:lang="en">Completed.</rdfs:comment>
    </owl:NamedIndividual>
    


    <!-- http://www.project-best.eu/owl/aixm-mod/airportheliport#CodeStatusConstructionBaseType-DEMOLITION_PLANNED -->

    <owl:NamedIndividual rdf:about="http://www.project-best.eu/owl/aixm-mod/airportheliport#CodeStatusConstructionBaseType-DEMOLITION_PLANNED">
        <rdf:type rdf:resource="http://www.project-best.eu/owl/aixm-mod/airportheliport#CodeStatusConstructionType"/>
        <rdfs:comment xml:lang="en">Removal is planned.</rdfs:comment>
    </owl:NamedIndividual>
    


    <!-- http://www.project-best.eu/owl/aixm-mod/airportheliport#CodeStatusConstructionBaseType-IN_CONSTRUCTION -->

    <owl:NamedIndividual rdf:about="http://www.project-best.eu/owl/aixm-mod/airportheliport#CodeStatusConstructionBaseType-IN_CONSTRUCTION">
        <rdf:type rdf:resource="http://www.project-best.eu/owl/aixm-mod/airportheliport#CodeStatusConstructionType"/>
        <rdfs:comment xml:lang="en">In Construction.</rdfs:comment>
    </owl:NamedIndividual>
    


    <!-- http://www.project-best.eu/owl/aixm-mod/airportheliport#CodeStatusConstructionBaseType-IN_DEMOLITION -->

    <owl:NamedIndividual rdf:about="http://www.project-best.eu/owl/aixm-mod/airportheliport#CodeStatusConstructionBaseType-IN_DEMOLITION">
        <rdf:type rdf:resource="http://www.project-best.eu/owl/aixm-mod/airportheliport#CodeStatusConstructionType"/>
        <rdfs:comment xml:lang="en">Work in progress to remove the item.</rdfs:comment>
    </owl:NamedIndividual>
    


    <!-- http://www.project-best.eu/owl/aixm-mod/airportheliport#CodeStatusConstructionBaseType-OTHER -->

    <owl:NamedIndividual rdf:about="http://www.project-best.eu/owl/aixm-mod/airportheliport#CodeStatusConstructionBaseType-OTHER">
        <rdf:type rdf:resource="http://www.project-best.eu/owl/aixm-mod/airportheliport#CodeStatusConstructionType"/>
        <rdfs:comment xml:lang="en">Other</rdfs:comment>
    </owl:NamedIndividual>
    


    <!-- http://www.project-best.eu/owl/aixm-mod/airportheliport#CodeStatusOperationsBaseType-DOWNGRADED -->

    <owl:NamedIndividual rdf:about="http://www.project-best.eu/owl/aixm-mod/airportheliport#CodeStatusOperationsBaseType-DOWNGRADED">
        <rdf:type rdf:resource="http://www.project-best.eu/owl/aixm-mod/airportheliport#CodeStatusOperationsType"/>
        <rdfs:comment xml:lang="en">The system is theoretically able to work at a higher level of service, but it is currently limited to the level described.</rdfs:comment>
    </owl:NamedIndividual>
    


    <!-- http://www.project-best.eu/owl/aixm-mod/airportheliport#CodeStatusOperationsBaseType-NORMAL -->

    <owl:NamedIndividual rdf:about="http://www.project-best.eu/owl/aixm-mod/airportheliport#CodeStatusOperationsBaseType-NORMAL">
        <rdf:type rdf:resource="http://www.project-best.eu/owl/aixm-mod/airportheliport#CodeStatusOperationsType"/>
        <rdfs:comment xml:lang="en">Normal operations.</rdfs:comment>
    </owl:NamedIndividual>
    


    <!-- http://www.project-best.eu/owl/aixm-mod/airportheliport#CodeStatusOperationsBaseType-OTHER -->

    <owl:NamedIndividual rdf:about="http://www.project-best.eu/owl/aixm-mod/airportheliport#CodeStatusOperationsBaseType-OTHER">
        <rdf:type rdf:resource="http://www.project-best.eu/owl/aixm-mod/airportheliport#CodeStatusOperationsType"/>
        <rdfs:comment xml:lang="en">Other.</rdfs:comment>
    </owl:NamedIndividual>
    


    <!-- http://www.project-best.eu/owl/aixm-mod/airportheliport#CodeStatusOperationsBaseType-UNSERVICEABLE -->

    <owl:NamedIndividual rdf:about="http://www.project-best.eu/owl/aixm-mod/airportheliport#CodeStatusOperationsBaseType-UNSERVICEABLE">
        <rdf:type rdf:resource="http://www.project-best.eu/owl/aixm-mod/airportheliport#CodeStatusOperationsType"/>
        <rdfs:comment xml:lang="en">Operation is unserviceable (unavailable).</rdfs:comment>
    </owl:NamedIndividual>
    


    <!-- http://www.project-best.eu/owl/aixm-mod/airportheliport#CodeStatusOperationsBaseType-WORK_IN_PROGRESS -->

    <owl:NamedIndividual rdf:about="http://www.project-best.eu/owl/aixm-mod/airportheliport#CodeStatusOperationsBaseType-WORK_IN_PROGRESS">
        <rdf:type rdf:resource="http://www.project-best.eu/owl/aixm-mod/airportheliport#CodeStatusOperationsType"/>
        <rdfs:comment xml:lang="en">Operation is under construction.</rdfs:comment>
    </owl:NamedIndividual>
    


    <!-- http://www.project-best.eu/owl/aixm-mod/airportheliport#CodeSurfaceCompositionBaseType-ASPH -->

    <owl:NamedIndividual rdf:about="http://www.project-best.eu/owl/aixm-mod/airportheliport#CodeSurfaceCompositionBaseType-ASPH">
        <rdf:type rdf:resource="http://www.project-best.eu/owl/aixm-mod/airportheliport#CodeSurfaceCompositionType"/>
        <rdfs:comment xml:lang="en">Asphalt.</rdfs:comment>
    </owl:NamedIndividual>
    


    <!-- http://www.project-best.eu/owl/aixm-mod/airportheliport#CodeSurfaceCompositionBaseType-ASPH_GRASS -->

    <owl:NamedIndividual rdf:about="http://www.project-best.eu/owl/aixm-mod/airportheliport#CodeSurfaceCompositionBaseType-ASPH_GRASS">
        <rdf:type rdf:resource="http://www.project-best.eu/owl/aixm-mod/airportheliport#CodeSurfaceCompositionType"/>
        <rdfs:comment xml:lang="en">Asphalt and grass.</rdfs:comment>
    </owl:NamedIndividual>
    


    <!-- http://www.project-best.eu/owl/aixm-mod/airportheliport#CodeSurfaceCompositionBaseType-BITUM -->

    <owl:NamedIndividual rdf:about="http://www.project-best.eu/owl/aixm-mod/airportheliport#CodeSurfaceCompositionBaseType-BITUM">
        <rdf:type rdf:resource="http://www.project-best.eu/owl/aixm-mod/airportheliport#CodeSurfaceCompositionType"/>
        <rdfs:comment xml:lang="en">Bituminous tar or asphalt and/or oil or bitumen bound, mix-in-place surfaces (often referred to as &quot;earth cement&quot;). </rdfs:comment>
    </owl:NamedIndividual>
    


    <!-- http://www.project-best.eu/owl/aixm-mod/airportheliport#CodeSurfaceCompositionBaseType-BRICK -->

    <owl:NamedIndividual rdf:about="http://www.project-best.eu/owl/aixm-mod/airportheliport#CodeSurfaceCompositionBaseType-BRICK">
        <rdf:type rdf:resource="http://www.project-best.eu/owl/aixm-mod/airportheliport#CodeSurfaceCompositionType"/>
        <rdfs:comment xml:lang="en">Brick.</rdfs:comment>
    </owl:NamedIndividual>
    


    <!-- http://www.project-best.eu/owl/aixm-mod/airportheliport#CodeSurfaceCompositionBaseType-CLAY -->

    <owl:NamedIndividual rdf:about="http://www.project-best.eu/owl/aixm-mod/airportheliport#CodeSurfaceCompositionBaseType-CLAY">
        <rdf:type rdf:resource="http://www.project-best.eu/owl/aixm-mod/airportheliport#CodeSurfaceCompositionType"/>
        <rdfs:comment xml:lang="en">Clay.</rdfs:comment>
    </owl:NamedIndividual>
    


    <!-- http://www.project-best.eu/owl/aixm-mod/airportheliport#CodeSurfaceCompositionBaseType-CONC -->

    <owl:NamedIndividual rdf:about="http://www.project-best.eu/owl/aixm-mod/airportheliport#CodeSurfaceCompositionBaseType-CONC">
        <rdf:type rdf:resource="http://www.project-best.eu/owl/aixm-mod/airportheliport#CodeSurfaceCompositionType"/>
        <rdfs:comment xml:lang="en">Concrete.</rdfs:comment>
    </owl:NamedIndividual>
    


    <!-- http://www.project-best.eu/owl/aixm-mod/airportheliport#CodeSurfaceCompositionBaseType-CONC_ASPH -->

    <owl:NamedIndividual rdf:about="http://www.project-best.eu/owl/aixm-mod/airportheliport#CodeSurfaceCompositionBaseType-CONC_ASPH">
        <rdf:type rdf:resource="http://www.project-best.eu/owl/aixm-mod/airportheliport#CodeSurfaceCompositionType"/>
        <rdfs:comment xml:lang="en">Concrete and asphalt.</rdfs:comment>
    </owl:NamedIndividual>
    


    <!-- http://www.project-best.eu/owl/aixm-mod/airportheliport#CodeSurfaceCompositionBaseType-CONC_GRS -->

    <owl:NamedIndividual rdf:about="http://www.project-best.eu/owl/aixm-mod/airportheliport#CodeSurfaceCompositionBaseType-CONC_GRS">
        <rdf:type rdf:resource="http://www.project-best.eu/owl/aixm-mod/airportheliport#CodeSurfaceCompositionType"/>
        <rdfs:comment xml:lang="en">Concrete and grass.</rdfs:comment>
    </owl:NamedIndividual>
    


    <!-- http://www.project-best.eu/owl/aixm-mod/airportheliport#CodeSurfaceCompositionBaseType-CORAL -->

    <owl:NamedIndividual rdf:about="http://www.project-best.eu/owl/aixm-mod/airportheliport#CodeSurfaceCompositionBaseType-CORAL">
        <rdf:type rdf:resource="http://www.project-best.eu/owl/aixm-mod/airportheliport#CodeSurfaceCompositionType"/>
        <rdfs:comment xml:lang="en">Coral.</rdfs:comment>
    </owl:NamedIndividual>
    


    <!-- http://www.project-best.eu/owl/aixm-mod/airportheliport#CodeSurfaceCompositionBaseType-EARTH -->

    <owl:NamedIndividual rdf:about="http://www.project-best.eu/owl/aixm-mod/airportheliport#CodeSurfaceCompositionBaseType-EARTH">
        <rdf:type rdf:resource="http://www.project-best.eu/owl/aixm-mod/airportheliport#CodeSurfaceCompositionType"/>
        <rdfs:comment xml:lang="en">Earth (in general).</rdfs:comment>
    </owl:NamedIndividual>
    


    <!-- http://www.project-best.eu/owl/aixm-mod/airportheliport#CodeSurfaceCompositionBaseType-GRASS -->

    <owl:NamedIndividual rdf:about="http://www.project-best.eu/owl/aixm-mod/airportheliport#CodeSurfaceCompositionBaseType-GRASS">
        <rdf:type rdf:resource="http://www.project-best.eu/owl/aixm-mod/airportheliport#CodeSurfaceCompositionType"/>
        <rdfs:comment xml:lang="en">Grass including portions of turf or bare earth.</rdfs:comment>
    </owl:NamedIndividual>
    


    <!-- http://www.project-best.eu/owl/aixm-mod/airportheliport#CodeSurfaceCompositionBaseType-GRAVEL -->

    <owl:NamedIndividual rdf:about="http://www.project-best.eu/owl/aixm-mod/airportheliport#CodeSurfaceCompositionBaseType-GRAVEL">
        <rdf:type rdf:resource="http://www.project-best.eu/owl/aixm-mod/airportheliport#CodeSurfaceCompositionType"/>
        <rdfs:comment xml:lang="en">Gravel.</rdfs:comment>
    </owl:NamedIndividual>
    


    <!-- http://www.project-best.eu/owl/aixm-mod/airportheliport#CodeSurfaceCompositionBaseType-ICE -->

    <owl:NamedIndividual rdf:about="http://www.project-best.eu/owl/aixm-mod/airportheliport#CodeSurfaceCompositionBaseType-ICE">
        <rdf:type rdf:resource="http://www.project-best.eu/owl/aixm-mod/airportheliport#CodeSurfaceCompositionType"/>
        <rdfs:comment xml:lang="en">Ice.</rdfs:comment>
    </owl:NamedIndividual>
    


    <!-- http://www.project-best.eu/owl/aixm-mod/airportheliport#CodeSurfaceCompositionBaseType-LATERITE -->

    <owl:NamedIndividual rdf:about="http://www.project-best.eu/owl/aixm-mod/airportheliport#CodeSurfaceCompositionBaseType-LATERITE">
        <rdf:type rdf:resource="http://www.project-best.eu/owl/aixm-mod/airportheliport#CodeSurfaceCompositionType"/>
        <rdfs:comment xml:lang="en">Laterite - a high iron clay formed in tropical areas.</rdfs:comment>
    </owl:NamedIndividual>
    


    <!-- http://www.project-best.eu/owl/aixm-mod/airportheliport#CodeSurfaceCompositionBaseType-MACADAM -->

    <owl:NamedIndividual rdf:about="http://www.project-best.eu/owl/aixm-mod/airportheliport#CodeSurfaceCompositionBaseType-MACADAM">
        <rdf:type rdf:resource="http://www.project-best.eu/owl/aixm-mod/airportheliport#CodeSurfaceCompositionType"/>
        <rdfs:comment xml:lang="en">A macadam or tarmac surface consisting of water-bound crushed rock.</rdfs:comment>
    </owl:NamedIndividual>
    


    <!-- http://www.project-best.eu/owl/aixm-mod/airportheliport#CodeSurfaceCompositionBaseType-MATS -->

    <owl:NamedIndividual rdf:about="http://www.project-best.eu/owl/aixm-mod/airportheliport#CodeSurfaceCompositionBaseType-MATS">
        <rdf:type rdf:resource="http://www.project-best.eu/owl/aixm-mod/airportheliport#CodeSurfaceCompositionType"/>
        <rdfs:comment xml:lang="en">Landing mat portable system usually made of aluminium.</rdfs:comment>
    </owl:NamedIndividual>
    


    <!-- http://www.project-best.eu/owl/aixm-mod/airportheliport#CodeSurfaceCompositionBaseType-MEMBRANE -->

    <owl:NamedIndividual rdf:about="http://www.project-best.eu/owl/aixm-mod/airportheliport#CodeSurfaceCompositionBaseType-MEMBRANE">
        <rdf:type rdf:resource="http://www.project-best.eu/owl/aixm-mod/airportheliport#CodeSurfaceCompositionType"/>
        <rdfs:comment xml:lang="en">A protective laminate usually made of rubber.</rdfs:comment>
    </owl:NamedIndividual>
    


    <!-- http://www.project-best.eu/owl/aixm-mod/airportheliport#CodeSurfaceCompositionBaseType-METAL -->

    <owl:NamedIndividual rdf:about="http://www.project-best.eu/owl/aixm-mod/airportheliport#CodeSurfaceCompositionBaseType-METAL">
        <rdf:type rdf:resource="http://www.project-best.eu/owl/aixm-mod/airportheliport#CodeSurfaceCompositionType"/>
        <rdfs:comment xml:lang="en">Metal - steel, aluminium.</rdfs:comment>
    </owl:NamedIndividual>
    


    <!-- http://www.project-best.eu/owl/aixm-mod/airportheliport#CodeSurfaceCompositionBaseType-NON_BITUM_MIX -->

    <owl:NamedIndividual rdf:about="http://www.project-best.eu/owl/aixm-mod/airportheliport#CodeSurfaceCompositionBaseType-NON_BITUM_MIX">
        <rdf:type rdf:resource="http://www.project-best.eu/owl/aixm-mod/airportheliport#CodeSurfaceCompositionType"/>
        <rdfs:comment xml:lang="en">Non Bituminous mix.</rdfs:comment>
    </owl:NamedIndividual>
    


    <!-- http://www.project-best.eu/owl/aixm-mod/airportheliport#CodeSurfaceCompositionBaseType-OTHER -->

    <owl:NamedIndividual rdf:about="http://www.project-best.eu/owl/aixm-mod/airportheliport#CodeSurfaceCompositionBaseType-OTHER">
        <rdf:type rdf:resource="http://www.project-best.eu/owl/aixm-mod/airportheliport#CodeSurfaceCompositionType"/>
        <rdfs:comment xml:lang="en">Other.</rdfs:comment>
    </owl:NamedIndividual>
    


    <!-- http://www.project-best.eu/owl/aixm-mod/airportheliport#CodeSurfaceCompositionBaseType-PIERCED_STEEL -->

    <owl:NamedIndividual rdf:about="http://www.project-best.eu/owl/aixm-mod/airportheliport#CodeSurfaceCompositionBaseType-PIERCED_STEEL">
        <rdf:type rdf:resource="http://www.project-best.eu/owl/aixm-mod/airportheliport#CodeSurfaceCompositionType"/>
        <rdfs:comment xml:lang="en">Pierced steel planking.</rdfs:comment>
    </owl:NamedIndividual>
    


    <!-- http://www.project-best.eu/owl/aixm-mod/airportheliport#CodeSurfaceCompositionBaseType-SAND -->

    <owl:NamedIndividual rdf:about="http://www.project-best.eu/owl/aixm-mod/airportheliport#CodeSurfaceCompositionBaseType-SAND">
        <rdf:type rdf:resource="http://www.project-best.eu/owl/aixm-mod/airportheliport#CodeSurfaceCompositionType"/>
        <rdfs:comment xml:lang="en">Sand.</rdfs:comment>
    </owl:NamedIndividual>
    


    <!-- http://www.project-best.eu/owl/aixm-mod/airportheliport#CodeSurfaceCompositionBaseType-SNOW -->

    <owl:NamedIndividual rdf:about="http://www.project-best.eu/owl/aixm-mod/airportheliport#CodeSurfaceCompositionBaseType-SNOW">
        <rdf:type rdf:resource="http://www.project-best.eu/owl/aixm-mod/airportheliport#CodeSurfaceCompositionType"/>
        <rdfs:comment xml:lang="en">Snow.</rdfs:comment>
    </owl:NamedIndividual>
    


    <!-- http://www.project-best.eu/owl/aixm-mod/airportheliport#CodeSurfaceCompositionBaseType-STONE -->

    <owl:NamedIndividual rdf:about="http://www.project-best.eu/owl/aixm-mod/airportheliport#CodeSurfaceCompositionBaseType-STONE">
        <rdf:type rdf:resource="http://www.project-best.eu/owl/aixm-mod/airportheliport#CodeSurfaceCompositionType"/>
        <rdfs:comment xml:lang="en">Stone.</rdfs:comment>
    </owl:NamedIndividual>
    


    <!-- http://www.project-best.eu/owl/aixm-mod/airportheliport#CodeSurfaceCompositionBaseType-WATER -->

    <owl:NamedIndividual rdf:about="http://www.project-best.eu/owl/aixm-mod/airportheliport#CodeSurfaceCompositionBaseType-WATER">
        <rdf:type rdf:resource="http://www.project-best.eu/owl/aixm-mod/airportheliport#CodeSurfaceCompositionType"/>
        <rdfs:comment xml:lang="en">Water.</rdfs:comment>
    </owl:NamedIndividual>
    


    <!-- http://www.project-best.eu/owl/aixm-mod/airportheliport#CodeSurfaceCompositionBaseType-WOOD -->

    <owl:NamedIndividual rdf:about="http://www.project-best.eu/owl/aixm-mod/airportheliport#CodeSurfaceCompositionBaseType-WOOD">
        <rdf:type rdf:resource="http://www.project-best.eu/owl/aixm-mod/airportheliport#CodeSurfaceCompositionType"/>
        <rdfs:comment xml:lang="en">Wood.</rdfs:comment>
    </owl:NamedIndividual>
    


    <!-- http://www.project-best.eu/owl/aixm-mod/airportheliport#CodeSurfaceConditionBaseType-DEFORMED -->

    <owl:NamedIndividual rdf:about="http://www.project-best.eu/owl/aixm-mod/airportheliport#CodeSurfaceConditionBaseType-DEFORMED">
        <rdf:type rdf:resource="http://www.project-best.eu/owl/aixm-mod/airportheliport#CodeSurfaceConditionType"/>
        <rdfs:comment xml:lang="en">Presenting deformations.</rdfs:comment>
    </owl:NamedIndividual>
    


    <!-- http://www.project-best.eu/owl/aixm-mod/airportheliport#CodeSurfaceConditionBaseType-FAIR -->

    <owl:NamedIndividual rdf:about="http://www.project-best.eu/owl/aixm-mod/airportheliport#CodeSurfaceConditionBaseType-FAIR">
        <rdf:type rdf:resource="http://www.project-best.eu/owl/aixm-mod/airportheliport#CodeSurfaceConditionType"/>
        <rdfs:comment xml:lang="en">Fair.</rdfs:comment>
    </owl:NamedIndividual>
    


    <!-- http://www.project-best.eu/owl/aixm-mod/airportheliport#CodeSurfaceConditionBaseType-GOOD -->

    <owl:NamedIndividual rdf:about="http://www.project-best.eu/owl/aixm-mod/airportheliport#CodeSurfaceConditionBaseType-GOOD">
        <rdf:type rdf:resource="http://www.project-best.eu/owl/aixm-mod/airportheliport#CodeSurfaceConditionType"/>
        <rdfs:comment xml:lang="en">Good.</rdfs:comment>
    </owl:NamedIndividual>
    


    <!-- http://www.project-best.eu/owl/aixm-mod/airportheliport#CodeSurfaceConditionBaseType-OTHER -->

    <owl:NamedIndividual rdf:about="http://www.project-best.eu/owl/aixm-mod/airportheliport#CodeSurfaceConditionBaseType-OTHER">
        <rdf:type rdf:resource="http://www.project-best.eu/owl/aixm-mod/airportheliport#CodeSurfaceConditionType"/>
        <rdfs:comment xml:lang="en">Other.</rdfs:comment>
    </owl:NamedIndividual>
    


    <!-- http://www.project-best.eu/owl/aixm-mod/airportheliport#CodeSurfaceConditionBaseType-POOR -->

    <owl:NamedIndividual rdf:about="http://www.project-best.eu/owl/aixm-mod/airportheliport#CodeSurfaceConditionBaseType-POOR">
        <rdf:type rdf:resource="http://www.project-best.eu/owl/aixm-mod/airportheliport#CodeSurfaceConditionType"/>
        <rdfs:comment xml:lang="en">Poor.</rdfs:comment>
    </owl:NamedIndividual>
    


    <!-- http://www.project-best.eu/owl/aixm-mod/airportheliport#CodeSurfaceConditionBaseType-UNSAFE -->

    <owl:NamedIndividual rdf:about="http://www.project-best.eu/owl/aixm-mod/airportheliport#CodeSurfaceConditionBaseType-UNSAFE">
        <rdf:type rdf:resource="http://www.project-best.eu/owl/aixm-mod/airportheliport#CodeSurfaceConditionType"/>
        <rdfs:comment xml:lang="en">Unsafe for use.</rdfs:comment>
    </owl:NamedIndividual>
    


    <!-- http://www.project-best.eu/owl/aixm-mod/airportheliport#CodeSurfacePreparationBaseType-AFSC -->

    <owl:NamedIndividual rdf:about="http://www.project-best.eu/owl/aixm-mod/airportheliport#CodeSurfacePreparationBaseType-AFSC">
        <rdf:type rdf:resource="http://www.project-best.eu/owl/aixm-mod/airportheliport#CodeSurfacePreparationType"/>
        <rdfs:comment xml:lang="en">Aggregate friction seal coat.</rdfs:comment>
    </owl:NamedIndividual>
    


    <!-- http://www.project-best.eu/owl/aixm-mod/airportheliport#CodeSurfacePreparationBaseType-COMPACTED -->

    <owl:NamedIndividual rdf:about="http://www.project-best.eu/owl/aixm-mod/airportheliport#CodeSurfacePreparationBaseType-COMPACTED">
        <rdf:type rdf:resource="http://www.project-best.eu/owl/aixm-mod/airportheliport#CodeSurfacePreparationType"/>
        <rdfs:comment xml:lang="en">Compacted</rdfs:comment>
    </owl:NamedIndividual>
    


    <!-- http://www.project-best.eu/owl/aixm-mod/airportheliport#CodeSurfacePreparationBaseType-GRADED -->

    <owl:NamedIndividual rdf:about="http://www.project-best.eu/owl/aixm-mod/airportheliport#CodeSurfacePreparationBaseType-GRADED">
        <rdf:type rdf:resource="http://www.project-best.eu/owl/aixm-mod/airportheliport#CodeSurfacePreparationType"/>
        <rdfs:comment xml:lang="en">Graded.</rdfs:comment>
    </owl:NamedIndividual>
    


    <!-- http://www.project-best.eu/owl/aixm-mod/airportheliport#CodeSurfacePreparationBaseType-GROOVED -->

    <owl:NamedIndividual rdf:about="http://www.project-best.eu/owl/aixm-mod/airportheliport#CodeSurfacePreparationBaseType-GROOVED">
        <rdf:type rdf:resource="http://www.project-best.eu/owl/aixm-mod/airportheliport#CodeSurfacePreparationType"/>
        <rdfs:comment xml:lang="en">Cut or plastic grooved.</rdfs:comment>
    </owl:NamedIndividual>
    


    <!-- http://www.project-best.eu/owl/aixm-mod/airportheliport#CodeSurfacePreparationBaseType-NATURAL -->

    <owl:NamedIndividual rdf:about="http://www.project-best.eu/owl/aixm-mod/airportheliport#CodeSurfacePreparationBaseType-NATURAL">
        <rdf:type rdf:resource="http://www.project-best.eu/owl/aixm-mod/airportheliport#CodeSurfacePreparationType"/>
        <rdfs:comment xml:lang="en">Natural surface; no treatment.</rdfs:comment>
    </owl:NamedIndividual>
    


    <!-- http://www.project-best.eu/owl/aixm-mod/airportheliport#CodeSurfacePreparationBaseType-NON_GROOVED -->

    <owl:NamedIndividual rdf:about="http://www.project-best.eu/owl/aixm-mod/airportheliport#CodeSurfacePreparationBaseType-NON_GROOVED">
        <rdf:type rdf:resource="http://www.project-best.eu/owl/aixm-mod/airportheliport#CodeSurfacePreparationType"/>
        <rdfs:comment xml:lang="en">This covers such items as &apos;APSHALT NON GROOVED&apos; .</rdfs:comment>
    </owl:NamedIndividual>
    


    <!-- http://www.project-best.eu/owl/aixm-mod/airportheliport#CodeSurfacePreparationBaseType-OILED -->

    <owl:NamedIndividual rdf:about="http://www.project-best.eu/owl/aixm-mod/airportheliport#CodeSurfacePreparationBaseType-OILED">
        <rdf:type rdf:resource="http://www.project-best.eu/owl/aixm-mod/airportheliport#CodeSurfacePreparationType"/>
        <rdfs:comment xml:lang="en">Oiled.</rdfs:comment>
    </owl:NamedIndividual>
    


    <!-- http://www.project-best.eu/owl/aixm-mod/airportheliport#CodeSurfacePreparationBaseType-OTHER -->

    <owl:NamedIndividual rdf:about="http://www.project-best.eu/owl/aixm-mod/airportheliport#CodeSurfacePreparationBaseType-OTHER">
        <rdf:type rdf:resource="http://www.project-best.eu/owl/aixm-mod/airportheliport#CodeSurfacePreparationType"/>
        <rdfs:comment xml:lang="en">Other.</rdfs:comment>
    </owl:NamedIndividual>
    


    <!-- http://www.project-best.eu/owl/aixm-mod/airportheliport#CodeSurfacePreparationBaseType-PAVED -->

    <owl:NamedIndividual rdf:about="http://www.project-best.eu/owl/aixm-mod/airportheliport#CodeSurfacePreparationBaseType-PAVED">
        <rdf:type rdf:resource="http://www.project-best.eu/owl/aixm-mod/airportheliport#CodeSurfacePreparationType"/>
        <rdfs:comment xml:lang="en">Paved.</rdfs:comment>
    </owl:NamedIndividual>
    


    <!-- http://www.project-best.eu/owl/aixm-mod/airportheliport#CodeSurfacePreparationBaseType-PFC -->

    <owl:NamedIndividual rdf:about="http://www.project-best.eu/owl/aixm-mod/airportheliport#CodeSurfacePreparationBaseType-PFC">
        <rdf:type rdf:resource="http://www.project-best.eu/owl/aixm-mod/airportheliport#CodeSurfacePreparationType"/>
        <rdfs:comment xml:lang="en">Porous friction coat.</rdfs:comment>
    </owl:NamedIndividual>
    


    <!-- http://www.project-best.eu/owl/aixm-mod/airportheliport#CodeSurfacePreparationBaseType-RFSC -->

    <owl:NamedIndividual rdf:about="http://www.project-best.eu/owl/aixm-mod/airportheliport#CodeSurfacePreparationBaseType-RFSC">
        <rdf:type rdf:resource="http://www.project-best.eu/owl/aixm-mod/airportheliport#CodeSurfacePreparationType"/>
        <rdfs:comment xml:lang="en">Rubberised friction seal coat.</rdfs:comment>
    </owl:NamedIndividual>
    


    <!-- http://www.project-best.eu/owl/aixm-mod/airportheliport#CodeSurfacePreparationBaseType-ROLLED -->

    <owl:NamedIndividual rdf:about="http://www.project-best.eu/owl/aixm-mod/airportheliport#CodeSurfacePreparationBaseType-ROLLED">
        <rdf:type rdf:resource="http://www.project-best.eu/owl/aixm-mod/airportheliport#CodeSurfacePreparationType"/>
        <rdfs:comment xml:lang="en">Rolled.</rdfs:comment>
    </owl:NamedIndividual>
    


    <!-- http://www.project-best.eu/owl/aixm-mod/airportheliport#CodeSystemActivationBaseType-OFF -->

    <owl:NamedIndividual rdf:about="http://www.project-best.eu/owl/aixm-mod/airportheliport#CodeSystemActivationBaseType-OFF">
        <rdf:type rdf:resource="http://www.project-best.eu/owl/aixm-mod/airportheliport#CodeSystemActivationType"/>
        <rdfs:comment xml:lang="en">System in status &quot;off-line&quot;.</rdfs:comment>
    </owl:NamedIndividual>
    


    <!-- http://www.project-best.eu/owl/aixm-mod/airportheliport#CodeSystemActivationBaseType-ON -->

    <owl:NamedIndividual rdf:about="http://www.project-best.eu/owl/aixm-mod/airportheliport#CodeSystemActivationBaseType-ON">
        <rdf:type rdf:resource="http://www.project-best.eu/owl/aixm-mod/airportheliport#CodeSystemActivationType"/>
        <rdfs:comment xml:lang="en">System in status &quot;on-line&quot;.</rdfs:comment>
    </owl:NamedIndividual>
    


    <!-- http://www.project-best.eu/owl/aixm-mod/airportheliport#CodeSystemActivationBaseType-ON_OR_OFF -->

    <owl:NamedIndividual rdf:about="http://www.project-best.eu/owl/aixm-mod/airportheliport#CodeSystemActivationBaseType-ON_OR_OFF">
        <rdf:type rdf:resource="http://www.project-best.eu/owl/aixm-mod/airportheliport#CodeSystemActivationType"/>
        <rdfs:comment xml:lang="en">System changes between &quot;ON&quot; and &quot;OFF&quot;, depending on the previous state.</rdfs:comment>
    </owl:NamedIndividual>
    


    <!-- http://www.project-best.eu/owl/aixm-mod/airportheliport#CodeSystemActivationBaseType-OTHER -->

    <owl:NamedIndividual rdf:about="http://www.project-best.eu/owl/aixm-mod/airportheliport#CodeSystemActivationBaseType-OTHER">
        <rdf:type rdf:resource="http://www.project-best.eu/owl/aixm-mod/airportheliport#CodeSystemActivationType"/>
        <rdfs:comment xml:lang="en">Other</rdfs:comment>
    </owl:NamedIndividual>
    


    <!-- http://www.project-best.eu/owl/aixm-mod/airportheliport#CodeTLOFSectionBaseType-AIM -->

    <owl:NamedIndividual rdf:about="http://www.project-best.eu/owl/aixm-mod/airportheliport#CodeTLOFSectionBaseType-AIM">
        <rdf:type rdf:resource="http://www.project-best.eu/owl/aixm-mod/airportheliport#CodeTLOFSectionType"/>
        <rdfs:comment xml:lang="en">Aiming point.</rdfs:comment>
    </owl:NamedIndividual>
    


    <!-- http://www.project-best.eu/owl/aixm-mod/airportheliport#CodeTLOFSectionBaseType-EDGE -->

    <owl:NamedIndividual rdf:about="http://www.project-best.eu/owl/aixm-mod/airportheliport#CodeTLOFSectionBaseType-EDGE">
        <rdf:type rdf:resource="http://www.project-best.eu/owl/aixm-mod/airportheliport#CodeTLOFSectionType"/>
        <rdfs:comment xml:lang="en">TLOF edge.</rdfs:comment>
    </owl:NamedIndividual>
    


    <!-- http://www.project-best.eu/owl/aixm-mod/airportheliport#CodeTLOFSectionBaseType-OTHER -->

    <owl:NamedIndividual rdf:about="http://www.project-best.eu/owl/aixm-mod/airportheliport#CodeTLOFSectionBaseType-OTHER">
        <rdf:type rdf:resource="http://www.project-best.eu/owl/aixm-mod/airportheliport#CodeTLOFSectionType"/>
        <rdfs:comment xml:lang="en">Other.</rdfs:comment>
    </owl:NamedIndividual>
    


    <!-- http://www.project-best.eu/owl/aixm-mod/airportheliport#CodeTaxiwayBaseType-AIR -->

    <owl:NamedIndividual rdf:about="http://www.project-best.eu/owl/aixm-mod/airportheliport#CodeTaxiwayBaseType-AIR">
        <rdf:type rdf:resource="http://www.project-best.eu/owl/aixm-mod/airportheliport#CodeTaxiwayType"/>
        <rdfs:comment xml:lang="en">Air taxiway.</rdfs:comment>
    </owl:NamedIndividual>
    


    <!-- http://www.project-best.eu/owl/aixm-mod/airportheliport#CodeTaxiwayBaseType-BYPASS -->

    <owl:NamedIndividual rdf:about="http://www.project-best.eu/owl/aixm-mod/airportheliport#CodeTaxiwayBaseType-BYPASS">
        <rdf:type rdf:resource="http://www.project-best.eu/owl/aixm-mod/airportheliport#CodeTaxiwayType"/>
        <rdfs:comment xml:lang="en">Bypass holding bay.</rdfs:comment>
    </owl:NamedIndividual>
    


    <!-- http://www.project-best.eu/owl/aixm-mod/airportheliport#CodeTaxiwayBaseType-EXIT -->

    <owl:NamedIndividual rdf:about="http://www.project-best.eu/owl/aixm-mod/airportheliport#CodeTaxiwayBaseType-EXIT">
        <rdf:type rdf:resource="http://www.project-best.eu/owl/aixm-mod/airportheliport#CodeTaxiwayType"/>
        <rdfs:comment xml:lang="en">Exit/turnoff taxiway.</rdfs:comment>
    </owl:NamedIndividual>
    


    <!-- http://www.project-best.eu/owl/aixm-mod/airportheliport#CodeTaxiwayBaseType-FASTEXIT -->

    <owl:NamedIndividual rdf:about="http://www.project-best.eu/owl/aixm-mod/airportheliport#CodeTaxiwayBaseType-FASTEXIT">
        <rdf:type rdf:resource="http://www.project-best.eu/owl/aixm-mod/airportheliport#CodeTaxiwayType"/>
        <rdfs:comment xml:lang="en">Rapid exit/turnoff taxiway.</rdfs:comment>
    </owl:NamedIndividual>
    


    <!-- http://www.project-best.eu/owl/aixm-mod/airportheliport#CodeTaxiwayBaseType-GND -->

    <owl:NamedIndividual rdf:about="http://www.project-best.eu/owl/aixm-mod/airportheliport#CodeTaxiwayBaseType-GND">
        <rdf:type rdf:resource="http://www.project-best.eu/owl/aixm-mod/airportheliport#CodeTaxiwayType"/>
        <rdfs:comment xml:lang="en">Ground taxiway.</rdfs:comment>
    </owl:NamedIndividual>
    


    <!-- http://www.project-best.eu/owl/aixm-mod/airportheliport#CodeTaxiwayBaseType-OTHER -->

    <owl:NamedIndividual rdf:about="http://www.project-best.eu/owl/aixm-mod/airportheliport#CodeTaxiwayBaseType-OTHER">
        <rdf:type rdf:resource="http://www.project-best.eu/owl/aixm-mod/airportheliport#CodeTaxiwayType"/>
        <rdfs:comment xml:lang="en">Other.</rdfs:comment>
    </owl:NamedIndividual>
    


    <!-- http://www.project-best.eu/owl/aixm-mod/airportheliport#CodeTaxiwayBaseType-PARALLEL -->

    <owl:NamedIndividual rdf:about="http://www.project-best.eu/owl/aixm-mod/airportheliport#CodeTaxiwayBaseType-PARALLEL">
        <rdf:type rdf:resource="http://www.project-best.eu/owl/aixm-mod/airportheliport#CodeTaxiwayType"/>
        <rdfs:comment xml:lang="en">Parallel taxiway.</rdfs:comment>
    </owl:NamedIndividual>
    


    <!-- http://www.project-best.eu/owl/aixm-mod/airportheliport#CodeTaxiwayBaseType-STUB -->

    <owl:NamedIndividual rdf:about="http://www.project-best.eu/owl/aixm-mod/airportheliport#CodeTaxiwayBaseType-STUB">
        <rdf:type rdf:resource="http://www.project-best.eu/owl/aixm-mod/airportheliport#CodeTaxiwayType"/>
        <rdfs:comment xml:lang="en">Stub taxiway.</rdfs:comment>
    </owl:NamedIndividual>
    


    <!-- http://www.project-best.eu/owl/aixm-mod/airportheliport#CodeTaxiwayBaseType-TURN_AROUND -->

    <owl:NamedIndividual rdf:about="http://www.project-best.eu/owl/aixm-mod/airportheliport#CodeTaxiwayBaseType-TURN_AROUND">
        <rdf:type rdf:resource="http://www.project-best.eu/owl/aixm-mod/airportheliport#CodeTaxiwayType"/>
        <rdfs:comment xml:lang="en">Turn around.</rdfs:comment>
    </owl:NamedIndividual>
    


    <!-- http://www.project-best.eu/owl/aixm-mod/airportheliport#CodeTaxiwayElementBaseType-HOLDING_BAY -->

    <owl:NamedIndividual rdf:about="http://www.project-best.eu/owl/aixm-mod/airportheliport#CodeTaxiwayElementBaseType-HOLDING_BAY">
        <rdf:type rdf:resource="http://www.project-best.eu/owl/aixm-mod/airportheliport#CodeTaxiwayElementType"/>
        <rdfs:comment xml:lang="en">A defined area, on the side of a taxiway, where aircraft can be held, or bypassed, to facilitate efficient surface movement of aircraft.</rdfs:comment>
    </owl:NamedIndividual>
    


    <!-- http://www.project-best.eu/owl/aixm-mod/airportheliport#CodeTaxiwayElementBaseType-INTERSECTION -->

    <owl:NamedIndividual rdf:about="http://www.project-best.eu/owl/aixm-mod/airportheliport#CodeTaxiwayElementBaseType-INTERSECTION">
        <rdf:type rdf:resource="http://www.project-best.eu/owl/aixm-mod/airportheliport#CodeTaxiwayElementType"/>
        <rdfs:comment xml:lang="en">Intersection element - with a runway or with a taxiway.</rdfs:comment>
    </owl:NamedIndividual>
    


    <!-- http://www.project-best.eu/owl/aixm-mod/airportheliport#CodeTaxiwayElementBaseType-NORMAL -->

    <owl:NamedIndividual rdf:about="http://www.project-best.eu/owl/aixm-mod/airportheliport#CodeTaxiwayElementBaseType-NORMAL">
        <rdf:type rdf:resource="http://www.project-best.eu/owl/aixm-mod/airportheliport#CodeTaxiwayElementType"/>
        <rdfs:comment xml:lang="en">The default/regular type.</rdfs:comment>
    </owl:NamedIndividual>
    


    <!-- http://www.project-best.eu/owl/aixm-mod/airportheliport#CodeTaxiwayElementBaseType-OTHER -->

    <owl:NamedIndividual rdf:about="http://www.project-best.eu/owl/aixm-mod/airportheliport#CodeTaxiwayElementBaseType-OTHER">
        <rdf:type rdf:resource="http://www.project-best.eu/owl/aixm-mod/airportheliport#CodeTaxiwayElementType"/>
        <rdfs:comment xml:lang="en">Other.</rdfs:comment>
    </owl:NamedIndividual>
    


    <!-- http://www.project-best.eu/owl/aixm-mod/airportheliport#CodeTaxiwayElementBaseType-SHOULDER -->

    <owl:NamedIndividual rdf:about="http://www.project-best.eu/owl/aixm-mod/airportheliport#CodeTaxiwayElementBaseType-SHOULDER">
        <rdf:type rdf:resource="http://www.project-best.eu/owl/aixm-mod/airportheliport#CodeTaxiwayElementType"/>
        <rdfs:comment xml:lang="en">Intersection element - with a runway or with another taxiway.</rdfs:comment>
    </owl:NamedIndividual>
    


    <!-- http://www.project-best.eu/owl/aixm-mod/airportheliport#CodeTaxiwaySectionBaseType-CL -->

    <owl:NamedIndividual rdf:about="http://www.project-best.eu/owl/aixm-mod/airportheliport#CodeTaxiwaySectionBaseType-CL">
        <rdf:type rdf:resource="http://www.project-best.eu/owl/aixm-mod/airportheliport#CodeTaxiwaySectionType"/>
        <rdfs:comment xml:lang="en">Centre line.</rdfs:comment>
    </owl:NamedIndividual>
    


    <!-- http://www.project-best.eu/owl/aixm-mod/airportheliport#CodeTaxiwaySectionBaseType-EDGE -->

    <owl:NamedIndividual rdf:about="http://www.project-best.eu/owl/aixm-mod/airportheliport#CodeTaxiwaySectionBaseType-EDGE">
        <rdf:type rdf:resource="http://www.project-best.eu/owl/aixm-mod/airportheliport#CodeTaxiwaySectionType"/>
        <rdfs:comment xml:lang="en">Edge.</rdfs:comment>
    </owl:NamedIndividual>
    


    <!-- http://www.project-best.eu/owl/aixm-mod/airportheliport#CodeTaxiwaySectionBaseType-END -->

    <owl:NamedIndividual rdf:about="http://www.project-best.eu/owl/aixm-mod/airportheliport#CodeTaxiwaySectionBaseType-END">
        <rdf:type rdf:resource="http://www.project-best.eu/owl/aixm-mod/airportheliport#CodeTaxiwaySectionType"/>
        <rdfs:comment xml:lang="en">Taxiway end.</rdfs:comment>
    </owl:NamedIndividual>
    


    <!-- http://www.project-best.eu/owl/aixm-mod/airportheliport#CodeTaxiwaySectionBaseType-OTHER -->

    <owl:NamedIndividual rdf:about="http://www.project-best.eu/owl/aixm-mod/airportheliport#CodeTaxiwaySectionBaseType-OTHER">
        <rdf:type rdf:resource="http://www.project-best.eu/owl/aixm-mod/airportheliport#CodeTaxiwaySectionType"/>
        <rdfs:comment xml:lang="en">Other.</rdfs:comment>
    </owl:NamedIndividual>
    


    <!-- http://www.project-best.eu/owl/aixm-mod/airportheliport#CodeTaxiwaySectionBaseType-RWY_INT -->

    <owl:NamedIndividual rdf:about="http://www.project-best.eu/owl/aixm-mod/airportheliport#CodeTaxiwaySectionBaseType-RWY_INT">
        <rdf:type rdf:resource="http://www.project-best.eu/owl/aixm-mod/airportheliport#CodeTaxiwaySectionType"/>
        <rdfs:comment xml:lang="en">Runway intersections.</rdfs:comment>
    </owl:NamedIndividual>
    


    <!-- http://www.project-best.eu/owl/aixm-mod/airportheliport#CodeTaxiwaySectionBaseType-TWY_INT -->

    <owl:NamedIndividual rdf:about="http://www.project-best.eu/owl/aixm-mod/airportheliport#CodeTaxiwaySectionBaseType-TWY_INT">
        <rdf:type rdf:resource="http://www.project-best.eu/owl/aixm-mod/airportheliport#CodeTaxiwaySectionType"/>
        <rdfs:comment xml:lang="en">Taxiway intersections.</rdfs:comment>
    </owl:NamedIndividual>
    


    <!-- http://www.project-best.eu/owl/aixm-mod/airportheliport#CodeTelecomNetworkBaseType-ACARS -->

    <owl:NamedIndividual rdf:about="http://www.project-best.eu/owl/aixm-mod/airportheliport#CodeTelecomNetworkBaseType-ACARS">
        <rdf:type rdf:resource="http://www.project-best.eu/owl/aixm-mod/airportheliport#CodeTelecomNetworkType"/>
        <rdfs:comment xml:lang="en">Aircraft Communications Addressing and Reporting System. A datalink system that enables ground stations (airports, aircraft maintenance bases, etc.) and commercial aircraft to communicate without voice using a datalink system.</rdfs:comment>
    </owl:NamedIndividual>
    


    <!-- http://www.project-best.eu/owl/aixm-mod/airportheliport#CodeTelecomNetworkBaseType-ADNS -->

    <owl:NamedIndividual rdf:about="http://www.project-best.eu/owl/aixm-mod/airportheliport#CodeTelecomNetworkBaseType-ADNS">
        <rdf:type rdf:resource="http://www.project-best.eu/owl/aixm-mod/airportheliport#CodeTelecomNetworkType"/>
        <rdfs:comment xml:lang="en">ARINC Data Network Service (retired Mar 2007)</rdfs:comment>
    </owl:NamedIndividual>
    


    <!-- http://www.project-best.eu/owl/aixm-mod/airportheliport#CodeTelecomNetworkBaseType-AFTN -->

    <owl:NamedIndividual rdf:about="http://www.project-best.eu/owl/aixm-mod/airportheliport#CodeTelecomNetworkBaseType-AFTN">
        <rdf:type rdf:resource="http://www.project-best.eu/owl/aixm-mod/airportheliport#CodeTelecomNetworkType"/>
        <rdfs:comment xml:lang="en">The data interchange in the AFS is performed by the Aeronautical Fixed Telecommunications Network, AFTN. This is a message handling network running according to ICAO Standards documented in Annex 10 to the ICAO Convention</rdfs:comment>
    </owl:NamedIndividual>
    


    <!-- http://www.project-best.eu/owl/aixm-mod/airportheliport#CodeTelecomNetworkBaseType-AMHS -->

    <owl:NamedIndividual rdf:about="http://www.project-best.eu/owl/aixm-mod/airportheliport#CodeTelecomNetworkBaseType-AMHS">
        <rdf:type rdf:resource="http://www.project-best.eu/owl/aixm-mod/airportheliport#CodeTelecomNetworkType"/>
        <rdfs:comment xml:lang="en">Aeronautical Message Handling System. A standard for aeronautical ground-ground communications (e.g. for the transmission of NOTAM, Flight Plans or Meteorological Data) based on X.400 profiles. It has been defined by the International Civil Aviation Organization (ICAO)</rdfs:comment>
    </owl:NamedIndividual>
    


    <!-- http://www.project-best.eu/owl/aixm-mod/airportheliport#CodeTelecomNetworkBaseType-INTERNET -->

    <owl:NamedIndividual rdf:about="http://www.project-best.eu/owl/aixm-mod/airportheliport#CodeTelecomNetworkBaseType-INTERNET">
        <rdf:type rdf:resource="http://www.project-best.eu/owl/aixm-mod/airportheliport#CodeTelecomNetworkType"/>
        <rdfs:comment xml:lang="en">The Internet is a worldwide, publicly accessible series of interconnected computer networks that transmit data by packet switching using the standard Internet Protocol (IP)</rdfs:comment>
    </owl:NamedIndividual>
    


    <!-- http://www.project-best.eu/owl/aixm-mod/airportheliport#CodeTelecomNetworkBaseType-OTHER -->

    <owl:NamedIndividual rdf:about="http://www.project-best.eu/owl/aixm-mod/airportheliport#CodeTelecomNetworkBaseType-OTHER">
        <rdf:type rdf:resource="http://www.project-best.eu/owl/aixm-mod/airportheliport#CodeTelecomNetworkType"/>
        <rdfs:comment xml:lang="en">Other</rdfs:comment>
    </owl:NamedIndividual>
    


    <!-- http://www.project-best.eu/owl/aixm-mod/airportheliport#CodeTelecomNetworkBaseType-SITA -->

    <owl:NamedIndividual rdf:about="http://www.project-best.eu/owl/aixm-mod/airportheliport#CodeTelecomNetworkBaseType-SITA">
        <rdf:type rdf:resource="http://www.project-best.eu/owl/aixm-mod/airportheliport#CodeTelecomNetworkType"/>
        <rdfs:comment xml:lang="en">SITA network</rdfs:comment>
    </owl:NamedIndividual>
    


    <!-- http://www.project-best.eu/owl/aixm-mod/airportheliport#CodeUsageLimitationBaseType-CONDITIONAL -->

    <owl:NamedIndividual rdf:about="http://www.project-best.eu/owl/aixm-mod/airportheliport#CodeUsageLimitationBaseType-CONDITIONAL">
        <rdf:type rdf:resource="http://www.project-best.eu/owl/aixm-mod/airportheliport#CodeUsageLimitationType"/>
        <rdfs:comment xml:lang="en">Permission but with additional instructions. Failure to comply with the additional instructions invalidates the permission.</rdfs:comment>
    </owl:NamedIndividual>
    


    <!-- http://www.project-best.eu/owl/aixm-mod/airportheliport#CodeUsageLimitationBaseType-FORBID -->

    <owl:NamedIndividual rdf:about="http://www.project-best.eu/owl/aixm-mod/airportheliport#CodeUsageLimitationBaseType-FORBID">
        <rdf:type rdf:resource="http://www.project-best.eu/owl/aixm-mod/airportheliport#CodeUsageLimitationType"/>
        <rdfs:comment xml:lang="en">Interdiction.</rdfs:comment>
    </owl:NamedIndividual>
    


    <!-- http://www.project-best.eu/owl/aixm-mod/airportheliport#CodeUsageLimitationBaseType-OTHER -->

    <owl:NamedIndividual rdf:about="http://www.project-best.eu/owl/aixm-mod/airportheliport#CodeUsageLimitationBaseType-OTHER">
        <rdf:type rdf:resource="http://www.project-best.eu/owl/aixm-mod/airportheliport#CodeUsageLimitationType"/>
        <rdfs:comment xml:lang="en">Other.</rdfs:comment>
    </owl:NamedIndividual>
    


    <!-- http://www.project-best.eu/owl/aixm-mod/airportheliport#CodeUsageLimitationBaseType-PERMIT -->

    <owl:NamedIndividual rdf:about="http://www.project-best.eu/owl/aixm-mod/airportheliport#CodeUsageLimitationBaseType-PERMIT">
        <rdf:type rdf:resource="http://www.project-best.eu/owl/aixm-mod/airportheliport#CodeUsageLimitationType"/>
        <rdfs:comment xml:lang="en">Permission.</rdfs:comment>
    </owl:NamedIndividual>
    


    <!-- http://www.project-best.eu/owl/aixm-mod/airportheliport#CodeUsageLimitationBaseType-RESERV -->

    <owl:NamedIndividual rdf:about="http://www.project-best.eu/owl/aixm-mod/airportheliport#CodeUsageLimitationBaseType-RESERV">
        <rdf:type rdf:resource="http://www.project-best.eu/owl/aixm-mod/airportheliport#CodeUsageLimitationType"/>
        <rdfs:comment xml:lang="en">Exclusive usage (reservation).</rdfs:comment>
    </owl:NamedIndividual>
    


    <!-- http://www.project-best.eu/owl/aixm-mod/airportheliport#CodeVASISBaseType-3B_ATVASIS -->

    <owl:NamedIndividual rdf:about="http://www.project-best.eu/owl/aixm-mod/airportheliport#CodeVASISBaseType-3B_ATVASIS">
        <rdf:type rdf:resource="http://www.project-best.eu/owl/aixm-mod/airportheliport#CodeVASISType"/>
        <rdfs:comment xml:lang="en">3 bar ATVASIS.</rdfs:comment>
    </owl:NamedIndividual>
    


    <!-- http://www.project-best.eu/owl/aixm-mod/airportheliport#CodeVASISBaseType-3B_AVASIS -->

    <owl:NamedIndividual rdf:about="http://www.project-best.eu/owl/aixm-mod/airportheliport#CodeVASISBaseType-3B_AVASIS">
        <rdf:type rdf:resource="http://www.project-best.eu/owl/aixm-mod/airportheliport#CodeVASISType"/>
        <rdfs:comment xml:lang="en">3 bar AVASIS</rdfs:comment>
    </owl:NamedIndividual>
    


    <!-- http://www.project-best.eu/owl/aixm-mod/airportheliport#CodeVASISBaseType-3B_VASIS -->

    <owl:NamedIndividual rdf:about="http://www.project-best.eu/owl/aixm-mod/airportheliport#CodeVASISBaseType-3B_VASIS">
        <rdf:type rdf:resource="http://www.project-best.eu/owl/aixm-mod/airportheliport#CodeVASISType"/>
        <rdfs:comment xml:lang="en">3 bar VASIS.</rdfs:comment>
    </owl:NamedIndividual>
    


    <!-- http://www.project-best.eu/owl/aixm-mod/airportheliport#CodeVASISBaseType-APAPI -->

    <owl:NamedIndividual rdf:about="http://www.project-best.eu/owl/aixm-mod/airportheliport#CodeVASISBaseType-APAPI">
        <rdf:type rdf:resource="http://www.project-best.eu/owl/aixm-mod/airportheliport#CodeVASISType"/>
        <rdfs:comment xml:lang="en">Abbreviated precision approach path indicator.</rdfs:comment>
    </owl:NamedIndividual>
    


    <!-- http://www.project-best.eu/owl/aixm-mod/airportheliport#CodeVASISBaseType-ATVASIS -->

    <owl:NamedIndividual rdf:about="http://www.project-best.eu/owl/aixm-mod/airportheliport#CodeVASISBaseType-ATVASIS">
        <rdf:type rdf:resource="http://www.project-best.eu/owl/aixm-mod/airportheliport#CodeVASISType"/>
        <rdfs:comment xml:lang="en">Abbreviated TVASIS</rdfs:comment>
    </owl:NamedIndividual>
    


    <!-- http://www.project-best.eu/owl/aixm-mod/airportheliport#CodeVASISBaseType-AVASIS -->

    <owl:NamedIndividual rdf:about="http://www.project-best.eu/owl/aixm-mod/airportheliport#CodeVASISBaseType-AVASIS">
        <rdf:type rdf:resource="http://www.project-best.eu/owl/aixm-mod/airportheliport#CodeVASISType"/>
        <rdfs:comment xml:lang="en">Abbreviated visual approach slow indicator system.</rdfs:comment>
    </owl:NamedIndividual>
    


    <!-- http://www.project-best.eu/owl/aixm-mod/airportheliport#CodeVASISBaseType-HAPI -->

    <owl:NamedIndividual rdf:about="http://www.project-best.eu/owl/aixm-mod/airportheliport#CodeVASISBaseType-HAPI">
        <rdf:type rdf:resource="http://www.project-best.eu/owl/aixm-mod/airportheliport#CodeVASISType"/>
        <rdfs:comment xml:lang="en">Helicopter approach path indicator.</rdfs:comment>
    </owl:NamedIndividual>
    


    <!-- http://www.project-best.eu/owl/aixm-mod/airportheliport#CodeVASISBaseType-ILU -->

    <owl:NamedIndividual rdf:about="http://www.project-best.eu/owl/aixm-mod/airportheliport#CodeVASISBaseType-ILU">
        <rdf:type rdf:resource="http://www.project-best.eu/owl/aixm-mod/airportheliport#CodeVASISType"/>
        <rdfs:comment xml:lang="en">A number of identical light units.</rdfs:comment>
    </owl:NamedIndividual>
    


    <!-- http://www.project-best.eu/owl/aixm-mod/airportheliport#CodeVASISBaseType-LCVASI -->

    <owl:NamedIndividual rdf:about="http://www.project-best.eu/owl/aixm-mod/airportheliport#CodeVASISBaseType-LCVASI">
        <rdf:type rdf:resource="http://www.project-best.eu/owl/aixm-mod/airportheliport#CodeVASISType"/>
        <rdfs:comment xml:lang="en">Low cost visual approach slope indicator: 3 sets of 4 white lights on 3 mounts usually on only one side of the runway.</rdfs:comment>
    </owl:NamedIndividual>
    


    <!-- http://www.project-best.eu/owl/aixm-mod/airportheliport#CodeVASISBaseType-OLS -->

    <owl:NamedIndividual rdf:about="http://www.project-best.eu/owl/aixm-mod/airportheliport#CodeVASISBaseType-OLS">
        <rdf:type rdf:resource="http://www.project-best.eu/owl/aixm-mod/airportheliport#CodeVASISType"/>
        <rdfs:comment xml:lang="en">Optical landing system for strip decks and aircraft carriers (sometimes available on ground air bases for training purposes).</rdfs:comment>
    </owl:NamedIndividual>
    


    <!-- http://www.project-best.eu/owl/aixm-mod/airportheliport#CodeVASISBaseType-OTHER -->

    <owl:NamedIndividual rdf:about="http://www.project-best.eu/owl/aixm-mod/airportheliport#CodeVASISBaseType-OTHER">
        <rdf:type rdf:resource="http://www.project-best.eu/owl/aixm-mod/airportheliport#CodeVASISType"/>
        <rdfs:comment xml:lang="en">Other type of visual approach slope indicator.</rdfs:comment>
    </owl:NamedIndividual>
    


    <!-- http://www.project-best.eu/owl/aixm-mod/airportheliport#CodeVASISBaseType-PAPI -->

    <owl:NamedIndividual rdf:about="http://www.project-best.eu/owl/aixm-mod/airportheliport#CodeVASISBaseType-PAPI">
        <rdf:type rdf:resource="http://www.project-best.eu/owl/aixm-mod/airportheliport#CodeVASISType"/>
        <rdfs:comment xml:lang="en">Precision approach path indicator.</rdfs:comment>
    </owl:NamedIndividual>
    


    <!-- http://www.project-best.eu/owl/aixm-mod/airportheliport#CodeVASISBaseType-PNI -->

    <owl:NamedIndividual rdf:about="http://www.project-best.eu/owl/aixm-mod/airportheliport#CodeVASISBaseType-PNI">
        <rdf:type rdf:resource="http://www.project-best.eu/owl/aixm-mod/airportheliport#CodeVASISType"/>
        <rdfs:comment xml:lang="en">Alignment of elements system.</rdfs:comment>
    </owl:NamedIndividual>
    


    <!-- http://www.project-best.eu/owl/aixm-mod/airportheliport#CodeVASISBaseType-PVASI -->

    <owl:NamedIndividual rdf:about="http://www.project-best.eu/owl/aixm-mod/airportheliport#CodeVASISBaseType-PVASI">
        <rdf:type rdf:resource="http://www.project-best.eu/owl/aixm-mod/airportheliport#CodeVASISType"/>
        <rdfs:comment xml:lang="en">Pulsating/steady burning visual approach slope indicator, normally a single light unit projecting two colours.</rdfs:comment>
    </owl:NamedIndividual>
    


    <!-- http://www.project-best.eu/owl/aixm-mod/airportheliport#CodeVASISBaseType-TRCV -->

    <owl:NamedIndividual rdf:about="http://www.project-best.eu/owl/aixm-mod/airportheliport#CodeVASISBaseType-TRCV">
        <rdf:type rdf:resource="http://www.project-best.eu/owl/aixm-mod/airportheliport#CodeVASISType"/>
        <rdfs:comment xml:lang="en">Tri-colour visual approach slope indicator, normally a single light unit projecting three colours.</rdfs:comment>
    </owl:NamedIndividual>
    


    <!-- http://www.project-best.eu/owl/aixm-mod/airportheliport#CodeVASISBaseType-TVASIS -->

    <owl:NamedIndividual rdf:about="http://www.project-best.eu/owl/aixm-mod/airportheliport#CodeVASISBaseType-TVASIS">
        <rdf:type rdf:resource="http://www.project-best.eu/owl/aixm-mod/airportheliport#CodeVASISType"/>
        <rdfs:comment xml:lang="en">T-shaped VASIS</rdfs:comment>
    </owl:NamedIndividual>
    


    <!-- http://www.project-best.eu/owl/aixm-mod/airportheliport#CodeVASISBaseType-VASIS -->

    <owl:NamedIndividual rdf:about="http://www.project-best.eu/owl/aixm-mod/airportheliport#CodeVASISBaseType-VASIS">
        <rdf:type rdf:resource="http://www.project-best.eu/owl/aixm-mod/airportheliport#CodeVASISType"/>
        <rdfs:comment xml:lang="en">Visual approach slope indicator system.</rdfs:comment>
    </owl:NamedIndividual>
    


    <!-- http://www.project-best.eu/owl/aixm-mod/airportheliport#CodeValueInterpretationBaseType-ABOVE -->

    <owl:NamedIndividual rdf:about="http://www.project-best.eu/owl/aixm-mod/airportheliport#CodeValueInterpretationBaseType-ABOVE">
        <rdf:type rdf:resource="http://www.project-best.eu/owl/aixm-mod/airportheliport#CodeValueInterpretationType"/>
        <rdfs:comment xml:lang="en">Higher than the value.</rdfs:comment>
    </owl:NamedIndividual>
    


    <!-- http://www.project-best.eu/owl/aixm-mod/airportheliport#CodeValueInterpretationBaseType-AT_OR_ABOVE -->

    <owl:NamedIndividual rdf:about="http://www.project-best.eu/owl/aixm-mod/airportheliport#CodeValueInterpretationBaseType-AT_OR_ABOVE">
        <rdf:type rdf:resource="http://www.project-best.eu/owl/aixm-mod/airportheliport#CodeValueInterpretationType"/>
        <rdfs:comment xml:lang="en">Equal or higher than the value.</rdfs:comment>
    </owl:NamedIndividual>
    


    <!-- http://www.project-best.eu/owl/aixm-mod/airportheliport#CodeValueInterpretationBaseType-AT_OR_BELOW -->

    <owl:NamedIndividual rdf:about="http://www.project-best.eu/owl/aixm-mod/airportheliport#CodeValueInterpretationBaseType-AT_OR_BELOW">
        <rdf:type rdf:resource="http://www.project-best.eu/owl/aixm-mod/airportheliport#CodeValueInterpretationType"/>
        <rdfs:comment xml:lang="en">Equal or lower than the value.</rdfs:comment>
    </owl:NamedIndividual>
    


    <!-- http://www.project-best.eu/owl/aixm-mod/airportheliport#CodeValueInterpretationBaseType-BELOW -->

    <owl:NamedIndividual rdf:about="http://www.project-best.eu/owl/aixm-mod/airportheliport#CodeValueInterpretationBaseType-BELOW">
        <rdf:type rdf:resource="http://www.project-best.eu/owl/aixm-mod/airportheliport#CodeValueInterpretationType"/>
        <rdfs:comment xml:lang="en">Lower than the value.</rdfs:comment>
    </owl:NamedIndividual>
    


    <!-- http://www.project-best.eu/owl/aixm-mod/airportheliport#CodeValueInterpretationBaseType-OTHER -->

    <owl:NamedIndividual rdf:about="http://www.project-best.eu/owl/aixm-mod/airportheliport#CodeValueInterpretationBaseType-OTHER">
        <rdf:type rdf:resource="http://www.project-best.eu/owl/aixm-mod/airportheliport#CodeValueInterpretationType"/>
        <rdfs:comment xml:lang="en">Other.</rdfs:comment>
    </owl:NamedIndividual>
    


    <!-- http://www.project-best.eu/owl/aixm-mod/airportheliport#CodeVerticalDatumBaseType-AHD -->

    <owl:NamedIndividual rdf:about="http://www.project-best.eu/owl/aixm-mod/airportheliport#CodeVerticalDatumBaseType-AHD">
        <rdf:type rdf:resource="http://www.project-best.eu/owl/aixm-mod/airportheliport#CodeVerticalDatumType"/>
        <rdfs:comment xml:lang="en">Australian Height Datum</rdfs:comment>
    </owl:NamedIndividual>
    


    <!-- http://www.project-best.eu/owl/aixm-mod/airportheliport#CodeVerticalDatumBaseType-EGM_96 -->

    <owl:NamedIndividual rdf:about="http://www.project-best.eu/owl/aixm-mod/airportheliport#CodeVerticalDatumBaseType-EGM_96">
        <rdf:type rdf:resource="http://www.project-best.eu/owl/aixm-mod/airportheliport#CodeVerticalDatumType"/>
        <rdfs:comment xml:lang="en">(ICAO Doc 9674) Earth gravitational model 1996.  ICAO recommended vertical datum.</rdfs:comment>
    </owl:NamedIndividual>
    


    <!-- http://www.project-best.eu/owl/aixm-mod/airportheliport#CodeVerticalDatumBaseType-NAVD88 -->

    <owl:NamedIndividual rdf:about="http://www.project-best.eu/owl/aixm-mod/airportheliport#CodeVerticalDatumBaseType-NAVD88">
        <rdf:type rdf:resource="http://www.project-best.eu/owl/aixm-mod/airportheliport#CodeVerticalDatumType"/>
        <rdfs:comment xml:lang="en">North American Vertical Datum of 1988</rdfs:comment>
    </owl:NamedIndividual>
    


    <!-- http://www.project-best.eu/owl/aixm-mod/airportheliport#CodeVerticalDatumBaseType-OTHER -->

    <owl:NamedIndividual rdf:about="http://www.project-best.eu/owl/aixm-mod/airportheliport#CodeVerticalDatumBaseType-OTHER">
        <rdf:type rdf:resource="http://www.project-best.eu/owl/aixm-mod/airportheliport#CodeVerticalDatumType"/>
        <rdfs:comment xml:lang="en">Other</rdfs:comment>
    </owl:NamedIndividual>
    


    <!-- http://www.project-best.eu/owl/aixm-mod/airportheliport#CodeVisualDockingGuidanceBaseType-AGNIS -->

    <owl:NamedIndividual rdf:about="http://www.project-best.eu/owl/aixm-mod/airportheliport#CodeVisualDockingGuidanceBaseType-AGNIS">
        <rdf:type rdf:resource="http://www.project-best.eu/owl/aixm-mod/airportheliport#CodeVisualDockingGuidanceType"/>
        <rdfs:comment xml:lang="en">Azimuth Guidance for Nose-In Stand, providing centreline guidance only by using two coloured lights mounted side by side.</rdfs:comment>
    </owl:NamedIndividual>
    


    <!-- http://www.project-best.eu/owl/aixm-mod/airportheliport#CodeVisualDockingGuidanceBaseType-AGNIS_PAPA -->

    <owl:NamedIndividual rdf:about="http://www.project-best.eu/owl/aixm-mod/airportheliport#CodeVisualDockingGuidanceBaseType-AGNIS_PAPA">
        <rdf:type rdf:resource="http://www.project-best.eu/owl/aixm-mod/airportheliport#CodeVisualDockingGuidanceType"/>
        <rdfs:comment xml:lang="en">Combined AGNIS and PAPA device.</rdfs:comment>
    </owl:NamedIndividual>
    


    <!-- http://www.project-best.eu/owl/aixm-mod/airportheliport#CodeVisualDockingGuidanceBaseType-AGNIS_STOP -->

    <owl:NamedIndividual rdf:about="http://www.project-best.eu/owl/aixm-mod/airportheliport#CodeVisualDockingGuidanceBaseType-AGNIS_STOP">
        <rdf:type rdf:resource="http://www.project-best.eu/owl/aixm-mod/airportheliport#CodeVisualDockingGuidanceType"/>
        <rdfs:comment xml:lang="en">AGNIS system complemented with a simple stop light, on the side of the AGNIS display.</rdfs:comment>
    </owl:NamedIndividual>
    


    <!-- http://www.project-best.eu/owl/aixm-mod/airportheliport#CodeVisualDockingGuidanceBaseType-APIS -->

    <owl:NamedIndividual rdf:about="http://www.project-best.eu/owl/aixm-mod/airportheliport#CodeVisualDockingGuidanceBaseType-APIS">
        <rdf:type rdf:resource="http://www.project-best.eu/owl/aixm-mod/airportheliport#CodeVisualDockingGuidanceType"/>
        <rdfs:comment xml:lang="en">Aircraft Positioning and Information System that shows azimuth information using a series of parallel and black bars which kink at their midpoint.</rdfs:comment>
    </owl:NamedIndividual>
    


    <!-- http://www.project-best.eu/owl/aixm-mod/airportheliport#CodeVisualDockingGuidanceBaseType-A_VDGS -->

    <owl:NamedIndividual rdf:about="http://www.project-best.eu/owl/aixm-mod/airportheliport#CodeVisualDockingGuidanceBaseType-A_VDGS">
        <rdf:type rdf:resource="http://www.project-best.eu/owl/aixm-mod/airportheliport#CodeVisualDockingGuidanceType"/>
        <rdfs:comment xml:lang="en">(Generic) Advanced Visual Docking Guidance System that features electronic displays which perform the functions of an AGNIS/PAPA installation, although with much greater accuracy.  They may also provide collision avoidance from static objects.</rdfs:comment>
    </owl:NamedIndividual>
    


    <!-- http://www.project-best.eu/owl/aixm-mod/airportheliport#CodeVisualDockingGuidanceBaseType-OTHER -->

    <owl:NamedIndividual rdf:about="http://www.project-best.eu/owl/aixm-mod/airportheliport#CodeVisualDockingGuidanceBaseType-OTHER">
        <rdf:type rdf:resource="http://www.project-best.eu/owl/aixm-mod/airportheliport#CodeVisualDockingGuidanceType"/>
        <rdfs:comment xml:lang="en">Other</rdfs:comment>
    </owl:NamedIndividual>
    


    <!-- http://www.project-best.eu/owl/aixm-mod/airportheliport#CodeVisualDockingGuidanceBaseType-PAPA -->

    <owl:NamedIndividual rdf:about="http://www.project-best.eu/owl/aixm-mod/airportheliport#CodeVisualDockingGuidanceBaseType-PAPA">
        <rdf:type rdf:resource="http://www.project-best.eu/owl/aixm-mod/airportheliport#CodeVisualDockingGuidanceType"/>
        <rdfs:comment xml:lang="en">Parallax Aircraft Parking Aid consisting of a large grey/black box that uses the effect of perspective in order to indicate the relative position of the aircraft along the centreline.</rdfs:comment>
    </owl:NamedIndividual>
    


    <!-- http://www.project-best.eu/owl/aixm-mod/airportheliport#CodeVisualDockingGuidanceBaseType-SAFE_DOC -->

    <owl:NamedIndividual rdf:about="http://www.project-best.eu/owl/aixm-mod/airportheliport#CodeVisualDockingGuidanceBaseType-SAFE_DOC">
        <rdf:type rdf:resource="http://www.project-best.eu/owl/aixm-mod/airportheliport#CodeVisualDockingGuidanceType"/>
        <rdfs:comment xml:lang="en">Safe dock allows aircraft to park up to an accuracy of 10 cm using lasers to attain the aircraft&apos;s position.</rdfs:comment>
    </owl:NamedIndividual>
    


    <!-- http://www.project-best.eu/owl/aixm-mod/airportheliport#CodeVisualDockingGuidanceBaseType-SAFE_GATE -->

    <owl:NamedIndividual rdf:about="http://www.project-best.eu/owl/aixm-mod/airportheliport#CodeVisualDockingGuidanceBaseType-SAFE_GATE">
        <rdf:type rdf:resource="http://www.project-best.eu/owl/aixm-mod/airportheliport#CodeVisualDockingGuidanceType"/>
        <rdfs:comment xml:lang="en">A type of A-VDGS that uses an aircraft symbol on a display indicating the relative position along the centreline.</rdfs:comment>
    </owl:NamedIndividual>
    


    <!-- http://www.project-best.eu/owl/aixm-mod/airportheliport#CodeWorkAreaBaseType-CONSTRUCTION -->

    <owl:NamedIndividual rdf:about="http://www.project-best.eu/owl/aixm-mod/airportheliport#CodeWorkAreaBaseType-CONSTRUCTION">
        <rdf:type rdf:resource="http://www.project-best.eu/owl/aixm-mod/airportheliport#CodeWorkAreaType"/>
        <rdfs:comment xml:lang="en">The work area is used for construction.</rdfs:comment>
    </owl:NamedIndividual>
    


    <!-- http://www.project-best.eu/owl/aixm-mod/airportheliport#CodeWorkAreaBaseType-OTHER -->

    <owl:NamedIndividual rdf:about="http://www.project-best.eu/owl/aixm-mod/airportheliport#CodeWorkAreaBaseType-OTHER">
        <rdf:type rdf:resource="http://www.project-best.eu/owl/aixm-mod/airportheliport#CodeWorkAreaType"/>
        <rdfs:comment xml:lang="en">The work area is used for other activities.</rdfs:comment>
    </owl:NamedIndividual>
    


    <!-- http://www.project-best.eu/owl/aixm-mod/airportheliport#CodeWorkAreaBaseType-PARKED -->

    <owl:NamedIndividual rdf:about="http://www.project-best.eu/owl/aixm-mod/airportheliport#CodeWorkAreaBaseType-PARKED">
        <rdf:type rdf:resource="http://www.project-best.eu/owl/aixm-mod/airportheliport#CodeWorkAreaType"/>
        <rdfs:comment xml:lang="en">Parked or disabled aircraft or machinery.</rdfs:comment>
    </owl:NamedIndividual>
    


    <!-- http://www.project-best.eu/owl/aixm-mod/airportheliport#CodeWorkAreaBaseType-SURFACEWORK -->

    <owl:NamedIndividual rdf:about="http://www.project-best.eu/owl/aixm-mod/airportheliport#CodeWorkAreaBaseType-SURFACEWORK">
        <rdf:type rdf:resource="http://www.project-best.eu/owl/aixm-mod/airportheliport#CodeWorkAreaType"/>
        <rdfs:comment xml:lang="en">The work area is used for surface improvements.</rdfs:comment>
    </owl:NamedIndividual>
</rdf:RDF>



<!-- Generated by the OWL API (version 1.3.8.1099) http://owlapi.sourceforge.net -->

